#################################################################
###                    Created by Javad Chamanara             ###
#################################################################

@prefix : 		    <http://stream-ontology.com/matvoc-core/> .
@prefix rdf: 		<http://www.w3.org/1999/02/22-rdf-syntax-ns#> .
@prefix rdfs: 	    <http://www.w3.org/2000/01/rdf-schema#> .
@prefix owl: 		<http://www.w3.org/2002/07/owl#> .
@prefix xsd: 		<http://www.w3.org/2001/XMLSchema#> .
@prefix dc: 		<http://purl.org/dc/elements/1.1/> .
@prefix xml: 		<http://www.w3.org/XML/1998/namespace> .
@prefix oboe: 	    <http://ecoinformatics.org/oboe/oboe.1.2/oboe-core.owl#> .
@prefix sosa:       <http://www.w3.org/ns/sosa/> .
@prefix ssn:        <http://www.w3.org/ns/ssn/> .
@prefix wot: 		<http://xmlns.com/wot/0.1/> .
@prefix swrlb: 	    <http://www.w3.org/2003/11/swrlb#> .
@prefix swrl: 	    <http://www.w3.org/2003/11/swrl#> .
@prefix dul:        <http://www.loa-cnr.it/ontologies/DUL.owl#> .
@prefix cc: 		<http://creativecommons.org/ns#> .
@prefix vs: 		<http://www.w3.org/2003/06/sw-vocab-status/ns#> .
@prefix foaf: 	    <http://xmlns.com/foaf/0.1/> .
@prefix owl2xml: 	<http://www.w3.org/2006/12/owl2-xml#> .
@prefix emmo:       <http://stream-ontology.com/matvoc-emmo> .
@prefix skos:       <http://www.w3.org/2004/02/skos/core#> .
@prefix dcat:       <http://www.w3.org/ns/dcat#> .
@prefix mvc: 		<http://stream-ontology.com/matvoc-core/> .
@base 			    <http://stream-ontology.com/matvoc-core/> .

<http://stream-ontology.com/matvoc-core/> rdf:type owl:Ontology ;
    dc:title "Materials Vocabulary: MatVoc-Core"@en; 
    dc:description "The Materials RDF vocabulary, described using W3C RDF Schema and the Web Ontology Language to satisfy the requirements of the STREAM project."@en . 

#################################################################
###                     Class Definitions                     ###

:Study rdf:type owl:Class; 
    #owl:equivalentClass dul:Process ; # needs more investigation for possible alternatives, PSL, ...
    #owl:equivalentClass bpmn1:FlowNode ; # https://www.researchgate.net/publication/221448529_Towards_a_BPMN_20_ontology/figures
    #owl:equivalentClass bpmn2:Process ; # https://dkm.fbk.eu/bpmn-ontology
    rdfs:comment "An endeavor that adheres to scientific research design to obtain a result or an insight."@en ;
    rdfs:label "Study"@IRI-based; 
    rdfs:label "Study"@en .

:Experiment rdf:type owl:Class; 
    rdfs:subClassOf  :Study ;
    rdfs:comment "A single, unique, and identifiable experiment."@en ;
    rdfs:label "Experiment"@IRI-based; 
    rdfs:label "Experiment"@en .

:Simulation rdf:type owl:Class; 
    rdfs:subClassOf :Study ;
    rdfs:comment "A single, unique, and identifiable simulation."@en ;
    rdfs:label "Simulation"@IRI-based; 
    rdfs:label "Simulation"@en .

:Run rdf:type owl:Class; 
    #owl:equivalentClass psl:Flow ;
    rdfs:comment "A single, unique, and identifiable execution of an experiment or simulation under defined terms and settings."@en ;
    rdfs:label "Run"@IRI-based; 
    rdfs:label "Run"@en .

# Add triples to say emmo:Item is a/sub of oboe:Entity to allow observations to apply to the characteristics of EMMO's items.
:Entity rdf:type owl:Class; 
    rdfs:comment "Entity class is an abstract entity which is being processed within an experiment or simulated."@en ;    
    owl:equivalentClass oboe:Entity ;
    owl:equivalentClass emmo:Item ;
    owl:equivalentClass sosa:FeatureOfInterest .

:Material rdf:type owl:Class; 
    rdfs:comment "Material class is a representative of a feature of interest on which an experiment or a simulation is made."@en ;  
    rdfs:subClassOf :Entity .

:Sample rdf:type owl:Class; 
    rdfs:comment "Sample is a class representing a subset of a material that is the object of an experiment or a simulation."@en ;      
    #owl:equivalentClass oboe:Entity ;
    owl:equivalentClass sosa:Sample .
    
:Observer rdf:type owl:Class; 
    rdfs:subClassOf foaf:Agent ;
    #owl:equivalentClass ssn:System ;
    rdfs:comment "An agent that can observe an observation. It can be a human, device, sensor, or software."@en ;
    rdfs:label "Observer"@IRI-based; 
    rdfs:label "Observer"@en .

:Dataset rdf:type owl:Class; 
    owl:equivalentClass oboe:ObservationCollection ;
    rdfs:comment "A set of related observations with their measurements and values, obtained by a single run."@en ;
    rdfs:label "Dataset"@IRI-based; 
    rdfs:label "Dataset"@en . 

:Term rdf:type owl:Class; 
    owl:subClassOf oboe:Standard ;
    rdfs:comment "A term or condition that applies to an observation or a run."@en ;
    rdfs:label "Term"@IRI-based; 
    rdfs:label "Term"@en .

:Enumeration rdf:type owl:Class; 
    rdfs:subClassOf :Term ;
    owl:equivalentClass skos:Concept ;
    rdfs:comment "A terminology, e.g., a closed list of vocabularies that can be used to limit the valid values of a measurement."@en ;
    rdfs:label "Enumeration"@IRI-based; 
    rdfs:label "Enumeration"@en .            

:Configuration rdf:type owl:Class; 
    rdfs:subClassOf :Term ;
    rdfs:comment "A specific setting or arrangement of the observers, entities, and/or charcteristics. This can be e.g., an atom topology in a smulation."@en ;
    rdfs:label "Configuration"@IRI-based; 
    rdfs:label "Configuration"@en .

:Method rdf:type owl:Class;
    owl:equivalentClass oboe:Protocol ;
    rdfs:comment "The method of performing an experiment, observation, or measurement."@en ;
    rdfs:label "Method"@IRI-based; 
    rdfs:label "Method"@en . 
	
:Formula rdf:type owl:Class;
    rdfs:comment "define formula's associated with the material."@en ;
    rdfs:label "Formula"@IRI-based; 
    rdfs:label "Formula"@en .

# MeasuredValue class has a data type property raw value, which its data type can be determined by xsd types, hence no need to have a type system here.
#:DataType rdf:type owl:Class; 
#    owl:equivalentClass ontodt:OntoDT_487147 ; # datatype from ontoDT
#    rdfs:comment "System type of the data, e.g., string, float, integer."@en ;
#    rdfs:label "DataType"@IRI-based; 
#    rdfs:label "Data Type"@en .

#:Integer rdf:type owl:Class; 
#    owl:equivalentClass ontodt:OntoDT_0000003 ; 
#    rdfs:comment "Integer Data Type"@en ;
#    rdfs:label "Integer"@IRI-based; 
#    rdfs:label "Integer"@en .

#:Real rdf:type owl:Class; 
#    owl:equivalentClass ontodt:OntoDT_488636 ; 
#    rdfs:comment "Real Data Type, e.g., float and double."@en ;
#    rdfs:label "Real"@IRI-based; 
#    rdfs:label "Real"@en .
       
#:String rdf:type owl:Class; 
#    #owl:equivalentClass ontodt:XXX ; 
#    rdfs:comment "String date type."@en ;
#    rdfs:label "String"@IRI-based; 
#    rdfs:label "String"@en .




###                 End of Class Definitions                  ###
#################################################################

#################################################################
###               Object Property Definitions                 ###
:hasRun rdf:type owl:ObjectProperty ;
    rdfs:comment "The hasRun property gives the runs of a simulation."@en ;
    rdfs:label "hasRun"@IRI-based; 
    rdfs:label "has run"@en; 
    rdfs:domain :Study;
    rdfs:range :Run . 

:isRunOf rdf:type owl:ObjectProperty ;
    owl:inverseOf :hasRun ;
    rdfs:comment "The isRunOf property gives the simulation of a run."@en ;
    rdfs:label "isRunOf"@IRI-based; 
    rdfs:label "is run of"@en; 
    rdfs:domain :Run;
    rdfs:range :Study . 

:hasProtocol rdf:type owl:ObjectProperty ;
    rdfs:comment "The hasProtocol property gives the protocol of an individual in the domain."@en ;
    rdfs:label "hasProtocol"@IRI-based; 
    rdfs:label "has protocol"@en; 
    #rdfs:domain :Run;  # The domain class can be a Run, an Observation, or a Measurement. Hence, I relaxed determining the domain.
    rdfs:domain :Run;
    rdfs:domain oboe:Observation;
    rdfs:domain oboe:Measurement;
    rdfs:range oboe:Protocol .         

:hasMethod rdf:type owl:ObjectProperty ;
    rdfs:comment "The hasMethod property gives the method of an individual in the domain."@en ;
    rdfs:label "hasMethod"@IRI-based; 
    rdfs:label "has method"@en; 
    #rdfs:domain :Run;  # The domain class can be a Run, an Observation, or a Measurement. Hence, I relaxed determining the domain.
    rdfs:domain :Run;
    rdfs:domain oboe:Observation;
    rdfs:domain oboe:Measurement;
    rdfs:range :Method .             

:restrictedBy rdf:type owl:ObjectProperty ;
    rdfs:comment "The restrictedBy property gives the terms that are applied to a Run, an Obervation, or a Measurement." ;
    rdfs:label "restrictedBy"@IRI-based; 
    rdfs:label "restricted by"@en; 
    #rdfs:domain :Run;  # The domain class can be a Run, an Observation, or a Measurement. Hence, I relaxed determining the domain.
    rdfs:domain :Run;
    rdfs:domain oboe:Observation;
    rdfs:domain oboe:Measurement;
    rdfs:range :Term .     

:resultsIn rdf:type owl:ObjectProperty ;
    rdfs:comment "The resultsIn property gives the observation collection of a run." ;
    rdfs:label "resultsIn"@IRI-based; 
    rdfs:label "results in"@en; 
    rdfs:domain :Run;
    rdfs:range  :Dataset .     

# can be removed or repurposed, as one run may have more than one observation, and they are captured via the resultsIn property.
:defines rdf:type owl:ObjectProperty ;
    rdfs:comment "The defines property gives the observations defined by a run." ;
    rdfs:label "defines"@IRI-based; 
    rdfs:label "defines"@en; 
    rdfs:domain :Run;
    rdfs:range oboe:Observation .     

:observes rdf:type owl:ObjectProperty ;
    rdfs:comment "The observes property gives the characteristic that has been observed by an observer." ;
    rdfs:label "observes"@IRI-based; 
    rdfs:label "observes"@en; 
    rdfs:domain :Observer;
    rdfs:range oboe:Characteristic . 

:isObservedBy rdf:type owl:ObjectProperty ;
    owl:inverseOf :observes ;
    rdfs:comment "The isObservedBy property gives the observer of a characteristic." ;
    rdfs:label "isObservedBy"@IRI-based; 
    rdfs:label "is observed by"@en; 
    rdfs:domain oboe:Characteristic;
    rdfs:range :Observer . 

:hasTag rdf:type owl:ObjectProperty ;
    rdfs:comment "The hasTag property gives allows the measurements to have classification, grouping, or thematic tags." ;
    rdfs:label "hasTag"@IRI-based; 
    rdfs:label "has tag"@en; 
    rdfs:domain oboe:measurement;
    rdfs:range skos:Concept . 

:hasMetadata rdf:type owl:ObjectProperty ;
    rdfs:comment "The hasMetadata property allows a dataset (observation collection) to be explained by a DCAT metadata." ;
    rdfs:label "hasMetadata"@IRI-based; 
    rdfs:label "has metadata"@en; 
    rdfs:domain :Dataset;
    rdfs:range dcat:Dataset. 

:isSampleOf rdf:type owl:ObjectProperty ;
    rdfs:comment "The isSampleOf property indicated the feature of interest that the sample is taken from" ;
    rdfs:label "isSampleOf"@IRI-based; 
    rdfs:label "is sample of"@en; 
    rdfs:domain :Sample;
    rdfs:range :Entity . 

#:hasDataType rdf:type owl:ObjectProperty ;
#    rdfs:comment "The hasDataType property give the data type of a measurement value." ;
#    rdfs:label "hasDataType"@IRI-based ; 
#    rdfs:label "has dataType"@en ; 
#    rdfs:domain oboe:MeasuredValue ;
#    rdfs:range :DataType . 

###            End of Object Property Definitions             ###
#################################################################

#################################################################
###                Data Property Definitions                  ###

:hasRawValue rdf:type owl:DataTypeProperty; 
    rdfs:comment "The hasRawValue property is the coded representation of the measured value."@en ;
    owl:equivalentProperty oboe:hasCode ;
    rdfs:domain oboe:MeasuredValue .

:startedAt rdf:type owl:DataTypeProperty; 
    rdfs:comment "The date and time when the ran started."@en ;
    rdfs:domain :Run ;
    rdfs:range xsd:dateTime .    

:fisnishedAt rdf:type owl:DataTypeProperty; 
    rdfs:comment "The date and time when the ran is finished."@en ;
    rdfs:domain :Run ;
    rdfs:range xsd:dateTime .    

###            End of Data Property Definitions               ###
#################################################################      
