@prefix : <https://nomad-coe.eu/ontology/metainfo/pure#> .
@prefix owl: <http://www.w3.org/2002/07/owl#> .
@prefix rdf: <http://www.w3.org/1999/02/22-rdf-syntax-ns#> .
@prefix rdfs: <http://www.w3.org/2000/01/rdf-schema#> .
@prefix xml: <http://www.w3.org/XML/1998/namespace> .
@prefix xsd: <http://www.w3.org/2001/XMLSchema#> .

<https://nomad-coe.eu/ontology/metainfo/pure> a owl:Ontology .

:basis_set_description a owl:Class ;
    rdfs:comment """One of the parts building the basis set of the system (e.g., some atom-centered basis
set, plane-waves or both)."""^^xsd:string ;
    rdfs:subClassOf :NMI_category .

:conserved_quantity a owl:Class ;
    rdfs:comment """A quantity that is preserved during the time propagation (for example,
kinetic+potential energy during NVE)."""^^xsd:string ;
    rdfs:subClassOf :NMI_category .

:error_estimate a owl:Class ;
    rdfs:comment "An estimate of the error on the converged (final) value."^^xsd:string ;
    rdfs:subClassOf :error_estimate_contribution .

:hasFixDim5 a owl:DatatypeProperty,
        owl:FunctionalProperty ;
    rdfs:domain :NMI_quantity ;
    rdfs:range [ a rdfs:Datatype ;
            owl:onDatatype xsd:integer ;
            owl:withRestrictions ( [ xsd:minInclusive 1 ] ) ] .

:hasReference a owl:ObjectProperty ;
    rdfs:domain :NMI_quantity ;
    rdfs:range :NMI_section ;
    rdfs:subPropertyOf <http://emmo.info/emmo/middle/holistic#EMMO_ae2d1a96_bfa1_409a_a7d2_03d69e8a125a> .

:hasSection a owl:ObjectProperty ;
    rdfs:domain :NOMADEntry ;
    rdfs:range :NMI_section .

:hasVarDim5 a owl:ObjectProperty ;
    rdfs:domain :NMI_quantity ;
    rdfs:range :NMI_dimension ;
    rdfs:subPropertyOf <http://emmo.info/emmo/middle/semiotics#EMMO_eb3518bf_f799_4f9e_8c3e_ce59af11453b> .

:section_run a owl:Class ;
    rdfs:comment """Every section_run represents a single call of a program. What exactly is contained in a run depends on the run type (see for example section_method and
section_single_configuration_calculation) and the program (see [program_info
](program_info))."""^^xsd:string ;
    rdfs:subClassOf [ a owl:Restriction ;
            owl:onProperty :hasQuantity ;
            owl:someValuesFrom :parsing_message_debug_run ],
        [ a owl:Restriction ;
            owl:onProperty :hasQuantity ;
            owl:someValuesFrom :parsing_message_warning_run ],
        [ a owl:Restriction ;
            owl:onProperty :hasQuantity ;
            owl:someValuesFrom :time_run_wall_end ],
        [ a owl:Restriction ;
            owl:onProperty :hasQuantity ;
            owl:someValuesFrom :parsing_message_error_run ],
        [ a owl:Restriction ;
            owl:onProperty :hasQuantity ;
            owl:someValuesFrom :run_clean_end ],
        [ a owl:Restriction ;
            owl:onProperty :hasSubSection ;
            owl:someValuesFrom :section_system ],
        [ a owl:Restriction ;
            owl:onProperty :hasSubSection ;
            owl:someValuesFrom :section_basis_set_cell_dependent ],
        [ a owl:Restriction ;
            owl:onProperty :hasQuantity ;
            owl:someValuesFrom :message_error_run ],
        [ a owl:Restriction ;
            owl:onProperty :hasQuantity ;
            owl:someValuesFrom :program_compilation_host ],
        [ a owl:Restriction ;
            owl:onProperty :hasQuantity ;
            owl:someValuesFrom :time_run_wall_start ],
        [ a owl:Restriction ;
            owl:onProperty :hasSubSection ;
            owl:someValuesFrom :section_basis_set_atom_centered ],
        [ a owl:Restriction ;
            owl:onProperty :hasQuantity ;
            owl:someValuesFrom :program_basis_set_type ],
        [ a owl:Restriction ;
            owl:onProperty :hasQuantity ;
            owl:someValuesFrom :message_info_run ],
        [ a owl:Restriction ;
            owl:onProperty :hasSubSection ;
            owl:someValuesFrom :section_method ],
        [ a owl:Restriction ;
            owl:onProperty :hasSubSection ;
            owl:someValuesFrom :section_topology ],
        [ a owl:Restriction ;
            owl:onProperty :hasQuantity ;
            owl:someValuesFrom :program_version ],
        [ a owl:Restriction ;
            owl:onProperty :hasSubSection ;
            owl:someValuesFrom :section_sampling_method ],
        [ a owl:Restriction ;
            owl:onProperty :hasSubSection ;
            owl:someValuesFrom :section_single_configuration_calculation ],
        [ a owl:Restriction ;
            owl:onProperty :hasQuantity ;
            owl:someValuesFrom :time_run_date_start ],
        [ a owl:Restriction ;
            owl:onProperty :hasQuantity ;
            owl:someValuesFrom :raw_id ],
        [ a owl:Restriction ;
            owl:onProperty :hasQuantity ;
            owl:someValuesFrom :parsing_message_info_run ],
        [ a owl:Restriction ;
            owl:onProperty :hasQuantity ;
            owl:someValuesFrom :program_name ],
        [ a owl:Restriction ;
            owl:onProperty :hasSubSection ;
            owl:someValuesFrom :section_frame_sequence ],
        [ a owl:Restriction ;
            owl:onProperty :hasQuantity ;
            owl:someValuesFrom :time_run_cpu1_start ],
        [ a owl:Restriction ;
            owl:onProperty :hasQuantity ;
            owl:someValuesFrom :run_hosts ],
        [ a owl:Restriction ;
            owl:onProperty :hasQuantity ;
            owl:someValuesFrom :program_compilation_datetime ],
        [ a owl:Restriction ;
            owl:onProperty :hasQuantity ;
            owl:someValuesFrom :time_run_cpu1_end ],
        [ a owl:Restriction ;
            owl:onProperty :hasQuantity ;
            owl:someValuesFrom :message_warning_run ],
        [ a owl:Restriction ;
            owl:onProperty :hasQuantity ;
            owl:someValuesFrom :message_debug_run ],
        [ a owl:Restriction ;
            owl:onProperty :hasQuantity ;
            owl:someValuesFrom :calculation_file_uri ],
        [ a owl:Restriction ;
            owl:onProperty :hasQuantity ;
            owl:someValuesFrom :time_run_date_end ],
        :NMI_section .

:settings_GW a owl:Class ;
    rdfs:comment """Contains parameters for the GW-method in the post Hartree-Fock step, that expands the
self-energy in terms of the single particle Green's function $G$ and the screened
Coulomb interaction $W$."""^^xsd:string ;
    rdfs:subClassOf :settings_post_hartree_fock .

:settings_MCSCF a owl:Class ;
    rdfs:comment """Contains parameters for the multi-configurational self-consistent-field (MCSCF)
method."""^^xsd:string ;
    rdfs:subClassOf :settings_post_hartree_fock .

:settings_Monte_Carlo a owl:Class ;
    rdfs:comment "Contains parameters that control the Monte-Carlo sampling."^^xsd:string ;
    rdfs:subClassOf :settings_sampling .

:settings_barostat a owl:Class ;
    rdfs:comment "Contains parameters controlling the barostat in a molecular dynamics calculation."^^xsd:string ;
    rdfs:subClassOf :settings_molecular_dynamics .

:settings_constraint a owl:Class ;
    rdfs:comment "Some parameters that describe a constraint"^^xsd:string ;
    rdfs:subClassOf :NMI_category .

:settings_coupled_cluster a owl:Class ;
    rdfs:comment "Contains parameters for the coupled-cluster method (CC) in the post Hartree-Fock step."^^xsd:string ;
    rdfs:subClassOf :settings_post_hartree_fock .

:settings_integrator a owl:Class ;
    rdfs:comment "Contains parameters that control the molecular dynamics (MD) integrator."^^xsd:string ;
    rdfs:subClassOf :settings_molecular_dynamics .

:settings_interaction a owl:Class ;
    rdfs:comment "Some parameters that describe a bonded interaction."^^xsd:string ;
    rdfs:subClassOf :NMI_category .

:settings_metadynamics a owl:Class ;
    rdfs:comment "Contains parameters that control the metadynamics sampling."^^xsd:string ;
    rdfs:subClassOf :settings_sampling .

:settings_moller_plesset_perturbation_theory a owl:Class ;
    rdfs:comment "Contains parameters for Møller–Plesset perturbation theory."^^xsd:string ;
    rdfs:subClassOf :settings_post_hartree_fock .

:settings_multi_reference a owl:Class ;
    rdfs:comment """Contains parameters for the multi-reference single and double configuration
interaction method."""^^xsd:string ;
    rdfs:subClassOf :settings_post_hartree_fock .

:settings_run a owl:Class ;
    rdfs:comment """Contains parameters that control the whole run (but not the *single configuration
calculation*, see section_single_configuration_calculation)."""^^xsd:string ;
    rdfs:subClassOf :NMI_category .

:settings_thermostat a owl:Class ;
    rdfs:comment """Contains parameters that control the thermostat in the molecular dynamics (MD)
calculations."""^^xsd:string ;
    rdfs:subClassOf :settings_molecular_dynamics .

:NOMADEntry a owl:Class ;
    rdfs:subClassOf owl:Thing .

:SC_matrix a owl:Class ;
    rdfs:comment """Specifies the matrix that transforms the unit-cell into the super-cell in which
the actual calculation is performed."""^^xsd:string ;
    rdfs:subClassOf [ a owl:Restriction ;
            owl:hasValue 3 ;
            owl:onProperty :hasFixDim2 ],
        [ a owl:Restriction ;
            owl:allValuesFrom <http://emmo.info/emmo/middle/math#EMMO_f8bd64d5_5d3e_4ad4_a46e_c30714fecb7f> ;
            owl:onProperty :hasDatatype ],
        [ a owl:Restriction ;
            owl:hasValue 2 ;
            owl:onProperty :hasNumberOfDimensions ],
        [ a owl:Restriction ;
            owl:hasValue 3 ;
            owl:onProperty :hasFixDim1 ],
        :NMI_quantity .

:XC_functional a owl:Class ;
    rdfs:comment """This value describes a DFT exchange-correlation (XC) functional used for
evaluating the energy value stored in energy_XC_functional and related quantities
(e.g., forces).

It is a unique short name obtained by combining the data stored in
section_XC_functionals, more specifically by combining different
XC_functional_name as described in the [XC_functional wiki
page](https://gitlab.mpcdf.mpg.de/nomad-lab/nomad-meta-info/wikis/metainfo/XC-
functional)."""^^xsd:string ;
    rdfs:subClassOf [ a owl:Restriction ;
            owl:onProperty :hasCategory ;
            owl:someValuesFrom :settings_XC ],
        [ a owl:Restriction ;
            owl:onProperty :hasCategory ;
            owl:someValuesFrom :settings_XC_functional ],
        [ a owl:Restriction ;
            owl:allValuesFrom <http://emmo.info/emmo/middle/perceptual#EMMO_50ea1ec5_f157_41b0_b46b_a9032f17ca10> ;
            owl:onProperty :hasDatatype ],
        [ a owl:Restriction ;
            owl:onProperty :hasCategory ;
            owl:someValuesFrom :settings_physical_parameter ],
        [ a owl:Restriction ;
            owl:hasValue 0 ;
            owl:onProperty :hasNumberOfDimensions ],
        [ a owl:Restriction ;
            owl:onProperty :hasCategory ;
            owl:someValuesFrom :settings_potential_energy_surface ],
        :NMI_quantity .

:XC_functional_name a owl:Class ;
    rdfs:comment """Provides the name of one of the exchange and/or correlation (XC) functionals
combined in XC_functional.

The valid unique names that can be used are listed in the [XC_functional wiki
page](https://gitlab.mpcdf.mpg.de/nomad-lab/nomad-meta-info/wikis/metainfo/XC-
functional).

*NOTE*: This value should refer to a correlation, an exchange or an exchange-
correlation functional only."""^^xsd:string ;
    rdfs:subClassOf [ a owl:Restriction ;
            owl:hasValue 0 ;
            owl:onProperty :hasNumberOfDimensions ],
        [ a owl:Restriction ;
            owl:allValuesFrom <http://emmo.info/emmo/middle/perceptual#EMMO_50ea1ec5_f157_41b0_b46b_a9032f17ca10> ;
            owl:onProperty :hasDatatype ],
        [ a owl:Restriction ;
            owl:onProperty :hasCategory ;
            owl:someValuesFrom :settings_physical_parameter ],
        :NMI_quantity .

:XC_functional_parameters a owl:Class ;
    rdfs:comment """Contains an associative list of non-default values of the parameters for the
functional declared in XC_functional_name of the section_XC_functionals section.

For example, if a calculations using a hybrid XC functional (e.g., HSE06)
specifies a user-given value of the mixing parameter between exact and GGA
exchange, then this non-default value is stored in this metadata.

The labels and units of these values are defined in the paragraph dedicated to the
specified functional declared in XC_functional_name of the [XC_functional wiki
page](https://gitlab.mpcdf.mpg.de/nomad-lab/nomad-meta-info/wikis/metainfo/XC-
functional).

If this metadata is not given, the default parameter values for the
XC_functional_name are assumed."""^^xsd:string ;
    rdfs:subClassOf [ a owl:Restriction ;
            owl:onProperty :hasCategory ;
            owl:someValuesFrom :settings_physical_parameter ],
        [ a owl:Restriction ;
            owl:hasValue 0 ;
            owl:onProperty :hasNumberOfDimensions ],
        :NMI_quantity .

:XC_functional_weight a owl:Class ;
    rdfs:comment """Provides the value of the weight for the exchange, correlation, or exchange-
correlation functional declared in XC_functional_name (see
section_XC_functionals).

This weight is used in the linear combination of the different XC functional names
(XC_functional_name) in different section_XC_functionals sections to form the
XC_functional used for evaluating energy_XC_functional and related quantities.

If not specified then the default is set to 1."""^^xsd:string ;
    rdfs:subClassOf [ a owl:Restriction ;
            owl:onProperty :hasCategory ;
            owl:someValuesFrom :settings_physical_parameter ],
        [ a owl:Restriction ;
            owl:allValuesFrom <http://emmo.info/emmo/middle/math#EMMO_18d180e4_5e3e_42f7_820c_e08951223486> ;
            owl:onProperty :hasDatatype ],
        [ a owl:Restriction ;
            owl:hasValue 0 ;
            owl:onProperty :hasNumberOfDimensions ],
        :NMI_quantity .

:XC_method a owl:Class ;
    rdfs:comment """Describes the exchange correlation (XC) method used for evaluating the XC energy
(energy_XC). Differently from XC_functional, perturbative treatments are also
accounted for, where the string contains the reference to both the perturbative
(e.g., MP2) and the starting point (e.g, Hartree-Fock) XC method defined in the
section section_method.

The value consists of XC_method_current concatenated with the `@` character and
the XC method (XC_method) defined in section_method that is referred to by
method_to_method_ref where method_to_method_kind = "starting_point_method"."""^^xsd:string ;
    rdfs:subClassOf [ a owl:Restriction ;
            owl:hasValue 0 ;
            owl:onProperty :hasNumberOfDimensions ],
        [ a owl:Restriction ;
            owl:onProperty :hasCategory ;
            owl:someValuesFrom :settings_potential_energy_surface ],
        [ a owl:Restriction ;
            owl:allValuesFrom <http://emmo.info/emmo/middle/perceptual#EMMO_50ea1ec5_f157_41b0_b46b_a9032f17ca10> ;
            owl:onProperty :hasDatatype ],
        [ a owl:Restriction ;
            owl:onProperty :hasCategory ;
            owl:someValuesFrom :settings_XC ],
        :NMI_quantity .

:XC_method_current a owl:Class ;
    rdfs:comment """Identifies the exchange correlation (XC) method used for energy_XC and related
quantities in a standardized short form as a string.

It is built by joining the values in the following order using the underscore `_`
character: electronic_structure_method, XC_functional,
self_interaction_correction_method, van_der_Waals_method and relativity_method.

If any of the methods listed in the string contain non-standard settings, then the
first 10 characters of the Base64 URL encoding of SHA 512 checksum of a normalized
JSON with all non-redundant non-derived settings_XC are appended to the the string
preceded by an underscore.

With empty strings, the underscore `_` character is skipped.

If the method defined in the section_method section is perturbative, the
XC_method_current contains only the perturbative method, not the starting point
(e.g. the DFT XC functional used as a starting point for a RPA perturbative
calculation). In this case, the string that contains both the perturbative and
starting point method is stored in XC_method."""^^xsd:string ;
    rdfs:subClassOf [ a owl:Restriction ;
            owl:hasValue 0 ;
            owl:onProperty :hasNumberOfDimensions ],
        [ a owl:Restriction ;
            owl:onProperty :hasCategory ;
            owl:someValuesFrom :settings_potential_energy_surface ],
        [ a owl:Restriction ;
            owl:onProperty :hasCategory ;
            owl:someValuesFrom :settings_XC ],
        [ a owl:Restriction ;
            owl:allValuesFrom <http://emmo.info/emmo/middle/perceptual#EMMO_50ea1ec5_f157_41b0_b46b_a9032f17ca10> ;
            owl:onProperty :hasDatatype ],
        :NMI_quantity .

:atom_atom_number a owl:Class ;
    rdfs:comment "Atomic number Z of the atom."^^xsd:string ;
    rdfs:subClassOf [ a owl:Restriction ;
            owl:hasValue 1 ;
            owl:onProperty :hasNumberOfDimensions ],
        [ a owl:Restriction ;
            owl:hasValue :number_of_sites ;
            owl:onProperty :hasVarDim1 ],
        [ a owl:Restriction ;
            owl:allValuesFrom <http://emmo.info/emmo/middle/math#EMMO_f8bd64d5_5d3e_4ad4_a46e_c30714fecb7f> ;
            owl:onProperty :hasDatatype ],
        :NMI_quantity .

:atom_concentrations a owl:Class ;
    rdfs:comment """concentration of the atom species in a variable composition, by default it should
be considered an array of ones. Summing these should give the number_of_sites"""^^xsd:string ;
    rdfs:subClassOf [ a owl:Restriction ;
            owl:hasValue 1 ;
            owl:onProperty :hasNumberOfDimensions ],
        [ a owl:Restriction ;
            owl:hasValue :number_of_atoms ;
            owl:onProperty :hasVarDim1 ],
        [ a owl:Restriction ;
            owl:allValuesFrom <http://emmo.info/emmo/middle/math#EMMO_18d180e4_5e3e_42f7_820c_e08951223486> ;
            owl:onProperty :hasDatatype ],
        :NMI_quantity .

:atom_forces a owl:Class ;
    rdfs:comment """Forces acting on the atoms, calculated as minus gradient of energy_total,
**including** constraints, if present. The derivatives with respect to
displacements of nuclei are evaluated in Cartesian coordinates. In addition, these
forces are obtained by filtering out the unitary transformations (center-of-mass
translations and rigid rotations for non-periodic systems, see
atom_forces_free_raw for the unfiltered counterpart). Forces due to constraints
such as fixed atoms, distances, angles, dihedrals, etc. are included (see
atom_forces_raw for the unfiltered counterpart)."""^^xsd:string ;
    rdfs:subClassOf [ a owl:Restriction ;
            owl:hasValue 2 ;
            owl:onProperty :hasNumberOfDimensions ],
        [ a owl:Restriction ;
            owl:allValuesFrom <http://emmo.info/emmo/middle/math#EMMO_18d180e4_5e3e_42f7_820c_e08951223486> ;
            owl:onProperty :hasDatatype ],
        [ a owl:Restriction ;
            owl:hasValue 3 ;
            owl:onProperty :hasFixDim2 ],
        [ a owl:Restriction ;
            owl:hasValue :number_of_atoms ;
            owl:onProperty :hasVarDim1 ],
        [ a owl:Restriction ;
            owl:allValuesFrom <http://emmo.info/emmo/middle/siunits#EMMO_a979c531_f9fa_4a6e_93c1.0.0-alpha2960241ca6> ;
            owl:onProperty <http://emmo.info/emmo/middle/metrology#EMMO_67fc0a36_8dcb_4ffa_9a43_31074efa3296> ],
        [ a owl:Restriction ;
            owl:onProperty :hasCategory ;
            owl:someValuesFrom :atom_forces_type ],
        :NMI_quantity .

:atom_forces_T0 a owl:Class ;
    rdfs:comment """Forces acting on the atoms, calculated as minus gradient of energy_total_T0,
**including** constraints, if present. The derivatives with respect to
displacements of the nuclei are evaluated in Cartesian coordinates. In addition,
these forces are obtained by filtering out the unitary transformations (center-of-
mass translations and rigid rotations for non-periodic systems, see
atom_forces_free_T0_raw for the unfiltered counterpart). Forces due to constraints
such as fixed atoms, distances, angles, dihedrals, etc. are also included (see
atom_forces_free_T0_raw for the unfiltered counterpart)."""^^xsd:string ;
    rdfs:subClassOf [ a owl:Restriction ;
            owl:onProperty :hasCategory ;
            owl:someValuesFrom :atom_forces_type ],
        [ a owl:Restriction ;
            owl:hasValue :number_of_atoms ;
            owl:onProperty :hasVarDim1 ],
        [ a owl:Restriction ;
            owl:allValuesFrom <http://emmo.info/emmo/middle/math#EMMO_18d180e4_5e3e_42f7_820c_e08951223486> ;
            owl:onProperty :hasDatatype ],
        [ a owl:Restriction ;
            owl:hasValue 2 ;
            owl:onProperty :hasNumberOfDimensions ],
        [ a owl:Restriction ;
            owl:hasValue 3 ;
            owl:onProperty :hasFixDim2 ],
        [ a owl:Restriction ;
            owl:allValuesFrom <http://emmo.info/emmo/middle/siunits#EMMO_a979c531_f9fa_4a6e_93c1.0.0-alpha2960241ca6> ;
            owl:onProperty <http://emmo.info/emmo/middle/metrology#EMMO_67fc0a36_8dcb_4ffa_9a43_31074efa3296> ],
        :NMI_quantity .

:atom_forces_T0_raw a owl:Class ;
    rdfs:comment """Forces acting on the atoms, calculated as minus gradient of energy_total_T0,
**without** constraints. The derivatives with respect to displacements of the
nuclei are evaluated in Cartesian coordinates. These forces may contain unitary
transformations (center-of-mass translations and rigid rotations for non-periodic
systems) that are normally filtered separately (see atom_forces_T0 for the
filtered counterpart). Forces due to constraints such as fixed atoms, distances,
angles, dihedrals, etc. are also considered separately (see atom_forces_T0 for the
filtered counterpart)."""^^xsd:string ;
    rdfs:subClassOf [ a owl:Restriction ;
            owl:hasValue 2 ;
            owl:onProperty :hasNumberOfDimensions ],
        [ a owl:Restriction ;
            owl:onProperty :hasCategory ;
            owl:someValuesFrom :atom_forces_type ],
        [ a owl:Restriction ;
            owl:hasValue :number_of_atoms ;
            owl:onProperty :hasVarDim1 ],
        [ a owl:Restriction ;
            owl:allValuesFrom <http://emmo.info/emmo/middle/math#EMMO_18d180e4_5e3e_42f7_820c_e08951223486> ;
            owl:onProperty :hasDatatype ],
        [ a owl:Restriction ;
            owl:allValuesFrom <http://emmo.info/emmo/middle/siunits#EMMO_a979c531_f9fa_4a6e_93c1.0.0-alpha2960241ca6> ;
            owl:onProperty <http://emmo.info/emmo/middle/metrology#EMMO_67fc0a36_8dcb_4ffa_9a43_31074efa3296> ],
        [ a owl:Restriction ;
            owl:hasValue 3 ;
            owl:onProperty :hasFixDim2 ],
        :NMI_quantity .

:atom_forces_free a owl:Class ;
    rdfs:comment """Forces acting on the atoms, calculated as minus gradient of energy_free,
**including** constraints, if present. The derivatives with respect to
displacements of the nuclei are evaluated in Cartesian coordinates. The
(electronic) energy_free contains the information on the change in (fractional)
occupation of the electronic eigenstates, which are accounted for in the
derivatives, yielding a truly energy-conserved quantity. In addition, these forces
are obtained by filtering out the unitary transformations (center-of-mass
translations and rigid rotations for non-periodic systems, see
atom_forces_free_raw for the unfiltered counterpart). Forces due to constraints
such as fixed atoms, distances, angles, dihedrals, etc. are included (see
atom_forces_free_raw for the unfiltered counterpart)."""^^xsd:string ;
    rdfs:subClassOf [ a owl:Restriction ;
            owl:hasValue 3 ;
            owl:onProperty :hasFixDim2 ],
        [ a owl:Restriction ;
            owl:hasValue 2 ;
            owl:onProperty :hasNumberOfDimensions ],
        [ a owl:Restriction ;
            owl:allValuesFrom <http://emmo.info/emmo/middle/siunits#EMMO_a979c531_f9fa_4a6e_93c1.0.0-alpha2960241ca6> ;
            owl:onProperty <http://emmo.info/emmo/middle/metrology#EMMO_67fc0a36_8dcb_4ffa_9a43_31074efa3296> ],
        [ a owl:Restriction ;
            owl:onProperty :hasCategory ;
            owl:someValuesFrom :atom_forces_type ],
        [ a owl:Restriction ;
            owl:allValuesFrom <http://emmo.info/emmo/middle/math#EMMO_18d180e4_5e3e_42f7_820c_e08951223486> ;
            owl:onProperty :hasDatatype ],
        [ a owl:Restriction ;
            owl:hasValue :number_of_atoms ;
            owl:onProperty :hasVarDim1 ],
        :NMI_quantity .

:atom_forces_free_raw a owl:Class ;
    rdfs:comment """Forces acting on the atoms, calculated as minus gradient of energy_free,
**without** constraints. The derivatives with respect to displacements of nuclei
are evaluated in Cartesian coordinates. The (electronic) energy_free contains the
change in (fractional) occupation of the electronic eigenstates, which are
accounted for in the derivatives, yielding a truly energy-conserved quantity.
These forces may contain unitary transformations (center-of-mass translations and
rigid rotations for non-periodic systems) that are normally filtered separately
(see atom_forces_free for the filtered counterpart). Forces due to constraints
such as fixed atoms, distances, angles, dihedrals, etc. are also considered
separately (see atom_forces_free for the filtered counterpart)."""^^xsd:string ;
    rdfs:subClassOf [ a owl:Restriction ;
            owl:allValuesFrom <http://emmo.info/emmo/middle/math#EMMO_18d180e4_5e3e_42f7_820c_e08951223486> ;
            owl:onProperty :hasDatatype ],
        [ a owl:Restriction ;
            owl:onProperty :hasCategory ;
            owl:someValuesFrom :atom_forces_type ],
        [ a owl:Restriction ;
            owl:hasValue 2 ;
            owl:onProperty :hasNumberOfDimensions ],
        [ a owl:Restriction ;
            owl:allValuesFrom <http://emmo.info/emmo/middle/siunits#EMMO_a979c531_f9fa_4a6e_93c1.0.0-alpha2960241ca6> ;
            owl:onProperty <http://emmo.info/emmo/middle/metrology#EMMO_67fc0a36_8dcb_4ffa_9a43_31074efa3296> ],
        [ a owl:Restriction ;
            owl:hasValue 3 ;
            owl:onProperty :hasFixDim2 ],
        [ a owl:Restriction ;
            owl:hasValue :number_of_atoms ;
            owl:onProperty :hasVarDim1 ],
        :NMI_quantity .

:atom_forces_raw a owl:Class ;
    rdfs:comment """Forces acting on the atoms, calculated as minus gradient of energy_total,
**without** constraints. The derivatives with respect to displacements of the
nuclei are evaluated in Cartesian coordinates. These forces may contain unitary
transformations (center-of-mass translations and rigid rotations for non-periodic
systems) that are normally filtered separately (see atom_forces for the filtered
counterpart). Forces due to constraints such as fixed atoms, distances, angles,
dihedrals, etc. are also considered separately (see atom_forces for the filtered
counterpart)."""^^xsd:string ;
    rdfs:subClassOf [ a owl:Restriction ;
            owl:onProperty :hasCategory ;
            owl:someValuesFrom :atom_forces_type ],
        [ a owl:Restriction ;
            owl:allValuesFrom <http://emmo.info/emmo/middle/siunits#EMMO_a979c531_f9fa_4a6e_93c1.0.0-alpha2960241ca6> ;
            owl:onProperty <http://emmo.info/emmo/middle/metrology#EMMO_67fc0a36_8dcb_4ffa_9a43_31074efa3296> ],
        [ a owl:Restriction ;
            owl:hasValue 2 ;
            owl:onProperty :hasNumberOfDimensions ],
        [ a owl:Restriction ;
            owl:hasValue 3 ;
            owl:onProperty :hasFixDim2 ],
        [ a owl:Restriction ;
            owl:allValuesFrom <http://emmo.info/emmo/middle/math#EMMO_18d180e4_5e3e_42f7_820c_e08951223486> ;
            owl:onProperty :hasDatatype ],
        [ a owl:Restriction ;
            owl:hasValue :number_of_atoms ;
            owl:onProperty :hasVarDim1 ],
        :NMI_quantity .

:atom_in_molecule_charge a owl:Class ;
    rdfs:comment "Charge of each atom in the molecule."^^xsd:string ;
    rdfs:subClassOf [ a owl:Restriction ;
            owl:allValuesFrom <http://emmo.info/emmo/middle/math#EMMO_18d180e4_5e3e_42f7_820c_e08951223486> ;
            owl:onProperty :hasDatatype ],
        [ a owl:Restriction ;
            owl:allValuesFrom <http://emmo.info/emmo/middle/siunits#EMMO_696ed548_9477_45ea_993c_6a8f5271914a> ;
            owl:onProperty <http://emmo.info/emmo/middle/metrology#EMMO_67fc0a36_8dcb_4ffa_9a43_31074efa3296> ],
        [ a owl:Restriction ;
            owl:hasValue 1 ;
            owl:onProperty :hasNumberOfDimensions ],
        [ a owl:Restriction ;
            owl:hasValue :number_of_atoms_in_molecule ;
            owl:onProperty :hasVarDim1 ],
        [ a owl:Restriction ;
            owl:onProperty :hasCategory ;
            owl:someValuesFrom :settings_atom_in_molecule ],
        :NMI_quantity .

:atom_in_molecule_name a owl:Class ;
    rdfs:comment "Name (label) of each atom in the molecule."^^xsd:string ;
    rdfs:subClassOf [ a owl:Restriction ;
            owl:allValuesFrom <http://emmo.info/emmo/middle/perceptual#EMMO_50ea1ec5_f157_41b0_b46b_a9032f17ca10> ;
            owl:onProperty :hasDatatype ],
        [ a owl:Restriction ;
            owl:onProperty :hasCategory ;
            owl:someValuesFrom :settings_atom_in_molecule ],
        [ a owl:Restriction ;
            owl:hasValue 1 ;
            owl:onProperty :hasNumberOfDimensions ],
        [ a owl:Restriction ;
            owl:hasValue :number_of_atoms_in_molecule ;
            owl:onProperty :hasVarDim1 ],
        :NMI_quantity .

:atom_in_molecule_to_atom_type_ref a owl:Class ;
    rdfs:comment "Reference to the atom type of each atom in the molecule."^^xsd:string ;
    rdfs:subClassOf [ a owl:Restriction ;
            owl:onProperty :hasCategory ;
            owl:someValuesFrom :settings_atom_in_molecule ],
        [ a owl:Restriction ;
            owl:hasValue 1 ;
            owl:onProperty :hasNumberOfDimensions ],
        [ a owl:Restriction ;
            owl:hasValue :number_of_atoms_in_molecule ;
            owl:onProperty :hasVarDim1 ],
        :NMI_quantity .

:atom_labels a owl:Class ;
    rdfs:comment """Labels of the atoms. These strings identify the atom kind and conventionally start
with the symbol of the atomic species, possibly followed by the atomic number. The
same atomic species can be labeled with more than one atom_labels in order to
distinguish, e.g., atoms of the same species assigned to different atom-centered
basis sets or pseudo-potentials, or simply atoms in different locations in the
structure (e.g., bulk and surface). These labels can also be used for *particles*
that do not correspond to physical atoms (e.g., ghost atoms in some codes using
atom-centered basis sets). This metadata defines a configuration and is therefore
required."""^^xsd:string ;
    rdfs:subClassOf [ a owl:Restriction ;
            owl:hasValue :number_of_atoms ;
            owl:onProperty :hasVarDim1 ],
        [ a owl:Restriction ;
            owl:allValuesFrom <http://emmo.info/emmo/middle/perceptual#EMMO_50ea1ec5_f157_41b0_b46b_a9032f17ca10> ;
            owl:onProperty :hasDatatype ],
        [ a owl:Restriction ;
            owl:hasValue 1 ;
            owl:onProperty :hasNumberOfDimensions ],
        [ a owl:Restriction ;
            owl:onProperty :hasCategory ;
            owl:someValuesFrom :configuration_core ],
        :NMI_quantity .

:atom_positions a owl:Class ;
    rdfs:comment """Positions of all the atoms, in Cartesian coordinates. This metadata defines a
configuration and is therefore required. For alloys where concentrations of
species are given for each site in the unit cell, it stores the position of the
sites."""^^xsd:string ;
    rdfs:subClassOf [ a owl:Restriction ;
            owl:hasValue :number_of_atoms ;
            owl:onProperty :hasVarDim1 ],
        [ a owl:Restriction ;
            owl:onProperty :hasCategory ;
            owl:someValuesFrom :configuration_core ],
        [ a owl:Restriction ;
            owl:allValuesFrom <http://emmo.info/emmo/middle/siunits#EMMO_7db11dbf_a643_464a_9b56_07eabcc3e9c5> ;
            owl:onProperty <http://emmo.info/emmo/middle/metrology#EMMO_67fc0a36_8dcb_4ffa_9a43_31074efa3296> ],
        [ a owl:Restriction ;
            owl:allValuesFrom <http://emmo.info/emmo/middle/math#EMMO_18d180e4_5e3e_42f7_820c_e08951223486> ;
            owl:onProperty :hasDatatype ],
        [ a owl:Restriction ;
            owl:hasValue 2 ;
            owl:onProperty :hasNumberOfDimensions ],
        [ a owl:Restriction ;
            owl:hasValue 3 ;
            owl:onProperty :hasFixDim2 ],
        :NMI_quantity .

:atom_positions_primitive a owl:Class ;
    rdfs:comment "Atom positions in the primitive cell in reduced units."^^xsd:string ;
    rdfs:subClassOf [ a owl:Restriction ;
            owl:hasValue 2 ;
            owl:onProperty :hasNumberOfDimensions ],
        [ a owl:Restriction ;
            owl:hasValue :number_of_atoms_primitive ;
            owl:onProperty :hasVarDim1 ],
        [ a owl:Restriction ;
            owl:hasValue 3 ;
            owl:onProperty :hasFixDim2 ],
        [ a owl:Restriction ;
            owl:allValuesFrom <http://emmo.info/emmo/middle/math#EMMO_18d180e4_5e3e_42f7_820c_e08951223486> ;
            owl:onProperty :hasDatatype ],
        :NMI_quantity .

:atom_positions_std a owl:Class ;
    rdfs:comment "Standardized atom positions in reduced units."^^xsd:string ;
    rdfs:subClassOf [ a owl:Restriction ;
            owl:hasValue 3 ;
            owl:onProperty :hasFixDim2 ],
        [ a owl:Restriction ;
            owl:hasValue 2 ;
            owl:onProperty :hasNumberOfDimensions ],
        [ a owl:Restriction ;
            owl:allValuesFrom <http://emmo.info/emmo/middle/math#EMMO_18d180e4_5e3e_42f7_820c_e08951223486> ;
            owl:onProperty :hasDatatype ],
        [ a owl:Restriction ;
            owl:hasValue :number_of_atoms_std ;
            owl:onProperty :hasVarDim1 ],
        :NMI_quantity .

:atom_projected_dos_energies a owl:Class ;
    rdfs:comment """Array containing the set of discrete energy values for the atom-projected density
(electronic-energy) of states (DOS)."""^^xsd:string ;
    rdfs:subClassOf [ a owl:Restriction ;
            owl:hasValue :number_of_atom_projected_dos_values ;
            owl:onProperty :hasVarDim1 ],
        [ a owl:Restriction ;
            owl:allValuesFrom <http://emmo.info/emmo/middle/math#EMMO_18d180e4_5e3e_42f7_820c_e08951223486> ;
            owl:onProperty :hasDatatype ],
        [ a owl:Restriction ;
            owl:allValuesFrom <http://emmo.info/emmo/middle/siunits#EMMO_8a70dea4_d6ab_4260_b931_a3e990982416> ;
            owl:onProperty <http://emmo.info/emmo/middle/metrology#EMMO_67fc0a36_8dcb_4ffa_9a43_31074efa3296> ],
        [ a owl:Restriction ;
            owl:hasValue 1 ;
            owl:onProperty :hasNumberOfDimensions ],
        :NMI_quantity .

:atom_projected_dos_lm a owl:Class ;
    rdfs:comment """Tuples of $l$ and $m$ values for which atom_projected_dos_values_lm are given. For
the quantum number $l$ the conventional meaning of azimuthal quantum number is
always adopted. For the integer number $m$, besides the conventional use as
magnetic quantum number ($l+1$ integer values from $-l$ to $l$), a set of
different conventions is accepted (see the [m_kind wiki
page](https://gitlab.rzg.mpg.de/nomad-lab/nomad-meta-info/wikis/metainfo/m-kind).
The adopted convention is specified by atom_projected_dos_m_kind."""^^xsd:string ;
    rdfs:subClassOf [ a owl:Restriction ;
            owl:allValuesFrom <http://emmo.info/emmo/middle/math#EMMO_f8bd64d5_5d3e_4ad4_a46e_c30714fecb7f> ;
            owl:onProperty :hasDatatype ],
        [ a owl:Restriction ;
            owl:hasValue 2 ;
            owl:onProperty :hasFixDim2 ],
        [ a owl:Restriction ;
            owl:hasValue :number_of_lm_atom_projected_dos ;
            owl:onProperty :hasVarDim1 ],
        [ a owl:Restriction ;
            owl:hasValue 2 ;
            owl:onProperty :hasNumberOfDimensions ],
        :NMI_quantity .

:atom_projected_dos_m_kind a owl:Class ;
    rdfs:comment """String describing what the integer numbers of $m$ in atom_projected_dos_lm mean.
The allowed values are listed in the [m_kind wiki
page](https://gitlab.rzg.mpg.de/nomad-lab/nomad-meta-info/wikis/metainfo/m-kind)."""^^xsd:string ;
    rdfs:subClassOf [ a owl:Restriction ;
            owl:allValuesFrom <http://emmo.info/emmo/middle/perceptual#EMMO_50ea1ec5_f157_41b0_b46b_a9032f17ca10> ;
            owl:onProperty :hasDatatype ],
        [ a owl:Restriction ;
            owl:hasValue 0 ;
            owl:onProperty :hasNumberOfDimensions ],
        :NMI_quantity .

:atom_projected_dos_values_lm a owl:Class ;
    rdfs:comment """Values correspond to the number of states for a given energy (the set of discrete
energy values is given in atom_projected_dos_energies) divided into contributions
from each $l,m$ channel for the atom-projected density (electronic-energy) of
states. Here, there are as many atom-projected DOS as the number_of_atoms, the
list of labels of the atoms and their meanings are in atom_labels."""^^xsd:string ;
    rdfs:subClassOf [ a owl:Restriction ;
            owl:hasValue :number_of_atoms ;
            owl:onProperty :hasVarDim3 ],
        [ a owl:Restriction ;
            owl:hasValue :number_of_atom_projected_dos_values ;
            owl:onProperty :hasVarDim4 ],
        [ a owl:Restriction ;
            owl:hasValue :number_of_spin_channels ;
            owl:onProperty :hasVarDim2 ],
        [ a owl:Restriction ;
            owl:hasValue :number_of_lm_atom_projected_dos ;
            owl:onProperty :hasVarDim1 ],
        [ a owl:Restriction ;
            owl:allValuesFrom <http://emmo.info/emmo/middle/math#EMMO_18d180e4_5e3e_42f7_820c_e08951223486> ;
            owl:onProperty :hasDatatype ],
        [ a owl:Restriction ;
            owl:hasValue 4 ;
            owl:onProperty :hasNumberOfDimensions ],
        :NMI_quantity .

:atom_projected_dos_values_total a owl:Class ;
    rdfs:comment """Values correspond to the number of states for a given energy (the set of discrete
energy values is given in atom_projected_dos_energies) divided into contributions
summed up over all $l$ channels for the atom-projected density (electronic-energy)
of states (DOS). Here, there are as many atom-projected DOS as the
number_of_atoms, the list of labels of the atoms and their meanings are in
atom_labels."""^^xsd:string ;
    rdfs:subClassOf [ a owl:Restriction ;
            owl:hasValue :number_of_spin_channels ;
            owl:onProperty :hasVarDim1 ],
        [ a owl:Restriction ;
            owl:hasValue :number_of_atoms ;
            owl:onProperty :hasVarDim2 ],
        [ a owl:Restriction ;
            owl:allValuesFrom <http://emmo.info/emmo/middle/math#EMMO_18d180e4_5e3e_42f7_820c_e08951223486> ;
            owl:onProperty :hasDatatype ],
        [ a owl:Restriction ;
            owl:hasValue 3 ;
            owl:onProperty :hasNumberOfDimensions ],
        [ a owl:Restriction ;
            owl:hasValue :number_of_atom_projected_dos_values ;
            owl:onProperty :hasVarDim3 ],
        :NMI_quantity .

:atom_species a owl:Class ;
    rdfs:comment """Species of the atom (normally the atomic number Z, 0 or negative for unidentifed
species or particles that are not atoms."""^^xsd:string ;
    rdfs:subClassOf [ a owl:Restriction ;
            owl:allValuesFrom <http://emmo.info/emmo/middle/math#EMMO_f8bd64d5_5d3e_4ad4_a46e_c30714fecb7f> ;
            owl:onProperty :hasDatatype ],
        [ a owl:Restriction ;
            owl:hasValue :number_of_atoms ;
            owl:onProperty :hasVarDim1 ],
        [ a owl:Restriction ;
            owl:hasValue 1 ;
            owl:onProperty :hasNumberOfDimensions ],
        :NMI_quantity .

:atom_to_molecule a owl:Class ;
    rdfs:comment """Table mapping atom to molecules: the first column is the index of the molecule and
the second column the index of the atom, signifying that the atom in the second
column belongs to the molecule in the first column in the same row."""^^xsd:string ;
    rdfs:subClassOf [ a owl:Restriction ;
            owl:hasValue :number_of_topology_atoms ;
            owl:onProperty :hasVarDim1 ],
        [ a owl:Restriction ;
            owl:allValuesFrom <http://emmo.info/emmo/middle/math#EMMO_f8bd64d5_5d3e_4ad4_a46e_c30714fecb7f> ;
            owl:onProperty :hasDatatype ],
        [ a owl:Restriction ;
            owl:hasValue 2 ;
            owl:onProperty :hasFixDim2 ],
        [ a owl:Restriction ;
            owl:hasValue 2 ;
            owl:onProperty :hasNumberOfDimensions ],
        :NMI_quantity .

:atom_type_charge a owl:Class ;
    rdfs:comment "Charge of the atom type."^^xsd:string ;
    rdfs:subClassOf [ a owl:Restriction ;
            owl:hasValue 0 ;
            owl:onProperty :hasNumberOfDimensions ],
        [ a owl:Restriction ;
            owl:allValuesFrom <http://emmo.info/emmo/middle/siunits#EMMO_696ed548_9477_45ea_993c_6a8f5271914a> ;
            owl:onProperty <http://emmo.info/emmo/middle/metrology#EMMO_67fc0a36_8dcb_4ffa_9a43_31074efa3296> ],
        [ a owl:Restriction ;
            owl:allValuesFrom <http://emmo.info/emmo/middle/math#EMMO_18d180e4_5e3e_42f7_820c_e08951223486> ;
            owl:onProperty :hasDatatype ],
        :NMI_quantity .

:atom_type_mass a owl:Class ;
    rdfs:comment "Mass of the atom type."^^xsd:string ;
    rdfs:subClassOf [ a owl:Restriction ;
            owl:hasValue 0 ;
            owl:onProperty :hasNumberOfDimensions ],
        [ a owl:Restriction ;
            owl:allValuesFrom <http://emmo.info/emmo/middle/siunits#EMMO_9bfd6f1e_b0ce_459c_beb7_8f1f41708bba> ;
            owl:onProperty <http://emmo.info/emmo/middle/metrology#EMMO_67fc0a36_8dcb_4ffa_9a43_31074efa3296> ],
        [ a owl:Restriction ;
            owl:allValuesFrom <http://emmo.info/emmo/middle/math#EMMO_18d180e4_5e3e_42f7_820c_e08951223486> ;
            owl:onProperty :hasDatatype ],
        :NMI_quantity .

:atom_type_name a owl:Class ;
    rdfs:comment "Name (label) of the atom type."^^xsd:string ;
    rdfs:subClassOf [ a owl:Restriction ;
            owl:hasValue 0 ;
            owl:onProperty :hasNumberOfDimensions ],
        [ a owl:Restriction ;
            owl:allValuesFrom <http://emmo.info/emmo/middle/perceptual#EMMO_50ea1ec5_f157_41b0_b46b_a9032f17ca10> ;
            owl:onProperty :hasDatatype ],
        :NMI_quantity .

:atom_velocities a owl:Class ;
    rdfs:comment """Velocities of the nuclei, defined as the change in Cartesian coordinates of the
nuclei with respect to time."""^^xsd:string ;
    rdfs:subClassOf [ a owl:Restriction ;
            owl:allValuesFrom <https://nomad-coe.eu/ontology/properties#MetrePerSecond> ;
            owl:onProperty <http://emmo.info/emmo/middle/metrology#EMMO_67fc0a36_8dcb_4ffa_9a43_31074efa3296> ],
        [ a owl:Restriction ;
            owl:hasValue 3 ;
            owl:onProperty :hasFixDim2 ],
        [ a owl:Restriction ;
            owl:allValuesFrom <http://emmo.info/emmo/middle/math#EMMO_18d180e4_5e3e_42f7_820c_e08951223486> ;
            owl:onProperty :hasDatatype ],
        [ a owl:Restriction ;
            owl:hasValue :number_of_atoms ;
            owl:onProperty :hasVarDim1 ],
        [ a owl:Restriction ;
            owl:hasValue 2 ;
            owl:onProperty :hasNumberOfDimensions ],
        :NMI_quantity .

:atomic_multipole_kind a owl:Class ;
    rdfs:comment """String describing the method used to obtain the electrostatic multipoles
(including the electric charge, dipole, etc.) for each atom. Such multipoles
require a charge-density partitioning scheme, specified by the value of this
metadata. Allowed values are listed in the [atomic_multipole_kind wiki
page](https://gitlab.mpcdf.mpg.de/nomad-lab/nomad-meta-info/wikis/metainfo/atomic-
multipole-kind)."""^^xsd:string ;
    rdfs:subClassOf [ a owl:Restriction ;
            owl:hasValue 0 ;
            owl:onProperty :hasNumberOfDimensions ],
        [ a owl:Restriction ;
            owl:allValuesFrom <http://emmo.info/emmo/middle/perceptual#EMMO_50ea1ec5_f157_41b0_b46b_a9032f17ca10> ;
            owl:onProperty :hasDatatype ],
        :NMI_quantity .

:atomic_multipole_lm a owl:Class ;
    rdfs:comment """Tuples of $l$ and $m$ values for which the atomic multipoles (including the
electric charge, dipole, etc.) are given. The method used to obtain the multipoles
is specified by atomic_multipole_kind. The meaning of the integer number $l$ is
monopole/charge for $l=0$, dipole for $l=1$, quadrupole for $l=2$, etc. The
meaning of the integer numbers $m$ is specified by atomic_multipole_m_kind."""^^xsd:string ;
    rdfs:subClassOf [ a owl:Restriction ;
            owl:hasValue 2 ;
            owl:onProperty :hasFixDim2 ],
        [ a owl:Restriction ;
            owl:hasValue :number_of_lm_atomic_multipoles ;
            owl:onProperty :hasVarDim1 ],
        [ a owl:Restriction ;
            owl:allValuesFrom <http://emmo.info/emmo/middle/math#EMMO_f8bd64d5_5d3e_4ad4_a46e_c30714fecb7f> ;
            owl:onProperty :hasDatatype ],
        [ a owl:Restriction ;
            owl:hasValue 2 ;
            owl:onProperty :hasNumberOfDimensions ],
        :NMI_quantity .

:atomic_multipole_m_kind a owl:Class ;
    rdfs:comment """String describing the definition for each integer number $m$ in
atomic_multipole_lm. Allowed values are listed in the [m_kind wiki
page](https://gitlab.rzg.mpg.de/nomad-lab/nomad-meta-info/wikis/metainfo/m-kind)."""^^xsd:string ;
    rdfs:subClassOf [ a owl:Restriction ;
            owl:allValuesFrom <http://emmo.info/emmo/middle/perceptual#EMMO_50ea1ec5_f157_41b0_b46b_a9032f17ca10> ;
            owl:onProperty :hasDatatype ],
        [ a owl:Restriction ;
            owl:hasValue 0 ;
            owl:onProperty :hasNumberOfDimensions ],
        :NMI_quantity .

:atomic_multipole_values a owl:Class ;
    rdfs:comment """Value of the multipoles (including the monopole/charge for $l$ = 0, the dipole for
$l$ = 1, etc.) for each atom, calculated as described in atomic_multipole_kind."""^^xsd:string ;
    rdfs:subClassOf [ a owl:Restriction ;
            owl:allValuesFrom <http://emmo.info/emmo/middle/math#EMMO_18d180e4_5e3e_42f7_820c_e08951223486> ;
            owl:onProperty :hasDatatype ],
        [ a owl:Restriction ;
            owl:hasValue 2 ;
            owl:onProperty :hasNumberOfDimensions ],
        [ a owl:Restriction ;
            owl:hasValue :number_of_lm_atomic_multipoles ;
            owl:onProperty :hasVarDim1 ],
        [ a owl:Restriction ;
            owl:hasValue :number_of_atoms ;
            owl:onProperty :hasVarDim2 ],
        :NMI_quantity .

:atomic_numbers_primitive a owl:Class ;
    rdfs:comment "Atomic numbers in the primitive cell."^^xsd:string ;
    rdfs:subClassOf [ a owl:Restriction ;
            owl:allValuesFrom <http://emmo.info/emmo/middle/math#EMMO_f8bd64d5_5d3e_4ad4_a46e_c30714fecb7f> ;
            owl:onProperty :hasDatatype ],
        [ a owl:Restriction ;
            owl:hasValue 1 ;
            owl:onProperty :hasNumberOfDimensions ],
        [ a owl:Restriction ;
            owl:hasValue :number_of_atoms_primitive ;
            owl:onProperty :hasVarDim1 ],
        :NMI_quantity .

:atomic_numbers_std a owl:Class ;
    rdfs:comment "Atomic numbers of the atoms in the standardized cell."^^xsd:string ;
    rdfs:subClassOf [ a owl:Restriction ;
            owl:allValuesFrom <http://emmo.info/emmo/middle/math#EMMO_f8bd64d5_5d3e_4ad4_a46e_c30714fecb7f> ;
            owl:onProperty :hasDatatype ],
        [ a owl:Restriction ;
            owl:hasValue 1 ;
            owl:onProperty :hasNumberOfDimensions ],
        [ a owl:Restriction ;
            owl:hasValue :number_of_atoms_std ;
            owl:onProperty :hasVarDim1 ],
        :NMI_quantity .

:band_energies a owl:Class ;
    rdfs:comment """$k$-dependent or $q$-dependent  energies of the electronic or vibrational band
segment (electronic/vibrational band structure). This is a third-order tensor,
with one dimension used for the spin channels (1 in case of a vibrational band
structure), one for the $k$ or $q$ points for each segment, and one for the
eigenvalue sequence."""^^xsd:string ;
    rdfs:subClassOf [ a owl:Restriction ;
            owl:allValuesFrom <http://emmo.info/emmo/middle/math#EMMO_18d180e4_5e3e_42f7_820c_e08951223486> ;
            owl:onProperty :hasDatatype ],
        [ a owl:Restriction ;
            owl:hasValue :number_of_band_segment_eigenvalues ;
            owl:onProperty :hasVarDim3 ],
        [ a owl:Restriction ;
            owl:hasValue 3 ;
            owl:onProperty :hasNumberOfDimensions ],
        [ a owl:Restriction ;
            owl:hasValue :number_of_spin_channels ;
            owl:onProperty :hasVarDim1 ],
        [ a owl:Restriction ;
            owl:allValuesFrom <http://emmo.info/emmo/middle/siunits#EMMO_8a70dea4_d6ab_4260_b931_a3e990982416> ;
            owl:onProperty <http://emmo.info/emmo/middle/metrology#EMMO_67fc0a36_8dcb_4ffa_9a43_31074efa3296> ],
        [ a owl:Restriction ;
            owl:hasValue :number_of_k_points_per_segment ;
            owl:onProperty :hasVarDim2 ],
        :NMI_quantity .

:band_energies_normalized a owl:Class ;
    rdfs:comment """$k$-dependent energies of the electronic band segment (electronic band structure)
with respect to the top of the valence band. This is a third-order tensor, with
one dimension used for the spin channels, one for the $k$ points for each segment,
and one for the eigenvalue sequence."""^^xsd:string ;
    rdfs:subClassOf [ a owl:Restriction ;
            owl:hasValue :number_of_spin_channels ;
            owl:onProperty :hasVarDim1 ],
        [ a owl:Restriction ;
            owl:allValuesFrom <http://emmo.info/emmo/middle/math#EMMO_18d180e4_5e3e_42f7_820c_e08951223486> ;
            owl:onProperty :hasDatatype ],
        [ a owl:Restriction ;
            owl:allValuesFrom <http://emmo.info/emmo/middle/siunits#EMMO_8a70dea4_d6ab_4260_b931_a3e990982416> ;
            owl:onProperty <http://emmo.info/emmo/middle/metrology#EMMO_67fc0a36_8dcb_4ffa_9a43_31074efa3296> ],
        [ a owl:Restriction ;
            owl:hasValue :number_of_normalized_k_points_per_segment ;
            owl:onProperty :hasVarDim2 ],
        [ a owl:Restriction ;
            owl:hasValue 3 ;
            owl:onProperty :hasNumberOfDimensions ],
        [ a owl:Restriction ;
            owl:hasValue :number_of_normalized_band_segment_eigenvalues ;
            owl:onProperty :hasVarDim3 ],
        :NMI_quantity .

:band_k_points a owl:Class ;
    rdfs:comment """Fractional coordinates of the $k$ or $q$ points (in the basis of the reciprocal-
lattice vectors) for which the electronic energy are given."""^^xsd:string ;
    rdfs:subClassOf [ a owl:Restriction ;
            owl:allValuesFrom <http://emmo.info/emmo/middle/math#EMMO_18d180e4_5e3e_42f7_820c_e08951223486> ;
            owl:onProperty :hasDatatype ],
        [ a owl:Restriction ;
            owl:hasValue 2 ;
            owl:onProperty :hasNumberOfDimensions ],
        [ a owl:Restriction ;
            owl:hasValue 3 ;
            owl:onProperty :hasFixDim2 ],
        [ a owl:Restriction ;
            owl:hasValue :number_of_k_points_per_segment ;
            owl:onProperty :hasVarDim1 ],
        :NMI_quantity .

:band_k_points_normalized a owl:Class ;
    rdfs:comment """Fractional coordinates of the $k$ points (in the basis of the reciprocal-lattice
vectors) for which the normalized electronic energies are given."""^^xsd:string ;
    rdfs:subClassOf [ a owl:Restriction ;
            owl:hasValue 2 ;
            owl:onProperty :hasNumberOfDimensions ],
        [ a owl:Restriction ;
            owl:hasValue :number_of_normalized_k_points_per_segment ;
            owl:onProperty :hasVarDim1 ],
        [ a owl:Restriction ;
            owl:hasValue 3 ;
            owl:onProperty :hasFixDim2 ],
        [ a owl:Restriction ;
            owl:allValuesFrom <http://emmo.info/emmo/middle/math#EMMO_18d180e4_5e3e_42f7_820c_e08951223486> ;
            owl:onProperty :hasDatatype ],
        :NMI_quantity .

:band_occupations a owl:Class ;
    rdfs:comment """Occupation of the $k$-points along the electronic band. The size of the dimensions
of this third-order tensor are the same as for the tensor in band_energies."""^^xsd:string ;
    rdfs:subClassOf [ a owl:Restriction ;
            owl:allValuesFrom <http://emmo.info/emmo/middle/math#EMMO_18d180e4_5e3e_42f7_820c_e08951223486> ;
            owl:onProperty :hasDatatype ],
        [ a owl:Restriction ;
            owl:hasValue :number_of_spin_channels ;
            owl:onProperty :hasVarDim1 ],
        [ a owl:Restriction ;
            owl:hasValue :number_of_band_segment_eigenvalues ;
            owl:onProperty :hasVarDim3 ],
        [ a owl:Restriction ;
            owl:hasValue 3 ;
            owl:onProperty :hasNumberOfDimensions ],
        [ a owl:Restriction ;
            owl:hasValue :number_of_k_points_per_segment ;
            owl:onProperty :hasVarDim2 ],
        :NMI_quantity .

:band_occupations_normalized a owl:Class ;
    rdfs:comment """Occupation of the $k$-points along the normalized electronic band. The size of the
dimensions of this third-order tensor are the same as for the tensor in
band_energies."""^^xsd:string ;
    rdfs:subClassOf [ a owl:Restriction ;
            owl:hasValue :number_of_normalized_k_points_per_segment ;
            owl:onProperty :hasVarDim2 ],
        [ a owl:Restriction ;
            owl:allValuesFrom <http://emmo.info/emmo/middle/math#EMMO_18d180e4_5e3e_42f7_820c_e08951223486> ;
            owl:onProperty :hasDatatype ],
        [ a owl:Restriction ;
            owl:hasValue :number_of_normalized_band_segment_eigenvalues ;
            owl:onProperty :hasVarDim3 ],
        [ a owl:Restriction ;
            owl:hasValue 3 ;
            owl:onProperty :hasNumberOfDimensions ],
        [ a owl:Restriction ;
            owl:hasValue :number_of_spin_channels ;
            owl:onProperty :hasVarDim1 ],
        :NMI_quantity .

:band_segm_labels a owl:Class ;
    rdfs:comment """Start and end labels of the points in the segment (one-dimensional pathways)
sampled in the $k$-space or $q$-space, using the conventional symbols, e.g.,
Gamma, K, L. The coordinates (fractional, in the reciprocal space) of the start
and end points for each segment are given in band_segm_start_end"""^^xsd:string ;
    rdfs:subClassOf [ a owl:Restriction ;
            owl:allValuesFrom <http://emmo.info/emmo/middle/perceptual#EMMO_50ea1ec5_f157_41b0_b46b_a9032f17ca10> ;
            owl:onProperty :hasDatatype ],
        [ a owl:Restriction ;
            owl:hasValue 2 ;
            owl:onProperty :hasFixDim1 ],
        [ a owl:Restriction ;
            owl:hasValue 1 ;
            owl:onProperty :hasNumberOfDimensions ],
        :NMI_quantity .

:band_segm_labels_normalized a owl:Class ;
    rdfs:comment """Start and end labels of the points in the segment (one-dimensional pathways)
sampled in the $k$-space, using the conventional symbols, e.g., Gamma, K, L. The
coordinates (fractional, in the reciprocal space) of the start and end points for
each segment are given in band_segm_start_end_normalized"""^^xsd:string ;
    rdfs:subClassOf [ a owl:Restriction ;
            owl:hasValue 1 ;
            owl:onProperty :hasNumberOfDimensions ],
        [ a owl:Restriction ;
            owl:hasValue 2 ;
            owl:onProperty :hasFixDim1 ],
        [ a owl:Restriction ;
            owl:allValuesFrom <http://emmo.info/emmo/middle/perceptual#EMMO_50ea1ec5_f157_41b0_b46b_a9032f17ca10> ;
            owl:onProperty :hasDatatype ],
        :NMI_quantity .

:band_segm_start_end a owl:Class ;
    rdfs:comment """Fractional coordinates of the start and end point (in the basis of the reciprocal
lattice vectors) of the segment sampled in the $k$ space. The conventional symbols
(e.g., Gamma, K, L) of the same points are given in band_segm_labels"""^^xsd:string ;
    rdfs:subClassOf [ a owl:Restriction ;
            owl:hasValue 3 ;
            owl:onProperty :hasFixDim2 ],
        [ a owl:Restriction ;
            owl:hasValue 2 ;
            owl:onProperty :hasFixDim1 ],
        [ a owl:Restriction ;
            owl:hasValue 2 ;
            owl:onProperty :hasNumberOfDimensions ],
        [ a owl:Restriction ;
            owl:allValuesFrom <http://emmo.info/emmo/middle/math#EMMO_18d180e4_5e3e_42f7_820c_e08951223486> ;
            owl:onProperty :hasDatatype ],
        :NMI_quantity .

:band_segm_start_end_normalized a owl:Class ;
    rdfs:comment """Fractional coordinates of the start and end point (in the basis of the reciprocal
lattice vectors) of the segment sampled in the $k$ space. The conventional symbols
(e.g., Gamma, K, L) of the same points are given in band_segm_labels"""^^xsd:string ;
    rdfs:subClassOf [ a owl:Restriction ;
            owl:allValuesFrom <http://emmo.info/emmo/middle/math#EMMO_18d180e4_5e3e_42f7_820c_e08951223486> ;
            owl:onProperty :hasDatatype ],
        [ a owl:Restriction ;
            owl:hasValue 3 ;
            owl:onProperty :hasFixDim2 ],
        [ a owl:Restriction ;
            owl:hasValue 2 ;
            owl:onProperty :hasFixDim1 ],
        [ a owl:Restriction ;
            owl:hasValue 2 ;
            owl:onProperty :hasNumberOfDimensions ],
        :NMI_quantity .

:band_structure_kind a owl:Class ;
    rdfs:comment "String to specify the kind of band structure (either electronic or vibrational)."^^xsd:string ;
    rdfs:subClassOf [ a owl:Restriction ;
            owl:hasValue 0 ;
            owl:onProperty :hasNumberOfDimensions ],
        [ a owl:Restriction ;
            owl:allValuesFrom <http://emmo.info/emmo/middle/perceptual#EMMO_50ea1ec5_f157_41b0_b46b_a9032f17ca10> ;
            owl:onProperty :hasDatatype ],
        :NMI_quantity .

:basis_set a owl:Class ;
    rdfs:comment """Unique string identifying the basis set used for the final wavefunctions
calculated with XC_method. It might identify a class of basis sets, often matches
one of the strings given in any of basis_set_name."""^^xsd:string ;
    rdfs:subClassOf [ a owl:Restriction ;
            owl:hasValue 0 ;
            owl:onProperty :hasNumberOfDimensions ],
        [ a owl:Restriction ;
            owl:onProperty :hasCategory ;
            owl:someValuesFrom :settings_numerical_parameter ],
        [ a owl:Restriction ;
            owl:allValuesFrom <http://emmo.info/emmo/middle/perceptual#EMMO_50ea1ec5_f157_41b0_b46b_a9032f17ca10> ;
            owl:onProperty :hasDatatype ],
        [ a owl:Restriction ;
            owl:onProperty :hasCategory ;
            owl:someValuesFrom :settings_potential_energy_surface ],
        :NMI_quantity .

:basis_set_atom_centered_ls a owl:Class ;
    rdfs:comment """Azimuthal quantum number ($l$) values (of the angular part given by the spherical
harmonic $Y_{lm}$) of the atom-centered basis function defined in the current
section_basis_set_atom_centered."""^^xsd:string ;
    rdfs:subClassOf [ a owl:Restriction ;
            owl:hasValue 1 ;
            owl:onProperty :hasNumberOfDimensions ],
        [ a owl:Restriction ;
            owl:hasValue :number_of_kinds_in_basis_set_atom_centered ;
            owl:onProperty :hasVarDim1 ],
        [ a owl:Restriction ;
            owl:allValuesFrom <http://emmo.info/emmo/middle/math#EMMO_f8bd64d5_5d3e_4ad4_a46e_c30714fecb7f> ;
            owl:onProperty :hasDatatype ],
        :NMI_quantity .

:basis_set_atom_centered_radial_functions a owl:Class ;
    rdfs:comment """Values of the radial function of the different basis function kinds. The values
are numerically tabulated on a default 0.01-nm equally spaced grid from 0 to 4 nm.
The 5 tabulated values are $r$, $f(r)$, $f'(r)$, $f(r) \\cdot r$,
$\\frac{d}{dr}(f(r) \\cdot r)$."""^^xsd:string ;
    rdfs:subClassOf [ a owl:Restriction ;
            owl:hasValue :number_of_kinds_in_basis_set_atom_centered ;
            owl:onProperty :hasVarDim1 ],
        [ a owl:Restriction ;
            owl:hasValue 401 ;
            owl:onProperty :hasFixDim2 ],
        [ a owl:Restriction ;
            owl:allValuesFrom <http://emmo.info/emmo/middle/math#EMMO_18d180e4_5e3e_42f7_820c_e08951223486> ;
            owl:onProperty :hasDatatype ],
        [ a owl:Restriction ;
            owl:hasValue 5 ;
            owl:onProperty :hasFixDim3 ],
        [ a owl:Restriction ;
            owl:hasValue 3 ;
            owl:onProperty :hasNumberOfDimensions ],
        :NMI_quantity .

:basis_set_atom_centered_short_name a owl:Class ;
    rdfs:comment """Code-specific, but explicative, base name for the basis set (not unique). Details
are explained in the [basis_set_atom_centered_short_name wiki
page](https://gitlab.mpcdf.mpg.de/nomad-lab/nomad-meta-info/wikis/metainfo/basis-
set-atom-centered-short-name), this name should not contain the *atom kind* (to
simplify the use of a single name for multiple elements)."""^^xsd:string ;
    rdfs:subClassOf [ a owl:Restriction ;
            owl:allValuesFrom <http://emmo.info/emmo/middle/perceptual#EMMO_50ea1ec5_f157_41b0_b46b_a9032f17ca10> ;
            owl:onProperty :hasDatatype ],
        [ a owl:Restriction ;
            owl:hasValue 0 ;
            owl:onProperty :hasNumberOfDimensions ],
        :NMI_quantity .

:basis_set_atom_centered_unique_name a owl:Class ;
    rdfs:comment """Code-specific, but explicative, base name for the basis set (not unique). This
string starts with basis_set_atom_centered_short_name. If the basis set defined in
this section_basis_set_atom_centered is not identical to the default definition
(stored in a database) of the basis set with the same name stored in a database,
then the string is extended by 10 identifiable characters as explained in the
[basis_set_atom_centered_name wiki page](https://gitlab.mpcdf.mpg.de/nomad-
lab/nomad-meta-info/wikis/metainfo/basis-set-atom-centered-unique-name). The
reason for this procedure is that often atom-centered basis sets are obtained by
fine tuning basis sets provided by the code developers or other sources. Each
basis sets, which has normally a standard name, often reported in publications,
has also several parameters that can be tuned. This metadata tries to keep track
of the original basis set and its modifications. This string here defined should
not contain the *atom kind* for which this basis set is intended for, in order to
simplify the use of a single name for multiple *atom kinds* (see atom_labels for
the actual meaning of *atom kind*)."""^^xsd:string ;
    rdfs:subClassOf [ a owl:Restriction ;
            owl:allValuesFrom <http://emmo.info/emmo/middle/perceptual#EMMO_50ea1ec5_f157_41b0_b46b_a9032f17ca10> ;
            owl:onProperty :hasDatatype ],
        [ a owl:Restriction ;
            owl:hasValue 0 ;
            owl:onProperty :hasNumberOfDimensions ],
        :NMI_quantity .

:basis_set_atom_number a owl:Class ;
    rdfs:comment """Atomic number (i.e., number of protons) of the atom for which this basis set is
constructed (0 means unspecified or a pseudo atom)."""^^xsd:string ;
    rdfs:subClassOf [ a owl:Restriction ;
            owl:allValuesFrom <http://emmo.info/emmo/middle/math#EMMO_f8bd64d5_5d3e_4ad4_a46e_c30714fecb7f> ;
            owl:onProperty <http://emmo.info/emmo/middle/metrology#EMMO_67fc0a36_8dcb_4ffa_9a43_31074efa3296> ],
        [ a owl:Restriction ;
            owl:hasValue 0 ;
            owl:onProperty :hasNumberOfDimensions ],
        [ a owl:Restriction ;
            owl:allValuesFrom <http://emmo.info/emmo/middle/math#EMMO_f8bd64d5_5d3e_4ad4_a46e_c30714fecb7f> ;
            owl:onProperty :hasDatatype ],
        :NMI_dimension,
        :NMI_quantity .

:basis_set_cell_dependent_kind a owl:Class ;
    rdfs:comment """A string defining the type of the cell-dependent basis set (i.e., non atom
centered such as plane-waves). Allowed values are listed in the
[basis_set_cell_dependent_kind wiki page](https://gitlab.mpcdf.mpg.de/nomad-
lab/nomad-meta-info/wikis/metainfo/basis-set-cell-dependent-kind)."""^^xsd:string ;
    rdfs:subClassOf [ a owl:Restriction ;
            owl:allValuesFrom <http://emmo.info/emmo/middle/perceptual#EMMO_50ea1ec5_f157_41b0_b46b_a9032f17ca10> ;
            owl:onProperty :hasDatatype ],
        [ a owl:Restriction ;
            owl:hasValue 0 ;
            owl:onProperty :hasNumberOfDimensions ],
        :NMI_quantity .

:basis_set_cell_dependent_name a owl:Class ;
    rdfs:comment """A label identifying the cell-dependent basis set (i.e., non atom centered such as
plane-waves). Allowed values are listed in the [basis_set_cell_dependent_name wiki
page](https://gitlab.mpcdf.mpg.de/nomad-lab/nomad-meta-info/wikis/metainfo/basis-
set-cell-dependent-name)."""^^xsd:string ;
    rdfs:subClassOf [ a owl:Restriction ;
            owl:allValuesFrom <http://emmo.info/emmo/middle/perceptual#EMMO_50ea1ec5_f157_41b0_b46b_a9032f17ca10> ;
            owl:onProperty :hasDatatype ],
        [ a owl:Restriction ;
            owl:hasValue 0 ;
            owl:onProperty :hasNumberOfDimensions ],
        :NMI_quantity .

:basis_set_kind a owl:Class ;
    rdfs:comment """String describing the use of the basis set, i.e, if it used for expanding a wave-
function or an electron density. Allowed values are listed in the [basis_set_kind
wiki page](https://gitlab.mpcdf.mpg.de/nomad-lab/nomad-meta-
info/wikis/metainfo/basis-set-kind)."""^^xsd:string ;
    rdfs:subClassOf [ a owl:Restriction ;
            owl:hasValue 0 ;
            owl:onProperty :hasNumberOfDimensions ],
        [ a owl:Restriction ;
            owl:allValuesFrom <http://emmo.info/emmo/middle/perceptual#EMMO_50ea1ec5_f157_41b0_b46b_a9032f17ca10> ;
            owl:onProperty :hasDatatype ],
        :NMI_quantity .

:basis_set_name a owl:Class ;
    rdfs:comment """String identifying the basis set in an unique way. The rules for building this
string are specified in the [basis_set_name wiki
page](https://gitlab.mpcdf.mpg.de/nomad-lab/nomad-meta-info/wikis/metainfo/basis-
set-name)."""^^xsd:string ;
    rdfs:subClassOf [ a owl:Restriction ;
            owl:hasValue 0 ;
            owl:onProperty :hasNumberOfDimensions ],
        [ a owl:Restriction ;
            owl:allValuesFrom <http://emmo.info/emmo/middle/perceptual#EMMO_50ea1ec5_f157_41b0_b46b_a9032f17ca10> ;
            owl:onProperty :hasDatatype ],
        :NMI_quantity .

:basis_set_planewave_cutoff a owl:Class ;
    rdfs:comment """Spherical cutoff  in reciprocal space for a plane-wave basis set. It is the energy
of the highest plan-ewave ($\\frac{\\hbar^2|k+G|^2}{2m_e}$) included in the basis
set. Note that normally this basis set is used for the wavefunctions, and the
density would have 4 times the cutoff, but this actually depends on the use of the
basis set by the method."""^^xsd:string ;
    rdfs:subClassOf [ a owl:Restriction ;
            owl:allValuesFrom <http://emmo.info/emmo/middle/math#EMMO_18d180e4_5e3e_42f7_820c_e08951223486> ;
            owl:onProperty :hasDatatype ],
        [ a owl:Restriction ;
            owl:allValuesFrom <http://emmo.info/emmo/middle/siunits#EMMO_8a70dea4_d6ab_4260_b931_a3e990982416> ;
            owl:onProperty <http://emmo.info/emmo/middle/metrology#EMMO_67fc0a36_8dcb_4ffa_9a43_31074efa3296> ],
        [ a owl:Restriction ;
            owl:hasValue 0 ;
            owl:onProperty :hasNumberOfDimensions ],
        :NMI_quantity .

:bins a owl:Class ;
    rdfs:comment "Byte representation of the DOS fingerprint."^^xsd:string ;
    rdfs:subClassOf [ a owl:Restriction ;
            owl:allValuesFrom <http://emmo.info/emmo/middle/perceptual#EMMO_50ea1ec5_f157_41b0_b46b_a9032f17ca10> ;
            owl:onProperty :hasDatatype ],
        [ a owl:Restriction ;
            owl:hasValue 0 ;
            owl:onProperty :hasNumberOfDimensions ],
        :NMI_quantity .

:bravais_lattice a owl:Class ;
    rdfs:comment """Identifier for the Bravais lattice in Pearson notation. The first lowercase letter
identifies the crystal family and can be one of the following: a (triclinic), b
(monoclinic), o (orthorhombic), t (tetragonal), h (hexagonal) or c (cubic). The
second uppercase letter identifies the centring and can be one of the following: P
(primitive), S (face centred), I (body centred), R (rhombohedral centring) or F
(all faces centred)."""^^xsd:string ;
    rdfs:subClassOf [ a owl:Restriction ;
            owl:allValuesFrom <http://emmo.info/emmo/middle/perceptual#EMMO_50ea1ec5_f157_41b0_b46b_a9032f17ca10> ;
            owl:onProperty :hasDatatype ],
        [ a owl:Restriction ;
            owl:hasValue 0 ;
            owl:onProperty :hasNumberOfDimensions ],
        :NMI_quantity .

:calculation_file_uri a owl:Class ;
    rdfs:comment """Contains the nomad uri of a raw the data file connected to the current run. There
should be an value for the main_file_uri and all ancillary files."""^^xsd:string ;
    rdfs:subClassOf [ a owl:Restriction ;
            owl:allValuesFrom <http://emmo.info/emmo/middle/perceptual#EMMO_50ea1ec5_f157_41b0_b46b_a9032f17ca10> ;
            owl:onProperty :hasDatatype ],
        [ a owl:Restriction ;
            owl:hasValue 0 ;
            owl:onProperty :hasNumberOfDimensions ],
        :NMI_quantity .

:calculation_method a owl:Class ;
    rdfs:comment """String that uniquely represents the method used to calculate energy_total, If the
present calculation_method_current is a perturbative method Y that uses method X
as starting point, this string is automatically created as X@Y, where X is taken
from calculation_method_current and Y from method_to_method_ref. In order to
activate this, method_to_method_kind must have the value starting_point (see the
[method_to_method_kind wiki page](https://gitlab.mpcdf.mpg.de/nomad-lab/nomad-
meta-info/wikis/metainfo/method-to-method-kind))."""^^xsd:string ;
    rdfs:subClassOf [ a owl:Restriction ;
            owl:hasValue 0 ;
            owl:onProperty :hasNumberOfDimensions ],
        [ a owl:Restriction ;
            owl:allValuesFrom <http://emmo.info/emmo/middle/perceptual#EMMO_50ea1ec5_f157_41b0_b46b_a9032f17ca10> ;
            owl:onProperty :hasDatatype ],
        :NMI_quantity .

:calculation_method_current a owl:Class ;
    rdfs:comment """String that represents the method used to calculate the energy_current. If the
method is perturbative, this string does not describe the starting point method,
the latter being referenced to by section_method_to_method_refs. For self-
consistent field (SCF) ab initio calculations, for example, this is composed by
concatenating XC_method_current and basis_set. See [calculation_method_current
wiki page](https://gitlab.mpcdf.mpg.de/nomad-lab/nomad-meta-
info/wikis/metainfo/calculation-method-current) for the details."""^^xsd:string ;
    rdfs:subClassOf [ a owl:Restriction ;
            owl:allValuesFrom <http://emmo.info/emmo/middle/perceptual#EMMO_50ea1ec5_f157_41b0_b46b_a9032f17ca10> ;
            owl:onProperty :hasDatatype ],
        [ a owl:Restriction ;
            owl:hasValue 0 ;
            owl:onProperty :hasNumberOfDimensions ],
        :NMI_quantity .

:calculation_method_kind a owl:Class ;
    rdfs:comment """Kind of method in calculation_method_current.

Accepted values are:

- absolute

- perturbative."""^^xsd:string ;
    rdfs:subClassOf [ a owl:Restriction ;
            owl:allValuesFrom <http://emmo.info/emmo/middle/perceptual#EMMO_50ea1ec5_f157_41b0_b46b_a9032f17ca10> ;
            owl:onProperty :hasDatatype ],
        [ a owl:Restriction ;
            owl:hasValue 0 ;
            owl:onProperty :hasNumberOfDimensions ],
        :NMI_quantity .

:calculation_to_calculation_external_url a owl:Class ;
    rdfs:comment """URL used to reference an externally stored calculation. The kind of relationship
between the present and the referenced section_single_configuration_calculation is
specified by calculation_to_calculation_kind."""^^xsd:string ;
    rdfs:subClassOf [ a owl:Restriction ;
            owl:allValuesFrom <http://emmo.info/emmo/middle/perceptual#EMMO_50ea1ec5_f157_41b0_b46b_a9032f17ca10> ;
            owl:onProperty :hasDatatype ],
        [ a owl:Restriction ;
            owl:hasValue 0 ;
            owl:onProperty :hasNumberOfDimensions ],
        :NMI_quantity .

:calculation_to_calculation_kind a owl:Class ;
    rdfs:comment """String defining the relationship between the referenced
section_single_configuration_calculation and the present
section_single_configuration_calculation. Valid values are described in the
[calculation_to_calculation_kind wiki page](https://gitlab.mpcdf.mpg.de/nomad-
lab/nomad-meta-info/wikis/metainfo/calculation-to-calculation-kind). Often
calculations are connected, for instance, one calculation is a perturbation
performed using a self-consistent field (SCF) calculation as starting point, or a
simulated system is partitioned in regions with different but connected
Hamiltonians (e.g., QM/MM, or a region treated via Kohn-Sham DFT embedded into a
region treated via orbital-free DFT). Hence, the need of keeping track of these
connected calculations. The referenced calculation is identified via
calculation_to_calculation_ref (typically used for a calculation in the same
section_run) or calculation_to_calculation_external_url."""^^xsd:string ;
    rdfs:subClassOf [ a owl:Restriction ;
            owl:hasValue 0 ;
            owl:onProperty :hasNumberOfDimensions ],
        [ a owl:Restriction ;
            owl:allValuesFrom <http://emmo.info/emmo/middle/perceptual#EMMO_50ea1ec5_f157_41b0_b46b_a9032f17ca10> ;
            owl:onProperty :hasDatatype ],
        :NMI_quantity .

:calculation_to_calculation_ref a owl:Class ;
    rdfs:comment """Reference to another calculation. If both this and
calculation_to_calculation_external_url are given, then
calculation_to_calculation_ref is a local copy of the URL given in
calculation_to_calculation_external_url. The kind of relationship between the
present and the referenced section_single_configuration_calculation is specified
by calculation_to_calculation_kind."""^^xsd:string ;
    rdfs:subClassOf [ a owl:Restriction ;
            owl:hasValue 0 ;
            owl:onProperty :hasNumberOfDimensions ],
        :NMI_quantity .

:calculation_to_folder_external_url a owl:Class ;
    rdfs:comment """URL used to reference a folder containing external calculations. The kind of
relationship between the present and the referenced
section_single_configuration_calculation is specified by
calculation_to_folder_kind."""^^xsd:string ;
    rdfs:subClassOf [ a owl:Restriction ;
            owl:hasValue 0 ;
            owl:onProperty :hasNumberOfDimensions ],
        [ a owl:Restriction ;
            owl:allValuesFrom <http://emmo.info/emmo/middle/perceptual#EMMO_50ea1ec5_f157_41b0_b46b_a9032f17ca10> ;
            owl:onProperty :hasDatatype ],
        :NMI_quantity .

:calculation_to_folder_kind a owl:Class ;
    rdfs:comment """String defining the relationship between the referenced
section_single_configuration_calculation and a folder containing calculations."""^^xsd:string ;
    rdfs:subClassOf [ a owl:Restriction ;
            owl:allValuesFrom <http://emmo.info/emmo/middle/perceptual#EMMO_50ea1ec5_f157_41b0_b46b_a9032f17ca10> ;
            owl:onProperty :hasDatatype ],
        [ a owl:Restriction ;
            owl:hasValue 0 ;
            owl:onProperty :hasNumberOfDimensions ],
        :NMI_quantity .

:chemical_composition a owl:Class ;
    rdfs:comment "The chemical composition as full formula of the system, based on atom species."^^xsd:string ;
    rdfs:subClassOf [ a owl:Restriction ;
            owl:hasValue 0 ;
            owl:onProperty :hasNumberOfDimensions ],
        [ a owl:Restriction ;
            owl:allValuesFrom <http://emmo.info/emmo/middle/perceptual#EMMO_50ea1ec5_f157_41b0_b46b_a9032f17ca10> ;
            owl:onProperty :hasDatatype ],
        :NMI_quantity .

:chemical_composition_bulk_reduced a owl:Class ;
    rdfs:comment """The chemical composition as reduced bulk formula of the system, based on atom
species."""^^xsd:string ;
    rdfs:subClassOf [ a owl:Restriction ;
            owl:allValuesFrom <http://emmo.info/emmo/middle/perceptual#EMMO_50ea1ec5_f157_41b0_b46b_a9032f17ca10> ;
            owl:onProperty :hasDatatype ],
        [ a owl:Restriction ;
            owl:hasValue 0 ;
            owl:onProperty :hasNumberOfDimensions ],
        :NMI_quantity .

:chemical_composition_reduced a owl:Class ;
    rdfs:comment "The chemical composition as reduced formula of the system, based on atom species."^^xsd:string ;
    rdfs:subClassOf [ a owl:Restriction ;
            owl:allValuesFrom <http://emmo.info/emmo/middle/perceptual#EMMO_50ea1ec5_f157_41b0_b46b_a9032f17ca10> ;
            owl:onProperty :hasDatatype ],
        [ a owl:Restriction ;
            owl:hasValue 0 ;
            owl:onProperty :hasNumberOfDimensions ],
        :NMI_quantity .

:choice a owl:Class ;
    rdfs:comment """String that specifies the centering, origin and basis vector settings of the 3D
space group that defines the symmetry group of the simulated physical system (see
section_system). Values are as defined by spglib."""^^xsd:string ;
    rdfs:subClassOf [ a owl:Restriction ;
            owl:hasValue 0 ;
            owl:onProperty :hasNumberOfDimensions ],
        [ a owl:Restriction ;
            owl:allValuesFrom <http://emmo.info/emmo/middle/perceptual#EMMO_50ea1ec5_f157_41b0_b46b_a9032f17ca10> ;
            owl:onProperty :hasDatatype ],
        :NMI_quantity .

:conduction_band_min_energy a owl:Class ;
    rdfs:comment "Conduction band minimum energy."^^xsd:string ;
    rdfs:subClassOf [ a owl:Restriction ;
            owl:allValuesFrom <http://emmo.info/emmo/middle/siunits#EMMO_8a70dea4_d6ab_4260_b931_a3e990982416> ;
            owl:onProperty <http://emmo.info/emmo/middle/metrology#EMMO_67fc0a36_8dcb_4ffa_9a43_31074efa3296> ],
        [ a owl:Restriction ;
            owl:allValuesFrom <http://emmo.info/emmo/middle/math#EMMO_18d180e4_5e3e_42f7_820c_e08951223486> ;
            owl:onProperty :hasDatatype ],
        [ a owl:Restriction ;
            owl:hasValue 0 ;
            owl:onProperty :hasNumberOfDimensions ],
        :NMI_quantity .

:conduction_band_min_k_point a owl:Class ;
    rdfs:comment "Coordinate of the conduction band minimum in k-space."^^xsd:string ;
    rdfs:subClassOf [ a owl:Restriction ;
            owl:allValuesFrom <http://emmo.info/emmo/middle/math#EMMO_18d180e4_5e3e_42f7_820c_e08951223486> ;
            owl:onProperty :hasDatatype ],
        [ a owl:Restriction ;
            owl:hasValue 3 ;
            owl:onProperty :hasFixDim1 ],
        [ a owl:Restriction ;
            owl:allValuesFrom <https://nomad-coe.eu/ontology/properties#PerMetre> ;
            owl:onProperty <http://emmo.info/emmo/middle/metrology#EMMO_67fc0a36_8dcb_4ffa_9a43_31074efa3296> ],
        [ a owl:Restriction ;
            owl:hasValue 1 ;
            owl:onProperty :hasNumberOfDimensions ],
        :NMI_quantity .

:configuration_periodic_dimensions a owl:Class ;
    rdfs:comment """Array labeling which of the lattice vectors use periodic boundary conditions. Note
for the parser developers: This value is not expected to be given for each
section_single_configuration_calculation. It is assumed to be valid from the
section_single_configuration_calculation where it is defined for all subsequent
section_single_configuration_calculation in section_run, until redefined."""^^xsd:string ;
    rdfs:subClassOf [ a owl:Restriction ;
            owl:allValuesFrom <http://emmo.info/emmo/middle/math#EMMO_54dc83cb_06e1_4739_9e45_bc09cead7f48> ;
            owl:onProperty :hasDatatype ],
        [ a owl:Restriction ;
            owl:hasValue 1 ;
            owl:onProperty :hasNumberOfDimensions ],
        [ a owl:Restriction ;
            owl:hasValue 3 ;
            owl:onProperty :hasFixDim1 ],
        [ a owl:Restriction ;
            owl:onProperty :hasCategory ;
            owl:someValuesFrom :configuration_core ],
        :NMI_quantity .

:configuration_raw_gid a owl:Class ;
    rdfs:comment """checksum of the configuration_core, i.e. the geometry of the system. The values
are not normalized in any way so equivalent configurations might have different
values"""^^xsd:string ;
    rdfs:subClassOf [ a owl:Restriction ;
            owl:allValuesFrom <http://emmo.info/emmo/middle/perceptual#EMMO_50ea1ec5_f157_41b0_b46b_a9032f17ca10> ;
            owl:onProperty :hasDatatype ],
        [ a owl:Restriction ;
            owl:hasValue 0 ;
            owl:onProperty :hasNumberOfDimensions ],
        :NMI_quantity .

:constraint_atoms a owl:Class ;
    rdfs:comment """List of the indexes involved in this constraint. The fist atom has index 1, the
last number_of_topology_atoms."""^^xsd:string ;
    rdfs:subClassOf [ a owl:Restriction ;
            owl:hasValue :number_of_constraints ;
            owl:onProperty :hasVarDim1 ],
        [ a owl:Restriction ;
            owl:hasValue :number_of_atoms_per_constraint ;
            owl:onProperty :hasVarDim2 ],
        [ a owl:Restriction ;
            owl:hasValue 2 ;
            owl:onProperty :hasNumberOfDimensions ],
        [ a owl:Restriction ;
            owl:allValuesFrom <http://emmo.info/emmo/middle/math#EMMO_f8bd64d5_5d3e_4ad4_a46e_c30714fecb7f> ;
            owl:onProperty :hasDatatype ],
        :NMI_quantity .

:constraint_kind a owl:Class ;
    rdfs:comment """Short and unique name for this constraint type. Valid names are described in the
[constraint\\_kind wiki page](https://gitlab.mpcdf.mpg.de/nomad-lab/nomad-meta-
info/wikis/metainfo/constraint-kind)."""^^xsd:string ;
    rdfs:subClassOf [ a owl:Restriction ;
            owl:allValuesFrom <http://emmo.info/emmo/middle/perceptual#EMMO_50ea1ec5_f157_41b0_b46b_a9032f17ca10> ;
            owl:onProperty :hasDatatype ],
        [ a owl:Restriction ;
            owl:hasValue 0 ;
            owl:onProperty :hasNumberOfDimensions ],
        :NMI_quantity .

:constraint_parameters a owl:Class ;
    rdfs:comment """Explicit constraint parameters for this kind of constraint (depending on the
constraint type, some might be given implicitly through other means)."""^^xsd:string ;
    rdfs:subClassOf [ a owl:Restriction ;
            owl:hasValue 0 ;
            owl:onProperty :hasNumberOfDimensions ],
        :NMI_quantity .

:crystal_system a owl:Class ;
    rdfs:comment """Name of the crystal system. Can be one of the following: triclinic, monoclinic,
orthorhombic, tetragonal, trigonal, hexagonal or cubic."""^^xsd:string ;
    rdfs:subClassOf [ a owl:Restriction ;
            owl:allValuesFrom <http://emmo.info/emmo/middle/perceptual#EMMO_50ea1ec5_f157_41b0_b46b_a9032f17ca10> ;
            owl:onProperty :hasDatatype ],
        [ a owl:Restriction ;
            owl:hasValue 0 ;
            owl:onProperty :hasNumberOfDimensions ],
        :NMI_quantity .

:dft_plus_u_functional a owl:Class ;
    rdfs:comment """Type of DFT+U functional (such as DFT/DFT+U double-counting compensation). Valid
names are described in the [dft\\_plus\\_u\\_functional wiki
page](https://gitlab.mpcdf.mpg.de/nomad-lab/nomad-meta-info/wikis/metainfo/dft-
plus-u-functional)."""^^xsd:string ;
    rdfs:subClassOf [ a owl:Restriction ;
            owl:allValuesFrom <http://emmo.info/emmo/middle/perceptual#EMMO_50ea1ec5_f157_41b0_b46b_a9032f17ca10> ;
            owl:onProperty :hasDatatype ],
        [ a owl:Restriction ;
            owl:hasValue 0 ;
            owl:onProperty :hasNumberOfDimensions ],
        :NMI_quantity .

:dft_plus_u_orbital_J a owl:Class ;
    rdfs:comment "DFT+U-orbital setting: value J (exchange interaction)"^^xsd:string ;
    rdfs:subClassOf [ a owl:Restriction ;
            owl:allValuesFrom <http://emmo.info/emmo/middle/math#EMMO_18d180e4_5e3e_42f7_820c_e08951223486> ;
            owl:onProperty :hasDatatype ],
        [ a owl:Restriction ;
            owl:onProperty :hasCategory ;
            owl:someValuesFrom :energy_value ],
        [ a owl:Restriction ;
            owl:hasValue 0 ;
            owl:onProperty :hasNumberOfDimensions ],
        :NMI_quantity .

:dft_plus_u_orbital_U a owl:Class ;
    rdfs:comment "DFT+U-orbital setting: value U (on-site Coulomb interaction)"^^xsd:string ;
    rdfs:subClassOf [ a owl:Restriction ;
            owl:allValuesFrom <http://emmo.info/emmo/middle/math#EMMO_18d180e4_5e3e_42f7_820c_e08951223486> ;
            owl:onProperty :hasDatatype ],
        [ a owl:Restriction ;
            owl:hasValue 0 ;
            owl:onProperty :hasNumberOfDimensions ],
        [ a owl:Restriction ;
            owl:onProperty :hasCategory ;
            owl:someValuesFrom :energy_value ],
        :NMI_quantity .

:dft_plus_u_orbital_U_effective a owl:Class ;
    rdfs:comment "DFT+U-orbital setting: value U_{effective} (U-J), if implementation uses it"^^xsd:string ;
    rdfs:subClassOf [ a owl:Restriction ;
            owl:hasValue 0 ;
            owl:onProperty :hasNumberOfDimensions ],
        [ a owl:Restriction ;
            owl:allValuesFrom <http://emmo.info/emmo/middle/math#EMMO_18d180e4_5e3e_42f7_820c_e08951223486> ;
            owl:onProperty :hasDatatype ],
        [ a owl:Restriction ;
            owl:onProperty :hasCategory ;
            owl:someValuesFrom :energy_value ],
        :NMI_quantity .

:dft_plus_u_orbital_atom a owl:Class ;
    rdfs:comment "DFT+U-orbital setting: atom index (references index of atom_labels/atom_positions)"^^xsd:string ;
    rdfs:subClassOf [ a owl:Restriction ;
            owl:hasValue 0 ;
            owl:onProperty :hasNumberOfDimensions ],
        [ a owl:Restriction ;
            owl:allValuesFrom <http://emmo.info/emmo/middle/math#EMMO_f8bd64d5_5d3e_4ad4_a46e_c30714fecb7f> ;
            owl:onProperty :hasDatatype ],
        [ a owl:Restriction ;
            owl:allValuesFrom <http://emmo.info/emmo/middle/math#EMMO_f8bd64d5_5d3e_4ad4_a46e_c30714fecb7f> ;
            owl:onProperty <http://emmo.info/emmo/middle/metrology#EMMO_67fc0a36_8dcb_4ffa_9a43_31074efa3296> ],
        :NMI_dimension,
        :NMI_quantity .

:dft_plus_u_orbital_label a owl:Class ;
    rdfs:comment "DFT+U-orbital setting: orbital label (normally (n,l)), notation: '3d', '4f', ..."^^xsd:string ;
    rdfs:subClassOf [ a owl:Restriction ;
            owl:hasValue 0 ;
            owl:onProperty :hasNumberOfDimensions ],
        [ a owl:Restriction ;
            owl:allValuesFrom <http://emmo.info/emmo/middle/perceptual#EMMO_50ea1ec5_f157_41b0_b46b_a9032f17ca10> ;
            owl:onProperty :hasDatatype ],
        :NMI_quantity .

:dft_plus_u_projection_type a owl:Class ;
    rdfs:comment """DFT+U: Type of orbitals used for projection in order to calculate occupation
numbers. Valid names are described in the [dft\\_plus\\_u\\_projection\\_type wiki
page](https://gitlab.mpcdf.mpg.de/nomad-lab/nomad-meta-info/wikis/metainfo/dft-
plus-u-projection-type)."""^^xsd:string ;
    rdfs:subClassOf [ a owl:Restriction ;
            owl:hasValue 0 ;
            owl:onProperty :hasNumberOfDimensions ],
        [ a owl:Restriction ;
            owl:allValuesFrom <http://emmo.info/emmo/middle/perceptual#EMMO_50ea1ec5_f157_41b0_b46b_a9032f17ca10> ;
            owl:onProperty :hasDatatype ],
        :NMI_quantity .

:dos_energies a owl:Class ;
    rdfs:comment """Array containing the set of discrete energy values for the density (electronic-
energy or vibrational energy) of states (DOS). This is the total DOS, see
atom_projected_dos_energies and species_projected_dos_energies for partial density
of states."""^^xsd:string ;
    rdfs:subClassOf [ a owl:Restriction ;
            owl:allValuesFrom <http://emmo.info/emmo/middle/siunits#EMMO_8a70dea4_d6ab_4260_b931_a3e990982416> ;
            owl:onProperty <http://emmo.info/emmo/middle/metrology#EMMO_67fc0a36_8dcb_4ffa_9a43_31074efa3296> ],
        [ a owl:Restriction ;
            owl:hasValue :number_of_dos_values ;
            owl:onProperty :hasVarDim1 ],
        [ a owl:Restriction ;
            owl:hasValue 1 ;
            owl:onProperty :hasNumberOfDimensions ],
        [ a owl:Restriction ;
            owl:allValuesFrom <http://emmo.info/emmo/middle/math#EMMO_18d180e4_5e3e_42f7_820c_e08951223486> ;
            owl:onProperty :hasDatatype ],
        :NMI_quantity .

:dos_energies_normalized a owl:Class ;
    rdfs:comment """Array containing the set of discrete energy values with respect to the top of the
valence band for the density (electronic-energy) of states (DOS). This is the
total DOS, see atom_projected_dos_energies and species_projected_dos_energies for
partial density of states."""^^xsd:string ;
    rdfs:subClassOf [ a owl:Restriction ;
            owl:allValuesFrom <http://emmo.info/emmo/middle/siunits#EMMO_8a70dea4_d6ab_4260_b931_a3e990982416> ;
            owl:onProperty <http://emmo.info/emmo/middle/metrology#EMMO_67fc0a36_8dcb_4ffa_9a43_31074efa3296> ],
        [ a owl:Restriction ;
            owl:hasValue 1 ;
            owl:onProperty :hasNumberOfDimensions ],
        [ a owl:Restriction ;
            owl:hasValue :number_of_dos_values ;
            owl:onProperty :hasVarDim1 ],
        [ a owl:Restriction ;
            owl:allValuesFrom <http://emmo.info/emmo/middle/math#EMMO_18d180e4_5e3e_42f7_820c_e08951223486> ;
            owl:onProperty :hasDatatype ],
        :NMI_quantity .

:dos_fermi_energy a owl:Class ;
    rdfs:comment "Stores the Fermi energy of the density of states."^^xsd:string ;
    rdfs:subClassOf [ a owl:Restriction ;
            owl:allValuesFrom <http://emmo.info/emmo/middle/math#EMMO_18d180e4_5e3e_42f7_820c_e08951223486> ;
            owl:onProperty :hasDatatype ],
        [ a owl:Restriction ;
            owl:hasValue 0 ;
            owl:onProperty :hasNumberOfDimensions ],
        :NMI_quantity .

:dos_integrated_values a owl:Class ;
    rdfs:comment """Integrated density of states (starting at $-\\infty$), pseudo potential
calculations should start with the number of core electrons if they cover only the
active electrons"""^^xsd:string ;
    rdfs:subClassOf [ a owl:Restriction ;
            owl:hasValue :number_of_spin_channels ;
            owl:onProperty :hasVarDim1 ],
        [ a owl:Restriction ;
            owl:hasValue 2 ;
            owl:onProperty :hasNumberOfDimensions ],
        [ a owl:Restriction ;
            owl:hasValue :number_of_dos_values ;
            owl:onProperty :hasVarDim2 ],
        [ a owl:Restriction ;
            owl:allValuesFrom <http://emmo.info/emmo/middle/math#EMMO_18d180e4_5e3e_42f7_820c_e08951223486> ;
            owl:onProperty :hasDatatype ],
        :NMI_quantity .

:dos_kind a owl:Class ;
    rdfs:comment """String to specify the kind of density of states (either electronic or
vibrational)."""^^xsd:string ;
    rdfs:subClassOf [ a owl:Restriction ;
            owl:allValuesFrom <http://emmo.info/emmo/middle/perceptual#EMMO_50ea1ec5_f157_41b0_b46b_a9032f17ca10> ;
            owl:onProperty :hasDatatype ],
        [ a owl:Restriction ;
            owl:hasValue 0 ;
            owl:onProperty :hasNumberOfDimensions ],
        :NMI_quantity .

:dos_lm a owl:Class ;
    rdfs:comment """Tuples of $l$ and $m$ values for which dos_values_lm are given. For the quantum
number $l$ the conventional meaning of azimuthal quantum number is always adopted.
For the integer number $m$, besides the conventional use as magnetic quantum
number ($l+1$ integer values from $-l$ to $l$), a set of different conventions is
accepted (see the [m_kind wiki page](https://gitlab.rzg.mpg.de/nomad-lab/nomad-
meta-info/wikis/metainfo/m-kind). The actual adopted convention is specified by
dos_m_kind."""^^xsd:string ;
    rdfs:subClassOf [ a owl:Restriction ;
            owl:allValuesFrom <http://emmo.info/emmo/middle/math#EMMO_f8bd64d5_5d3e_4ad4_a46e_c30714fecb7f> ;
            owl:onProperty :hasDatatype ],
        [ a owl:Restriction ;
            owl:hasValue 2 ;
            owl:onProperty :hasNumberOfDimensions ],
        [ a owl:Restriction ;
            owl:hasValue 2 ;
            owl:onProperty :hasFixDim2 ],
        [ a owl:Restriction ;
            owl:hasValue :number_of_dos_lms ;
            owl:onProperty :hasVarDim1 ],
        :NMI_quantity .

:dos_m_kind a owl:Class ;
    rdfs:comment """String describing what the integer numbers of $m$ in dos_lm mean. The allowed
values are listed in the [m_kind wiki page](https://gitlab.rzg.mpg.de/nomad-
lab/nomad-meta-info/wikis/metainfo/m-kind)."""^^xsd:string ;
    rdfs:subClassOf [ a owl:Restriction ;
            owl:hasValue 0 ;
            owl:onProperty :hasNumberOfDimensions ],
        [ a owl:Restriction ;
            owl:allValuesFrom <http://emmo.info/emmo/middle/perceptual#EMMO_50ea1ec5_f157_41b0_b46b_a9032f17ca10> ;
            owl:onProperty :hasDatatype ],
        :NMI_quantity .

:dos_values a owl:Class ;
    rdfs:comment """Values (number of states for a given energy, the set of discrete energy values is
given in dos_energies) of density (electronic-energy or vibrational-energy) of
states. This refers to the simulation cell, i.e. integrating over all energies
will give the number of electrons in the simulation cell."""^^xsd:string ;
    rdfs:subClassOf [ a owl:Restriction ;
            owl:hasValue :number_of_dos_values ;
            owl:onProperty :hasVarDim2 ],
        [ a owl:Restriction ;
            owl:allValuesFrom <http://emmo.info/emmo/middle/math#EMMO_18d180e4_5e3e_42f7_820c_e08951223486> ;
            owl:onProperty :hasDatatype ],
        [ a owl:Restriction ;
            owl:hasValue 2 ;
            owl:onProperty :hasNumberOfDimensions ],
        [ a owl:Restriction ;
            owl:hasValue :number_of_spin_channels ;
            owl:onProperty :hasVarDim1 ],
        :NMI_quantity .

:dos_values_lm a owl:Class ;
    rdfs:comment """Array containing the density (electronic-energy) of states values projected on the
various spherical harmonics (integrated on all atoms), see
atom_projected_dos_values_lm for atom values."""^^xsd:string ;
    rdfs:subClassOf [ a owl:Restriction ;
            owl:hasValue 4 ;
            owl:onProperty :hasNumberOfDimensions ],
        [ a owl:Restriction ;
            owl:hasValue :number_of_atoms ;
            owl:onProperty :hasVarDim3 ],
        [ a owl:Restriction ;
            owl:hasValue :number_of_spin_channels ;
            owl:onProperty :hasVarDim2 ],
        [ a owl:Restriction ;
            owl:hasValue :number_of_dos_values ;
            owl:onProperty :hasVarDim4 ],
        [ a owl:Restriction ;
            owl:hasValue :number_of_dos_lms ;
            owl:onProperty :hasVarDim1 ],
        [ a owl:Restriction ;
            owl:allValuesFrom <http://emmo.info/emmo/middle/math#EMMO_18d180e4_5e3e_42f7_820c_e08951223486> ;
            owl:onProperty :hasDatatype ],
        [ a owl:Restriction ;
            owl:allValuesFrom <http://emmo.info/emmo/middle/siunits#EMMO_8a70dea4_d6ab_4260_b931_a3e990982416> ;
            owl:onProperty <http://emmo.info/emmo/middle/metrology#EMMO_67fc0a36_8dcb_4ffa_9a43_31074efa3296> ],
        :NMI_quantity .

:dos_values_normalized a owl:Class ;
    rdfs:comment """Density of states (DOS) values divided by the unit cell volume and by the number
of atoms."""^^xsd:string ;
    rdfs:subClassOf [ a owl:Restriction ;
            owl:hasValue :number_of_spin_channels ;
            owl:onProperty :hasVarDim1 ],
        [ a owl:Restriction ;
            owl:allValuesFrom <http://emmo.info/emmo/middle/math#EMMO_18d180e4_5e3e_42f7_820c_e08951223486> ;
            owl:onProperty :hasDatatype ],
        [ a owl:Restriction ;
            owl:hasValue 2 ;
            owl:onProperty :hasNumberOfDimensions ],
        [ a owl:Restriction ;
            owl:hasValue :number_of_dos_values ;
            owl:onProperty :hasVarDim2 ],
        :NMI_quantity .

:eigenvalues_kind a owl:Class ;
    rdfs:comment """A short string describing the kind of eigenvalues, as defined in the
[eigenvalues_kind wiki page](https://gitlab.mpcdf.mpg.de/nomad-lab/nomad-meta-
info/wikis/metainfo/eigenvalues-kind)."""^^xsd:string ;
    rdfs:subClassOf [ a owl:Restriction ;
            owl:hasValue 0 ;
            owl:onProperty :hasNumberOfDimensions ],
        [ a owl:Restriction ;
            owl:allValuesFrom <http://emmo.info/emmo/middle/perceptual#EMMO_50ea1ec5_f157_41b0_b46b_a9032f17ca10> ;
            owl:onProperty :hasDatatype ],
        :NMI_quantity .

:eigenvalues_kpoints a owl:Class ;
    rdfs:comment """Coordinates of the $k$ points (in the basis of the reciprocal lattice vectors)
used for the evaluation of the eigenvalues tabulated in eigenvalues_values."""^^xsd:string ;
    rdfs:subClassOf [ a owl:Restriction ;
            owl:hasValue :number_of_eigenvalues_kpoints ;
            owl:onProperty :hasVarDim1 ],
        [ a owl:Restriction ;
            owl:hasValue 3 ;
            owl:onProperty :hasFixDim2 ],
        [ a owl:Restriction ;
            owl:allValuesFrom <http://emmo.info/emmo/middle/math#EMMO_18d180e4_5e3e_42f7_820c_e08951223486> ;
            owl:onProperty :hasDatatype ],
        [ a owl:Restriction ;
            owl:hasValue 2 ;
            owl:onProperty :hasNumberOfDimensions ],
        :NMI_quantity .

:eigenvalues_kpoints_multiplicity a owl:Class ;
    rdfs:comment """Multiplicity of the $k$ point (i.e., how many distinct points per cell this
expands to after applying all symmetries). This defaults to 1. If expansion is
preformed then each point will have weight
eigenvalues_kpoints_weights/eigenvalues_kpoints_multiplicity."""^^xsd:string ;
    rdfs:subClassOf [ a owl:Restriction ;
            owl:hasValue :number_of_eigenvalues_kpoints ;
            owl:onProperty :hasVarDim1 ],
        [ a owl:Restriction ;
            owl:allValuesFrom <http://emmo.info/emmo/middle/math#EMMO_18d180e4_5e3e_42f7_820c_e08951223486> ;
            owl:onProperty :hasDatatype ],
        [ a owl:Restriction ;
            owl:hasValue 1 ;
            owl:onProperty :hasNumberOfDimensions ],
        :NMI_quantity .

:eigenvalues_kpoints_weights a owl:Class ;
    rdfs:comment """Weights of the $k$ points (in the basis of the reciprocal lattice vectors) used
for the evaluation of the eigenvalues tabulated in eigenvalues_values, should
account for symmetry too."""^^xsd:string ;
    rdfs:subClassOf [ a owl:Restriction ;
            owl:allValuesFrom <http://emmo.info/emmo/middle/math#EMMO_18d180e4_5e3e_42f7_820c_e08951223486> ;
            owl:onProperty :hasDatatype ],
        [ a owl:Restriction ;
            owl:hasValue 1 ;
            owl:onProperty :hasNumberOfDimensions ],
        [ a owl:Restriction ;
            owl:hasValue :number_of_eigenvalues_kpoints ;
            owl:onProperty :hasVarDim1 ],
        :NMI_quantity .

:eigenvalues_occupation a owl:Class ;
    rdfs:comment """Occupation of the eigenstates. The corresponding eigenvalues (energy) are given in
eigenvalues_values. The coordinates in the reciprocal space are defined in
eigenvalues_kpoints."""^^xsd:string ;
    rdfs:subClassOf [ a owl:Restriction ;
            owl:hasValue 3 ;
            owl:onProperty :hasNumberOfDimensions ],
        [ a owl:Restriction ;
            owl:hasValue :number_of_eigenvalues ;
            owl:onProperty :hasVarDim3 ],
        [ a owl:Restriction ;
            owl:hasValue :number_of_spin_channels ;
            owl:onProperty :hasVarDim1 ],
        [ a owl:Restriction ;
            owl:allValuesFrom <http://emmo.info/emmo/middle/math#EMMO_18d180e4_5e3e_42f7_820c_e08951223486> ;
            owl:onProperty :hasDatatype ],
        [ a owl:Restriction ;
            owl:hasValue :number_of_eigenvalues_kpoints ;
            owl:onProperty :hasVarDim2 ],
        :NMI_quantity .

:eigenvalues_values a owl:Class ;
    rdfs:comment """Values of the (electronic-energy) eigenvalues. The coordinates of the
corresponding eigenstates in the reciprocal space are defined in
eigenvalues_kpoints and their occupations are given in eigenvalues_occupation."""^^xsd:string ;
    rdfs:subClassOf [ a owl:Restriction ;
            owl:hasValue 3 ;
            owl:onProperty :hasNumberOfDimensions ],
        [ a owl:Restriction ;
            owl:hasValue :number_of_spin_channels ;
            owl:onProperty :hasVarDim1 ],
        [ a owl:Restriction ;
            owl:allValuesFrom <http://emmo.info/emmo/middle/siunits#EMMO_8a70dea4_d6ab_4260_b931_a3e990982416> ;
            owl:onProperty <http://emmo.info/emmo/middle/metrology#EMMO_67fc0a36_8dcb_4ffa_9a43_31074efa3296> ],
        [ a owl:Restriction ;
            owl:allValuesFrom <http://emmo.info/emmo/middle/math#EMMO_18d180e4_5e3e_42f7_820c_e08951223486> ;
            owl:onProperty :hasDatatype ],
        [ a owl:Restriction ;
            owl:hasValue :number_of_eigenvalues_kpoints ;
            owl:onProperty :hasVarDim2 ],
        [ a owl:Restriction ;
            owl:hasValue :number_of_eigenvalues ;
            owl:onProperty :hasVarDim3 ],
        :NMI_quantity .

:electronic_kinetic_energy a owl:Class ;
    rdfs:comment "Self-consistent electronic kinetic energy as defined in XC_method."^^xsd:string ;
    rdfs:subClassOf [ a owl:Restriction ;
            owl:allValuesFrom <http://emmo.info/emmo/middle/siunits#EMMO_8a70dea4_d6ab_4260_b931_a3e990982416> ;
            owl:onProperty <http://emmo.info/emmo/middle/metrology#EMMO_67fc0a36_8dcb_4ffa_9a43_31074efa3296> ],
        [ a owl:Restriction ;
            owl:hasValue 0 ;
            owl:onProperty :hasNumberOfDimensions ],
        [ a owl:Restriction ;
            owl:allValuesFrom <http://emmo.info/emmo/middle/math#EMMO_18d180e4_5e3e_42f7_820c_e08951223486> ;
            owl:onProperty :hasDatatype ],
        [ a owl:Restriction ;
            owl:onProperty :hasCategory ;
            owl:someValuesFrom :energy_value ],
        [ a owl:Restriction ;
            owl:onProperty :hasCategory ;
            owl:someValuesFrom :energy_component ],
        :NMI_quantity .

:electronic_kinetic_energy_scf_iteration a owl:Class ;
    rdfs:comment """Electronic kinetic energy as defined in XC_method during the self-consistent field
(SCF) iterations."""^^xsd:string ;
    rdfs:subClassOf [ a owl:Restriction ;
            owl:allValuesFrom <http://emmo.info/emmo/middle/siunits#EMMO_8a70dea4_d6ab_4260_b931_a3e990982416> ;
            owl:onProperty <http://emmo.info/emmo/middle/metrology#EMMO_67fc0a36_8dcb_4ffa_9a43_31074efa3296> ],
        [ a owl:Restriction ;
            owl:allValuesFrom <http://emmo.info/emmo/middle/math#EMMO_18d180e4_5e3e_42f7_820c_e08951223486> ;
            owl:onProperty :hasDatatype ],
        [ a owl:Restriction ;
            owl:onProperty :hasCategory ;
            owl:someValuesFrom :energy_component ],
        [ a owl:Restriction ;
            owl:onProperty :hasCategory ;
            owl:someValuesFrom :energy_value ],
        [ a owl:Restriction ;
            owl:hasValue 0 ;
            owl:onProperty :hasNumberOfDimensions ],
        :NMI_quantity .

:electronic_structure_method a owl:Class ;
    rdfs:comment """Non-unique string identifying the used electronic structure method. It is not
unique in the sense that two calculations with the same
electronic_structure_method string may have not been performed with exactly the
same method. The allowed strings are given in the [electronic structure method
wiki page](https://gitlab.mpcdf.mpg.de/nomad-lab/nomad-meta-
info/wikis/metainfo/electronic-structure-method)."""^^xsd:string ;
    rdfs:subClassOf [ a owl:Restriction ;
            owl:onProperty :hasCategory ;
            owl:someValuesFrom :settings_XC ],
        [ a owl:Restriction ;
            owl:hasValue 0 ;
            owl:onProperty :hasNumberOfDimensions ],
        [ a owl:Restriction ;
            owl:allValuesFrom <http://emmo.info/emmo/middle/perceptual#EMMO_50ea1ec5_f157_41b0_b46b_a9032f17ca10> ;
            owl:onProperty :hasDatatype ],
        [ a owl:Restriction ;
            owl:onProperty :hasCategory ;
            owl:someValuesFrom :settings_potential_energy_surface ],
        :NMI_quantity .

:embedded_system a owl:Class ;
    rdfs:comment "Is the system embedded into a host geometry?."^^xsd:string ;
    rdfs:subClassOf [ a owl:Restriction ;
            owl:allValuesFrom <http://emmo.info/emmo/middle/math#EMMO_54dc83cb_06e1_4739_9e45_bc09cead7f48> ;
            owl:onProperty :hasDatatype ],
        [ a owl:Restriction ;
            owl:hasValue 0 ;
            owl:onProperty :hasNumberOfDimensions ],
        [ a owl:Restriction ;
            owl:onProperty :hasCategory ;
            owl:someValuesFrom :configuration_core ],
        :NMI_quantity .

:energy_C a owl:Class ;
    rdfs:comment "Correlation (C) energy calculated with the method described in XC_functional."^^xsd:string ;
    rdfs:subClassOf [ a owl:Restriction ;
            owl:hasValue 0 ;
            owl:onProperty :hasNumberOfDimensions ],
        [ a owl:Restriction ;
            owl:allValuesFrom <http://emmo.info/emmo/middle/siunits#EMMO_8a70dea4_d6ab_4260_b931_a3e990982416> ;
            owl:onProperty <http://emmo.info/emmo/middle/metrology#EMMO_67fc0a36_8dcb_4ffa_9a43_31074efa3296> ],
        [ a owl:Restriction ;
            owl:onProperty :hasCategory ;
            owl:someValuesFrom :energy_component ],
        [ a owl:Restriction ;
            owl:onProperty :hasCategory ;
            owl:someValuesFrom :energy_value ],
        [ a owl:Restriction ;
            owl:allValuesFrom <http://emmo.info/emmo/middle/math#EMMO_18d180e4_5e3e_42f7_820c_e08951223486> ;
            owl:onProperty :hasDatatype ],
        [ a owl:Restriction ;
            owl:onProperty :hasCategory ;
            owl:someValuesFrom :energy_type_C ],
        :NMI_quantity .

:energy_C_mGGA a owl:Class ;
    rdfs:comment """Component of the correlation (C) energy at the GGA (or MetaGGA) level using the
self-consistent density of the target XC functional (full unscaled value, i.e.,
not scaled due to exact-exchange mixing)."""^^xsd:string ;
    rdfs:subClassOf [ a owl:Restriction ;
            owl:onProperty :hasCategory ;
            owl:someValuesFrom :energy_type_C ],
        [ a owl:Restriction ;
            owl:onProperty :hasCategory ;
            owl:someValuesFrom :energy_value ],
        [ a owl:Restriction ;
            owl:allValuesFrom <http://emmo.info/emmo/middle/math#EMMO_18d180e4_5e3e_42f7_820c_e08951223486> ;
            owl:onProperty :hasDatatype ],
        [ a owl:Restriction ;
            owl:allValuesFrom <http://emmo.info/emmo/middle/siunits#EMMO_8a70dea4_d6ab_4260_b931_a3e990982416> ;
            owl:onProperty <http://emmo.info/emmo/middle/metrology#EMMO_67fc0a36_8dcb_4ffa_9a43_31074efa3296> ],
        [ a owl:Restriction ;
            owl:onProperty :hasCategory ;
            owl:someValuesFrom :energy_component ],
        [ a owl:Restriction ;
            owl:hasValue 0 ;
            owl:onProperty :hasNumberOfDimensions ],
        :NMI_quantity .

:energy_T0_per_atom a owl:Class ;
    rdfs:comment """Value of the total energy per atom, calculated with the method described in
XC_method and extrapolated to $T=0$, based on a free-electron gas argument."""^^xsd:string ;
    rdfs:subClassOf [ a owl:Restriction ;
            owl:onProperty :hasCategory ;
            owl:someValuesFrom :energy_total_potential_per_atom ],
        [ a owl:Restriction ;
            owl:hasValue 0 ;
            owl:onProperty :hasNumberOfDimensions ],
        [ a owl:Restriction ;
            owl:onProperty :hasCategory ;
            owl:someValuesFrom :energy_value ],
        [ a owl:Restriction ;
            owl:onProperty :hasCategory ;
            owl:someValuesFrom :energy_component ],
        [ a owl:Restriction ;
            owl:allValuesFrom <http://emmo.info/emmo/middle/math#EMMO_18d180e4_5e3e_42f7_820c_e08951223486> ;
            owl:onProperty :hasDatatype ],
        [ a owl:Restriction ;
            owl:allValuesFrom <http://emmo.info/emmo/middle/siunits#EMMO_8a70dea4_d6ab_4260_b931_a3e990982416> ;
            owl:onProperty <http://emmo.info/emmo/middle/metrology#EMMO_67fc0a36_8dcb_4ffa_9a43_31074efa3296> ],
        :NMI_quantity .

:energy_X a owl:Class ;
    rdfs:comment """Value fo the exchange (X) energy calculated with the method described in
XC_method."""^^xsd:string ;
    rdfs:subClassOf [ a owl:Restriction ;
            owl:allValuesFrom <http://emmo.info/emmo/middle/siunits#EMMO_8a70dea4_d6ab_4260_b931_a3e990982416> ;
            owl:onProperty <http://emmo.info/emmo/middle/metrology#EMMO_67fc0a36_8dcb_4ffa_9a43_31074efa3296> ],
        [ a owl:Restriction ;
            owl:onProperty :hasCategory ;
            owl:someValuesFrom :energy_component ],
        [ a owl:Restriction ;
            owl:onProperty :hasCategory ;
            owl:someValuesFrom :energy_value ],
        [ a owl:Restriction ;
            owl:allValuesFrom <http://emmo.info/emmo/middle/math#EMMO_18d180e4_5e3e_42f7_820c_e08951223486> ;
            owl:onProperty :hasDatatype ],
        [ a owl:Restriction ;
            owl:onProperty :hasCategory ;
            owl:someValuesFrom :energy_type_X ],
        [ a owl:Restriction ;
            owl:hasValue 0 ;
            owl:onProperty :hasNumberOfDimensions ],
        :NMI_quantity .

:energy_XC a owl:Class ;
    rdfs:comment """Value of the exchange-correlation (XC) energy calculated with the method described
in XC_method."""^^xsd:string ;
    rdfs:subClassOf [ a owl:Restriction ;
            owl:onProperty :hasCategory ;
            owl:someValuesFrom :energy_type_XC ],
        [ a owl:Restriction ;
            owl:allValuesFrom <http://emmo.info/emmo/middle/siunits#EMMO_8a70dea4_d6ab_4260_b931_a3e990982416> ;
            owl:onProperty <http://emmo.info/emmo/middle/metrology#EMMO_67fc0a36_8dcb_4ffa_9a43_31074efa3296> ],
        [ a owl:Restriction ;
            owl:onProperty :hasCategory ;
            owl:someValuesFrom :energy_value ],
        [ a owl:Restriction ;
            owl:onProperty :hasCategory ;
            owl:someValuesFrom :energy_component ],
        [ a owl:Restriction ;
            owl:allValuesFrom <http://emmo.info/emmo/middle/math#EMMO_18d180e4_5e3e_42f7_820c_e08951223486> ;
            owl:onProperty :hasDatatype ],
        [ a owl:Restriction ;
            owl:hasValue 0 ;
            owl:onProperty :hasNumberOfDimensions ],
        :NMI_quantity .

:energy_XC_functional a owl:Class ;
    rdfs:comment """Value of the exchange-correlation (XC) energy calculated with the functional
stored in XC_functional."""^^xsd:string ;
    rdfs:subClassOf [ a owl:Restriction ;
            owl:onProperty :hasCategory ;
            owl:someValuesFrom :energy_value ],
        [ a owl:Restriction ;
            owl:allValuesFrom <http://emmo.info/emmo/middle/siunits#EMMO_8a70dea4_d6ab_4260_b931_a3e990982416> ;
            owl:onProperty <http://emmo.info/emmo/middle/metrology#EMMO_67fc0a36_8dcb_4ffa_9a43_31074efa3296> ],
        [ a owl:Restriction ;
            owl:allValuesFrom <http://emmo.info/emmo/middle/math#EMMO_18d180e4_5e3e_42f7_820c_e08951223486> ;
            owl:onProperty :hasDatatype ],
        [ a owl:Restriction ;
            owl:onProperty :hasCategory ;
            owl:someValuesFrom :energy_type_XC ],
        [ a owl:Restriction ;
            owl:hasValue 0 ;
            owl:onProperty :hasNumberOfDimensions ],
        [ a owl:Restriction ;
            owl:onProperty :hasCategory ;
            owl:someValuesFrom :energy_component ],
        :NMI_quantity .

:energy_XC_potential a owl:Class ;
    rdfs:comment """Value of the exchange-correlation (XC) potential energy: the integral of the first
order derivative of the functional stored in XC_functional (integral of
v_xc*electron_density), i.e., the component of XC that is in the sum of the
eigenvalues. Value associated with the configuration, should be the most converged
value."""^^xsd:string ;
    rdfs:subClassOf [ a owl:Restriction ;
            owl:allValuesFrom <http://emmo.info/emmo/middle/math#EMMO_18d180e4_5e3e_42f7_820c_e08951223486> ;
            owl:onProperty :hasDatatype ],
        [ a owl:Restriction ;
            owl:allValuesFrom <http://emmo.info/emmo/middle/siunits#EMMO_8a70dea4_d6ab_4260_b931_a3e990982416> ;
            owl:onProperty <http://emmo.info/emmo/middle/metrology#EMMO_67fc0a36_8dcb_4ffa_9a43_31074efa3296> ],
        [ a owl:Restriction ;
            owl:hasValue 0 ;
            owl:onProperty :hasNumberOfDimensions ],
        [ a owl:Restriction ;
            owl:onProperty :hasCategory ;
            owl:someValuesFrom :energy_value ],
        [ a owl:Restriction ;
            owl:onProperty :hasCategory ;
            owl:someValuesFrom :energy_component ],
        :NMI_quantity .

:energy_XC_potential_scf_iteration a owl:Class ;
    rdfs:comment """Value for exchange-correlation (XC) potential energy: the integral of the first
order derivative of the functional stored in XC_functional (integral of
v_xc*electron_density), i.e., the component of XC that is in the sum of the
eigenvalues. Values are given for each self-consistent field (SCF) iteration
(i.e., not the converged value, the latter being stored in energy_XC_potential)."""^^xsd:string ;
    rdfs:subClassOf [ a owl:Restriction ;
            owl:hasValue 0 ;
            owl:onProperty :hasNumberOfDimensions ],
        [ a owl:Restriction ;
            owl:onProperty :hasCategory ;
            owl:someValuesFrom :energy_component ],
        [ a owl:Restriction ;
            owl:allValuesFrom <http://emmo.info/emmo/middle/siunits#EMMO_8a70dea4_d6ab_4260_b931_a3e990982416> ;
            owl:onProperty <http://emmo.info/emmo/middle/metrology#EMMO_67fc0a36_8dcb_4ffa_9a43_31074efa3296> ],
        [ a owl:Restriction ;
            owl:onProperty :hasCategory ;
            owl:someValuesFrom :energy_value ],
        [ a owl:Restriction ;
            owl:allValuesFrom <http://emmo.info/emmo/middle/math#EMMO_18d180e4_5e3e_42f7_820c_e08951223486> ;
            owl:onProperty :hasDatatype ],
        :NMI_quantity .

:energy_XC_scf_iteration a owl:Class ;
    rdfs:comment """Value for exchange-correlation (XC) energy obtained during each self-consistent
field (SCF) iteration, using the method described in XC_method."""^^xsd:string ;
    rdfs:subClassOf [ a owl:Restriction ;
            owl:onProperty :hasCategory ;
            owl:someValuesFrom :energy_component ],
        [ a owl:Restriction ;
            owl:allValuesFrom <http://emmo.info/emmo/middle/math#EMMO_18d180e4_5e3e_42f7_820c_e08951223486> ;
            owl:onProperty :hasDatatype ],
        [ a owl:Restriction ;
            owl:hasValue 0 ;
            owl:onProperty :hasNumberOfDimensions ],
        [ a owl:Restriction ;
            owl:allValuesFrom <http://emmo.info/emmo/middle/siunits#EMMO_8a70dea4_d6ab_4260_b931_a3e990982416> ;
            owl:onProperty <http://emmo.info/emmo/middle/metrology#EMMO_67fc0a36_8dcb_4ffa_9a43_31074efa3296> ],
        [ a owl:Restriction ;
            owl:onProperty :hasCategory ;
            owl:someValuesFrom :energy_value ],
        :NMI_quantity .

:energy_X_mGGA a owl:Class ;
    rdfs:comment """Component of the exchange (X) energy at the GGA (or MetaGGA) level using the self
consistent density of the target functional (full unscaled value, i.e., not scaled
due to exact-exchange mixing)."""^^xsd:string ;
    rdfs:subClassOf [ a owl:Restriction ;
            owl:onProperty :hasCategory ;
            owl:someValuesFrom :energy_type_X ],
        [ a owl:Restriction ;
            owl:hasValue 0 ;
            owl:onProperty :hasNumberOfDimensions ],
        [ a owl:Restriction ;
            owl:onProperty :hasCategory ;
            owl:someValuesFrom :energy_component ],
        [ a owl:Restriction ;
            owl:allValuesFrom <http://emmo.info/emmo/middle/siunits#EMMO_8a70dea4_d6ab_4260_b931_a3e990982416> ;
            owl:onProperty <http://emmo.info/emmo/middle/metrology#EMMO_67fc0a36_8dcb_4ffa_9a43_31074efa3296> ],
        [ a owl:Restriction ;
            owl:allValuesFrom <http://emmo.info/emmo/middle/math#EMMO_18d180e4_5e3e_42f7_820c_e08951223486> ;
            owl:onProperty :hasDatatype ],
        [ a owl:Restriction ;
            owl:onProperty :hasCategory ;
            owl:someValuesFrom :energy_value ],
        :NMI_quantity .

:energy_X_mGGA_scaled a owl:Class ;
    rdfs:comment """Component of the exchange (X) energy at the GGA (or MetaGGA) level, using the self
consistent density of the target functional, scaled accordingly to the mixing
parameter."""^^xsd:string ;
    rdfs:subClassOf [ a owl:Restriction ;
            owl:hasValue 0 ;
            owl:onProperty :hasNumberOfDimensions ],
        [ a owl:Restriction ;
            owl:onProperty :hasCategory ;
            owl:someValuesFrom :energy_component ],
        [ a owl:Restriction ;
            owl:onProperty :hasCategory ;
            owl:someValuesFrom :energy_value ],
        [ a owl:Restriction ;
            owl:allValuesFrom <http://emmo.info/emmo/middle/math#EMMO_18d180e4_5e3e_42f7_820c_e08951223486> ;
            owl:onProperty :hasDatatype ],
        [ a owl:Restriction ;
            owl:allValuesFrom <http://emmo.info/emmo/middle/siunits#EMMO_8a70dea4_d6ab_4260_b931_a3e990982416> ;
            owl:onProperty <http://emmo.info/emmo/middle/metrology#EMMO_67fc0a36_8dcb_4ffa_9a43_31074efa3296> ],
        :NMI_quantity .

:energy_change_scf_iteration a owl:Class ;
    rdfs:comment """Stores the change of total energy with respect to the previous self-consistent
field (SCF) iteration."""^^xsd:string ;
    rdfs:subClassOf [ a owl:Restriction ;
            owl:allValuesFrom <http://emmo.info/emmo/middle/math#EMMO_18d180e4_5e3e_42f7_820c_e08951223486> ;
            owl:onProperty :hasDatatype ],
        [ a owl:Restriction ;
            owl:onProperty :hasCategory ;
            owl:someValuesFrom :energy_value ],
        [ a owl:Restriction ;
            owl:hasValue 0 ;
            owl:onProperty :hasNumberOfDimensions ],
        [ a owl:Restriction ;
            owl:allValuesFrom <http://emmo.info/emmo/middle/siunits#EMMO_8a70dea4_d6ab_4260_b931_a3e990982416> ;
            owl:onProperty <http://emmo.info/emmo/middle/metrology#EMMO_67fc0a36_8dcb_4ffa_9a43_31074efa3296> ],
        [ a owl:Restriction ;
            owl:onProperty :hasCategory ;
            owl:someValuesFrom :error_estimate_contribution ],
        :NMI_quantity .

:energy_code_independent_kind a owl:Class ;
    rdfs:comment """Type of the code-independent total energy (obtained by subtracting a reference
energy calculated with the same code), created to be comparable among different
codes and numerical settings. Details can be found on the [energy_code_independent
wiki page](https://gitlab.mpcdf.mpg.de/nomad-lab/nomad-meta-
info/wikis/metainfo/energy-code-independent)."""^^xsd:string ;
    rdfs:subClassOf [ a owl:Restriction ;
            owl:allValuesFrom <http://emmo.info/emmo/middle/perceptual#EMMO_50ea1ec5_f157_41b0_b46b_a9032f17ca10> ;
            owl:onProperty :hasDatatype ],
        [ a owl:Restriction ;
            owl:hasValue 0 ;
            owl:onProperty :hasNumberOfDimensions ],
        :NMI_quantity .

:energy_code_independent_value a owl:Class ;
    rdfs:comment """Value of the code-independent total energy (obtained by subtracting a reference
energy calculated with the same code). This value is created to be comparable
among different codes and numerical settings. Details can be found on the
[energy_code_independent wiki page](https://gitlab.mpcdf.mpg.de/nomad-lab/nomad-
meta-info/wikis/metainfo/energy-code-independent)."""^^xsd:string ;
    rdfs:subClassOf [ a owl:Restriction ;
            owl:onProperty :hasCategory ;
            owl:someValuesFrom :energy_value ],
        [ a owl:Restriction ;
            owl:allValuesFrom <http://emmo.info/emmo/middle/siunits#EMMO_8a70dea4_d6ab_4260_b931_a3e990982416> ;
            owl:onProperty <http://emmo.info/emmo/middle/metrology#EMMO_67fc0a36_8dcb_4ffa_9a43_31074efa3296> ],
        [ a owl:Restriction ;
            owl:allValuesFrom <http://emmo.info/emmo/middle/math#EMMO_18d180e4_5e3e_42f7_820c_e08951223486> ;
            owl:onProperty :hasDatatype ],
        [ a owl:Restriction ;
            owl:onProperty :hasCategory ;
            owl:someValuesFrom :energy_total_potential ],
        [ a owl:Restriction ;
            owl:hasValue 0 ;
            owl:onProperty :hasNumberOfDimensions ],
        [ a owl:Restriction ;
            owl:onProperty :hasCategory ;
            owl:someValuesFrom :energy_component ],
        :NMI_quantity .

:energy_correction_entropy a owl:Class ;
    rdfs:comment """Entropy correction to the potential energy to compensate for the change in
occupation so that forces at finite T do not need to keep the change of occupation
in account. Defined consistently with XC_method."""^^xsd:string ;
    rdfs:subClassOf [ a owl:Restriction ;
            owl:allValuesFrom <http://emmo.info/emmo/middle/siunits#EMMO_8a70dea4_d6ab_4260_b931_a3e990982416> ;
            owl:onProperty <http://emmo.info/emmo/middle/metrology#EMMO_67fc0a36_8dcb_4ffa_9a43_31074efa3296> ],
        [ a owl:Restriction ;
            owl:hasValue 0 ;
            owl:onProperty :hasNumberOfDimensions ],
        [ a owl:Restriction ;
            owl:onProperty :hasCategory ;
            owl:someValuesFrom :energy_component ],
        [ a owl:Restriction ;
            owl:allValuesFrom <http://emmo.info/emmo/middle/math#EMMO_18d180e4_5e3e_42f7_820c_e08951223486> ;
            owl:onProperty :hasDatatype ],
        [ a owl:Restriction ;
            owl:onProperty :hasCategory ;
            owl:someValuesFrom :energy_value ],
        :NMI_quantity .

:energy_correction_entropy_scf_iteration a owl:Class ;
    rdfs:comment """Entropy correction to the potential energy to compensate for the change in
occupation so that forces at finite T do not need to keep the change of occupation
in account. The array lists the values of the entropy correction for each self-
consistent field (SCF) iteration. Defined consistently with XC_method."""^^xsd:string ;
    rdfs:subClassOf [ a owl:Restriction ;
            owl:allValuesFrom <http://emmo.info/emmo/middle/math#EMMO_18d180e4_5e3e_42f7_820c_e08951223486> ;
            owl:onProperty :hasDatatype ],
        [ a owl:Restriction ;
            owl:hasValue 0 ;
            owl:onProperty :hasNumberOfDimensions ],
        [ a owl:Restriction ;
            owl:onProperty :hasCategory ;
            owl:someValuesFrom :energy_component ],
        [ a owl:Restriction ;
            owl:onProperty :hasCategory ;
            owl:someValuesFrom :energy_value ],
        [ a owl:Restriction ;
            owl:allValuesFrom <http://emmo.info/emmo/middle/siunits#EMMO_8a70dea4_d6ab_4260_b931_a3e990982416> ;
            owl:onProperty <http://emmo.info/emmo/middle/metrology#EMMO_67fc0a36_8dcb_4ffa_9a43_31074efa3296> ],
        :NMI_quantity .

:energy_correction_hartree a owl:Class ;
    rdfs:comment """Correction to the density-density electrostatic energy in the sum of eigenvalues
(that uses the mixed density on one side), and the fully consistent density-
density electrostatic energy. Defined consistently with XC_method."""^^xsd:string ;
    rdfs:subClassOf [ a owl:Restriction ;
            owl:onProperty :hasCategory ;
            owl:someValuesFrom :energy_component ],
        [ a owl:Restriction ;
            owl:allValuesFrom <http://emmo.info/emmo/middle/siunits#EMMO_8a70dea4_d6ab_4260_b931_a3e990982416> ;
            owl:onProperty <http://emmo.info/emmo/middle/metrology#EMMO_67fc0a36_8dcb_4ffa_9a43_31074efa3296> ],
        [ a owl:Restriction ;
            owl:allValuesFrom <http://emmo.info/emmo/middle/math#EMMO_18d180e4_5e3e_42f7_820c_e08951223486> ;
            owl:onProperty :hasDatatype ],
        [ a owl:Restriction ;
            owl:hasValue 0 ;
            owl:onProperty :hasNumberOfDimensions ],
        [ a owl:Restriction ;
            owl:onProperty :hasCategory ;
            owl:someValuesFrom :energy_value ],
        :NMI_quantity .

:energy_correction_hartree_scf_iteration a owl:Class ;
    rdfs:comment """Correction to the density-density electrostatic energy in the sum of eigenvalues
(that uses the mixed density on one side), and the fully consistent density-
density electrostatic energy during the self-consistent field (SCF) iterations.
Defined consistently with XC_method."""^^xsd:string ;
    rdfs:subClassOf [ a owl:Restriction ;
            owl:hasValue 0 ;
            owl:onProperty :hasNumberOfDimensions ],
        [ a owl:Restriction ;
            owl:allValuesFrom <http://emmo.info/emmo/middle/math#EMMO_18d180e4_5e3e_42f7_820c_e08951223486> ;
            owl:onProperty :hasDatatype ],
        [ a owl:Restriction ;
            owl:allValuesFrom <http://emmo.info/emmo/middle/siunits#EMMO_8a70dea4_d6ab_4260_b931_a3e990982416> ;
            owl:onProperty <http://emmo.info/emmo/middle/metrology#EMMO_67fc0a36_8dcb_4ffa_9a43_31074efa3296> ],
        [ a owl:Restriction ;
            owl:onProperty :hasCategory ;
            owl:someValuesFrom :energy_value ],
        [ a owl:Restriction ;
            owl:onProperty :hasCategory ;
            owl:someValuesFrom :energy_component ],
        :NMI_quantity .

:energy_current a owl:Class ;
    rdfs:comment """Value of the energy calculated with calculation_method_current. energy_current is
equal to energy_total for non-perturbative methods. For perturbative methods,
energy_current is equal to the correction: energy_total minus energy_total of the
calculation_to_calculation_ref with calculation_to_calculation_kind =
starting_point (see the [method_to_method_kind wiki
page](https://gitlab.mpcdf.mpg.de/nomad-lab/nomad-meta-info/wikis/metainfo/method-
to-method-kind)). See also [energy_current wiki
page](https://gitlab.mpcdf.mpg.de/nomad-lab/nomad-meta-info/wikis/metainfo/energy-
current)."""^^xsd:string ;
    rdfs:subClassOf [ a owl:Restriction ;
            owl:allValuesFrom <http://emmo.info/emmo/middle/siunits#EMMO_8a70dea4_d6ab_4260_b931_a3e990982416> ;
            owl:onProperty <http://emmo.info/emmo/middle/metrology#EMMO_67fc0a36_8dcb_4ffa_9a43_31074efa3296> ],
        [ a owl:Restriction ;
            owl:onProperty :hasCategory ;
            owl:someValuesFrom :energy_component ],
        [ a owl:Restriction ;
            owl:onProperty :hasCategory ;
            owl:someValuesFrom :energy_total_potential ],
        [ a owl:Restriction ;
            owl:allValuesFrom <http://emmo.info/emmo/middle/math#EMMO_18d180e4_5e3e_42f7_820c_e08951223486> ;
            owl:onProperty :hasDatatype ],
        [ a owl:Restriction ;
            owl:hasValue 0 ;
            owl:onProperty :hasNumberOfDimensions ],
        [ a owl:Restriction ;
            owl:onProperty :hasCategory ;
            owl:someValuesFrom :energy_value ],
        :NMI_quantity .

:energy_electrostatic a owl:Class ;
    rdfs:comment """Total electrostatic energy (nuclei + electrons), defined consistently with
calculation_method."""^^xsd:string ;
    rdfs:subClassOf [ a owl:Restriction ;
            owl:hasValue 0 ;
            owl:onProperty :hasNumberOfDimensions ],
        [ a owl:Restriction ;
            owl:onProperty :hasCategory ;
            owl:someValuesFrom :energy_value ],
        [ a owl:Restriction ;
            owl:allValuesFrom <http://emmo.info/emmo/middle/math#EMMO_18d180e4_5e3e_42f7_820c_e08951223486> ;
            owl:onProperty :hasDatatype ],
        [ a owl:Restriction ;
            owl:allValuesFrom <http://emmo.info/emmo/middle/siunits#EMMO_8a70dea4_d6ab_4260_b931_a3e990982416> ;
            owl:onProperty <http://emmo.info/emmo/middle/metrology#EMMO_67fc0a36_8dcb_4ffa_9a43_31074efa3296> ],
        [ a owl:Restriction ;
            owl:onProperty :hasCategory ;
            owl:someValuesFrom :energy_component ],
        :NMI_quantity .

:energy_electrostatic_scf_iteration a owl:Class ;
    rdfs:comment """Total electrostatic energy (nuclei + electrons) during each self-consistent field
(SCF) iteration."""^^xsd:string ;
    rdfs:subClassOf [ a owl:Restriction ;
            owl:onProperty :hasCategory ;
            owl:someValuesFrom :energy_component ],
        [ a owl:Restriction ;
            owl:allValuesFrom <http://emmo.info/emmo/middle/math#EMMO_18d180e4_5e3e_42f7_820c_e08951223486> ;
            owl:onProperty :hasDatatype ],
        [ a owl:Restriction ;
            owl:onProperty :hasCategory ;
            owl:someValuesFrom :energy_value ],
        [ a owl:Restriction ;
            owl:allValuesFrom <http://emmo.info/emmo/middle/siunits#EMMO_8a70dea4_d6ab_4260_b931_a3e990982416> ;
            owl:onProperty <http://emmo.info/emmo/middle/metrology#EMMO_67fc0a36_8dcb_4ffa_9a43_31074efa3296> ],
        [ a owl:Restriction ;
            owl:hasValue 0 ;
            owl:onProperty :hasNumberOfDimensions ],
        :NMI_quantity .

:energy_free a owl:Class ;
    rdfs:comment """Free energy (nuclei + electrons) (whose minimum gives the smeared occupation
density calculated with smearing_kind) calculated with the method described in
XC_method."""^^xsd:string ;
    rdfs:subClassOf [ a owl:Restriction ;
            owl:allValuesFrom <http://emmo.info/emmo/middle/siunits#EMMO_8a70dea4_d6ab_4260_b931_a3e990982416> ;
            owl:onProperty <http://emmo.info/emmo/middle/metrology#EMMO_67fc0a36_8dcb_4ffa_9a43_31074efa3296> ],
        [ a owl:Restriction ;
            owl:onProperty :hasCategory ;
            owl:someValuesFrom :energy_value ],
        [ a owl:Restriction ;
            owl:onProperty :hasCategory ;
            owl:someValuesFrom :energy_total_potential ],
        [ a owl:Restriction ;
            owl:hasValue 0 ;
            owl:onProperty :hasNumberOfDimensions ],
        [ a owl:Restriction ;
            owl:onProperty :hasCategory ;
            owl:someValuesFrom :energy_component ],
        [ a owl:Restriction ;
            owl:allValuesFrom <http://emmo.info/emmo/middle/math#EMMO_18d180e4_5e3e_42f7_820c_e08951223486> ;
            owl:onProperty :hasDatatype ],
        :NMI_quantity .

:energy_free_per_atom a owl:Class ;
    rdfs:comment """Free energy per atom (whose minimum gives the smeared occupation density
calculated with smearing_kind) calculated with XC_method."""^^xsd:string ;
    rdfs:subClassOf [ a owl:Restriction ;
            owl:allValuesFrom <http://emmo.info/emmo/middle/math#EMMO_18d180e4_5e3e_42f7_820c_e08951223486> ;
            owl:onProperty :hasDatatype ],
        [ a owl:Restriction ;
            owl:allValuesFrom <http://emmo.info/emmo/middle/siunits#EMMO_8a70dea4_d6ab_4260_b931_a3e990982416> ;
            owl:onProperty <http://emmo.info/emmo/middle/metrology#EMMO_67fc0a36_8dcb_4ffa_9a43_31074efa3296> ],
        [ a owl:Restriction ;
            owl:onProperty :hasCategory ;
            owl:someValuesFrom :energy_value ],
        [ a owl:Restriction ;
            owl:onProperty :hasCategory ;
            owl:someValuesFrom :energy_component_per_atom ],
        [ a owl:Restriction ;
            owl:hasValue 0 ;
            owl:onProperty :hasNumberOfDimensions ],
        :NMI_quantity .

:energy_free_per_atom_scf_iteration a owl:Class ;
    rdfs:comment """Free energy per atom (whose minimum gives the smeared occupation density
calculated with smearing_kind) calculated with XC_method during the self-
consistent field (SCF) iterations."""^^xsd:string ;
    rdfs:subClassOf [ a owl:Restriction ;
            owl:onProperty :hasCategory ;
            owl:someValuesFrom :energy_value ],
        [ a owl:Restriction ;
            owl:hasValue 0 ;
            owl:onProperty :hasNumberOfDimensions ],
        [ a owl:Restriction ;
            owl:allValuesFrom <http://emmo.info/emmo/middle/math#EMMO_18d180e4_5e3e_42f7_820c_e08951223486> ;
            owl:onProperty :hasDatatype ],
        [ a owl:Restriction ;
            owl:onProperty :hasCategory ;
            owl:someValuesFrom :energy_component_per_atom ],
        [ a owl:Restriction ;
            owl:allValuesFrom <http://emmo.info/emmo/middle/siunits#EMMO_8a70dea4_d6ab_4260_b931_a3e990982416> ;
            owl:onProperty <http://emmo.info/emmo/middle/metrology#EMMO_67fc0a36_8dcb_4ffa_9a43_31074efa3296> ],
        :NMI_quantity .

:energy_free_scf_iteration a owl:Class ;
    rdfs:comment """Free energy (whose minimum gives the smeared occupation density calculated with
smearing_kind) calculated with the method described in XC_method during the self-
consistent field (SCF) iterations."""^^xsd:string ;
    rdfs:subClassOf [ a owl:Restriction ;
            owl:allValuesFrom <http://emmo.info/emmo/middle/math#EMMO_18d180e4_5e3e_42f7_820c_e08951223486> ;
            owl:onProperty :hasDatatype ],
        [ a owl:Restriction ;
            owl:onProperty :hasCategory ;
            owl:someValuesFrom :energy_value ],
        [ a owl:Restriction ;
            owl:onProperty :hasCategory ;
            owl:someValuesFrom :energy_total_potential ],
        [ a owl:Restriction ;
            owl:allValuesFrom <http://emmo.info/emmo/middle/siunits#EMMO_8a70dea4_d6ab_4260_b931_a3e990982416> ;
            owl:onProperty <http://emmo.info/emmo/middle/metrology#EMMO_67fc0a36_8dcb_4ffa_9a43_31074efa3296> ],
        [ a owl:Restriction ;
            owl:onProperty :hasCategory ;
            owl:someValuesFrom :energy_component ],
        [ a owl:Restriction ;
            owl:hasValue 0 ;
            owl:onProperty :hasNumberOfDimensions ],
        :NMI_quantity .

:energy_hartree_error a owl:Class ;
    rdfs:comment """Error in the Hartree (electrostatic) potential energy. Defined consistently with
XC_method."""^^xsd:string ;
    rdfs:subClassOf [ a owl:Restriction ;
            owl:hasValue 0 ;
            owl:onProperty :hasNumberOfDimensions ],
        [ a owl:Restriction ;
            owl:onProperty :hasCategory ;
            owl:someValuesFrom :energy_value ],
        [ a owl:Restriction ;
            owl:onProperty :hasCategory ;
            owl:someValuesFrom :error_estimate_contribution ],
        [ a owl:Restriction ;
            owl:allValuesFrom <http://emmo.info/emmo/middle/math#EMMO_18d180e4_5e3e_42f7_820c_e08951223486> ;
            owl:onProperty :hasDatatype ],
        [ a owl:Restriction ;
            owl:allValuesFrom <http://emmo.info/emmo/middle/siunits#EMMO_8a70dea4_d6ab_4260_b931_a3e990982416> ;
            owl:onProperty <http://emmo.info/emmo/middle/metrology#EMMO_67fc0a36_8dcb_4ffa_9a43_31074efa3296> ],
        :NMI_quantity .

:energy_hartree_error_scf_iteration a owl:Class ;
    rdfs:comment """Error in the Hartree (electrostatic) potential energy during each self-consistent
field (SCF) iteration. Defined consistently with XC_method."""^^xsd:string ;
    rdfs:subClassOf [ a owl:Restriction ;
            owl:hasValue 0 ;
            owl:onProperty :hasNumberOfDimensions ],
        [ a owl:Restriction ;
            owl:onProperty :hasCategory ;
            owl:someValuesFrom :energy_value ],
        [ a owl:Restriction ;
            owl:allValuesFrom <http://emmo.info/emmo/middle/math#EMMO_18d180e4_5e3e_42f7_820c_e08951223486> ;
            owl:onProperty :hasDatatype ],
        [ a owl:Restriction ;
            owl:onProperty :hasCategory ;
            owl:someValuesFrom :error_estimate_contribution ],
        [ a owl:Restriction ;
            owl:allValuesFrom <http://emmo.info/emmo/middle/siunits#EMMO_8a70dea4_d6ab_4260_b931_a3e990982416> ;
            owl:onProperty <http://emmo.info/emmo/middle/metrology#EMMO_67fc0a36_8dcb_4ffa_9a43_31074efa3296> ],
        :NMI_quantity .

:energy_hartree_fock_X a owl:Class ;
    rdfs:comment """Converged exact-exchange (Hartree-Fock) energy. Defined consistently with
XC_method."""^^xsd:string ;
    rdfs:subClassOf [ a owl:Restriction ;
            owl:hasValue 0 ;
            owl:onProperty :hasNumberOfDimensions ],
        [ a owl:Restriction ;
            owl:onProperty :hasCategory ;
            owl:someValuesFrom :energy_component ],
        [ a owl:Restriction ;
            owl:allValuesFrom <http://emmo.info/emmo/middle/math#EMMO_18d180e4_5e3e_42f7_820c_e08951223486> ;
            owl:onProperty :hasDatatype ],
        [ a owl:Restriction ;
            owl:allValuesFrom <http://emmo.info/emmo/middle/siunits#EMMO_8a70dea4_d6ab_4260_b931_a3e990982416> ;
            owl:onProperty <http://emmo.info/emmo/middle/metrology#EMMO_67fc0a36_8dcb_4ffa_9a43_31074efa3296> ],
        [ a owl:Restriction ;
            owl:onProperty :hasCategory ;
            owl:someValuesFrom :energy_type_X ],
        [ a owl:Restriction ;
            owl:onProperty :hasCategory ;
            owl:someValuesFrom :energy_value ],
        :NMI_quantity .

:energy_hartree_fock_X_scaled a owl:Class ;
    rdfs:comment """Scaled exact-exchange energy that depends on the mixing parameter of the
functional. For example in hybrid functionals, the exchange energy is given as a
linear combination of exact-energy and exchange energy of an approximate DFT
functional; the exact exchange energy multiplied by the mixing coefficient of the
hybrid functional would be stored in this metadata. Defined consistently with
XC_method."""^^xsd:string ;
    rdfs:subClassOf [ a owl:Restriction ;
            owl:onProperty :hasCategory ;
            owl:someValuesFrom :energy_value ],
        [ a owl:Restriction ;
            owl:allValuesFrom <http://emmo.info/emmo/middle/math#EMMO_18d180e4_5e3e_42f7_820c_e08951223486> ;
            owl:onProperty :hasDatatype ],
        [ a owl:Restriction ;
            owl:hasValue 0 ;
            owl:onProperty :hasNumberOfDimensions ],
        [ a owl:Restriction ;
            owl:onProperty :hasCategory ;
            owl:someValuesFrom :energy_component ],
        [ a owl:Restriction ;
            owl:allValuesFrom <http://emmo.info/emmo/middle/siunits#EMMO_8a70dea4_d6ab_4260_b931_a3e990982416> ;
            owl:onProperty <http://emmo.info/emmo/middle/metrology#EMMO_67fc0a36_8dcb_4ffa_9a43_31074efa3296> ],
        :NMI_quantity .

:energy_method_current a owl:Class ;
    rdfs:comment """Value of the energy calculated with the method calculation_method_current.
Depending on calculation_method_kind it might be a total energy or only a
correction."""^^xsd:string ;
    rdfs:subClassOf [ a owl:Restriction ;
            owl:onProperty :hasCategory ;
            owl:someValuesFrom :energy_value ],
        [ a owl:Restriction ;
            owl:allValuesFrom <http://emmo.info/emmo/middle/math#EMMO_18d180e4_5e3e_42f7_820c_e08951223486> ;
            owl:onProperty :hasDatatype ],
        [ a owl:Restriction ;
            owl:allValuesFrom <http://emmo.info/emmo/middle/siunits#EMMO_8a70dea4_d6ab_4260_b931_a3e990982416> ;
            owl:onProperty <http://emmo.info/emmo/middle/metrology#EMMO_67fc0a36_8dcb_4ffa_9a43_31074efa3296> ],
        [ a owl:Restriction ;
            owl:onProperty :hasCategory ;
            owl:someValuesFrom :energy_component ],
        [ a owl:Restriction ;
            owl:hasValue 0 ;
            owl:onProperty :hasNumberOfDimensions ],
        :NMI_quantity .

:energy_reference_fermi a owl:Class ;
    rdfs:comment "Fermi energy (separates occupied from unoccupied single-particle states in metals)"^^xsd:string ;
    rdfs:subClassOf [ a owl:Restriction ;
            owl:hasValue 1 ;
            owl:onProperty :hasNumberOfDimensions ],
        [ a owl:Restriction ;
            owl:allValuesFrom <http://emmo.info/emmo/middle/siunits#EMMO_8a70dea4_d6ab_4260_b931_a3e990982416> ;
            owl:onProperty <http://emmo.info/emmo/middle/metrology#EMMO_67fc0a36_8dcb_4ffa_9a43_31074efa3296> ],
        [ a owl:Restriction ;
            owl:onProperty :hasCategory ;
            owl:someValuesFrom :energy_type_reference ],
        [ a owl:Restriction ;
            owl:allValuesFrom <http://emmo.info/emmo/middle/math#EMMO_18d180e4_5e3e_42f7_820c_e08951223486> ;
            owl:onProperty :hasDatatype ],
        [ a owl:Restriction ;
            owl:hasValue :number_of_spin_channels ;
            owl:onProperty :hasVarDim1 ],
        [ a owl:Restriction ;
            owl:onProperty :hasCategory ;
            owl:someValuesFrom :energy_value ],
        :NMI_quantity .

:energy_reference_fermi_iteration a owl:Class ;
    rdfs:comment """Fermi energy (separates occupied from unoccupied single-particle states in metals)
during the self-consistent field (SCF) iterations."""^^xsd:string ;
    rdfs:subClassOf [ a owl:Restriction ;
            owl:hasValue 1 ;
            owl:onProperty :hasNumberOfDimensions ],
        [ a owl:Restriction ;
            owl:hasValue :number_of_spin_channels ;
            owl:onProperty :hasVarDim1 ],
        [ a owl:Restriction ;
            owl:onProperty :hasCategory ;
            owl:someValuesFrom :energy_type_reference ],
        [ a owl:Restriction ;
            owl:onProperty :hasCategory ;
            owl:someValuesFrom :energy_value ],
        [ a owl:Restriction ;
            owl:allValuesFrom <http://emmo.info/emmo/middle/siunits#EMMO_8a70dea4_d6ab_4260_b931_a3e990982416> ;
            owl:onProperty <http://emmo.info/emmo/middle/metrology#EMMO_67fc0a36_8dcb_4ffa_9a43_31074efa3296> ],
        [ a owl:Restriction ;
            owl:allValuesFrom <http://emmo.info/emmo/middle/math#EMMO_18d180e4_5e3e_42f7_820c_e08951223486> ;
            owl:onProperty :hasDatatype ],
        :NMI_quantity .

:energy_reference_highest_occupied a owl:Class ;
    rdfs:comment """Highest occupied single-particle state energy (in insulators or HOMO energy in
finite systems)"""^^xsd:string ;
    rdfs:subClassOf [ a owl:Restriction ;
            owl:hasValue 1 ;
            owl:onProperty :hasNumberOfDimensions ],
        [ a owl:Restriction ;
            owl:hasValue :number_of_spin_channels ;
            owl:onProperty :hasVarDim1 ],
        [ a owl:Restriction ;
            owl:allValuesFrom <http://emmo.info/emmo/middle/math#EMMO_18d180e4_5e3e_42f7_820c_e08951223486> ;
            owl:onProperty :hasDatatype ],
        [ a owl:Restriction ;
            owl:onProperty :hasCategory ;
            owl:someValuesFrom :energy_value ],
        [ a owl:Restriction ;
            owl:onProperty :hasCategory ;
            owl:someValuesFrom :energy_type_reference ],
        [ a owl:Restriction ;
            owl:allValuesFrom <http://emmo.info/emmo/middle/siunits#EMMO_8a70dea4_d6ab_4260_b931_a3e990982416> ;
            owl:onProperty <http://emmo.info/emmo/middle/metrology#EMMO_67fc0a36_8dcb_4ffa_9a43_31074efa3296> ],
        :NMI_quantity .

:energy_reference_highest_occupied_iteration a owl:Class ;
    rdfs:comment """Highest occupied single-particle state energy (in insulators or HOMO energy in
finite systems) during the self-consistent field (SCF) iterations."""^^xsd:string ;
    rdfs:subClassOf [ a owl:Restriction ;
            owl:onProperty :hasCategory ;
            owl:someValuesFrom :energy_value ],
        [ a owl:Restriction ;
            owl:onProperty :hasCategory ;
            owl:someValuesFrom :energy_type_reference ],
        [ a owl:Restriction ;
            owl:allValuesFrom <http://emmo.info/emmo/middle/math#EMMO_18d180e4_5e3e_42f7_820c_e08951223486> ;
            owl:onProperty :hasDatatype ],
        [ a owl:Restriction ;
            owl:hasValue 1 ;
            owl:onProperty :hasNumberOfDimensions ],
        [ a owl:Restriction ;
            owl:hasValue :number_of_spin_channels ;
            owl:onProperty :hasVarDim1 ],
        [ a owl:Restriction ;
            owl:allValuesFrom <http://emmo.info/emmo/middle/siunits#EMMO_8a70dea4_d6ab_4260_b931_a3e990982416> ;
            owl:onProperty <http://emmo.info/emmo/middle/metrology#EMMO_67fc0a36_8dcb_4ffa_9a43_31074efa3296> ],
        :NMI_quantity .

:energy_reference_lowest_unoccupied a owl:Class ;
    rdfs:comment """Lowest unoccupied single-particle state energy (in insulators or LUMO energy in
finite systems)"""^^xsd:string ;
    rdfs:subClassOf [ a owl:Restriction ;
            owl:hasValue :number_of_spin_channels ;
            owl:onProperty :hasVarDim1 ],
        [ a owl:Restriction ;
            owl:hasValue 1 ;
            owl:onProperty :hasNumberOfDimensions ],
        [ a owl:Restriction ;
            owl:allValuesFrom <http://emmo.info/emmo/middle/siunits#EMMO_8a70dea4_d6ab_4260_b931_a3e990982416> ;
            owl:onProperty <http://emmo.info/emmo/middle/metrology#EMMO_67fc0a36_8dcb_4ffa_9a43_31074efa3296> ],
        [ a owl:Restriction ;
            owl:onProperty :hasCategory ;
            owl:someValuesFrom :energy_value ],
        [ a owl:Restriction ;
            owl:allValuesFrom <http://emmo.info/emmo/middle/math#EMMO_18d180e4_5e3e_42f7_820c_e08951223486> ;
            owl:onProperty :hasDatatype ],
        [ a owl:Restriction ;
            owl:onProperty :hasCategory ;
            owl:someValuesFrom :energy_type_reference ],
        :NMI_quantity .

:energy_reference_lowest_unoccupied_iteration a owl:Class ;
    rdfs:comment """Lowest unoccupied single-particle state energy (in insulators or LUMO energy in
finite systems) during the self-consistent field (SCF) iterations."""^^xsd:string ;
    rdfs:subClassOf [ a owl:Restriction ;
            owl:allValuesFrom <http://emmo.info/emmo/middle/siunits#EMMO_8a70dea4_d6ab_4260_b931_a3e990982416> ;
            owl:onProperty <http://emmo.info/emmo/middle/metrology#EMMO_67fc0a36_8dcb_4ffa_9a43_31074efa3296> ],
        [ a owl:Restriction ;
            owl:hasValue :number_of_spin_channels ;
            owl:onProperty :hasVarDim1 ],
        [ a owl:Restriction ;
            owl:onProperty :hasCategory ;
            owl:someValuesFrom :energy_type_reference ],
        [ a owl:Restriction ;
            owl:hasValue 1 ;
            owl:onProperty :hasNumberOfDimensions ],
        [ a owl:Restriction ;
            owl:allValuesFrom <http://emmo.info/emmo/middle/math#EMMO_18d180e4_5e3e_42f7_820c_e08951223486> ;
            owl:onProperty :hasDatatype ],
        [ a owl:Restriction ;
            owl:onProperty :hasCategory ;
            owl:someValuesFrom :energy_value ],
        :NMI_quantity .

:energy_sum_eigenvalues a owl:Class ;
    rdfs:comment "Sum of the eigenvalues of the Hamiltonian matrix defined by XC_method."^^xsd:string ;
    rdfs:subClassOf [ a owl:Restriction ;
            owl:hasValue 0 ;
            owl:onProperty :hasNumberOfDimensions ],
        [ a owl:Restriction ;
            owl:onProperty :hasCategory ;
            owl:someValuesFrom :energy_component ],
        [ a owl:Restriction ;
            owl:allValuesFrom <http://emmo.info/emmo/middle/math#EMMO_18d180e4_5e3e_42f7_820c_e08951223486> ;
            owl:onProperty :hasDatatype ],
        [ a owl:Restriction ;
            owl:onProperty :hasCategory ;
            owl:someValuesFrom :energy_value ],
        [ a owl:Restriction ;
            owl:allValuesFrom <http://emmo.info/emmo/middle/siunits#EMMO_8a70dea4_d6ab_4260_b931_a3e990982416> ;
            owl:onProperty <http://emmo.info/emmo/middle/metrology#EMMO_67fc0a36_8dcb_4ffa_9a43_31074efa3296> ],
        :NMI_quantity .

:energy_sum_eigenvalues_per_atom a owl:Class ;
    rdfs:comment """Value of the energy per atom, where the energy is defined as the sum of the
eigenvalues of the Hamiltonian matrix given by XC_method."""^^xsd:string ;
    rdfs:subClassOf [ a owl:Restriction ;
            owl:onProperty :hasCategory ;
            owl:someValuesFrom :energy_component_per_atom ],
        [ a owl:Restriction ;
            owl:allValuesFrom <http://emmo.info/emmo/middle/siunits#EMMO_8a70dea4_d6ab_4260_b931_a3e990982416> ;
            owl:onProperty <http://emmo.info/emmo/middle/metrology#EMMO_67fc0a36_8dcb_4ffa_9a43_31074efa3296> ],
        [ a owl:Restriction ;
            owl:onProperty :hasCategory ;
            owl:someValuesFrom :energy_value ],
        [ a owl:Restriction ;
            owl:allValuesFrom <http://emmo.info/emmo/middle/math#EMMO_18d180e4_5e3e_42f7_820c_e08951223486> ;
            owl:onProperty :hasDatatype ],
        [ a owl:Restriction ;
            owl:hasValue 0 ;
            owl:onProperty :hasNumberOfDimensions ],
        :NMI_quantity .

:energy_sum_eigenvalues_per_atom_scf_iteration a owl:Class ;
    rdfs:comment """Value of the energy per atom, where the energy is defined as the sum of the
eigenvalues of the Hamiltonian matrix given by XC_method, during each self-
consistent field (SCF) iteration."""^^xsd:string ;
    rdfs:subClassOf [ a owl:Restriction ;
            owl:allValuesFrom <http://emmo.info/emmo/middle/siunits#EMMO_8a70dea4_d6ab_4260_b931_a3e990982416> ;
            owl:onProperty <http://emmo.info/emmo/middle/metrology#EMMO_67fc0a36_8dcb_4ffa_9a43_31074efa3296> ],
        [ a owl:Restriction ;
            owl:allValuesFrom <http://emmo.info/emmo/middle/math#EMMO_18d180e4_5e3e_42f7_820c_e08951223486> ;
            owl:onProperty :hasDatatype ],
        [ a owl:Restriction ;
            owl:hasValue 0 ;
            owl:onProperty :hasNumberOfDimensions ],
        [ a owl:Restriction ;
            owl:onProperty :hasCategory ;
            owl:someValuesFrom :energy_component_per_atom ],
        [ a owl:Restriction ;
            owl:onProperty :hasCategory ;
            owl:someValuesFrom :energy_value ],
        :NMI_quantity .

:energy_sum_eigenvalues_scf_iteration a owl:Class ;
    rdfs:comment """Sum of the eigenvalues of the Hamiltonian matrix defined by XC_method, during each
self-consistent field (SCF) iteration."""^^xsd:string ;
    rdfs:subClassOf [ a owl:Restriction ;
            owl:onProperty :hasCategory ;
            owl:someValuesFrom :energy_component ],
        [ a owl:Restriction ;
            owl:hasValue 0 ;
            owl:onProperty :hasNumberOfDimensions ],
        [ a owl:Restriction ;
            owl:onProperty :hasCategory ;
            owl:someValuesFrom :energy_value ],
        [ a owl:Restriction ;
            owl:allValuesFrom <http://emmo.info/emmo/middle/siunits#EMMO_8a70dea4_d6ab_4260_b931_a3e990982416> ;
            owl:onProperty <http://emmo.info/emmo/middle/metrology#EMMO_67fc0a36_8dcb_4ffa_9a43_31074efa3296> ],
        [ a owl:Restriction ;
            owl:allValuesFrom <http://emmo.info/emmo/middle/math#EMMO_18d180e4_5e3e_42f7_820c_e08951223486> ;
            owl:onProperty :hasDatatype ],
        :NMI_quantity .

:energy_total a owl:Class ;
    rdfs:comment """Value of the total energy, calculated with the method described in XC_method and
extrapolated to $T=0$, based on a free-electron gas argument."""^^xsd:string ;
    rdfs:subClassOf [ a owl:Restriction ;
            owl:allValuesFrom <http://emmo.info/emmo/middle/siunits#EMMO_8a70dea4_d6ab_4260_b931_a3e990982416> ;
            owl:onProperty <http://emmo.info/emmo/middle/metrology#EMMO_67fc0a36_8dcb_4ffa_9a43_31074efa3296> ],
        [ a owl:Restriction ;
            owl:onProperty :hasCategory ;
            owl:someValuesFrom :energy_value ],
        [ a owl:Restriction ;
            owl:onProperty :hasCategory ;
            owl:someValuesFrom :energy_total_potential ],
        [ a owl:Restriction ;
            owl:allValuesFrom <http://emmo.info/emmo/middle/math#EMMO_18d180e4_5e3e_42f7_820c_e08951223486> ;
            owl:onProperty :hasDatatype ],
        [ a owl:Restriction ;
            owl:hasValue 0 ;
            owl:onProperty :hasNumberOfDimensions ],
        [ a owl:Restriction ;
            owl:onProperty :hasCategory ;
            owl:someValuesFrom :energy_component ],
        :NMI_quantity .

:energy_total_T0 a owl:Class ;
    rdfs:comment """Value of the total energy (or equivalently free energy), calculated with the
method described in XC_method and extrapolated to $T=0$, based on a free-electron
gas argument."""^^xsd:string ;
    rdfs:subClassOf [ a owl:Restriction ;
            owl:allValuesFrom <http://emmo.info/emmo/middle/math#EMMO_18d180e4_5e3e_42f7_820c_e08951223486> ;
            owl:onProperty :hasDatatype ],
        [ a owl:Restriction ;
            owl:onProperty :hasCategory ;
            owl:someValuesFrom :energy_total_potential ],
        [ a owl:Restriction ;
            owl:allValuesFrom <http://emmo.info/emmo/middle/siunits#EMMO_8a70dea4_d6ab_4260_b931_a3e990982416> ;
            owl:onProperty <http://emmo.info/emmo/middle/metrology#EMMO_67fc0a36_8dcb_4ffa_9a43_31074efa3296> ],
        [ a owl:Restriction ;
            owl:onProperty :hasCategory ;
            owl:someValuesFrom :energy_value ],
        [ a owl:Restriction ;
            owl:hasValue 0 ;
            owl:onProperty :hasNumberOfDimensions ],
        [ a owl:Restriction ;
            owl:onProperty :hasCategory ;
            owl:someValuesFrom :energy_component ],
        :NMI_quantity .

:energy_total_T0_per_atom a owl:Class ;
    rdfs:comment """Value of the total energy, calculated with the method described in XC_method per
atom extrapolated to $T=0$, based on a free-electron gas argument."""^^xsd:string ;
    rdfs:subClassOf [ a owl:Restriction ;
            owl:onProperty :hasCategory ;
            owl:someValuesFrom :energy_value ],
        [ a owl:Restriction ;
            owl:allValuesFrom <http://emmo.info/emmo/middle/siunits#EMMO_8a70dea4_d6ab_4260_b931_a3e990982416> ;
            owl:onProperty <http://emmo.info/emmo/middle/metrology#EMMO_67fc0a36_8dcb_4ffa_9a43_31074efa3296> ],
        [ a owl:Restriction ;
            owl:onProperty :hasCategory ;
            owl:someValuesFrom :energy_total_potential_per_atom ],
        [ a owl:Restriction ;
            owl:onProperty :hasCategory ;
            owl:someValuesFrom :energy_component ],
        [ a owl:Restriction ;
            owl:allValuesFrom <http://emmo.info/emmo/middle/math#EMMO_18d180e4_5e3e_42f7_820c_e08951223486> ;
            owl:onProperty :hasDatatype ],
        [ a owl:Restriction ;
            owl:hasValue 0 ;
            owl:onProperty :hasNumberOfDimensions ],
        :NMI_quantity .

:energy_total_T0_per_atom_scf_iteration a owl:Class ;
    rdfs:comment """Value of the total energy, calculated with the method described in XC_method per
atom extrapolated to $T=0$, based on a free-electron gas argument, during each
self-consistent field (SCF) iteration."""^^xsd:string ;
    rdfs:subClassOf [ a owl:Restriction ;
            owl:onProperty :hasCategory ;
            owl:someValuesFrom :energy_component ],
        [ a owl:Restriction ;
            owl:onProperty :hasCategory ;
            owl:someValuesFrom :energy_total_potential_per_atom ],
        [ a owl:Restriction ;
            owl:allValuesFrom <http://emmo.info/emmo/middle/math#EMMO_18d180e4_5e3e_42f7_820c_e08951223486> ;
            owl:onProperty :hasDatatype ],
        [ a owl:Restriction ;
            owl:onProperty :hasCategory ;
            owl:someValuesFrom :energy_value ],
        [ a owl:Restriction ;
            owl:allValuesFrom <http://emmo.info/emmo/middle/siunits#EMMO_8a70dea4_d6ab_4260_b931_a3e990982416> ;
            owl:onProperty <http://emmo.info/emmo/middle/metrology#EMMO_67fc0a36_8dcb_4ffa_9a43_31074efa3296> ],
        [ a owl:Restriction ;
            owl:hasValue 0 ;
            owl:onProperty :hasNumberOfDimensions ],
        :NMI_quantity .

:energy_total_T0_scf_iteration a owl:Class ;
    rdfs:comment """Value of the total energy (or equivalently free energy), calculated with the
method described in XC_method and extrapolated to $T=0$, based on a free-electron
gas argument, during each self-consistent field (SCF) iteration."""^^xsd:string ;
    rdfs:subClassOf [ a owl:Restriction ;
            owl:allValuesFrom <http://emmo.info/emmo/middle/math#EMMO_18d180e4_5e3e_42f7_820c_e08951223486> ;
            owl:onProperty :hasDatatype ],
        [ a owl:Restriction ;
            owl:allValuesFrom <http://emmo.info/emmo/middle/siunits#EMMO_8a70dea4_d6ab_4260_b931_a3e990982416> ;
            owl:onProperty <http://emmo.info/emmo/middle/metrology#EMMO_67fc0a36_8dcb_4ffa_9a43_31074efa3296> ],
        [ a owl:Restriction ;
            owl:onProperty :hasCategory ;
            owl:someValuesFrom :energy_value ],
        [ a owl:Restriction ;
            owl:onProperty :hasCategory ;
            owl:someValuesFrom :energy_component ],
        [ a owl:Restriction ;
            owl:onProperty :hasCategory ;
            owl:someValuesFrom :energy_total_potential ],
        [ a owl:Restriction ;
            owl:hasValue 0 ;
            owl:onProperty :hasNumberOfDimensions ],
        :NMI_quantity .

:energy_total_scf_iteration a owl:Class ;
    rdfs:comment """Value of the total electronic energy calculated with the method described in
XC_method during each self-consistent field (SCF) iteration."""^^xsd:string ;
    rdfs:subClassOf [ a owl:Restriction ;
            owl:allValuesFrom <http://emmo.info/emmo/middle/math#EMMO_18d180e4_5e3e_42f7_820c_e08951223486> ;
            owl:onProperty :hasDatatype ],
        [ a owl:Restriction ;
            owl:hasValue 0 ;
            owl:onProperty :hasNumberOfDimensions ],
        [ a owl:Restriction ;
            owl:onProperty :hasCategory ;
            owl:someValuesFrom :energy_component ],
        [ a owl:Restriction ;
            owl:onProperty :hasCategory ;
            owl:someValuesFrom :energy_value ],
        [ a owl:Restriction ;
            owl:onProperty :hasCategory ;
            owl:someValuesFrom :energy_total_potential ],
        [ a owl:Restriction ;
            owl:allValuesFrom <http://emmo.info/emmo/middle/siunits#EMMO_8a70dea4_d6ab_4260_b931_a3e990982416> ;
            owl:onProperty <http://emmo.info/emmo/middle/metrology#EMMO_67fc0a36_8dcb_4ffa_9a43_31074efa3296> ],
        :NMI_quantity .

:energy_van_der_Waals a owl:Class ;
    rdfs:comment """Value for the converged van der Waals energy calculated using the method described
in van_der_Waals_method, and used in energy_current. This is the van der Waals
method consistent with, e.g., forces used for relaxation or dynamics. Alternative
methods are listed in section_energy_van_der_Waals."""^^xsd:string ;
    rdfs:subClassOf [ a owl:Restriction ;
            owl:onProperty :hasCategory ;
            owl:someValuesFrom :energy_type_van_der_Waals ],
        [ a owl:Restriction ;
            owl:hasValue 0 ;
            owl:onProperty :hasNumberOfDimensions ],
        [ a owl:Restriction ;
            owl:onProperty :hasCategory ;
            owl:someValuesFrom :energy_value ],
        [ a owl:Restriction ;
            owl:allValuesFrom <http://emmo.info/emmo/middle/math#EMMO_18d180e4_5e3e_42f7_820c_e08951223486> ;
            owl:onProperty :hasDatatype ],
        [ a owl:Restriction ;
            owl:allValuesFrom <http://emmo.info/emmo/middle/siunits#EMMO_8a70dea4_d6ab_4260_b931_a3e990982416> ;
            owl:onProperty <http://emmo.info/emmo/middle/metrology#EMMO_67fc0a36_8dcb_4ffa_9a43_31074efa3296> ],
        [ a owl:Restriction ;
            owl:onProperty :hasCategory ;
            owl:someValuesFrom :energy_component ],
        :NMI_quantity .

:energy_van_der_Waals_kind a owl:Class ;
    rdfs:comment """Method used to compute van der Waals energy stored in energy_van_der_Waals_value.
This metadata is used when more than one van der Waals method is applied in the
same *single configuration calculation* (see
section_single_configuration_calculation). The method used for van der Waals  (the
one consistent with energy_current and, e.g., for evaluating the forces for a
relaxation or dynamics) is defined in settings_van_der_Waals."""^^xsd:string ;
    rdfs:subClassOf [ a owl:Restriction ;
            owl:hasValue 0 ;
            owl:onProperty :hasNumberOfDimensions ],
        [ a owl:Restriction ;
            owl:allValuesFrom <http://emmo.info/emmo/middle/perceptual#EMMO_50ea1ec5_f157_41b0_b46b_a9032f17ca10> ;
            owl:onProperty :hasDatatype ],
        :NMI_quantity .

:energy_van_der_Waals_value a owl:Class ;
    rdfs:comment """Value of van der Waals energy, calculated with the method defined in
energy_van_der_Waals_kind. This metadata is used when more than one van der Waals
method is applied in the same *single configuration calculation* (see
section_single_configuration_calculation). The value of the van der Waals energy
consistent with energy_current and used, e.g., for evaluating the forces for a
relaxation or dynamics, is given in energy_van_der_Waals and defined in
settings_van_der_Waals."""^^xsd:string ;
    rdfs:subClassOf [ a owl:Restriction ;
            owl:allValuesFrom <http://emmo.info/emmo/middle/siunits#EMMO_8a70dea4_d6ab_4260_b931_a3e990982416> ;
            owl:onProperty <http://emmo.info/emmo/middle/metrology#EMMO_67fc0a36_8dcb_4ffa_9a43_31074efa3296> ],
        [ a owl:Restriction ;
            owl:onProperty :hasCategory ;
            owl:someValuesFrom :energy_component ],
        [ a owl:Restriction ;
            owl:hasValue 0 ;
            owl:onProperty :hasNumberOfDimensions ],
        [ a owl:Restriction ;
            owl:onProperty :hasCategory ;
            owl:someValuesFrom :energy_type_van_der_Waals ],
        [ a owl:Restriction ;
            owl:allValuesFrom <http://emmo.info/emmo/middle/math#EMMO_18d180e4_5e3e_42f7_820c_e08951223486> ;
            owl:onProperty :hasDatatype ],
        [ a owl:Restriction ;
            owl:onProperty :hasCategory ;
            owl:someValuesFrom :energy_value ],
        :NMI_quantity .

:energy_zero_point a owl:Class ;
    rdfs:comment """Value for the converged zero-point vibrations energy calculated using the method
described in zero_point_method , and used in energy_current ."""^^xsd:string ;
    rdfs:subClassOf [ a owl:Restriction ;
            owl:allValuesFrom <http://emmo.info/emmo/middle/math#EMMO_18d180e4_5e3e_42f7_820c_e08951223486> ;
            owl:onProperty :hasDatatype ],
        [ a owl:Restriction ;
            owl:hasValue 0 ;
            owl:onProperty :hasNumberOfDimensions ],
        :NMI_quantity .

:ensemble_type a owl:Class ;
    rdfs:comment """Kind of sampled ensemble stored in section_frame_sequence; valid values are
defined in [ensemble_type wiki page](https://gitlab.mpcdf.mpg.de/nomad-lab/nomad-
meta-info/wikis/metainfo/ensemble-type)."""^^xsd:string ;
    rdfs:subClassOf [ a owl:Restriction ;
            owl:hasValue 0 ;
            owl:onProperty :hasNumberOfDimensions ],
        [ a owl:Restriction ;
            owl:allValuesFrom <http://emmo.info/emmo/middle/perceptual#EMMO_50ea1ec5_f157_41b0_b46b_a9032f17ca10> ;
            owl:onProperty :hasDatatype ],
        :NMI_quantity .

:equivalent_atoms_original a owl:Class ;
    rdfs:comment """Gives a mapping table of atoms to symmetrically independent atoms in the original
cell. This is used to find symmetrically equivalent atoms."""^^xsd:string ;
    rdfs:subClassOf [ a owl:Restriction ;
            owl:hasValue :number_of_atoms ;
            owl:onProperty :hasVarDim1 ],
        [ a owl:Restriction ;
            owl:allValuesFrom <http://emmo.info/emmo/middle/math#EMMO_f8bd64d5_5d3e_4ad4_a46e_c30714fecb7f> ;
            owl:onProperty :hasDatatype ],
        [ a owl:Restriction ;
            owl:hasValue 1 ;
            owl:onProperty :hasNumberOfDimensions ],
        :NMI_quantity .

:equivalent_atoms_primitive a owl:Class ;
    rdfs:comment """Gives a mapping table of atoms to symmetrically independent atoms in the primitive
cell. This is used to find symmetrically equivalent atoms."""^^xsd:string ;
    rdfs:subClassOf [ a owl:Restriction ;
            owl:hasValue :number_of_atoms_primitive ;
            owl:onProperty :hasVarDim1 ],
        [ a owl:Restriction ;
            owl:hasValue 1 ;
            owl:onProperty :hasNumberOfDimensions ],
        [ a owl:Restriction ;
            owl:allValuesFrom <http://emmo.info/emmo/middle/math#EMMO_f8bd64d5_5d3e_4ad4_a46e_c30714fecb7f> ;
            owl:onProperty :hasDatatype ],
        :NMI_quantity .

:equivalent_atoms_std a owl:Class ;
    rdfs:comment """Gives a mapping table of atoms to symmetrically independent atoms in the
standardized cell. This is used to find symmetrically equivalent atoms."""^^xsd:string ;
    rdfs:subClassOf [ a owl:Restriction ;
            owl:allValuesFrom <http://emmo.info/emmo/middle/math#EMMO_f8bd64d5_5d3e_4ad4_a46e_c30714fecb7f> ;
            owl:onProperty :hasDatatype ],
        [ a owl:Restriction ;
            owl:hasValue :number_of_atoms_std ;
            owl:onProperty :hasVarDim1 ],
        [ a owl:Restriction ;
            owl:hasValue 1 ;
            owl:onProperty :hasNumberOfDimensions ],
        :NMI_quantity .

:excitation_energies a owl:Class ;
    rdfs:comment "Excitation energies."^^xsd:string ;
    rdfs:subClassOf [ a owl:Restriction ;
            owl:allValuesFrom <http://emmo.info/emmo/middle/math#EMMO_18d180e4_5e3e_42f7_820c_e08951223486> ;
            owl:onProperty :hasDatatype ],
        [ a owl:Restriction ;
            owl:hasValue 1 ;
            owl:onProperty :hasNumberOfDimensions ],
        [ a owl:Restriction ;
            owl:onProperty :hasCategory ;
            owl:someValuesFrom :energy_value ],
        [ a owl:Restriction ;
            owl:hasValue :number_of_excited_states ;
            owl:onProperty :hasVarDim1 ],
        :NMI_quantity .

:faces a owl:Class ;
    rdfs:comment """The faces of the Brillouin zone polyhedron as vertex indices. The
surface normal is determined by a right-hand ordering of the points."""^^xsd:string ;
    rdfs:subClassOf [ a owl:Restriction ;
            owl:allValuesFrom <http://emmo.info/emmo/middle/math#EMMO_f8bd64d5_5d3e_4ad4_a46e_c30714fecb7f> ;
            owl:onProperty :hasDatatype ],
        [ a owl:Restriction ;
            owl:hasValue 2 ;
            owl:onProperty :hasNumberOfDimensions ],
        :NMI_quantity .

:filling_factor a owl:Class ;
    rdfs:comment "Proportion of 1 bins in the DOS fingerprint."^^xsd:string ;
    rdfs:subClassOf [ a owl:Restriction ;
            owl:allValuesFrom <http://emmo.info/emmo/middle/math#EMMO_18d180e4_5e3e_42f7_820c_e08951223486> ;
            owl:onProperty :hasDatatype ],
        [ a owl:Restriction ;
            owl:hasValue 0 ;
            owl:onProperty :hasNumberOfDimensions ],
        :NMI_quantity .

:frame_sequence_conserved_quantity a owl:Class ;
    rdfs:comment """Array containing the values of a quantity that should be conserved,  along a
sequence of frames (i.e., a trajectory). A frame is one
section_single_configuration_calculation), for example the total energy in the NVE
ensemble. If not all frames have a value the indices of the frames that have a
value are stored in frame_sequence_conserved_quantity_frames."""^^xsd:string ;
    rdfs:subClassOf [ a owl:Restriction ;
            owl:hasValue :number_of_conserved_quantity_evaluations_in_sequence ;
            owl:onProperty :hasVarDim1 ],
        [ a owl:Restriction ;
            owl:hasValue 1 ;
            owl:onProperty :hasNumberOfDimensions ],
        [ a owl:Restriction ;
            owl:allValuesFrom <http://emmo.info/emmo/middle/math#EMMO_18d180e4_5e3e_42f7_820c_e08951223486> ;
            owl:onProperty :hasDatatype ],
        [ a owl:Restriction ;
            owl:allValuesFrom <http://emmo.info/emmo/middle/siunits#EMMO_8a70dea4_d6ab_4260_b931_a3e990982416> ;
            owl:onProperty <http://emmo.info/emmo/middle/metrology#EMMO_67fc0a36_8dcb_4ffa_9a43_31074efa3296> ],
        :NMI_quantity .

:frame_sequence_conserved_quantity_frames a owl:Class ;
    rdfs:comment """Array containing the strictly increasing indices of the frames the
frame_sequence_conserved_quantity values refers to. If not given it defaults to
the trivial mapping 0,1,..."""^^xsd:string ;
    rdfs:subClassOf [ a owl:Restriction ;
            owl:hasValue 1 ;
            owl:onProperty :hasNumberOfDimensions ],
        [ a owl:Restriction ;
            owl:allValuesFrom <http://emmo.info/emmo/middle/math#EMMO_f8bd64d5_5d3e_4ad4_a46e_c30714fecb7f> ;
            owl:onProperty :hasDatatype ],
        [ a owl:Restriction ;
            owl:hasValue :number_of_conserved_quantity_evaluations_in_sequence ;
            owl:onProperty :hasVarDim1 ],
        :NMI_quantity .

:frame_sequence_conserved_quantity_stats a owl:Class ;
    rdfs:comment """Average value of energy-like frame_sequence_conserved_quantity, and its standard
deviation, over this sequence of frames (i.e., a trajectory, a frame is one
section_single_configuration_calculation)."""^^xsd:string ;
    rdfs:subClassOf [ a owl:Restriction ;
            owl:hasValue 1 ;
            owl:onProperty :hasNumberOfDimensions ],
        [ a owl:Restriction ;
            owl:hasValue 2 ;
            owl:onProperty :hasFixDim1 ],
        [ a owl:Restriction ;
            owl:allValuesFrom <http://emmo.info/emmo/middle/math#EMMO_18d180e4_5e3e_42f7_820c_e08951223486> ;
            owl:onProperty :hasDatatype ],
        [ a owl:Restriction ;
            owl:allValuesFrom <http://emmo.info/emmo/middle/siunits#EMMO_8a70dea4_d6ab_4260_b931_a3e990982416> ;
            owl:onProperty <http://emmo.info/emmo/middle/metrology#EMMO_67fc0a36_8dcb_4ffa_9a43_31074efa3296> ],
        :NMI_quantity .

:frame_sequence_continuation_kind a owl:Class ;
    rdfs:comment """Type of continuation that has been performed from the previous sequence of frames
(i.e., a trajectory, a frame is one section_single_configuration_calculation),
upon restart."""^^xsd:string ;
    rdfs:subClassOf [ a owl:Restriction ;
            owl:hasValue 0 ;
            owl:onProperty :hasNumberOfDimensions ],
        :NMI_quantity .

:frame_sequence_external_url a owl:Class ;
    rdfs:comment """If the energy, forces, and other quantities for the frames (a frame is one
section_single_configuration_calculation) in  section_frame_sequence are obtained
by calling a different code than the code that drives the sequence (e.g., a
wrapper that drives a molecular dynamics, Monte Carlo, geometry optimization and
calls an electronic-structure code for energy and forces for each configuration),
this metadata holds the reference to where the
section_single_configuration_calculation for each frame are located. The format
for this reference is described in the [frame_sequence_external_url wiki
page](https://gitlab.mpcdf.mpg.de/nomad-lab/nomad-meta-info/wikis/metainfo/frame-
sequence-external-url)."""^^xsd:string ;
    rdfs:subClassOf [ a owl:Restriction ;
            owl:hasValue 0 ;
            owl:onProperty :hasNumberOfDimensions ],
        [ a owl:Restriction ;
            owl:allValuesFrom <http://emmo.info/emmo/middle/perceptual#EMMO_50ea1ec5_f157_41b0_b46b_a9032f17ca10> ;
            owl:onProperty :hasDatatype ],
        :NMI_quantity .

:frame_sequence_kinetic_energy a owl:Class ;
    rdfs:comment """Array containing the values of the kinetic energy along this sequence of frames
(i.e., a trajectory, a frame is one section_single_configuration_calculation). If
not all frames have a value the indices of the frames that have a value are stored
in frame_sequence_kinetic_energy_frames."""^^xsd:string ;
    rdfs:subClassOf [ a owl:Restriction ;
            owl:allValuesFrom <http://emmo.info/emmo/middle/siunits#EMMO_8a70dea4_d6ab_4260_b931_a3e990982416> ;
            owl:onProperty <http://emmo.info/emmo/middle/metrology#EMMO_67fc0a36_8dcb_4ffa_9a43_31074efa3296> ],
        [ a owl:Restriction ;
            owl:allValuesFrom <http://emmo.info/emmo/middle/math#EMMO_18d180e4_5e3e_42f7_820c_e08951223486> ;
            owl:onProperty :hasDatatype ],
        [ a owl:Restriction ;
            owl:hasValue 1 ;
            owl:onProperty :hasNumberOfDimensions ],
        [ a owl:Restriction ;
            owl:hasValue :number_of_kinetic_energies_in_sequence ;
            owl:onProperty :hasVarDim1 ],
        :NMI_quantity .

:frame_sequence_kinetic_energy_frames a owl:Class ;
    rdfs:comment """Array containing the strictly increasing indices referring to the frames of
frame_sequence_kinetic_energy. If not given it defaults to the trivial mapping
0,1,..."""^^xsd:string ;
    rdfs:subClassOf [ a owl:Restriction ;
            owl:hasValue 1 ;
            owl:onProperty :hasNumberOfDimensions ],
        [ a owl:Restriction ;
            owl:allValuesFrom <http://emmo.info/emmo/middle/math#EMMO_f8bd64d5_5d3e_4ad4_a46e_c30714fecb7f> ;
            owl:onProperty :hasDatatype ],
        [ a owl:Restriction ;
            owl:hasValue :number_of_kinetic_energies_in_sequence ;
            owl:onProperty :hasVarDim1 ],
        :NMI_quantity .

:frame_sequence_kinetic_energy_stats a owl:Class ;
    rdfs:comment """Average kinetic energy and its standard deviation over this sequence of frames
(i.e., a trajectory, a frame is one section_single_configuration_calculation)."""^^xsd:string ;
    rdfs:subClassOf [ a owl:Restriction ;
            owl:hasValue 1 ;
            owl:onProperty :hasNumberOfDimensions ],
        [ a owl:Restriction ;
            owl:allValuesFrom <http://emmo.info/emmo/middle/math#EMMO_18d180e4_5e3e_42f7_820c_e08951223486> ;
            owl:onProperty :hasDatatype ],
        [ a owl:Restriction ;
            owl:hasValue 2 ;
            owl:onProperty :hasFixDim1 ],
        [ a owl:Restriction ;
            owl:allValuesFrom <http://emmo.info/emmo/middle/siunits#EMMO_8a70dea4_d6ab_4260_b931_a3e990982416> ;
            owl:onProperty <http://emmo.info/emmo/middle/metrology#EMMO_67fc0a36_8dcb_4ffa_9a43_31074efa3296> ],
        :NMI_quantity .

:frame_sequence_local_frames_ref a owl:Class ;
    rdfs:comment """Reference from each frame (a frame is one
section_single_configuration_calculation) in this section_frame_sequence to the
corresponding section_single_configuration_calculation. Each
section_frame_sequence binds a collection of
section_single_configuration_calculation, because they all belong to, e.g., a
molecular dynamics trajectory, or geometry optimization. The full information for
each frame is stored in section_single_configuration_calculation and this metadata
establishes the link for each frame."""^^xsd:string ;
    rdfs:subClassOf [ a owl:Restriction ;
            owl:hasValue 1 ;
            owl:onProperty :hasNumberOfDimensions ],
        [ a owl:Restriction ;
            owl:hasValue :number_of_frames_in_sequence ;
            owl:onProperty :hasVarDim1 ],
        :NMI_quantity .

:frame_sequence_potential_energy a owl:Class ;
    rdfs:comment """Array containing the value of the potential energy along this sequence of frames
(i.e., a trajectory, a frame is one section_single_configuration_calculation).
This is equal to energy_total of the corresponding
section_single_configuration_calculation and repeated here in a summary array for
easier access. If not all frames have a value the indices of the frames that have
a value are stored in frame_sequence_potential_energy_frames."""^^xsd:string ;
    rdfs:subClassOf [ a owl:Restriction ;
            owl:allValuesFrom <http://emmo.info/emmo/middle/siunits#EMMO_8a70dea4_d6ab_4260_b931_a3e990982416> ;
            owl:onProperty <http://emmo.info/emmo/middle/metrology#EMMO_67fc0a36_8dcb_4ffa_9a43_31074efa3296> ],
        [ a owl:Restriction ;
            owl:allValuesFrom <http://emmo.info/emmo/middle/math#EMMO_18d180e4_5e3e_42f7_820c_e08951223486> ;
            owl:onProperty :hasDatatype ],
        [ a owl:Restriction ;
            owl:hasValue :number_of_potential_energies_in_sequence ;
            owl:onProperty :hasVarDim1 ],
        [ a owl:Restriction ;
            owl:hasValue 1 ;
            owl:onProperty :hasNumberOfDimensions ],
        :NMI_quantity .

:frame_sequence_potential_energy_frames a owl:Class ;
    rdfs:comment """Array containing the strictly increasing indices referring to the frames of
frame_sequence_potential_energy. If not given it defaults to the trivial mapping
0,1,..."""^^xsd:string ;
    rdfs:subClassOf [ a owl:Restriction ;
            owl:hasValue :number_of_potential_energies_in_sequence ;
            owl:onProperty :hasVarDim1 ],
        [ a owl:Restriction ;
            owl:hasValue 1 ;
            owl:onProperty :hasNumberOfDimensions ],
        [ a owl:Restriction ;
            owl:allValuesFrom <http://emmo.info/emmo/middle/math#EMMO_f8bd64d5_5d3e_4ad4_a46e_c30714fecb7f> ;
            owl:onProperty :hasDatatype ],
        :NMI_quantity .

:frame_sequence_potential_energy_stats a owl:Class ;
    rdfs:comment """Average potential energy and its standard deviation over this sequence of frames
(i.e., a trajectory, a frame is one section_single_configuration_calculation)."""^^xsd:string ;
    rdfs:subClassOf [ a owl:Restriction ;
            owl:hasValue 2 ;
            owl:onProperty :hasFixDim1 ],
        [ a owl:Restriction ;
            owl:allValuesFrom <http://emmo.info/emmo/middle/siunits#EMMO_8a70dea4_d6ab_4260_b931_a3e990982416> ;
            owl:onProperty <http://emmo.info/emmo/middle/metrology#EMMO_67fc0a36_8dcb_4ffa_9a43_31074efa3296> ],
        [ a owl:Restriction ;
            owl:allValuesFrom <http://emmo.info/emmo/middle/math#EMMO_18d180e4_5e3e_42f7_820c_e08951223486> ;
            owl:onProperty :hasDatatype ],
        [ a owl:Restriction ;
            owl:hasValue 1 ;
            owl:onProperty :hasNumberOfDimensions ],
        :NMI_quantity .

:frame_sequence_pressure a owl:Class ;
    rdfs:comment """Array containing the values of the pressure (one third of the trace of the stress
tensor) along this sequence of frames (a frame is one
section_single_configuration_calculation). If not all frames have a value the
indices of the frames that have a value are stored in
frame_sequence_pressure_frames."""^^xsd:string ;
    rdfs:subClassOf [ a owl:Restriction ;
            owl:allValuesFrom <http://emmo.info/emmo/middle/math#EMMO_18d180e4_5e3e_42f7_820c_e08951223486> ;
            owl:onProperty :hasDatatype ],
        [ a owl:Restriction ;
            owl:hasValue :number_of_pressure_evaluations_in_sequence ;
            owl:onProperty :hasVarDim1 ],
        [ a owl:Restriction ;
            owl:hasValue 1 ;
            owl:onProperty :hasNumberOfDimensions ],
        [ a owl:Restriction ;
            owl:allValuesFrom <http://emmo.info/emmo/middle/siunits#EMMO_a80dc6f5_b1aa_41a7_a3a8_cd5040da2162> ;
            owl:onProperty <http://emmo.info/emmo/middle/metrology#EMMO_67fc0a36_8dcb_4ffa_9a43_31074efa3296> ],
        :NMI_quantity .

:frame_sequence_pressure_frames a owl:Class ;
    rdfs:comment """Array containing the strictly increasing indices referring to the frames of
frame_sequence_pressure. If not given it defaults to the trivial mapping 0,1,..."""^^xsd:string ;
    rdfs:subClassOf [ a owl:Restriction ;
            owl:hasValue :number_of_pressure_evaluations_in_sequence ;
            owl:onProperty :hasVarDim1 ],
        [ a owl:Restriction ;
            owl:hasValue 1 ;
            owl:onProperty :hasNumberOfDimensions ],
        [ a owl:Restriction ;
            owl:allValuesFrom <http://emmo.info/emmo/middle/math#EMMO_f8bd64d5_5d3e_4ad4_a46e_c30714fecb7f> ;
            owl:onProperty :hasDatatype ],
        :NMI_quantity .

:frame_sequence_pressure_stats a owl:Class ;
    rdfs:comment """Average pressure (one third of the trace of the stress tensor) and standard
deviation over this sequence of frames (i.e., a trajectory, a frame is one
section_single_configuration_calculation)."""^^xsd:string ;
    rdfs:subClassOf [ a owl:Restriction ;
            owl:allValuesFrom <http://emmo.info/emmo/middle/math#EMMO_18d180e4_5e3e_42f7_820c_e08951223486> ;
            owl:onProperty :hasDatatype ],
        [ a owl:Restriction ;
            owl:hasValue 1 ;
            owl:onProperty :hasNumberOfDimensions ],
        [ a owl:Restriction ;
            owl:hasValue 2 ;
            owl:onProperty :hasFixDim1 ],
        [ a owl:Restriction ;
            owl:allValuesFrom <http://emmo.info/emmo/middle/siunits#EMMO_a80dc6f5_b1aa_41a7_a3a8_cd5040da2162> ;
            owl:onProperty <http://emmo.info/emmo/middle/metrology#EMMO_67fc0a36_8dcb_4ffa_9a43_31074efa3296> ],
        :NMI_quantity .

:frame_sequence_temperature a owl:Class ;
    rdfs:comment """Array containing the values of the instantaneous temperature (a quantity,
proportional to frame_sequence_kinetic_energy, whose ensemble average equals the
thermodynamic temperature) along this sequence of frames (i.e., a trajectory, a
frame is one section_single_configuration_calculation). If not all frames have a
value the indices of the frames that have a value are stored in
frame_sequence_temperature_frames."""^^xsd:string ;
    rdfs:subClassOf [ a owl:Restriction ;
            owl:allValuesFrom <http://emmo.info/emmo/middle/siunits#EMMO_2e5e45fc_f52c_4294_bdc2_5ed7a06dfce7> ;
            owl:onProperty <http://emmo.info/emmo/middle/metrology#EMMO_67fc0a36_8dcb_4ffa_9a43_31074efa3296> ],
        [ a owl:Restriction ;
            owl:hasValue :number_of_temperatures_in_sequence ;
            owl:onProperty :hasVarDim1 ],
        [ a owl:Restriction ;
            owl:hasValue 1 ;
            owl:onProperty :hasNumberOfDimensions ],
        [ a owl:Restriction ;
            owl:allValuesFrom <http://emmo.info/emmo/middle/math#EMMO_18d180e4_5e3e_42f7_820c_e08951223486> ;
            owl:onProperty :hasDatatype ],
        :NMI_quantity .

:frame_sequence_temperature_frames a owl:Class ;
    rdfs:comment """Array containing the strictly increasing indices referring to the frames of
frame_sequence_temperature. If not given it defaults to the trivial mapping
0,1,..."""^^xsd:string ;
    rdfs:subClassOf [ a owl:Restriction ;
            owl:hasValue 1 ;
            owl:onProperty :hasNumberOfDimensions ],
        [ a owl:Restriction ;
            owl:hasValue :number_of_temperatures_in_sequence ;
            owl:onProperty :hasVarDim1 ],
        [ a owl:Restriction ;
            owl:allValuesFrom <http://emmo.info/emmo/middle/math#EMMO_f8bd64d5_5d3e_4ad4_a46e_c30714fecb7f> ;
            owl:onProperty :hasDatatype ],
        :NMI_quantity .

:frame_sequence_temperature_stats a owl:Class ;
    rdfs:comment """Average temperature and its standard deviation over this sequence of frames (i.e.,
a trajectory, a frame is one section_single_configuration_calculation)."""^^xsd:string ;
    rdfs:subClassOf [ a owl:Restriction ;
            owl:hasValue 1 ;
            owl:onProperty :hasNumberOfDimensions ],
        [ a owl:Restriction ;
            owl:allValuesFrom <http://emmo.info/emmo/middle/siunits#EMMO_2e5e45fc_f52c_4294_bdc2_5ed7a06dfce7> ;
            owl:onProperty <http://emmo.info/emmo/middle/metrology#EMMO_67fc0a36_8dcb_4ffa_9a43_31074efa3296> ],
        [ a owl:Restriction ;
            owl:hasValue 2 ;
            owl:onProperty :hasFixDim1 ],
        [ a owl:Restriction ;
            owl:allValuesFrom <http://emmo.info/emmo/middle/math#EMMO_18d180e4_5e3e_42f7_820c_e08951223486> ;
            owl:onProperty :hasDatatype ],
        :NMI_quantity .

:frame_sequence_time a owl:Class ;
    rdfs:comment """Time along this sequence of frames (i.e., a trajectory, a frame is one
section_single_configuration_calculation). Time start is arbitrary, but when a
sequence is a continuation of another time should be continued too."""^^xsd:string ;
    rdfs:subClassOf [ a owl:Restriction ;
            owl:hasValue 1 ;
            owl:onProperty :hasNumberOfDimensions ],
        [ a owl:Restriction ;
            owl:hasValue :number_of_frames_in_sequence ;
            owl:onProperty :hasVarDim1 ],
        [ a owl:Restriction ;
            owl:allValuesFrom <http://emmo.info/emmo/middle/math#EMMO_18d180e4_5e3e_42f7_820c_e08951223486> ;
            owl:onProperty :hasDatatype ],
        [ a owl:Restriction ;
            owl:allValuesFrom <http://emmo.info/emmo/middle/siunits#EMMO_314ba716_2d3d_4462_9a4f_d3419ae1df43> ;
            owl:onProperty <http://emmo.info/emmo/middle/metrology#EMMO_67fc0a36_8dcb_4ffa_9a43_31074efa3296> ],
        :NMI_quantity .

:frame_sequence_to_sampling_ref a owl:Class ;
    rdfs:comment """Reference from the present section_frame_sequence to the section_sampling_method,
that defines the parameters used in this sequence of frames (i.e., a trajectory, a
frame is one section_single_configuration_calculation)."""^^xsd:string ;
    rdfs:subClassOf [ a owl:Restriction ;
            owl:hasValue 0 ;
            owl:onProperty :hasNumberOfDimensions ],
        :NMI_quantity .

:frame_sequence_user_quantity a owl:Class ;
    rdfs:comment """Array containing the values of the user-defined quantity defined in
frame_sequence_user_quantity_name, evaluated along this sequence of frames (i.e.,
trajectory, a frame is one section_single_configuration_calculation). If not all
frames have a value the indices of the frames that have a value are stored in
frame_sequence_kinetic_energy_frames. If not all frames have a value the indices
of the frames that have a value are stored in
frame_sequence_kinetic_energy_frames."""^^xsd:string ;
    rdfs:subClassOf [ a owl:Restriction ;
            owl:hasValue 2 ;
            owl:onProperty :hasNumberOfDimensions ],
        [ a owl:Restriction ;
            owl:allValuesFrom <http://emmo.info/emmo/middle/math#EMMO_18d180e4_5e3e_42f7_820c_e08951223486> ;
            owl:onProperty :hasDatatype ],
        [ a owl:Restriction ;
            owl:hasValue :number_of_frame_sequence_user_quantity_components ;
            owl:onProperty :hasVarDim2 ],
        [ a owl:Restriction ;
            owl:hasValue :number_of_user_quantity_evaluations_in_sequence ;
            owl:onProperty :hasVarDim1 ],
        :NMI_quantity .

:frame_sequence_user_quantity_frames a owl:Class ;
    rdfs:comment """Array containing the strictly increasing indices referring to the frames of
frame_sequence_user_quantity. If not given it defaults to the trivial mapping
0,1,..."""^^xsd:string ;
    rdfs:subClassOf [ a owl:Restriction ;
            owl:hasValue :number_of_user_quantity_evaluations_in_sequence ;
            owl:onProperty :hasVarDim1 ],
        [ a owl:Restriction ;
            owl:hasValue 1 ;
            owl:onProperty :hasNumberOfDimensions ],
        [ a owl:Restriction ;
            owl:allValuesFrom <http://emmo.info/emmo/middle/math#EMMO_f8bd64d5_5d3e_4ad4_a46e_c30714fecb7f> ;
            owl:onProperty :hasDatatype ],
        :NMI_quantity .

:frame_sequence_user_quantity_name a owl:Class ;
    rdfs:comment """Descriptive name of a user-defined quantity, sampled along this sequence of frames
(i.e., a trajectory, a frame is one section_single_configuration_calculation).
Dedicated metadata are created for the conserved energy-like quantity
(frame_sequence_conserved_quantity), the kinetic and potential energies
(frame_sequence_kinetic_energy and frame_sequence_potential_energy), the
instantaneous temperature (frame_sequence_temperature) and pressure
(frame_sequence_pressure). This metadata should be used for other quantities that
are monitored along a sequence of frames."""^^xsd:string ;
    rdfs:subClassOf [ a owl:Restriction ;
            owl:hasValue 0 ;
            owl:onProperty :hasNumberOfDimensions ],
        [ a owl:Restriction ;
            owl:allValuesFrom <http://emmo.info/emmo/middle/perceptual#EMMO_50ea1ec5_f157_41b0_b46b_a9032f17ca10> ;
            owl:onProperty :hasDatatype ],
        :NMI_quantity .

:frame_sequence_user_quantity_stats a owl:Class ;
    rdfs:comment """Average of frame_sequence_user_quantity and its standard deviation in this
sequence of frames (i.e., a trajectory, a frame is one
section_single_configuration_calculation)."""^^xsd:string ;
    rdfs:subClassOf [ a owl:Restriction ;
            owl:allValuesFrom <http://emmo.info/emmo/middle/math#EMMO_18d180e4_5e3e_42f7_820c_e08951223486> ;
            owl:onProperty :hasDatatype ],
        [ a owl:Restriction ;
            owl:hasValue 2 ;
            owl:onProperty :hasFixDim1 ],
        [ a owl:Restriction ;
            owl:hasValue :number_of_frame_sequence_user_quantity_components ;
            owl:onProperty :hasVarDim2 ],
        [ a owl:Restriction ;
            owl:hasValue 2 ;
            owl:onProperty :hasNumberOfDimensions ],
        :NMI_quantity .

:gaussian_basis_group_contractions a owl:Class ;
    rdfs:comment """contraction coefficients $c_{i j}$ defining the contracted basis functions with
respect to *normalized* primitive Gaussian functions. They define the Gaussian
basis functions as described in section_gaussian_basis_group."""^^xsd:string ;
    rdfs:subClassOf [ a owl:Restriction ;
            owl:hasValue 2 ;
            owl:onProperty :hasNumberOfDimensions ],
        [ a owl:Restriction ;
            owl:hasValue :number_of_gaussian_basis_group_exponents ;
            owl:onProperty :hasVarDim2 ],
        [ a owl:Restriction ;
            owl:allValuesFrom <http://emmo.info/emmo/middle/math#EMMO_18d180e4_5e3e_42f7_820c_e08951223486> ;
            owl:onProperty :hasDatatype ],
        [ a owl:Restriction ;
            owl:hasValue :number_of_gaussian_basis_group_contractions ;
            owl:onProperty :hasVarDim1 ],
        :NMI_quantity .

:gaussian_basis_group_exponents a owl:Class ;
    rdfs:comment """Exponents $\\alpha_j$ of the Gaussian functions defining this basis set
$exp(-\\alpha_j r^2)$. One should be careful about the units of the coefficients."""^^xsd:string ;
    rdfs:subClassOf [ a owl:Restriction ;
            owl:hasValue 1 ;
            owl:onProperty :hasNumberOfDimensions ],
        [ a owl:Restriction ;
            owl:hasValue :number_of_gaussian_basis_group_exponents ;
            owl:onProperty :hasVarDim1 ],
        [ a owl:Restriction ;
            owl:allValuesFrom <http://emmo.info/emmo/middle/math#EMMO_18d180e4_5e3e_42f7_820c_e08951223486> ;
            owl:onProperty :hasDatatype ],
        [ a owl:Restriction ;
            owl:allValuesFrom <https://nomad-coe.eu/ontology/properties#PerSquareMetre> ;
            owl:onProperty <http://emmo.info/emmo/middle/metrology#EMMO_67fc0a36_8dcb_4ffa_9a43_31074efa3296> ],
        :NMI_quantity .

:gaussian_basis_group_ls a owl:Class ;
    rdfs:comment """Azimuthal quantum number ($l$) values (of the angular part given by the spherical
harmonic $Y_{l m}$ of the various contracted basis functions)."""^^xsd:string ;
    rdfs:subClassOf [ a owl:Restriction ;
            owl:hasValue :number_of_gaussian_basis_group_contractions ;
            owl:onProperty :hasVarDim1 ],
        [ a owl:Restriction ;
            owl:hasValue 1 ;
            owl:onProperty :hasNumberOfDimensions ],
        [ a owl:Restriction ;
            owl:allValuesFrom <http://emmo.info/emmo/middle/math#EMMO_18d180e4_5e3e_42f7_820c_e08951223486> ;
            owl:onProperty :hasDatatype ],
        :NMI_quantity .

:geometry_optimization_converged a owl:Class ;
    rdfs:comment "Arrays specify whether a geometry optimization is converged."^^xsd:string ;
    rdfs:subClassOf [ a owl:Restriction ;
            owl:allValuesFrom <http://emmo.info/emmo/middle/math#EMMO_54dc83cb_06e1_4739_9e45_bc09cead7f48> ;
            owl:onProperty :hasDatatype ],
        [ a owl:Restriction ;
            owl:hasValue 0 ;
            owl:onProperty :hasNumberOfDimensions ],
        :NMI_quantity .

:geometry_optimization_energy_change a owl:Class ;
    rdfs:comment """Value of threshold for the energy_total change between two geometry optimization
steps, as convergence criterion of the geometry_optimization_method. A geometry
optimization is considered converged when the energy_total change between two
geometry optimization steps is below the threshold (possibly in combination with
other criteria)"""^^xsd:string ;
    rdfs:subClassOf [ a owl:Restriction ;
            owl:allValuesFrom <http://emmo.info/emmo/middle/siunits#EMMO_8a70dea4_d6ab_4260_b931_a3e990982416> ;
            owl:onProperty <http://emmo.info/emmo/middle/metrology#EMMO_67fc0a36_8dcb_4ffa_9a43_31074efa3296> ],
        [ a owl:Restriction ;
            owl:onProperty :hasCategory ;
            owl:someValuesFrom :settings_geometry_optimization ],
        [ a owl:Restriction ;
            owl:hasValue 0 ;
            owl:onProperty :hasNumberOfDimensions ],
        [ a owl:Restriction ;
            owl:allValuesFrom <http://emmo.info/emmo/middle/math#EMMO_18d180e4_5e3e_42f7_820c_e08951223486> ;
            owl:onProperty :hasDatatype ],
        [ a owl:Restriction ;
            owl:onProperty :hasCategory ;
            owl:someValuesFrom :settings_sampling ],
        :NMI_quantity .

:geometry_optimization_geometry_change a owl:Class ;
    rdfs:comment """Value of threshold for the displacement of the nuclei between two geometry
optimization steps as convergence criterion of the geometry_optimization_method. A
geometry optimization is considered converged when the maximum among the
displacements of the nuclei between two geometry optimization steps is below the
threshold (possibly in combination with other criteria)"""^^xsd:string ;
    rdfs:subClassOf [ a owl:Restriction ;
            owl:allValuesFrom <http://emmo.info/emmo/middle/math#EMMO_18d180e4_5e3e_42f7_820c_e08951223486> ;
            owl:onProperty :hasDatatype ],
        [ a owl:Restriction ;
            owl:onProperty :hasCategory ;
            owl:someValuesFrom :settings_geometry_optimization ],
        [ a owl:Restriction ;
            owl:hasValue 0 ;
            owl:onProperty :hasNumberOfDimensions ],
        [ a owl:Restriction ;
            owl:allValuesFrom <http://emmo.info/emmo/middle/siunits#EMMO_7db11dbf_a643_464a_9b56_07eabcc3e9c5> ;
            owl:onProperty <http://emmo.info/emmo/middle/metrology#EMMO_67fc0a36_8dcb_4ffa_9a43_31074efa3296> ],
        [ a owl:Restriction ;
            owl:onProperty :hasCategory ;
            owl:someValuesFrom :settings_sampling ],
        :NMI_quantity .

:geometry_optimization_method a owl:Class ;
    rdfs:comment """Algorithm for the geometry optimization. Allowed values are listed in the
[geometry_optimization_method wiki page](https://gitlab.mpcdf.mpg.de/nomad-
lab/nomad-meta-info/wikis/metainfo/geometry-optimization-method)."""^^xsd:string ;
    rdfs:subClassOf [ a owl:Restriction ;
            owl:hasValue 0 ;
            owl:onProperty :hasNumberOfDimensions ],
        [ a owl:Restriction ;
            owl:onProperty :hasCategory ;
            owl:someValuesFrom :settings_geometry_optimization ],
        [ a owl:Restriction ;
            owl:allValuesFrom <http://emmo.info/emmo/middle/perceptual#EMMO_50ea1ec5_f157_41b0_b46b_a9032f17ca10> ;
            owl:onProperty :hasDatatype ],
        [ a owl:Restriction ;
            owl:onProperty :hasCategory ;
            owl:someValuesFrom :settings_sampling ],
        :NMI_quantity .

:geometry_optimization_threshold_force a owl:Class ;
    rdfs:comment """Value of threshold for the force modulus as convergence criterion of the
geometry_optimization_method. A geometry optimization is considered converged when
the maximum of the moduli of the force on each of the atoms is below this
threshold (possibly in combination with other criteria)"""^^xsd:string ;
    rdfs:subClassOf [ a owl:Restriction ;
            owl:allValuesFrom <http://emmo.info/emmo/middle/siunits#EMMO_a979c531_f9fa_4a6e_93c1.0.0-alpha2960241ca6> ;
            owl:onProperty <http://emmo.info/emmo/middle/metrology#EMMO_67fc0a36_8dcb_4ffa_9a43_31074efa3296> ],
        [ a owl:Restriction ;
            owl:onProperty :hasCategory ;
            owl:someValuesFrom :settings_sampling ],
        [ a owl:Restriction ;
            owl:onProperty :hasCategory ;
            owl:someValuesFrom :settings_geometry_optimization ],
        [ a owl:Restriction ;
            owl:allValuesFrom <http://emmo.info/emmo/middle/math#EMMO_18d180e4_5e3e_42f7_820c_e08951223486> ;
            owl:onProperty :hasDatatype ],
        [ a owl:Restriction ;
            owl:hasValue 0 ;
            owl:onProperty :hasNumberOfDimensions ],
        :NMI_quantity .

:grid_id a owl:Class ;
    rdfs:comment """Identifier of the DOS grid that was used for the creation of the fingerprint.
Similarity can only be calculated if the same grid was used for both fingerprints."""^^xsd:string ;
    rdfs:subClassOf [ a owl:Restriction ;
            owl:allValuesFrom <http://emmo.info/emmo/middle/perceptual#EMMO_50ea1ec5_f157_41b0_b46b_a9032f17ca10> ;
            owl:onProperty :hasDatatype ],
        [ a owl:Restriction ;
            owl:hasValue 0 ;
            owl:onProperty :hasNumberOfDimensions ],
        :NMI_quantity .

:gw_bare_coulomb_cutofftype a owl:Class ;
    rdfs:comment """Cutoff type for the calculation of the bare Coulomb potential: none, 0d, 1d, 2d.
See Rozzi et al., PRB 73, 205119 (2006)"""^^xsd:string ;
    rdfs:subClassOf [ a owl:Restriction ;
            owl:hasValue 0 ;
            owl:onProperty :hasNumberOfDimensions ],
        [ a owl:Restriction ;
            owl:allValuesFrom <http://emmo.info/emmo/middle/perceptual#EMMO_50ea1ec5_f157_41b0_b46b_a9032f17ca10> ;
            owl:onProperty :hasDatatype ],
        :NMI_quantity .

:gw_bare_coulomb_gmax a owl:Class ;
    rdfs:comment "Maximum G for the pw basis for the Coulomb potential."^^xsd:string ;
    rdfs:subClassOf [ a owl:Restriction ;
            owl:allValuesFrom <http://emmo.info/emmo/middle/math#EMMO_18d180e4_5e3e_42f7_820c_e08951223486> ;
            owl:onProperty :hasDatatype ],
        [ a owl:Restriction ;
            owl:allValuesFrom <https://nomad-coe.eu/ontology/properties#PerMetre> ;
            owl:onProperty <http://emmo.info/emmo/middle/metrology#EMMO_67fc0a36_8dcb_4ffa_9a43_31074efa3296> ],
        [ a owl:Restriction ;
            owl:hasValue 0 ;
            owl:onProperty :hasNumberOfDimensions ],
        :NMI_quantity .

:gw_basis_set a owl:Class ;
    rdfs:comment """Auxillary basis set used for non-local operators: mixed - mixed basis set, Kotani
and Schilfgaarde, Solid State Comm. 121, 461 (2002)."""^^xsd:string ;
    rdfs:subClassOf [ a owl:Restriction ;
            owl:allValuesFrom <http://emmo.info/emmo/middle/perceptual#EMMO_50ea1ec5_f157_41b0_b46b_a9032f17ca10> ;
            owl:onProperty :hasDatatype ],
        [ a owl:Restriction ;
            owl:hasValue 0 ;
            owl:onProperty :hasNumberOfDimensions ],
        :NMI_quantity .

:gw_core_treatment a owl:Class ;
    rdfs:comment """It specifies whether the core states are treated in the GW calculation: all - All
electron calculation; val - Valence electron only calculation; vab - Core
electrons are excluded from the mixed product basis; xal - All electron treatment
of the exchange self-energy only"""^^xsd:string ;
    rdfs:subClassOf [ a owl:Restriction ;
            owl:allValuesFrom <http://emmo.info/emmo/middle/perceptual#EMMO_50ea1ec5_f157_41b0_b46b_a9032f17ca10> ;
            owl:onProperty :hasDatatype ],
        [ a owl:Restriction ;
            owl:hasValue 0 ;
            owl:onProperty :hasNumberOfDimensions ],
        :NMI_quantity .

:gw_fermi_energy a owl:Class ;
    rdfs:comment "GW Fermi energy"^^xsd:string ;
    rdfs:subClassOf [ a owl:Restriction ;
            owl:allValuesFrom <http://emmo.info/emmo/middle/siunits#EMMO_8a70dea4_d6ab_4260_b931_a3e990982416> ;
            owl:onProperty <http://emmo.info/emmo/middle/metrology#EMMO_67fc0a36_8dcb_4ffa_9a43_31074efa3296> ],
        [ a owl:Restriction ;
            owl:hasValue 0 ;
            owl:onProperty :hasNumberOfDimensions ],
        [ a owl:Restriction ;
            owl:allValuesFrom <http://emmo.info/emmo/middle/math#EMMO_18d180e4_5e3e_42f7_820c_e08951223486> ;
            owl:onProperty :hasDatatype ],
        :NMI_quantity .

:gw_frequency_grid_type a owl:Class ;
    rdfs:comment """Frequency integration grid type for the correlational self energy: 'eqdis' -
equidistant frequencies from 0 to freqmax; 'gaulag' - Gauss-Laguerre quadrature
from 0 to infinity; 'gauleg' - Gauss-Legendre quadrature from 0 to freqmax;
'gaule2' (default) - double Gauss-Legendre quadrature from 0 to freqmax and from
freqmax to infinity."""^^xsd:string ;
    rdfs:subClassOf [ a owl:Restriction ;
            owl:hasValue 0 ;
            owl:onProperty :hasNumberOfDimensions ],
        [ a owl:Restriction ;
            owl:allValuesFrom <http://emmo.info/emmo/middle/perceptual#EMMO_50ea1ec5_f157_41b0_b46b_a9032f17ca10> ;
            owl:onProperty :hasDatatype ],
        :NMI_quantity .

:gw_frequency_number a owl:Class ;
    rdfs:comment "Number referring to the frequency used in the calculation of the self energy."^^xsd:string ;
    rdfs:subClassOf [ a owl:Restriction ;
            owl:allValuesFrom <http://emmo.info/emmo/middle/math#EMMO_f8bd64d5_5d3e_4ad4_a46e_c30714fecb7f> ;
            owl:onProperty <http://emmo.info/emmo/middle/metrology#EMMO_67fc0a36_8dcb_4ffa_9a43_31074efa3296> ],
        [ a owl:Restriction ;
            owl:hasValue 0 ;
            owl:onProperty :hasNumberOfDimensions ],
        [ a owl:Restriction ;
            owl:allValuesFrom <http://emmo.info/emmo/middle/math#EMMO_f8bd64d5_5d3e_4ad4_a46e_c30714fecb7f> ;
            owl:onProperty :hasDatatype ],
        :NMI_dimension,
        :NMI_quantity .

:gw_frequency_values a owl:Class ;
    rdfs:comment "Values of the frequency used in the calculation of the self energy."^^xsd:string ;
    rdfs:subClassOf [ a owl:Restriction ;
            owl:allValuesFrom <http://emmo.info/emmo/middle/siunits#EMMO_8a70dea4_d6ab_4260_b931_a3e990982416> ;
            owl:onProperty <http://emmo.info/emmo/middle/metrology#EMMO_67fc0a36_8dcb_4ffa_9a43_31074efa3296> ],
        [ a owl:Restriction ;
            owl:hasValue 0 ;
            owl:onProperty :hasNumberOfDimensions ],
        [ a owl:Restriction ;
            owl:allValuesFrom <http://emmo.info/emmo/middle/math#EMMO_18d180e4_5e3e_42f7_820c_e08951223486> ;
            owl:onProperty :hasDatatype ],
        :NMI_quantity .

:gw_frequency_weights a owl:Class ;
    rdfs:comment "Weights of the frequency used in the calculation of the self energy."^^xsd:string ;
    rdfs:subClassOf [ a owl:Restriction ;
            owl:allValuesFrom <http://emmo.info/emmo/middle/math#EMMO_18d180e4_5e3e_42f7_820c_e08951223486> ;
            owl:onProperty :hasDatatype ],
        [ a owl:Restriction ;
            owl:hasValue 0 ;
            owl:onProperty :hasNumberOfDimensions ],
        :NMI_quantity .

:gw_fundamental_gap a owl:Class ;
    rdfs:comment "GW fundamental band gap"^^xsd:string ;
    rdfs:subClassOf [ a owl:Restriction ;
            owl:hasValue 0 ;
            owl:onProperty :hasNumberOfDimensions ],
        [ a owl:Restriction ;
            owl:allValuesFrom <http://emmo.info/emmo/middle/siunits#EMMO_8a70dea4_d6ab_4260_b931_a3e990982416> ;
            owl:onProperty <http://emmo.info/emmo/middle/metrology#EMMO_67fc0a36_8dcb_4ffa_9a43_31074efa3296> ],
        [ a owl:Restriction ;
            owl:allValuesFrom <http://emmo.info/emmo/middle/math#EMMO_18d180e4_5e3e_42f7_820c_e08951223486> ;
            owl:onProperty :hasDatatype ],
        :NMI_quantity .

:gw_max_frequency a owl:Class ;
    rdfs:comment "Maximum frequency for the calculation of the self energy."^^xsd:string ;
    rdfs:subClassOf [ a owl:Restriction ;
            owl:hasValue 0 ;
            owl:onProperty :hasNumberOfDimensions ],
        [ a owl:Restriction ;
            owl:allValuesFrom <http://emmo.info/emmo/middle/math#EMMO_18d180e4_5e3e_42f7_820c_e08951223486> ;
            owl:onProperty :hasDatatype ],
        :NMI_quantity .

:gw_mixed_basis_gmax a owl:Class ;
    rdfs:comment """Cut-off parameter for the truncation of the expansion of the plane waves in the
interstitial region."""^^xsd:string ;
    rdfs:subClassOf [ a owl:Restriction ;
            owl:hasValue 0 ;
            owl:onProperty :hasNumberOfDimensions ],
        [ a owl:Restriction ;
            owl:allValuesFrom <https://nomad-coe.eu/ontology/properties#PerMetre> ;
            owl:onProperty <http://emmo.info/emmo/middle/metrology#EMMO_67fc0a36_8dcb_4ffa_9a43_31074efa3296> ],
        [ a owl:Restriction ;
            owl:allValuesFrom <http://emmo.info/emmo/middle/math#EMMO_18d180e4_5e3e_42f7_820c_e08951223486> ;
            owl:onProperty :hasDatatype ],
        :NMI_quantity .

:gw_mixed_basis_lmax a owl:Class ;
    rdfs:comment "Maximum l value used for the radial functions within the muffin-tin."^^xsd:string ;
    rdfs:subClassOf [ a owl:Restriction ;
            owl:allValuesFrom <http://emmo.info/emmo/middle/math#EMMO_f8bd64d5_5d3e_4ad4_a46e_c30714fecb7f> ;
            owl:onProperty :hasDatatype ],
        [ a owl:Restriction ;
            owl:allValuesFrom <http://emmo.info/emmo/middle/math#EMMO_f8bd64d5_5d3e_4ad4_a46e_c30714fecb7f> ;
            owl:onProperty <http://emmo.info/emmo/middle/metrology#EMMO_67fc0a36_8dcb_4ffa_9a43_31074efa3296> ],
        [ a owl:Restriction ;
            owl:hasValue 0 ;
            owl:onProperty :hasNumberOfDimensions ],
        :NMI_dimension,
        :NMI_quantity .

:gw_mixed_basis_tolerance a owl:Class ;
    rdfs:comment """Eigenvalue threshold below which the egenvectors are discarded in the construction
of the radial basis set."""^^xsd:string ;
    rdfs:subClassOf [ a owl:Restriction ;
            owl:hasValue 0 ;
            owl:onProperty :hasNumberOfDimensions ],
        [ a owl:Restriction ;
            owl:allValuesFrom <http://emmo.info/emmo/middle/math#EMMO_18d180e4_5e3e_42f7_820c_e08951223486> ;
            owl:onProperty :hasDatatype ],
        :NMI_quantity .

:gw_ngridq a owl:Class ;
    rdfs:comment "k/q-point grid size used in the GW calculation."^^xsd:string ;
    rdfs:subClassOf [ a owl:Restriction ;
            owl:hasValue 1 ;
            owl:onProperty :hasNumberOfDimensions ],
        [ a owl:Restriction ;
            owl:hasValue 3 ;
            owl:onProperty :hasFixDim1 ],
        [ a owl:Restriction ;
            owl:allValuesFrom <http://emmo.info/emmo/middle/math#EMMO_f8bd64d5_5d3e_4ad4_a46e_c30714fecb7f> ;
            owl:onProperty :hasDatatype ],
        :NMI_quantity .

:gw_number_of_frequencies a owl:Class ;
    rdfs:comment "Number of frequency points used in the calculation of the self energy."^^xsd:string ;
    rdfs:subClassOf [ a owl:Restriction ;
            owl:allValuesFrom <http://emmo.info/emmo/middle/math#EMMO_f8bd64d5_5d3e_4ad4_a46e_c30714fecb7f> ;
            owl:onProperty :hasDatatype ],
        [ a owl:Restriction ;
            owl:hasValue 0 ;
            owl:onProperty :hasNumberOfDimensions ],
        [ a owl:Restriction ;
            owl:allValuesFrom <http://emmo.info/emmo/middle/math#EMMO_f8bd64d5_5d3e_4ad4_a46e_c30714fecb7f> ;
            owl:onProperty <http://emmo.info/emmo/middle/metrology#EMMO_67fc0a36_8dcb_4ffa_9a43_31074efa3296> ],
        :NMI_dimension,
        :NMI_quantity .

:gw_optical_gap a owl:Class ;
    rdfs:comment "GW optical band gap"^^xsd:string ;
    rdfs:subClassOf [ a owl:Restriction ;
            owl:allValuesFrom <http://emmo.info/emmo/middle/siunits#EMMO_8a70dea4_d6ab_4260_b931_a3e990982416> ;
            owl:onProperty <http://emmo.info/emmo/middle/metrology#EMMO_67fc0a36_8dcb_4ffa_9a43_31074efa3296> ],
        [ a owl:Restriction ;
            owl:allValuesFrom <http://emmo.info/emmo/middle/math#EMMO_18d180e4_5e3e_42f7_820c_e08951223486> ;
            owl:onProperty :hasDatatype ],
        [ a owl:Restriction ;
            owl:hasValue 0 ;
            owl:onProperty :hasNumberOfDimensions ],
        :NMI_quantity .

:gw_polarizability_number_of_empty_states a owl:Class ;
    rdfs:comment "Number of empty states used to compute the polarizability P"^^xsd:string ;
    rdfs:subClassOf [ a owl:Restriction ;
            owl:allValuesFrom <http://emmo.info/emmo/middle/math#EMMO_f8bd64d5_5d3e_4ad4_a46e_c30714fecb7f> ;
            owl:onProperty :hasDatatype ],
        [ a owl:Restriction ;
            owl:hasValue 0 ;
            owl:onProperty :hasNumberOfDimensions ],
        [ a owl:Restriction ;
            owl:allValuesFrom <http://emmo.info/emmo/middle/math#EMMO_f8bd64d5_5d3e_4ad4_a46e_c30714fecb7f> ;
            owl:onProperty <http://emmo.info/emmo/middle/metrology#EMMO_67fc0a36_8dcb_4ffa_9a43_31074efa3296> ],
        :NMI_dimension,
        :NMI_quantity .

:gw_qp_equation_treatment a owl:Class ;
    rdfs:comment "Methods to solve the quasi-particle equation: 'linearization', 'self-consistent'"^^xsd:string ;
    rdfs:subClassOf [ a owl:Restriction ;
            owl:hasValue 0 ;
            owl:onProperty :hasNumberOfDimensions ],
        [ a owl:Restriction ;
            owl:allValuesFrom <http://emmo.info/emmo/middle/perceptual#EMMO_50ea1ec5_f157_41b0_b46b_a9032f17ca10> ;
            owl:onProperty :hasDatatype ],
        :NMI_quantity .

:gw_qp_linearization_prefactor a owl:Class ;
    rdfs:comment "Linearization prefactor"^^xsd:string ;
    rdfs:subClassOf [ a owl:Restriction ;
            owl:hasValue 3 ;
            owl:onProperty :hasNumberOfDimensions ],
        [ a owl:Restriction ;
            owl:allValuesFrom <http://emmo.info/emmo/middle/math#EMMO_18d180e4_5e3e_42f7_820c_e08951223486> ;
            owl:onProperty :hasDatatype ],
        [ a owl:Restriction ;
            owl:hasValue :number_of_eigenvalues ;
            owl:onProperty :hasVarDim3 ],
        [ a owl:Restriction ;
            owl:hasValue :number_of_eigenvalues_kpoints ;
            owl:onProperty :hasVarDim2 ],
        [ a owl:Restriction ;
            owl:hasValue :number_of_spin_channels ;
            owl:onProperty :hasVarDim1 ],
        :NMI_quantity .

:gw_screened_Coulomb a owl:Class ;
    rdfs:comment """Model used to calculate the dinamically-screened Coulomb potential: 'rpa' - Full-
frequency random-phase approximation; 'ppm' - Godby-Needs plasmon-pole model Godby
and Needs, Phys. Rev. Lett. 62, 1169 (1989); 'ppm_hl' - Hybertsen and Louie, Phys.
Rev. B 34, 5390 (1986); 'ppm_lh' - von der Linden and P. Horsh, Phys. Rev. B 37,
8351 (1988); 'ppm_fe' - Farid and Engel, Phys. Rev. B 47,15931 (1993); 'cdm' -
Contour deformation method, Phys. Rev. B 67, 155208 (2003).)"""^^xsd:string ;
    rdfs:subClassOf [ a owl:Restriction ;
            owl:allValuesFrom <http://emmo.info/emmo/middle/perceptual#EMMO_50ea1ec5_f157_41b0_b46b_a9032f17ca10> ;
            owl:onProperty :hasDatatype ],
        [ a owl:Restriction ;
            owl:hasValue 0 ;
            owl:onProperty :hasNumberOfDimensions ],
        :NMI_quantity .

:gw_screened_coulomb_volume_average a owl:Class ;
    rdfs:comment """Type of volume averaging for the dynamically screened Coulomb potential: isotropic
- Simple averaging along a specified direction using only diagonal components of
the dielectric tensor; anisotropic - Anisotropic screening by C. Freysoldt et al.,
CPC 176, 1-13 (2007)"""^^xsd:string ;
    rdfs:subClassOf [ a owl:Restriction ;
            owl:allValuesFrom <http://emmo.info/emmo/middle/perceptual#EMMO_50ea1ec5_f157_41b0_b46b_a9032f17ca10> ;
            owl:onProperty :hasDatatype ],
        [ a owl:Restriction ;
            owl:hasValue 0 ;
            owl:onProperty :hasNumberOfDimensions ],
        :NMI_quantity .

:gw_self_energy_c a owl:Class ;
    rdfs:comment "Diagonal matrix elements of the correlation self-energy"^^xsd:string ;
    rdfs:subClassOf [ a owl:Restriction ;
            owl:hasValue 3 ;
            owl:onProperty :hasNumberOfDimensions ],
        [ a owl:Restriction ;
            owl:hasValue :number_of_eigenvalues ;
            owl:onProperty :hasVarDim3 ],
        [ a owl:Restriction ;
            owl:allValuesFrom <http://emmo.info/emmo/middle/math#EMMO_18d180e4_5e3e_42f7_820c_e08951223486> ;
            owl:onProperty :hasDatatype ],
        [ a owl:Restriction ;
            owl:allValuesFrom <http://emmo.info/emmo/middle/siunits#EMMO_8a70dea4_d6ab_4260_b931_a3e990982416> ;
            owl:onProperty <http://emmo.info/emmo/middle/metrology#EMMO_67fc0a36_8dcb_4ffa_9a43_31074efa3296> ],
        [ a owl:Restriction ;
            owl:hasValue :number_of_spin_channels ;
            owl:onProperty :hasVarDim1 ],
        [ a owl:Restriction ;
            owl:hasValue :number_of_eigenvalues_kpoints ;
            owl:onProperty :hasVarDim2 ],
        :NMI_quantity .

:gw_self_energy_c_analytical_continuation a owl:Class ;
    rdfs:comment """Models for the correlation self-energy analytical continuation: 'pade' -  Pade's
approximant (by H. J. Vidberg and J. W. Serence, J. Low Temp. Phys. 29, 179
(1977)); 'mpf' -  Multi-Pole Fitting (by H. N Rojas, R. W. Godby and R. J. Needs,
Phys. Rev. Lett. 74, 1827 (1995)); 'cd' - contour deformation; 'ra' - real axis"""^^xsd:string ;
    rdfs:subClassOf [ a owl:Restriction ;
            owl:hasValue 0 ;
            owl:onProperty :hasNumberOfDimensions ],
        [ a owl:Restriction ;
            owl:allValuesFrom <http://emmo.info/emmo/middle/perceptual#EMMO_50ea1ec5_f157_41b0_b46b_a9032f17ca10> ;
            owl:onProperty :hasDatatype ],
        :NMI_quantity .

:gw_self_energy_c_number_of_empty_states a owl:Class ;
    rdfs:comment "Number of empty states to be used to calculate the correlation self energy."^^xsd:string ;
    rdfs:subClassOf [ a owl:Restriction ;
            owl:hasValue 0 ;
            owl:onProperty :hasNumberOfDimensions ],
        [ a owl:Restriction ;
            owl:allValuesFrom <http://emmo.info/emmo/middle/math#EMMO_f8bd64d5_5d3e_4ad4_a46e_c30714fecb7f> ;
            owl:onProperty <http://emmo.info/emmo/middle/metrology#EMMO_67fc0a36_8dcb_4ffa_9a43_31074efa3296> ],
        [ a owl:Restriction ;
            owl:allValuesFrom <http://emmo.info/emmo/middle/math#EMMO_f8bd64d5_5d3e_4ad4_a46e_c30714fecb7f> ;
            owl:onProperty :hasDatatype ],
        :NMI_dimension,
        :NMI_quantity .

:gw_self_energy_c_number_of_poles a owl:Class ;
    rdfs:comment "Number of poles used in the analytical continuation."^^xsd:string ;
    rdfs:subClassOf [ a owl:Restriction ;
            owl:allValuesFrom <http://emmo.info/emmo/middle/math#EMMO_f8bd64d5_5d3e_4ad4_a46e_c30714fecb7f> ;
            owl:onProperty <http://emmo.info/emmo/middle/metrology#EMMO_67fc0a36_8dcb_4ffa_9a43_31074efa3296> ],
        [ a owl:Restriction ;
            owl:allValuesFrom <http://emmo.info/emmo/middle/math#EMMO_f8bd64d5_5d3e_4ad4_a46e_c30714fecb7f> ;
            owl:onProperty :hasDatatype ],
        [ a owl:Restriction ;
            owl:hasValue 0 ;
            owl:onProperty :hasNumberOfDimensions ],
        :NMI_dimension,
        :NMI_quantity .

:gw_self_energy_singularity_treatment a owl:Class ;
    rdfs:comment """Treatment of the integrable singular terms in the calculation of the self energy.
Values: 'mpb' - Auxiliary function method by S. Massidda, M. Posternak, and A.
Baldereschi, PRB 48, 5058 (1993); 'crg' - Auxiliary function method by P. Carrier,
S. Rohra, and A. Goerling, PRB 75, 205126 (2007)."""^^xsd:string ;
    rdfs:subClassOf [ a owl:Restriction ;
            owl:hasValue 0 ;
            owl:onProperty :hasNumberOfDimensions ],
        [ a owl:Restriction ;
            owl:allValuesFrom <http://emmo.info/emmo/middle/perceptual#EMMO_50ea1ec5_f157_41b0_b46b_a9032f17ca10> ;
            owl:onProperty :hasDatatype ],
        :NMI_quantity .

:gw_self_energy_x a owl:Class ;
    rdfs:comment "Diagonal matrix elements of the exchange self-energy"^^xsd:string ;
    rdfs:subClassOf [ a owl:Restriction ;
            owl:hasValue :number_of_spin_channels ;
            owl:onProperty :hasVarDim1 ],
        [ a owl:Restriction ;
            owl:allValuesFrom <http://emmo.info/emmo/middle/math#EMMO_18d180e4_5e3e_42f7_820c_e08951223486> ;
            owl:onProperty :hasDatatype ],
        [ a owl:Restriction ;
            owl:hasValue :number_of_eigenvalues_kpoints ;
            owl:onProperty :hasVarDim2 ],
        [ a owl:Restriction ;
            owl:hasValue 3 ;
            owl:onProperty :hasNumberOfDimensions ],
        [ a owl:Restriction ;
            owl:hasValue :number_of_eigenvalues ;
            owl:onProperty :hasVarDim3 ],
        [ a owl:Restriction ;
            owl:allValuesFrom <http://emmo.info/emmo/middle/siunits#EMMO_8a70dea4_d6ab_4260_b931_a3e990982416> ;
            owl:onProperty <http://emmo.info/emmo/middle/metrology#EMMO_67fc0a36_8dcb_4ffa_9a43_31074efa3296> ],
        :NMI_quantity .

:gw_starting_point a owl:Class ;
    rdfs:comment """Exchange-correlation functional of the ground-state calculation. See XC_functional
list at https://gitlab.mpcdf.mpg.de/nomad-lab/nomad-meta-info/wikis/metainfo/XC-
functional"""^^xsd:string ;
    rdfs:subClassOf [ a owl:Restriction ;
            owl:allValuesFrom <http://emmo.info/emmo/middle/perceptual#EMMO_50ea1ec5_f157_41b0_b46b_a9032f17ca10> ;
            owl:onProperty :hasDatatype ],
        [ a owl:Restriction ;
            owl:hasValue 0 ;
            owl:onProperty :hasNumberOfDimensions ],
        :NMI_quantity .

:gw_type a owl:Class ;
    rdfs:comment """GW methodology: G0W0; ev-scGW: (eigenvalues self-consistent GW) – Phys.Rev.B 34,
5390 (1986); qp-scGW: (quasi-particle self-consistent GW) – Phys. Rev. Lett. 96,
226402 (2006)  scGW0: (self-consistent G with fixed W0) – Phys.Rev.B 54, 8411
(1996); scG0W: (self-consistent W with fixed G0); scGW: (self-consistent GW) –
Phys. Rev. B 88, 075105 (2013)"""^^xsd:string ;
    rdfs:subClassOf [ a owl:Restriction ;
            owl:hasValue 0 ;
            owl:onProperty :hasNumberOfDimensions ],
        [ a owl:Restriction ;
            owl:allValuesFrom <http://emmo.info/emmo/middle/perceptual#EMMO_50ea1ec5_f157_41b0_b46b_a9032f17ca10> ;
            owl:onProperty :hasDatatype ],
        :NMI_quantity .

:gw_type_test a owl:Class ;
    rdfs:comment "GW methodology: exciting test variable"^^xsd:string ;
    rdfs:subClassOf [ a owl:Restriction ;
            owl:allValuesFrom <http://emmo.info/emmo/middle/perceptual#EMMO_50ea1ec5_f157_41b0_b46b_a9032f17ca10> ;
            owl:onProperty :hasDatatype ],
        [ a owl:Restriction ;
            owl:hasValue 0 ;
            owl:onProperty :hasNumberOfDimensions ],
        :NMI_quantity .

:gw_xc_potential a owl:Class ;
    rdfs:comment "Diagonal matrix elements of the exchange-correlation potential"^^xsd:string ;
    rdfs:subClassOf [ a owl:Restriction ;
            owl:allValuesFrom <http://emmo.info/emmo/middle/siunits#EMMO_8a70dea4_d6ab_4260_b931_a3e990982416> ;
            owl:onProperty <http://emmo.info/emmo/middle/metrology#EMMO_67fc0a36_8dcb_4ffa_9a43_31074efa3296> ],
        [ a owl:Restriction ;
            owl:hasValue :number_of_eigenvalues ;
            owl:onProperty :hasVarDim3 ],
        [ a owl:Restriction ;
            owl:allValuesFrom <http://emmo.info/emmo/middle/math#EMMO_18d180e4_5e3e_42f7_820c_e08951223486> ;
            owl:onProperty :hasDatatype ],
        [ a owl:Restriction ;
            owl:hasValue 3 ;
            owl:onProperty :hasNumberOfDimensions ],
        [ a owl:Restriction ;
            owl:hasValue :number_of_spin_channels ;
            owl:onProperty :hasVarDim1 ],
        [ a owl:Restriction ;
            owl:hasValue :number_of_eigenvalues_kpoints ;
            owl:onProperty :hasVarDim2 ],
        :NMI_quantity .

:hall_number a owl:Class ;
    rdfs:comment "The Hall number for this system."^^xsd:string ;
    rdfs:subClassOf [ a owl:Restriction ;
            owl:allValuesFrom <http://emmo.info/emmo/middle/math#EMMO_f8bd64d5_5d3e_4ad4_a46e_c30714fecb7f> ;
            owl:onProperty :hasDatatype ],
        [ a owl:Restriction ;
            owl:hasValue 0 ;
            owl:onProperty :hasNumberOfDimensions ],
        [ a owl:Restriction ;
            owl:allValuesFrom <http://emmo.info/emmo/middle/math#EMMO_f8bd64d5_5d3e_4ad4_a46e_c30714fecb7f> ;
            owl:onProperty <http://emmo.info/emmo/middle/metrology#EMMO_67fc0a36_8dcb_4ffa_9a43_31074efa3296> ],
        :NMI_dimension,
        :NMI_quantity .

:hall_symbol a owl:Class ;
    rdfs:comment "The Hall symbol for this system."^^xsd:string ;
    rdfs:subClassOf [ a owl:Restriction ;
            owl:hasValue 0 ;
            owl:onProperty :hasNumberOfDimensions ],
        [ a owl:Restriction ;
            owl:allValuesFrom <http://emmo.info/emmo/middle/perceptual#EMMO_50ea1ec5_f157_41b0_b46b_a9032f17ca10> ;
            owl:onProperty :hasDatatype ],
        :NMI_quantity .

:hasFixDim4 a owl:DatatypeProperty,
        owl:FunctionalProperty ;
    rdfs:domain :NMI_quantity ;
    rdfs:range [ a rdfs:Datatype ;
            owl:onDatatype xsd:integer ;
            owl:withRestrictions ( [ xsd:minInclusive 1 ] ) ] .

:helmholz_free_energy a owl:Class ;
    rdfs:comment """Stores the Helmholtz free energy per unit cell at constant volume of a
thermodynamic calculation."""^^xsd:string ;
    rdfs:subClassOf [ a owl:Restriction ;
            owl:hasValue :number_of_thermodynamical_property_values ;
            owl:onProperty :hasVarDim1 ],
        [ a owl:Restriction ;
            owl:allValuesFrom <http://emmo.info/emmo/middle/math#EMMO_18d180e4_5e3e_42f7_820c_e08951223486> ;
            owl:onProperty :hasDatatype ],
        [ a owl:Restriction ;
            owl:allValuesFrom <http://emmo.info/emmo/middle/siunits#EMMO_8a70dea4_d6ab_4260_b931_a3e990982416> ;
            owl:onProperty <http://emmo.info/emmo/middle/metrology#EMMO_67fc0a36_8dcb_4ffa_9a43_31074efa3296> ],
        [ a owl:Restriction ;
            owl:hasValue 1 ;
            owl:onProperty :hasNumberOfDimensions ],
        :NMI_quantity .

:hessian_matrix a owl:Class ;
    rdfs:comment "The matrix with the second derivative with respect to atom displacements."^^xsd:string ;
    rdfs:subClassOf [ a owl:Restriction ;
            owl:hasValue 3 ;
            owl:onProperty :hasFixDim4 ],
        [ a owl:Restriction ;
            owl:hasValue :number_of_atoms ;
            owl:onProperty :hasVarDim2 ],
        [ a owl:Restriction ;
            owl:allValuesFrom <http://emmo.info/emmo/middle/math#EMMO_18d180e4_5e3e_42f7_820c_e08951223486> ;
            owl:onProperty :hasDatatype ],
        [ a owl:Restriction ;
            owl:hasValue 4 ;
            owl:onProperty :hasNumberOfDimensions ],
        [ a owl:Restriction ;
            owl:hasValue 3 ;
            owl:onProperty :hasFixDim3 ],
        [ a owl:Restriction ;
            owl:hasValue :number_of_atoms ;
            owl:onProperty :hasVarDim1 ],
        :NMI_quantity .

:indices a owl:Class ;
    rdfs:comment "Indices used to compare DOS fingerprints of different energy ranges."^^xsd:string ;
    rdfs:subClassOf [ a owl:Restriction ;
            owl:hasValue 2 ;
            owl:onProperty :hasNumberOfDimensions ],
        [ a owl:Restriction ;
            owl:allValuesFrom <http://emmo.info/emmo/middle/math#EMMO_f8bd64d5_5d3e_4ad4_a46e_c30714fecb7f> ;
            owl:onProperty :hasDatatype ],
        :NMI_quantity .

:interaction_atoms a owl:Class ;
    rdfs:comment """List of the indexes involved in this interaction. The fist atom has index 1, the
last atom index number_of_topology_atoms."""^^xsd:string ;
    rdfs:subClassOf [ a owl:Restriction ;
            owl:hasValue 2 ;
            owl:onProperty :hasNumberOfDimensions ],
        [ a owl:Restriction ;
            owl:allValuesFrom <http://emmo.info/emmo/middle/math#EMMO_f8bd64d5_5d3e_4ad4_a46e_c30714fecb7f> ;
            owl:onProperty :hasDatatype ],
        [ a owl:Restriction ;
            owl:hasValue :number_of_atoms_per_interaction ;
            owl:onProperty :hasVarDim2 ],
        [ a owl:Restriction ;
            owl:hasValue :number_of_interactions ;
            owl:onProperty :hasVarDim1 ],
        :NMI_quantity .

:interaction_kind a owl:Class ;
    rdfs:comment """Short and unique name for this interaction type. Valid names are described in the
[interaction\\_kind wiki page](https://gitlab.mpcdf.mpg.de/nomad-lab/nomad-meta-
info/wikis/metainfo/interaction-kind)."""^^xsd:string ;
    rdfs:subClassOf [ a owl:Restriction ;
            owl:allValuesFrom <http://emmo.info/emmo/middle/perceptual#EMMO_50ea1ec5_f157_41b0_b46b_a9032f17ca10> ;
            owl:onProperty :hasDatatype ],
        [ a owl:Restriction ;
            owl:hasValue 0 ;
            owl:onProperty :hasNumberOfDimensions ],
        :NMI_quantity .

:interaction_parameters a owl:Class ;
    rdfs:comment """Explicit interaction parameters for this kind of interaction (depending on the
interaction_kind some might be given implicitly through other means)."""^^xsd:string ;
    rdfs:subClassOf [ a owl:Restriction ;
            owl:hasValue 0 ;
            owl:onProperty :hasNumberOfDimensions ],
        :NMI_quantity .

:international_short_symbol a owl:Class ;
    rdfs:comment """Specifies the International Union of Crystallography (IUC) short symbol of the 3D
space group of this system"""^^xsd:string ;
    rdfs:subClassOf [ a owl:Restriction ;
            owl:allValuesFrom <http://emmo.info/emmo/middle/perceptual#EMMO_50ea1ec5_f157_41b0_b46b_a9032f17ca10> ;
            owl:onProperty :hasDatatype ],
        [ a owl:Restriction ;
            owl:hasValue 0 ;
            owl:onProperty :hasNumberOfDimensions ],
        :NMI_quantity .

:is_representative a owl:Class ;
    rdfs:comment """Most systems in a run are only minor variations of each other. Systems marked
representative where chosen to be representative for all systems in the run."""^^xsd:string ;
    rdfs:subClassOf [ a owl:Restriction ;
            owl:allValuesFrom <http://emmo.info/emmo/middle/math#EMMO_54dc83cb_06e1_4739_9e45_bc09cead7f48> ;
            owl:onProperty :hasDatatype ],
        [ a owl:Restriction ;
            owl:hasValue 0 ;
            owl:onProperty :hasNumberOfDimensions ],
        :NMI_quantity .

:is_standard_path a owl:Class ;
    rdfs:comment """Boolean indicating whether the path follows the standard path for this
bravais lattice. The AFLOW standard by Setyawan and Curtarolo is used
(https://doi.org/10.1016/j.commatsci.2010.05.010)."""^^xsd:string ;
    rdfs:subClassOf [ a owl:Restriction ;
            owl:allValuesFrom <http://emmo.info/emmo/middle/math#EMMO_54dc83cb_06e1_4739_9e45_bc09cead7f48> ;
            owl:onProperty :hasDatatype ],
        [ a owl:Restriction ;
            owl:hasValue 0 ;
            owl:onProperty :hasNumberOfDimensions ],
        :NMI_quantity .

:k_band_path_normalized_is_standard a owl:Class ;
    rdfs:comment """If the normalized path is along the default path defined in W. Setyawan and S.
Curtarolo, [Comput. Mater. Sci. **49**, 299-312
(2010)](http://dx.doi.org/10.1016/j.commatsci.2010.05.010)."""^^xsd:string ;
    rdfs:subClassOf [ a owl:Restriction ;
            owl:hasValue 0 ;
            owl:onProperty :hasNumberOfDimensions ],
        [ a owl:Restriction ;
            owl:allValuesFrom <http://emmo.info/emmo/middle/math#EMMO_54dc83cb_06e1_4739_9e45_bc09cead7f48> ;
            owl:onProperty :hasDatatype ],
        :NMI_quantity .

:k_mesh_points a owl:Class ;
    rdfs:comment """List of all the k points in the $k$-point mesh. These are the k point used to
evaluate energy_total, and are in fractional coordinates (in the basis of the
reciprocal-lattice vectors)."""^^xsd:string ;
    rdfs:subClassOf [ a owl:Restriction ;
            owl:hasValue 3 ;
            owl:onProperty :hasFixDim2 ],
        [ a owl:Restriction ;
            owl:onProperty :hasCategory ;
            owl:someValuesFrom :settings_k_points ],
        [ a owl:Restriction ;
            owl:hasValue 2 ;
            owl:onProperty :hasNumberOfDimensions ],
        [ a owl:Restriction ;
            owl:hasValue :number_of_k_mesh_points ;
            owl:onProperty :hasVarDim1 ],
        [ a owl:Restriction ;
            owl:onProperty :hasCategory ;
            owl:someValuesFrom :settings_potential_energy_surface ],
        [ a owl:Restriction ;
            owl:allValuesFrom <http://emmo.info/emmo/middle/math#EMMO_18d180e4_5e3e_42f7_820c_e08951223486> ;
            owl:onProperty :hasDatatype ],
        :NMI_quantity .

:k_mesh_weights a owl:Class ;
    rdfs:comment """Weights of all the k points in the $k$-point mesh. These are the weights for
k_mesh_points (i.e. the k point used to evaluate energy_total)."""^^xsd:string ;
    rdfs:subClassOf [ a owl:Restriction ;
            owl:hasValue 1 ;
            owl:onProperty :hasNumberOfDimensions ],
        [ a owl:Restriction ;
            owl:onProperty :hasCategory ;
            owl:someValuesFrom :settings_k_points ],
        [ a owl:Restriction ;
            owl:hasValue :number_of_k_mesh_points ;
            owl:onProperty :hasVarDim1 ],
        [ a owl:Restriction ;
            owl:onProperty :hasCategory ;
            owl:someValuesFrom :settings_potential_energy_surface ],
        [ a owl:Restriction ;
            owl:allValuesFrom <http://emmo.info/emmo/middle/math#EMMO_18d180e4_5e3e_42f7_820c_e08951223486> ;
            owl:onProperty :hasDatatype ],
        :NMI_quantity .

:lattice_vectors a owl:Class ;
    rdfs:comment """Holds the lattice vectors (in Cartesian coordinates) of the simulation cell. The
last (fastest) index runs over the $x,y,z$ Cartesian coordinates, and the first
index runs over the 3 lattice vectors."""^^xsd:string ;
    rdfs:subClassOf [ a owl:Restriction ;
            owl:hasValue 3 ;
            owl:onProperty :hasFixDim1 ],
        [ a owl:Restriction ;
            owl:hasValue 3 ;
            owl:onProperty :hasFixDim2 ],
        [ a owl:Restriction ;
            owl:onProperty :hasCategory ;
            owl:someValuesFrom :configuration_core ],
        [ a owl:Restriction ;
            owl:allValuesFrom <http://emmo.info/emmo/middle/siunits#EMMO_7db11dbf_a643_464a_9b56_07eabcc3e9c5> ;
            owl:onProperty <http://emmo.info/emmo/middle/metrology#EMMO_67fc0a36_8dcb_4ffa_9a43_31074efa3296> ],
        [ a owl:Restriction ;
            owl:allValuesFrom <http://emmo.info/emmo/middle/math#EMMO_18d180e4_5e3e_42f7_820c_e08951223486> ;
            owl:onProperty :hasDatatype ],
        [ a owl:Restriction ;
            owl:hasValue 2 ;
            owl:onProperty :hasNumberOfDimensions ],
        :NMI_quantity .

:lattice_vectors_primitive a owl:Class ;
    rdfs:comment "Primitive lattice vectors. The vectors are the rows of this matrix."^^xsd:string ;
    rdfs:subClassOf [ a owl:Restriction ;
            owl:allValuesFrom <http://emmo.info/emmo/middle/siunits#EMMO_7db11dbf_a643_464a_9b56_07eabcc3e9c5> ;
            owl:onProperty <http://emmo.info/emmo/middle/metrology#EMMO_67fc0a36_8dcb_4ffa_9a43_31074efa3296> ],
        [ a owl:Restriction ;
            owl:allValuesFrom <http://emmo.info/emmo/middle/math#EMMO_18d180e4_5e3e_42f7_820c_e08951223486> ;
            owl:onProperty :hasDatatype ],
        [ a owl:Restriction ;
            owl:hasValue 3 ;
            owl:onProperty :hasFixDim1 ],
        [ a owl:Restriction ;
            owl:hasValue 3 ;
            owl:onProperty :hasFixDim2 ],
        [ a owl:Restriction ;
            owl:hasValue 2 ;
            owl:onProperty :hasNumberOfDimensions ],
        :NMI_quantity .

:lattice_vectors_std a owl:Class ;
    rdfs:comment """Standardized lattice vectors of the conventional cell. The vectors are the rows of
this matrix."""^^xsd:string ;
    rdfs:subClassOf [ a owl:Restriction ;
            owl:allValuesFrom <http://emmo.info/emmo/middle/math#EMMO_18d180e4_5e3e_42f7_820c_e08951223486> ;
            owl:onProperty :hasDatatype ],
        [ a owl:Restriction ;
            owl:hasValue 2 ;
            owl:onProperty :hasNumberOfDimensions ],
        [ a owl:Restriction ;
            owl:allValuesFrom <http://emmo.info/emmo/middle/siunits#EMMO_7db11dbf_a643_464a_9b56_07eabcc3e9c5> ;
            owl:onProperty <http://emmo.info/emmo/middle/metrology#EMMO_67fc0a36_8dcb_4ffa_9a43_31074efa3296> ],
        [ a owl:Restriction ;
            owl:hasValue 3 ;
            owl:onProperty :hasFixDim1 ],
        [ a owl:Restriction ;
            owl:hasValue 3 ;
            owl:onProperty :hasFixDim2 ],
        :NMI_quantity .

:local_rotations a owl:Class ;
    rdfs:comment """A rotation matrix defining the orientation of each atom. If the rotation matrix
only needs to be specified for some atoms, the remaining atoms should set it to
the zero matrix (not the identity!)"""^^xsd:string ;
    rdfs:subClassOf [ a owl:Restriction ;
            owl:hasValue :number_of_atoms ;
            owl:onProperty :hasVarDim1 ],
        [ a owl:Restriction ;
            owl:hasValue 3 ;
            owl:onProperty :hasFixDim3 ],
        [ a owl:Restriction ;
            owl:hasValue 3 ;
            owl:onProperty :hasNumberOfDimensions ],
        [ a owl:Restriction ;
            owl:hasValue 3 ;
            owl:onProperty :hasFixDim2 ],
        [ a owl:Restriction ;
            owl:allValuesFrom <http://emmo.info/emmo/middle/math#EMMO_18d180e4_5e3e_42f7_820c_e08951223486> ;
            owl:onProperty :hasDatatype ],
        :NMI_quantity .

:mapping_section_basis_set_atom_centered a owl:Class ;
    rdfs:comment """An array of the dimension of number_of_atoms where each atom (identified by the
index in the array) is assigned to an atom-centered basis set, for this
section_single_configuration_calculation. The actual definition of the atom-
centered basis set is in the section_basis_set_atom_centered that is referred to
by this metadata."""^^xsd:string ;
    rdfs:subClassOf [ a owl:Restriction ;
            owl:hasValue :number_of_atoms ;
            owl:onProperty :hasVarDim1 ],
        [ a owl:Restriction ;
            owl:hasValue 1 ;
            owl:onProperty :hasNumberOfDimensions ],
        :NMI_quantity .

:mapping_section_basis_set_cell_dependent a owl:Class ;
    rdfs:comment """Assignment of the cell-dependent (i.e., non atom centered, e.g., plane-waves)
parts of the basis set, which is defined (type, parameters) in
section_basis_set_cell_dependent that is referred to by this metadata."""^^xsd:string ;
    rdfs:subClassOf [ a owl:Restriction ;
            owl:hasValue 0 ;
            owl:onProperty :hasNumberOfDimensions ],
        :NMI_quantity .

:mapping_section_method_basis_set_atom_centered a owl:Class ;
    rdfs:comment """Reference to an atom-centered basis set defined in section_basis_set_atom_centered
and to the atom kind as defined in section_method_atom_kind."""^^xsd:string ;
    rdfs:subClassOf [ a owl:Restriction ;
            owl:hasValue :number_of_basis_sets_atom_centered ;
            owl:onProperty :hasVarDim1 ],
        [ a owl:Restriction ;
            owl:hasValue 2 ;
            owl:onProperty :hasNumberOfDimensions ],
        [ a owl:Restriction ;
            owl:hasValue 2 ;
            owl:onProperty :hasFixDim2 ],
        [ a owl:Restriction ;
            owl:allValuesFrom <http://emmo.info/emmo/middle/math#EMMO_f8bd64d5_5d3e_4ad4_a46e_c30714fecb7f> ;
            owl:onProperty :hasDatatype ],
        :NMI_quantity .

:mapping_section_method_basis_set_cell_associated a owl:Class ;
    rdfs:comment "Reference to a cell-associated basis set."^^xsd:string ;
    rdfs:subClassOf [ a owl:Restriction ;
            owl:hasValue 0 ;
            owl:onProperty :hasNumberOfDimensions ],
        :NMI_quantity .

:message_debug_evaluation a owl:Class ;
    rdfs:comment """A debugging message of the computational program, associated with a *single
configuration calculation* (see section_single_configuration_calculation)."""^^xsd:string ;
    rdfs:subClassOf [ a owl:Restriction ;
            owl:allValuesFrom <http://emmo.info/emmo/middle/perceptual#EMMO_50ea1ec5_f157_41b0_b46b_a9032f17ca10> ;
            owl:onProperty :hasDatatype ],
        [ a owl:Restriction ;
            owl:onProperty :hasCategory ;
            owl:someValuesFrom :message_debug ],
        [ a owl:Restriction ;
            owl:hasValue 0 ;
            owl:onProperty :hasNumberOfDimensions ],
        :NMI_quantity .

:message_debug_run a owl:Class ;
    rdfs:comment "A debugging message of the computational program, associated with a run."^^xsd:string ;
    rdfs:subClassOf [ a owl:Restriction ;
            owl:hasValue 0 ;
            owl:onProperty :hasNumberOfDimensions ],
        [ a owl:Restriction ;
            owl:onProperty :hasCategory ;
            owl:someValuesFrom :message_debug ],
        [ a owl:Restriction ;
            owl:allValuesFrom <http://emmo.info/emmo/middle/perceptual#EMMO_50ea1ec5_f157_41b0_b46b_a9032f17ca10> ;
            owl:onProperty :hasDatatype ],
        :NMI_quantity .

:message_error_evaluation a owl:Class ;
    rdfs:comment """An error message of the computational program, associated with a *single
configuration calculation* (see section_single_configuration_calculation)."""^^xsd:string ;
    rdfs:subClassOf [ a owl:Restriction ;
            owl:hasValue 0 ;
            owl:onProperty :hasNumberOfDimensions ],
        [ a owl:Restriction ;
            owl:allValuesFrom <http://emmo.info/emmo/middle/perceptual#EMMO_50ea1ec5_f157_41b0_b46b_a9032f17ca10> ;
            owl:onProperty :hasDatatype ],
        [ a owl:Restriction ;
            owl:onProperty :hasCategory ;
            owl:someValuesFrom :message_warning ],
        [ a owl:Restriction ;
            owl:onProperty :hasCategory ;
            owl:someValuesFrom :message_info ],
        [ a owl:Restriction ;
            owl:onProperty :hasCategory ;
            owl:someValuesFrom :message_debug ],
        [ a owl:Restriction ;
            owl:onProperty :hasCategory ;
            owl:someValuesFrom :message_error ],
        :NMI_quantity .

:message_error_run a owl:Class ;
    rdfs:comment "An error message of the computational program, associated with a run."^^xsd:string ;
    rdfs:subClassOf [ a owl:Restriction ;
            owl:hasValue 0 ;
            owl:onProperty :hasNumberOfDimensions ],
        [ a owl:Restriction ;
            owl:onProperty :hasCategory ;
            owl:someValuesFrom :message_error ],
        [ a owl:Restriction ;
            owl:onProperty :hasCategory ;
            owl:someValuesFrom :message_info ],
        [ a owl:Restriction ;
            owl:onProperty :hasCategory ;
            owl:someValuesFrom :message_warning ],
        [ a owl:Restriction ;
            owl:onProperty :hasCategory ;
            owl:someValuesFrom :message_debug ],
        [ a owl:Restriction ;
            owl:allValuesFrom <http://emmo.info/emmo/middle/perceptual#EMMO_50ea1ec5_f157_41b0_b46b_a9032f17ca10> ;
            owl:onProperty :hasDatatype ],
        :NMI_quantity .

:message_info_evaluation a owl:Class ;
    rdfs:comment """An information message of the computational program, associated with a *single
configuration calculation* (see section_single_configuration_calculation)."""^^xsd:string ;
    rdfs:subClassOf [ a owl:Restriction ;
            owl:allValuesFrom <http://emmo.info/emmo/middle/perceptual#EMMO_50ea1ec5_f157_41b0_b46b_a9032f17ca10> ;
            owl:onProperty :hasDatatype ],
        [ a owl:Restriction ;
            owl:onProperty :hasCategory ;
            owl:someValuesFrom :message_debug ],
        [ a owl:Restriction ;
            owl:onProperty :hasCategory ;
            owl:someValuesFrom :message_info ],
        [ a owl:Restriction ;
            owl:hasValue 0 ;
            owl:onProperty :hasNumberOfDimensions ],
        :NMI_quantity .

:message_info_run a owl:Class ;
    rdfs:comment "An information message of the computational program, associated with a run."^^xsd:string ;
    rdfs:subClassOf [ a owl:Restriction ;
            owl:onProperty :hasCategory ;
            owl:someValuesFrom :message_debug ],
        [ a owl:Restriction ;
            owl:hasValue 0 ;
            owl:onProperty :hasNumberOfDimensions ],
        [ a owl:Restriction ;
            owl:allValuesFrom <http://emmo.info/emmo/middle/perceptual#EMMO_50ea1ec5_f157_41b0_b46b_a9032f17ca10> ;
            owl:onProperty :hasDatatype ],
        [ a owl:Restriction ;
            owl:onProperty :hasCategory ;
            owl:someValuesFrom :message_info ],
        :NMI_quantity .

:message_warning_evaluation a owl:Class ;
    rdfs:comment "A warning message of the computational program."^^xsd:string ;
    rdfs:subClassOf [ a owl:Restriction ;
            owl:onProperty :hasCategory ;
            owl:someValuesFrom :message_info ],
        [ a owl:Restriction ;
            owl:onProperty :hasCategory ;
            owl:someValuesFrom :message_debug ],
        [ a owl:Restriction ;
            owl:onProperty :hasCategory ;
            owl:someValuesFrom :message_warning ],
        [ a owl:Restriction ;
            owl:hasValue 0 ;
            owl:onProperty :hasNumberOfDimensions ],
        [ a owl:Restriction ;
            owl:allValuesFrom <http://emmo.info/emmo/middle/perceptual#EMMO_50ea1ec5_f157_41b0_b46b_a9032f17ca10> ;
            owl:onProperty :hasDatatype ],
        :NMI_quantity .

:message_warning_run a owl:Class ;
    rdfs:comment "A warning message of the computational program, associated with a run."^^xsd:string ;
    rdfs:subClassOf [ a owl:Restriction ;
            owl:hasValue 0 ;
            owl:onProperty :hasNumberOfDimensions ],
        [ a owl:Restriction ;
            owl:onProperty :hasCategory ;
            owl:someValuesFrom :message_info ],
        [ a owl:Restriction ;
            owl:onProperty :hasCategory ;
            owl:someValuesFrom :message_debug ],
        [ a owl:Restriction ;
            owl:onProperty :hasCategory ;
            owl:someValuesFrom :message_warning ],
        [ a owl:Restriction ;
            owl:allValuesFrom <http://emmo.info/emmo/middle/perceptual#EMMO_50ea1ec5_f157_41b0_b46b_a9032f17ca10> ;
            owl:onProperty :hasDatatype ],
        :NMI_quantity .

:method_atom_kind_atom_number a owl:Class ;
    rdfs:comment "Atomic number (number of protons) of this atom kind, use 0 if not an atom."^^xsd:string ;
    rdfs:subClassOf [ a owl:Restriction ;
            owl:allValuesFrom <http://emmo.info/emmo/middle/math#EMMO_f8bd64d5_5d3e_4ad4_a46e_c30714fecb7f> ;
            owl:onProperty :hasDatatype ],
        [ a owl:Restriction ;
            owl:allValuesFrom <http://emmo.info/emmo/middle/math#EMMO_f8bd64d5_5d3e_4ad4_a46e_c30714fecb7f> ;
            owl:onProperty <http://emmo.info/emmo/middle/metrology#EMMO_67fc0a36_8dcb_4ffa_9a43_31074efa3296> ],
        [ a owl:Restriction ;
            owl:hasValue 0 ;
            owl:onProperty :hasNumberOfDimensions ],
        :NMI_dimension,
        :NMI_quantity .

:method_atom_kind_explicit_electrons a owl:Class ;
    rdfs:comment "Number of explicit electrons (often called valence)."^^xsd:string ;
    rdfs:subClassOf [ a owl:Restriction ;
            owl:hasValue 0 ;
            owl:onProperty :hasNumberOfDimensions ],
        [ a owl:Restriction ;
            owl:allValuesFrom <http://emmo.info/emmo/middle/math#EMMO_18d180e4_5e3e_42f7_820c_e08951223486> ;
            owl:onProperty :hasDatatype ],
        :NMI_quantity .

:method_atom_kind_label a owl:Class ;
    rdfs:comment """String used to identify the atoms of this kind. This should correspond to the
atom_labels of the configuration. It is possible for one atom kind to have
multiple labels (in order to allow two atoms of the same kind to have two
differently defined sets of atom-centered basis functions or two different pseudo-
potentials). Atom kind is typically the symbol of the atomic species but it can be
also a ghost or pseudo-atom."""^^xsd:string ;
    rdfs:subClassOf [ a owl:Restriction ;
            owl:allValuesFrom <http://emmo.info/emmo/middle/perceptual#EMMO_50ea1ec5_f157_41b0_b46b_a9032f17ca10> ;
            owl:onProperty :hasDatatype ],
        [ a owl:Restriction ;
            owl:hasValue 0 ;
            owl:onProperty :hasNumberOfDimensions ],
        :NMI_quantity .

:method_atom_kind_mass a owl:Class ;
    rdfs:comment "Mass of the kind of this kind of atoms."^^xsd:string ;
    rdfs:subClassOf [ a owl:Restriction ;
            owl:allValuesFrom <http://emmo.info/emmo/middle/math#EMMO_18d180e4_5e3e_42f7_820c_e08951223486> ;
            owl:onProperty :hasDatatype ],
        [ a owl:Restriction ;
            owl:hasValue 0 ;
            owl:onProperty :hasNumberOfDimensions ],
        [ a owl:Restriction ;
            owl:allValuesFrom <https://nomad-coe.eu/ontology/properties#AtomicMass> ;
            owl:onProperty <http://emmo.info/emmo/middle/metrology#EMMO_67fc0a36_8dcb_4ffa_9a43_31074efa3296> ],
        :NMI_quantity .

:method_atom_kind_pseudopotential_name a owl:Class ;
    rdfs:comment "Name identifying the pseudopotential used."^^xsd:string ;
    rdfs:subClassOf [ a owl:Restriction ;
            owl:hasValue 0 ;
            owl:onProperty :hasNumberOfDimensions ],
        [ a owl:Restriction ;
            owl:allValuesFrom <http://emmo.info/emmo/middle/perceptual#EMMO_50ea1ec5_f157_41b0_b46b_a9032f17ca10> ;
            owl:onProperty :hasDatatype ],
        :NMI_quantity .

:method_basis_set_kind a owl:Class ;
    rdfs:comment """String describing the use of the basis set, i.e, if it used for expanding a
wavefunction or an electron density. Allowed values are listed in the
[basis\\_set\\_kind wiki page](https://gitlab.mpcdf.mpg.de/nomad-lab/nomad-meta-
info/wikis/metainfo/basis-set-kind)."""^^xsd:string ;
    rdfs:subClassOf [ a owl:Restriction ;
            owl:hasValue 0 ;
            owl:onProperty :hasNumberOfDimensions ],
        [ a owl:Restriction ;
            owl:allValuesFrom <http://emmo.info/emmo/middle/perceptual#EMMO_50ea1ec5_f157_41b0_b46b_a9032f17ca10> ;
            owl:onProperty :hasDatatype ],
        :NMI_quantity .

:method_to_method_external_url a owl:Class ;
    rdfs:comment """URL used to reference an externally stored section_method. The kind of
relationship between the present and the referenced section_method is specified by
method_to_method_kind."""^^xsd:string ;
    rdfs:subClassOf [ a owl:Restriction ;
            owl:allValuesFrom <http://emmo.info/emmo/middle/perceptual#EMMO_50ea1ec5_f157_41b0_b46b_a9032f17ca10> ;
            owl:onProperty :hasDatatype ],
        [ a owl:Restriction ;
            owl:hasValue 0 ;
            owl:onProperty :hasNumberOfDimensions ],
        :NMI_quantity .

:method_to_method_kind a owl:Class ;
    rdfs:comment """String defining the kind of relationship that the referenced section_method has
with the present section_method. Valid values are described in the
[method_to_method_kind wiki page](https://gitlab.mpcdf.mpg.de/nomad-lab/nomad-
meta-info/wikis/metainfo/method-to-method-kind). Often calculations are connected,
for instance, one calculation is a perturbation performed using a self-consistent
field (SCF) calculation as starting point, or a simulated system is partitioned in
regions with different but connected Hamiltonians (e.g., QM/MM, or a region
treated via Kohn-Sham DFT embedded into a region treated via orbital-free DFT).
Hence, the need of keeping track of these connected calculations. The referenced
section_method is identified via method_to_method_ref (typically used for a
section_method in the same section_run) or method_to_method_external_url."""^^xsd:string ;
    rdfs:subClassOf [ a owl:Restriction ;
            owl:hasValue 0 ;
            owl:onProperty :hasNumberOfDimensions ],
        [ a owl:Restriction ;
            owl:allValuesFrom <http://emmo.info/emmo/middle/perceptual#EMMO_50ea1ec5_f157_41b0_b46b_a9032f17ca10> ;
            owl:onProperty :hasDatatype ],
        :NMI_quantity .

:method_to_method_ref a owl:Class ;
    rdfs:comment """Reference to a local section_method. If both method_to_method_ref and
method_to_method_external_url are given, then method_to_method_ref is a local copy
of the value contained in method_to_method_external_url. The kind of relationship
between the method defined in the present section_method and the referenced one is
described by method_to_method_kind."""^^xsd:string ;
    rdfs:subClassOf [ a owl:Restriction ;
            owl:hasValue 0 ;
            owl:onProperty :hasNumberOfDimensions ],
        :NMI_quantity .

:method_to_topology_ref a owl:Class ;
    rdfs:comment "Reference to the topology and force fields to be used."^^xsd:string ;
    rdfs:subClassOf [ a owl:Restriction ;
            owl:hasValue 0 ;
            owl:onProperty :hasNumberOfDimensions ],
        :NMI_quantity .

:molecule_constraint_atoms a owl:Class ;
    rdfs:comment """List of the indexes involved in this constraint. The fist atom has index 1, the
last index is number_of_atoms_in_molecule."""^^xsd:string ;
    rdfs:subClassOf [ a owl:Restriction ;
            owl:hasValue 2 ;
            owl:onProperty :hasNumberOfDimensions ],
        [ a owl:Restriction ;
            owl:allValuesFrom <http://emmo.info/emmo/middle/math#EMMO_f8bd64d5_5d3e_4ad4_a46e_c30714fecb7f> ;
            owl:onProperty :hasDatatype ],
        [ a owl:Restriction ;
            owl:hasValue :number_of_atoms_per_molecule_constraint ;
            owl:onProperty :hasVarDim2 ],
        [ a owl:Restriction ;
            owl:hasValue :number_of_molecule_constraints ;
            owl:onProperty :hasVarDim1 ],
        :NMI_quantity .

:molecule_constraint_kind a owl:Class ;
    rdfs:comment """Short and unique name for this constraint type. Valid names are described in the
[constraint\\_kind wiki page](https://gitlab.mpcdf.mpg.de/nomad-lab/nomad-meta-
info/wikis/metainfo/constraint-kind)."""^^xsd:string ;
    rdfs:subClassOf [ a owl:Restriction ;
            owl:hasValue 0 ;
            owl:onProperty :hasNumberOfDimensions ],
        [ a owl:Restriction ;
            owl:allValuesFrom <http://emmo.info/emmo/middle/perceptual#EMMO_50ea1ec5_f157_41b0_b46b_a9032f17ca10> ;
            owl:onProperty :hasDatatype ],
        :NMI_quantity .

:molecule_constraint_parameters a owl:Class ;
    rdfs:comment """Explicit constraint parameters for this kind of constraint (depending on the
constraint type some might be given implicitly through other means)."""^^xsd:string ;
    rdfs:subClassOf [ a owl:Restriction ;
            owl:hasValue 0 ;
            owl:onProperty :hasNumberOfDimensions ],
        :NMI_quantity .

:molecule_interaction_atoms a owl:Class ;
    rdfs:comment """List of the indexes involved in this bonded interaction within a molecule. The
first atom has index 1, the last index is number_of_atoms_in_."""^^xsd:string ;
    rdfs:subClassOf [ a owl:Restriction ;
            owl:hasValue :number_of_molecule_interactions ;
            owl:onProperty :hasVarDim1 ],
        [ a owl:Restriction ;
            owl:allValuesFrom <http://emmo.info/emmo/middle/math#EMMO_f8bd64d5_5d3e_4ad4_a46e_c30714fecb7f> ;
            owl:onProperty :hasDatatype ],
        [ a owl:Restriction ;
            owl:hasValue 2 ;
            owl:onProperty :hasNumberOfDimensions ],
        [ a owl:Restriction ;
            owl:hasValue :number_of_atoms_per_molecule_interaction ;
            owl:onProperty :hasVarDim2 ],
        :NMI_quantity .

:molecule_interaction_kind a owl:Class ;
    rdfs:comment """Short and unique name for this interaction type, used for bonded interactions for
atoms in a molecule. Valid names are described in the [interaction\\_kind wiki
page](https://gitlab.mpcdf.mpg.de/nomad-lab/nomad-meta-
info/wikis/metainfo/interaction-kind)."""^^xsd:string ;
    rdfs:subClassOf [ a owl:Restriction ;
            owl:allValuesFrom <http://emmo.info/emmo/middle/perceptual#EMMO_50ea1ec5_f157_41b0_b46b_a9032f17ca10> ;
            owl:onProperty :hasDatatype ],
        [ a owl:Restriction ;
            owl:hasValue 0 ;
            owl:onProperty :hasNumberOfDimensions ],
        :NMI_quantity .

:molecule_interaction_parameters a owl:Class ;
    rdfs:comment """Explicit interaction parameters for this kind of interaction (depending on the
interaction type some might be given implicitly through other means), used for
bonded interactions for atoms in a molecule."""^^xsd:string ;
    rdfs:subClassOf [ a owl:Restriction ;
            owl:hasValue 0 ;
            owl:onProperty :hasNumberOfDimensions ],
        :NMI_quantity .

:molecule_to_molecule_type_map a owl:Class ;
    rdfs:comment "Mapping from molecules to molecule types."^^xsd:string ;
    rdfs:subClassOf [ a owl:Restriction ;
            owl:hasValue :number_of_topology_molecules ;
            owl:onProperty :hasVarDim1 ],
        [ a owl:Restriction ;
            owl:hasValue 1 ;
            owl:onProperty :hasNumberOfDimensions ],
        :NMI_quantity .

:molecule_type_name a owl:Class ;
    rdfs:comment "Name of the molecule."^^xsd:string ;
    rdfs:subClassOf [ a owl:Restriction ;
            owl:hasValue 0 ;
            owl:onProperty :hasNumberOfDimensions ],
        [ a owl:Restriction ;
            owl:allValuesFrom <http://emmo.info/emmo/middle/perceptual#EMMO_50ea1ec5_f157_41b0_b46b_a9032f17ca10> ;
            owl:onProperty :hasDatatype ],
        :NMI_quantity .

:number_of_basis_functions a owl:Class ;
    rdfs:comment "Stores the total number of basis functions in a section_basis_set section."^^xsd:string ;
    rdfs:subClassOf [ a owl:Restriction ;
            owl:allValuesFrom <http://emmo.info/emmo/middle/math#EMMO_f8bd64d5_5d3e_4ad4_a46e_c30714fecb7f> ;
            owl:onProperty <http://emmo.info/emmo/middle/metrology#EMMO_67fc0a36_8dcb_4ffa_9a43_31074efa3296> ],
        [ a owl:Restriction ;
            owl:allValuesFrom <http://emmo.info/emmo/middle/math#EMMO_f8bd64d5_5d3e_4ad4_a46e_c30714fecb7f> ;
            owl:onProperty :hasDatatype ],
        [ a owl:Restriction ;
            owl:hasValue 0 ;
            owl:onProperty :hasNumberOfDimensions ],
        :NMI_dimension,
        :NMI_quantity .

:number_of_basis_functions_in_basis_set_atom_centered a owl:Class ;
    rdfs:comment """Gives the number of different basis functions in a section_basis_set_atom_centered
section. This equals the number of actual coefficients that are specified when
using this basis set."""^^xsd:string ;
    rdfs:subClassOf [ a owl:Restriction ;
            owl:allValuesFrom <http://emmo.info/emmo/middle/math#EMMO_f8bd64d5_5d3e_4ad4_a46e_c30714fecb7f> ;
            owl:onProperty <http://emmo.info/emmo/middle/metrology#EMMO_67fc0a36_8dcb_4ffa_9a43_31074efa3296> ],
        [ a owl:Restriction ;
            owl:allValuesFrom <http://emmo.info/emmo/middle/math#EMMO_f8bd64d5_5d3e_4ad4_a46e_c30714fecb7f> ;
            owl:onProperty :hasDatatype ],
        [ a owl:Restriction ;
            owl:hasValue 0 ;
            owl:onProperty :hasNumberOfDimensions ],
        :NMI_dimension,
        :NMI_quantity .

:number_of_electrons a owl:Class ;
    rdfs:comment "Number of electrons in system"^^xsd:string ;
    rdfs:subClassOf [ a owl:Restriction ;
            owl:allValuesFrom <http://emmo.info/emmo/middle/math#EMMO_18d180e4_5e3e_42f7_820c_e08951223486> ;
            owl:onProperty :hasDatatype ],
        [ a owl:Restriction ;
            owl:hasValue 1 ;
            owl:onProperty :hasNumberOfDimensions ],
        [ a owl:Restriction ;
            owl:onProperty :hasCategory ;
            owl:someValuesFrom :configuration_core ],
        [ a owl:Restriction ;
            owl:hasValue :number_of_spin_channels ;
            owl:onProperty :hasVarDim1 ],
        :NMI_quantity .

:number_of_scf_iterations a owl:Class ;
    rdfs:comment """Gives the number of performed self-consistent field (SCF) iterations at a specfied
level of theory."""^^xsd:string ;
    rdfs:subClassOf [ a owl:Restriction ;
            owl:onProperty :hasCategory ;
            owl:someValuesFrom :scf_info ],
        [ a owl:Restriction ;
            owl:hasValue 0 ;
            owl:onProperty :hasNumberOfDimensions ],
        [ a owl:Restriction ;
            owl:allValuesFrom <http://emmo.info/emmo/middle/math#EMMO_f8bd64d5_5d3e_4ad4_a46e_c30714fecb7f> ;
            owl:onProperty :hasDatatype ],
        [ a owl:Restriction ;
            owl:allValuesFrom <http://emmo.info/emmo/middle/math#EMMO_f8bd64d5_5d3e_4ad4_a46e_c30714fecb7f> ;
            owl:onProperty <http://emmo.info/emmo/middle/metrology#EMMO_67fc0a36_8dcb_4ffa_9a43_31074efa3296> ],
        :NMI_dimension,
        :NMI_quantity .

:origin_shift a owl:Class ;
    rdfs:comment """Vector $\\mathbf{p}$ from the origin of the standardized system to the origin of
the original system. Together with the matrix $\\mathbf{P}$, found in
space_group_3D_transformation_matrix, the transformation between the standardized
coordinates $\\mathbf{x}_s$ and original coordinates $\\mathbf{x}$ is then given by
$\\mathbf{x}_s = \\mathbf{P} \\mathbf{x} + \\mathbf{p}$."""^^xsd:string ;
    rdfs:subClassOf [ a owl:Restriction ;
            owl:hasValue 1 ;
            owl:onProperty :hasNumberOfDimensions ],
        [ a owl:Restriction ;
            owl:allValuesFrom <http://emmo.info/emmo/middle/math#EMMO_18d180e4_5e3e_42f7_820c_e08951223486> ;
            owl:onProperty :hasDatatype ],
        [ a owl:Restriction ;
            owl:hasValue 3 ;
            owl:onProperty :hasFixDim1 ],
        :NMI_quantity .

:oscillator_strengths a owl:Class ;
    rdfs:comment "Excited states oscillator strengths."^^xsd:string ;
    rdfs:subClassOf [ a owl:Restriction ;
            owl:hasValue :number_of_excited_states ;
            owl:onProperty :hasVarDim1 ],
        [ a owl:Restriction ;
            owl:hasValue 1 ;
            owl:onProperty :hasNumberOfDimensions ],
        [ a owl:Restriction ;
            owl:allValuesFrom <http://emmo.info/emmo/middle/math#EMMO_18d180e4_5e3e_42f7_820c_e08951223486> ;
            owl:onProperty :hasDatatype ],
        :NMI_quantity .

:parallelization_info a owl:Class ;
    rdfs:comment """Contains information on the parallelization of the program, i.e. which parallel
programming language was used and its version, how many cores had been working on the
calculation and the flags and parameters needed to run the parallelization of the
code."""^^xsd:string ;
    rdfs:subClassOf :accessory_info .

:parsing_message_debug_evaluation a owl:Class ;
    rdfs:comment """This field is used for debugging messages of the parsing program associated with a
run, see section_run."""^^xsd:string ;
    rdfs:subClassOf [ a owl:Restriction ;
            owl:onProperty :hasCategory ;
            owl:someValuesFrom :parsing_message_debug ],
        [ a owl:Restriction ;
            owl:allValuesFrom <http://emmo.info/emmo/middle/perceptual#EMMO_50ea1ec5_f157_41b0_b46b_a9032f17ca10> ;
            owl:onProperty :hasDatatype ],
        [ a owl:Restriction ;
            owl:hasValue 0 ;
            owl:onProperty :hasNumberOfDimensions ],
        :NMI_quantity .

:parsing_message_debug_run a owl:Class ;
    rdfs:comment """This field is used for debugging messages of the parsing program associated with a
single configuration calculation, see section_single_configuration_calculation."""^^xsd:string ;
    rdfs:subClassOf [ a owl:Restriction ;
            owl:hasValue 0 ;
            owl:onProperty :hasNumberOfDimensions ],
        [ a owl:Restriction ;
            owl:onProperty :hasCategory ;
            owl:someValuesFrom :parsing_message_debug ],
        [ a owl:Restriction ;
            owl:allValuesFrom <http://emmo.info/emmo/middle/perceptual#EMMO_50ea1ec5_f157_41b0_b46b_a9032f17ca10> ;
            owl:onProperty :hasDatatype ],
        :NMI_quantity .

:parsing_message_error_run a owl:Class ;
    rdfs:comment """This field is used for error messages of the parsing program associated with a
run, see section_run."""^^xsd:string ;
    rdfs:subClassOf [ a owl:Restriction ;
            owl:onProperty :hasCategory ;
            owl:someValuesFrom :parsing_message_warning ],
        [ a owl:Restriction ;
            owl:onProperty :hasCategory ;
            owl:someValuesFrom :parsing_message_info ],
        [ a owl:Restriction ;
            owl:onProperty :hasCategory ;
            owl:someValuesFrom :parsing_message_error ],
        [ a owl:Restriction ;
            owl:allValuesFrom <http://emmo.info/emmo/middle/perceptual#EMMO_50ea1ec5_f157_41b0_b46b_a9032f17ca10> ;
            owl:onProperty :hasDatatype ],
        [ a owl:Restriction ;
            owl:hasValue 0 ;
            owl:onProperty :hasNumberOfDimensions ],
        [ a owl:Restriction ;
            owl:onProperty :hasCategory ;
            owl:someValuesFrom :parsing_message_debug ],
        :NMI_quantity .

:parsing_message_error_single_configuration a owl:Class ;
    rdfs:comment """This field is used for error messages of the parsing program associated with a
single configuration calculation, see section_single_configuration_calculation."""^^xsd:string ;
    rdfs:subClassOf [ a owl:Restriction ;
            owl:onProperty :hasCategory ;
            owl:someValuesFrom :parsing_message_warning ],
        [ a owl:Restriction ;
            owl:allValuesFrom <http://emmo.info/emmo/middle/perceptual#EMMO_50ea1ec5_f157_41b0_b46b_a9032f17ca10> ;
            owl:onProperty :hasDatatype ],
        [ a owl:Restriction ;
            owl:hasValue 0 ;
            owl:onProperty :hasNumberOfDimensions ],
        [ a owl:Restriction ;
            owl:onProperty :hasCategory ;
            owl:someValuesFrom :parsing_message_error ],
        [ a owl:Restriction ;
            owl:onProperty :hasCategory ;
            owl:someValuesFrom :parsing_message_info ],
        [ a owl:Restriction ;
            owl:onProperty :hasCategory ;
            owl:someValuesFrom :parsing_message_debug ],
        :NMI_quantity .

:parsing_message_info_run a owl:Class ;
    rdfs:comment """This field is used for info messages of the parsing program associated with a run,
see section_run."""^^xsd:string ;
    rdfs:subClassOf [ a owl:Restriction ;
            owl:allValuesFrom <http://emmo.info/emmo/middle/perceptual#EMMO_50ea1ec5_f157_41b0_b46b_a9032f17ca10> ;
            owl:onProperty :hasDatatype ],
        [ a owl:Restriction ;
            owl:onProperty :hasCategory ;
            owl:someValuesFrom :parsing_message_info ],
        [ a owl:Restriction ;
            owl:onProperty :hasCategory ;
            owl:someValuesFrom :parsing_message_debug ],
        [ a owl:Restriction ;
            owl:hasValue 0 ;
            owl:onProperty :hasNumberOfDimensions ],
        :NMI_quantity .

:parsing_message_info_single_configuration a owl:Class ;
    rdfs:comment """This field is used for info messages of the parsing program associated with a
single configuration calculation, see section_single_configuration_calculation."""^^xsd:string ;
    rdfs:subClassOf [ a owl:Restriction ;
            owl:allValuesFrom <http://emmo.info/emmo/middle/perceptual#EMMO_50ea1ec5_f157_41b0_b46b_a9032f17ca10> ;
            owl:onProperty :hasDatatype ],
        [ a owl:Restriction ;
            owl:hasValue 0 ;
            owl:onProperty :hasNumberOfDimensions ],
        [ a owl:Restriction ;
            owl:onProperty :hasCategory ;
            owl:someValuesFrom :parsing_message_debug ],
        [ a owl:Restriction ;
            owl:onProperty :hasCategory ;
            owl:someValuesFrom :parsing_message_info ],
        :NMI_quantity .

:parsing_message_warning_evaluation a owl:Class ;
    rdfs:comment """This field is used for warning messages of the parsing program associated with a
run, see section_run."""^^xsd:string ;
    rdfs:subClassOf [ a owl:Restriction ;
            owl:onProperty :hasCategory ;
            owl:someValuesFrom :parsing_message_warning ],
        [ a owl:Restriction ;
            owl:hasValue 0 ;
            owl:onProperty :hasNumberOfDimensions ],
        [ a owl:Restriction ;
            owl:onProperty :hasCategory ;
            owl:someValuesFrom :parsing_message_debug ],
        [ a owl:Restriction ;
            owl:allValuesFrom <http://emmo.info/emmo/middle/perceptual#EMMO_50ea1ec5_f157_41b0_b46b_a9032f17ca10> ;
            owl:onProperty :hasDatatype ],
        [ a owl:Restriction ;
            owl:onProperty :hasCategory ;
            owl:someValuesFrom :parsing_message_info ],
        :NMI_quantity .

:parsing_message_warning_run a owl:Class ;
    rdfs:comment """This field is used for warning messages of the parsing program associated with a
run, see section_run."""^^xsd:string ;
    rdfs:subClassOf [ a owl:Restriction ;
            owl:onProperty :hasCategory ;
            owl:someValuesFrom :parsing_message_info ],
        [ a owl:Restriction ;
            owl:onProperty :hasCategory ;
            owl:someValuesFrom :parsing_message_warning ],
        [ a owl:Restriction ;
            owl:onProperty :hasCategory ;
            owl:someValuesFrom :parsing_message_debug ],
        [ a owl:Restriction ;
            owl:hasValue 0 ;
            owl:onProperty :hasNumberOfDimensions ],
        [ a owl:Restriction ;
            owl:allValuesFrom <http://emmo.info/emmo/middle/perceptual#EMMO_50ea1ec5_f157_41b0_b46b_a9032f17ca10> ;
            owl:onProperty :hasDatatype ],
        :NMI_quantity .

:point_group a owl:Class ;
    rdfs:comment "Symbol of the crystallographic point group in the Hermann-Mauguin notation."^^xsd:string ;
    rdfs:subClassOf [ a owl:Restriction ;
            owl:allValuesFrom <http://emmo.info/emmo/middle/perceptual#EMMO_50ea1ec5_f157_41b0_b46b_a9032f17ca10> ;
            owl:onProperty :hasDatatype ],
        [ a owl:Restriction ;
            owl:hasValue 0 ;
            owl:onProperty :hasNumberOfDimensions ],
        :NMI_quantity .

:previous_sequence_ref a owl:Class ;
    rdfs:comment """Contains a reference to the previous sequence. A sequence is a trajectory, which
can have number_of_frames_in_sequence each representing one
section_single_configuration_calculation section. If not given, a start from an
initial configuration is assumed."""^^xsd:string ;
    rdfs:subClassOf [ a owl:Restriction ;
            owl:hasValue 0 ;
            owl:onProperty :hasNumberOfDimensions ],
        :NMI_quantity .

:program_basis_set_type a owl:Class ;
    rdfs:comment """The type of basis set used by the program to represent wave functions.

Valid values are:

* Numeric AOs

* Gaussians

* (L)APW+lo

* FLAPW (full-potential linearized augmented planewave)

* Plane waves

* Real-space grid

* Local-orbital minimum-basis"""^^xsd:string ;
    rdfs:subClassOf [ a owl:Restriction ;
            owl:allValuesFrom <http://emmo.info/emmo/middle/perceptual#EMMO_50ea1ec5_f157_41b0_b46b_a9032f17ca10> ;
            owl:onProperty :hasDatatype ],
        [ a owl:Restriction ;
            owl:hasValue 0 ;
            owl:onProperty :hasNumberOfDimensions ],
        :NMI_quantity .

:program_compilation_datetime a owl:Class ;
    rdfs:comment """Contains the program compilation date and time from *Unix epoch* (00:00:00 UTC on
1 January 1970) in seconds. For date and times without a timezone, the default
timezone GMT is used."""^^xsd:string ;
    rdfs:subClassOf [ a owl:Restriction ;
            owl:hasValue 0 ;
            owl:onProperty :hasNumberOfDimensions ],
        [ a owl:Restriction ;
            owl:onProperty :hasCategory ;
            owl:someValuesFrom :accessory_info ],
        [ a owl:Restriction ;
            owl:allValuesFrom <http://emmo.info/emmo/middle/math#EMMO_18d180e4_5e3e_42f7_820c_e08951223486> ;
            owl:onProperty :hasDatatype ],
        [ a owl:Restriction ;
            owl:onProperty :hasCategory ;
            owl:someValuesFrom :program_info ],
        [ a owl:Restriction ;
            owl:allValuesFrom <http://emmo.info/emmo/middle/siunits#EMMO_314ba716_2d3d_4462_9a4f_d3419ae1df43> ;
            owl:onProperty <http://emmo.info/emmo/middle/metrology#EMMO_67fc0a36_8dcb_4ffa_9a43_31074efa3296> ],
        :NMI_quantity .

:program_compilation_host a owl:Class ;
    rdfs:comment "Specifies the host on which the program was compiled."^^xsd:string ;
    rdfs:subClassOf [ a owl:Restriction ;
            owl:onProperty :hasCategory ;
            owl:someValuesFrom :program_info ],
        [ a owl:Restriction ;
            owl:onProperty :hasCategory ;
            owl:someValuesFrom :accessory_info ],
        [ a owl:Restriction ;
            owl:hasValue 0 ;
            owl:onProperty :hasNumberOfDimensions ],
        [ a owl:Restriction ;
            owl:allValuesFrom <http://emmo.info/emmo/middle/perceptual#EMMO_50ea1ec5_f157_41b0_b46b_a9032f17ca10> ;
            owl:onProperty :hasDatatype ],
        :NMI_quantity .

:program_name a owl:Class ;
    rdfs:comment "Specifies the name of the program that generated the data."^^xsd:string ;
    rdfs:subClassOf [ a owl:Restriction ;
            owl:hasValue 0 ;
            owl:onProperty :hasNumberOfDimensions ],
        [ a owl:Restriction ;
            owl:onProperty :hasCategory ;
            owl:someValuesFrom :program_info ],
        [ a owl:Restriction ;
            owl:allValuesFrom <http://emmo.info/emmo/middle/perceptual#EMMO_50ea1ec5_f157_41b0_b46b_a9032f17ca10> ;
            owl:onProperty :hasDatatype ],
        [ a owl:Restriction ;
            owl:onProperty :hasCategory ;
            owl:someValuesFrom :accessory_info ],
        :NMI_quantity .

:program_version a owl:Class ;
    rdfs:comment """Specifies the version of the program that was used. This should be the version
number of an official release, the version tag or a commit id as well as the
location of the repository."""^^xsd:string ;
    rdfs:subClassOf [ a owl:Restriction ;
            owl:allValuesFrom <http://emmo.info/emmo/middle/perceptual#EMMO_50ea1ec5_f157_41b0_b46b_a9032f17ca10> ;
            owl:onProperty :hasDatatype ],
        [ a owl:Restriction ;
            owl:onProperty :hasCategory ;
            owl:someValuesFrom :accessory_info ],
        [ a owl:Restriction ;
            owl:hasValue 0 ;
            owl:onProperty :hasNumberOfDimensions ],
        [ a owl:Restriction ;
            owl:onProperty :hasCategory ;
            owl:someValuesFrom :program_info ],
        :NMI_quantity .

:prototype_aflow_id a owl:Class ;
    rdfs:comment """AFLOW id of the prototype (see
http://aflowlib.org/CrystalDatabase/prototype_index.html) identified on the basis
of the space_group and normalized_wyckoff."""^^xsd:string ;
    rdfs:subClassOf [ a owl:Restriction ;
            owl:hasValue 0 ;
            owl:onProperty :hasNumberOfDimensions ],
        [ a owl:Restriction ;
            owl:allValuesFrom <http://emmo.info/emmo/middle/perceptual#EMMO_50ea1ec5_f157_41b0_b46b_a9032f17ca10> ;
            owl:onProperty :hasDatatype ],
        :NMI_quantity .

:prototype_aflow_url a owl:Class ;
    rdfs:comment """Url to the AFLOW definition of the prototype (see
http://aflowlib.org/CrystalDatabase/prototype_index.html) identified on the basis
of the space_group and normalized_wyckoff."""^^xsd:string ;
    rdfs:subClassOf [ a owl:Restriction ;
            owl:allValuesFrom <http://emmo.info/emmo/middle/perceptual#EMMO_50ea1ec5_f157_41b0_b46b_a9032f17ca10> ;
            owl:onProperty :hasDatatype ],
        [ a owl:Restriction ;
            owl:hasValue 0 ;
            owl:onProperty :hasNumberOfDimensions ],
        :NMI_quantity .

:prototype_assignment_method a owl:Class ;
    rdfs:comment "Method used to identify the prototype."^^xsd:string ;
    rdfs:subClassOf [ a owl:Restriction ;
            owl:hasValue 0 ;
            owl:onProperty :hasNumberOfDimensions ],
        [ a owl:Restriction ;
            owl:allValuesFrom <http://emmo.info/emmo/middle/perceptual#EMMO_50ea1ec5_f157_41b0_b46b_a9032f17ca10> ;
            owl:onProperty :hasDatatype ],
        :NMI_quantity .

:prototype_label a owl:Class ;
    rdfs:comment """Label of the prototype identified on the basis of the space_group and
normalized_wyckoff. The label is in the same format as in the read_prototypes
function: <space_group_number>-<prototype_name>-<Pearson's symbol>)."""^^xsd:string ;
    rdfs:subClassOf [ a owl:Restriction ;
            owl:hasValue 0 ;
            owl:onProperty :hasNumberOfDimensions ],
        [ a owl:Restriction ;
            owl:allValuesFrom <http://emmo.info/emmo/middle/perceptual#EMMO_50ea1ec5_f157_41b0_b46b_a9032f17ca10> ;
            owl:onProperty :hasDatatype ],
        :NMI_quantity .

:raw_id a owl:Class ;
    rdfs:comment "An optional calculation id, if one is found in the code input/output files."^^xsd:string ;
    rdfs:subClassOf [ a owl:Restriction ;
            owl:hasValue 0 ;
            owl:onProperty :hasNumberOfDimensions ],
        [ a owl:Restriction ;
            owl:allValuesFrom <http://emmo.info/emmo/middle/perceptual#EMMO_50ea1ec5_f157_41b0_b46b_a9032f17ca10> ;
            owl:onProperty :hasDatatype ],
        :NMI_quantity .

:reciprocal_cell a owl:Class ;
    rdfs:comment "The reciprocal cell within which the band structure is calculated."^^xsd:string ;
    rdfs:subClassOf [ a owl:Restriction ;
            owl:hasValue 3 ;
            owl:onProperty :hasFixDim2 ],
        [ a owl:Restriction ;
            owl:hasValue 3 ;
            owl:onProperty :hasFixDim1 ],
        [ a owl:Restriction ;
            owl:hasValue 2 ;
            owl:onProperty :hasNumberOfDimensions ],
        [ a owl:Restriction ;
            owl:allValuesFrom <https://nomad-coe.eu/ontology/properties#PerMetre> ;
            owl:onProperty <http://emmo.info/emmo/middle/metrology#EMMO_67fc0a36_8dcb_4ffa_9a43_31074efa3296> ],
        [ a owl:Restriction ;
            owl:allValuesFrom <http://emmo.info/emmo/middle/math#EMMO_18d180e4_5e3e_42f7_820c_e08951223486> ;
            owl:onProperty :hasDatatype ],
        :NMI_quantity .

:relativity_method a owl:Class ;
    rdfs:comment """Describes the relativistic treatment used for the calculation of the final energy
and related quantities. If skipped or empty, no relativistic treatment is applied."""^^xsd:string ;
    rdfs:subClassOf [ a owl:Restriction ;
            owl:onProperty :hasCategory ;
            owl:someValuesFrom :settings_XC ],
        [ a owl:Restriction ;
            owl:allValuesFrom <http://emmo.info/emmo/middle/perceptual#EMMO_50ea1ec5_f157_41b0_b46b_a9032f17ca10> ;
            owl:onProperty :hasDatatype ],
        [ a owl:Restriction ;
            owl:hasValue 0 ;
            owl:onProperty :hasNumberOfDimensions ],
        [ a owl:Restriction ;
            owl:onProperty :hasCategory ;
            owl:someValuesFrom :settings_relativity ],
        [ a owl:Restriction ;
            owl:onProperty :hasCategory ;
            owl:someValuesFrom :settings_potential_energy_surface ],
        :NMI_quantity .

:run_clean_end a owl:Class ;
    rdfs:comment """Indicates whether this run terminated properly (true), or if it was killed or
exited with an error code unequal to zero (false)."""^^xsd:string ;
    rdfs:subClassOf [ a owl:Restriction ;
            owl:hasValue 0 ;
            owl:onProperty :hasNumberOfDimensions ],
        [ a owl:Restriction ;
            owl:allValuesFrom <http://emmo.info/emmo/middle/math#EMMO_54dc83cb_06e1_4739_9e45_bc09cead7f48> ;
            owl:onProperty :hasDatatype ],
        :NMI_quantity .

:run_hosts a owl:Class ;
    rdfs:comment """An associative list of host(s) that performed this simulation. This is an
associative list that contains program-dependent information (*key*) on how the
host was used (*value*). Useful for debugging purposes."""^^xsd:string ;
    rdfs:subClassOf [ a owl:Restriction ;
            owl:onProperty :hasCategory ;
            owl:someValuesFrom :parallelization_info ],
        [ a owl:Restriction ;
            owl:onProperty :hasCategory ;
            owl:someValuesFrom :accessory_info ],
        [ a owl:Restriction ;
            owl:hasValue 0 ;
            owl:onProperty :hasNumberOfDimensions ],
        :NMI_quantity .

:sampling_method a owl:Class ;
    rdfs:comment """Type of method used to do the sampling.

Allowed values are:

| Sampling method                | Description                      |

| ------------------------------ | -------------------------------- |

| `"geometry_optimization"`      | Geometry optimization            |

| `"molecular_dynamics"`         | Molecular dynamics               |

| `"montecarlo"`                 | (Metropolis) Monte Carlo         |

| `"steered_molecular_dynamics"` | Steered molecular dynamics (with time dependent
external forces) |

| `"meta_dynamics"`              | Biased molecular dynamics with history-
dependent Hamiltonian |

| `"wang_landau_montecarlo"`     | Monte Carlo according to the Wang-Landau
formulation. |

| `"blue_moon"`                  | Blue Moon sampling               |

| `"langevin_dynamics"`          | Langevin dynamics                |

| `"taylor_expansion"`           | Taylor expansion of the potential energy
surface |"""^^xsd:string ;
    rdfs:subClassOf [ a owl:Restriction ;
            owl:hasValue 0 ;
            owl:onProperty :hasNumberOfDimensions ],
        [ a owl:Restriction ;
            owl:allValuesFrom <http://emmo.info/emmo/middle/perceptual#EMMO_50ea1ec5_f157_41b0_b46b_a9032f17ca10> ;
            owl:onProperty :hasDatatype ],
        :NMI_quantity .

:sampling_method_expansion_order a owl:Class ;
    rdfs:comment """Order up to which the potential energy surface was expanded in a Taylor series
(see sampling_method)."""^^xsd:string ;
    rdfs:subClassOf [ a owl:Restriction ;
            owl:allValuesFrom <http://emmo.info/emmo/middle/math#EMMO_f8bd64d5_5d3e_4ad4_a46e_c30714fecb7f> ;
            owl:onProperty :hasDatatype ],
        [ a owl:Restriction ;
            owl:allValuesFrom <http://emmo.info/emmo/middle/math#EMMO_f8bd64d5_5d3e_4ad4_a46e_c30714fecb7f> ;
            owl:onProperty <http://emmo.info/emmo/middle/metrology#EMMO_67fc0a36_8dcb_4ffa_9a43_31074efa3296> ],
        [ a owl:Restriction ;
            owl:hasValue 0 ;
            owl:onProperty :hasNumberOfDimensions ],
        :NMI_dimension,
        :NMI_quantity .

:scf_info a owl:Class ;
    rdfs:comment """Contains information on the self-consistent field (SCF) procedure, i.e. the number of
SCF iterations (number_of_scf_iterations) or a section_scf_iteration section with
detailed information on the SCF procedure of specified quantities."""^^xsd:string ;
    rdfs:subClassOf :NMI_category .

:scf_max_iteration a owl:Class ;
    rdfs:comment """Specifies the maximum number of allowed self-consistent field (SCF) iterations in
a calculation run, see section_run."""^^xsd:string ;
    rdfs:subClassOf [ a owl:Restriction ;
            owl:allValuesFrom <http://emmo.info/emmo/middle/math#EMMO_18d180e4_5e3e_42f7_820c_e08951223486> ;
            owl:onProperty :hasDatatype ],
        [ a owl:Restriction ;
            owl:hasValue 0 ;
            owl:onProperty :hasNumberOfDimensions ],
        [ a owl:Restriction ;
            owl:onProperty :hasCategory ;
            owl:someValuesFrom :settings_scf ],
        :NMI_quantity .

:scf_threshold_energy_change a owl:Class ;
    rdfs:comment """Specifies the threshold for the energy_total_scf_iteration change between two
subsequent self-consistent field (SCF) iterations. The SCF is considered converged
when the total-energy change between two SCF cycles is below the threshold
(possibly in combination with other criteria)."""^^xsd:string ;
    rdfs:subClassOf [ a owl:Restriction ;
            owl:allValuesFrom <http://emmo.info/emmo/middle/siunits#EMMO_8a70dea4_d6ab_4260_b931_a3e990982416> ;
            owl:onProperty <http://emmo.info/emmo/middle/metrology#EMMO_67fc0a36_8dcb_4ffa_9a43_31074efa3296> ],
        [ a owl:Restriction ;
            owl:onProperty :hasCategory ;
            owl:someValuesFrom :settings_scf ],
        [ a owl:Restriction ;
            owl:allValuesFrom <http://emmo.info/emmo/middle/math#EMMO_18d180e4_5e3e_42f7_820c_e08951223486> ;
            owl:onProperty :hasDatatype ],
        [ a owl:Restriction ;
            owl:hasValue 0 ;
            owl:onProperty :hasNumberOfDimensions ],
        :NMI_quantity .

:section_XC_functionals a owl:Class ;
    rdfs:comment "Section containing one of the exchange-correlation (XC) functionals for the present section_method that are combined to form the XC_functional."^^xsd:string ;
    rdfs:subClassOf [ a owl:Restriction ;
            owl:onProperty :hasQuantity ;
            owl:someValuesFrom :XC_functional_weight ],
        [ a owl:Restriction ;
            owl:onProperty :hasQuantity ;
            owl:someValuesFrom :XC_functional_parameters ],
        [ a owl:Restriction ;
            owl:onProperty :hasQuantity ;
            owl:someValuesFrom :XC_functional_name ],
        :NMI_section .

:section_atom_projected_dos a owl:Class ;
    rdfs:comment "Section collecting the information on an atom projected density of states (DOS) evaluation."^^xsd:string ;
    rdfs:subClassOf [ a owl:Restriction ;
            owl:onProperty :hasQuantity ;
            owl:someValuesFrom :atom_projected_dos_lm ],
        [ a owl:Restriction ;
            owl:onProperty :hasQuantity ;
            owl:someValuesFrom :atom_projected_dos_values_total ],
        [ a owl:Restriction ;
            owl:onProperty :hasQuantity ;
            owl:someValuesFrom :atom_projected_dos_values_lm ],
        [ a owl:Restriction ;
            owl:onProperty :hasQuantity ;
            owl:someValuesFrom :atom_projected_dos_m_kind ],
        [ a owl:Restriction ;
            owl:onProperty :hasQuantity ;
            owl:someValuesFrom :atom_projected_dos_energies ],
        [ a owl:Restriction ;
            owl:onProperty :hasQuantity ;
            owl:someValuesFrom :number_of_atom_projected_dos_values ],
        [ a owl:Restriction ;
            owl:onProperty :hasQuantity ;
            owl:someValuesFrom :number_of_lm_atom_projected_dos ],
        :NMI_section .

:section_atom_type a owl:Class ;
    rdfs:comment "Section describing a type of atom in the system."^^xsd:string ;
    rdfs:subClassOf [ a owl:Restriction ;
            owl:onProperty :hasQuantity ;
            owl:someValuesFrom :atom_type_mass ],
        [ a owl:Restriction ;
            owl:onProperty :hasQuantity ;
            owl:someValuesFrom :atom_type_name ],
        [ a owl:Restriction ;
            owl:onProperty :hasQuantity ;
            owl:someValuesFrom :atom_type_charge ],
        :NMI_section .

:section_atomic_multipoles a owl:Class ;
    rdfs:comment "Section describing multipoles (charges/monopoles, dipoles, quadrupoles, ...) for each atom."^^xsd:string ;
    rdfs:subClassOf [ a owl:Restriction ;
            owl:onProperty :hasQuantity ;
            owl:someValuesFrom :atomic_multipole_m_kind ],
        [ a owl:Restriction ;
            owl:onProperty :hasQuantity ;
            owl:someValuesFrom :atomic_multipole_lm ],
        [ a owl:Restriction ;
            owl:onProperty :hasQuantity ;
            owl:someValuesFrom :atomic_multipole_values ],
        [ a owl:Restriction ;
            owl:onProperty :hasQuantity ;
            owl:someValuesFrom :atomic_multipole_kind ],
        [ a owl:Restriction ;
            owl:onProperty :hasQuantity ;
            owl:someValuesFrom :number_of_lm_atomic_multipoles ],
        :NMI_section .

:section_band_gap a owl:Class ;
    rdfs:comment "This section stores information for a band gap within a band structure."^^xsd:string ;
    rdfs:subClassOf [ a owl:Restriction ;
            owl:onProperty :hasQuantity ;
            owl:someValuesFrom :valence_band_max_energy ],
        [ a owl:Restriction ;
            owl:onProperty :hasQuantity ;
            owl:someValuesFrom :type ],
        [ a owl:Restriction ;
            owl:onProperty :hasQuantity ;
            owl:someValuesFrom :conduction_band_min_energy ],
        [ a owl:Restriction ;
            owl:onProperty :hasQuantity ;
            owl:someValuesFrom :value ],
        [ a owl:Restriction ;
            owl:onProperty :hasQuantity ;
            owl:someValuesFrom :valence_band_max_k_point ],
        [ a owl:Restriction ;
            owl:onProperty :hasQuantity ;
            owl:someValuesFrom :conduction_band_min_k_point ],
        :NMI_section .

:section_basis_functions_atom_centered a owl:Class ;
    rdfs:comment "This section contains the description of the basis functions (at least one function) of the (atom-centered) basis set defined in section_basis_set_atom_centered."^^xsd:string ;
    rdfs:subClassOf :NMI_section .

:section_basis_set a owl:Class ;
    rdfs:comment """This section contains references to *all* basis sets used in this section_single_configuration_calculation. More than one basis set instance per *single
configuration calculation* (see section_single_configuration_calculation) may be
needed. This is true for example, for codes that implement adaptive basis sets along
the self-consistent field (SCF) convergence (e.g., exciting). In such cases, there is
a section_basis_set instance per SCF iteration, if necessary. Another example is
having a basis set for wavefunctions, a different one for the density, an auxiliary
basis set for resolution of identity (RI), etc.

Supported are the two broad classes of basis sets: *atom-centered* (e.g., Gaussian-
type, numerical atomic orbitals) and *cell-dependent* (like plane waves or real-space
grids, so named because they are typically used for periodic-system calculations and
dependent to the simulated cell as a whole).

Basis sets used in this section_single_configuration_calculation, belonging to either
class, are defined in the dedicated section: [section_basis_set_cell_dependent
](section_basis_set_cell_dependent) or section_basis_set_atom_centered. The
correspondence between the basis sets listed in this section and the definition given
in the dedicated sessions is given by the two concrete metadata:
mapping_section_basis_set_cell_dependent and mapping_section_basis_set_atom_centered.
The latter metadata is a list that connects each atom in the system with its basis
set, where the same basis set can be assigned to more than one atom."""^^xsd:string ;
    rdfs:subClassOf [ a owl:Restriction ;
            owl:onProperty :hasQuantity ;
            owl:someValuesFrom :basis_set_name ],
        [ a owl:Restriction ;
            owl:onProperty :hasQuantity ;
            owl:someValuesFrom :number_of_basis_functions ],
        [ a owl:Restriction ;
            owl:onProperty :hasQuantity ;
            owl:someValuesFrom :basis_set_kind ],
        [ a owl:Restriction ;
            owl:onProperty :hasQuantity ;
            owl:someValuesFrom :mapping_section_basis_set_atom_centered ],
        [ a owl:Restriction ;
            owl:onProperty :hasQuantity ;
            owl:someValuesFrom :mapping_section_basis_set_cell_dependent ],
        :NMI_section .

:section_basis_set_atom_centered a owl:Class ;
    rdfs:comment """This section describes the atom-centered basis set. The main contained information is a short, non unique but human-interpretable, name for identifying the basis set
(basis_set_atom_centered_short_name), a longer, unique name
(basis_set_atom_centered_unique_name), the atomic number of the atomic species the
basis set is meant for (basis_set_atom_number), and a list of actual basis functions
in the section_basis_functions_atom_centered section."""^^xsd:string ;
    rdfs:subClassOf [ a owl:Restriction ;
            owl:onProperty :hasSubSection ;
            owl:someValuesFrom :section_gaussian_basis_group ],
        [ a owl:Restriction ;
            owl:onProperty :hasQuantity ;
            owl:someValuesFrom :number_of_kinds_in_basis_set_atom_centered ],
        [ a owl:Restriction ;
            owl:onProperty :hasQuantity ;
            owl:someValuesFrom :basis_set_atom_centered_unique_name ],
        [ a owl:Restriction ;
            owl:onProperty :hasQuantity ;
            owl:someValuesFrom :basis_set_atom_number ],
        [ a owl:Restriction ;
            owl:onProperty :hasQuantity ;
            owl:someValuesFrom :number_of_basis_functions_in_basis_set_atom_centered ],
        [ a owl:Restriction ;
            owl:onProperty :hasQuantity ;
            owl:someValuesFrom :basis_set_atom_centered_ls ],
        [ a owl:Restriction ;
            owl:onProperty :hasQuantity ;
            owl:someValuesFrom :basis_set_atom_centered_short_name ],
        [ a owl:Restriction ;
            owl:onProperty :hasSubSection ;
            owl:someValuesFrom :section_basis_functions_atom_centered ],
        [ a owl:Restriction ;
            owl:onProperty :hasQuantity ;
            owl:someValuesFrom :basis_set_atom_centered_radial_functions ],
        :NMI_section .

:section_basis_set_cell_dependent a owl:Class ;
    rdfs:comment """Section describing a cell-dependent (atom-independent) basis set, e.g. plane waves. The contained information is the type of basis set (in basis_set_cell_dependent_kind),
its parameters (e.g., for plane waves in basis_set_planewave_cutoff), and a name that
identifies the actually used basis set (a string combining the type and the
parameter(s), stored in basis_set_cell_dependent_name)."""^^xsd:string ;
    rdfs:subClassOf [ a owl:Restriction ;
            owl:onProperty :hasQuantity ;
            owl:someValuesFrom :basis_set_planewave_cutoff ],
        [ a owl:Restriction ;
            owl:onProperty :hasQuantity ;
            owl:someValuesFrom :basis_set_cell_dependent_name ],
        [ a owl:Restriction ;
            owl:onProperty :hasQuantity ;
            owl:someValuesFrom :basis_set_cell_dependent_kind ],
        :NMI_section .

:section_brillouin_zone a owl:Class ;
    rdfs:comment "Defines a polyhedra for the Brillouin zone in reciprocal space."^^xsd:string ;
    rdfs:subClassOf [ a owl:Restriction ;
            owl:onProperty :hasQuantity ;
            owl:someValuesFrom :faces ],
        [ a owl:Restriction ;
            owl:onProperty :hasQuantity ;
            owl:someValuesFrom :vertices ],
        :NMI_section .

:section_calculation_to_calculation_refs a owl:Class ;
    rdfs:comment """Section that describes the relationship between different section_single_configuration_calculation sections.

For instance, one calculation is a perturbation performed using a self-consistent
field (SCF) calculation as starting point, or a simulated system is partitioned in
regions with different but connected Hamiltonians (e.g., QM/MM, or a region treated
via Kohn-Sham DFT embedded into a region treated via orbital-free DFT).

The kind of relationship between the calculation defined in this section and the
referenced one is described by calculation_to_calculation_kind. The referenced
section_single_configuration_calculation is identified via
calculation_to_calculation_ref (typically used for a
section_single_configuration_calculation in the same section_run) or
calculation_to_calculation_external_url."""^^xsd:string ;
    rdfs:subClassOf [ a owl:Restriction ;
            owl:onProperty :hasQuantity ;
            owl:someValuesFrom :calculation_to_calculation_kind ],
        [ a owl:Restriction ;
            owl:onProperty :hasQuantity ;
            owl:someValuesFrom :calculation_to_calculation_external_url ],
        [ a owl:Restriction ;
            owl:onProperty :hasQuantity ;
            owl:someValuesFrom :calculation_to_calculation_ref ],
        :NMI_section .

:section_calculation_to_folder_refs a owl:Class ;
    rdfs:comment """Section that describes the relationship between section_single_configuration_calculationa and the folder containing the original
calulations"""^^xsd:string ;
    rdfs:subClassOf [ a owl:Restriction ;
            owl:onProperty :hasQuantity ;
            owl:someValuesFrom :calculation_to_folder_external_url ],
        [ a owl:Restriction ;
            owl:onProperty :hasQuantity ;
            owl:someValuesFrom :calculation_to_folder_kind ],
        :NMI_section .

:section_constraint a owl:Class ;
    rdfs:comment "Section describing a constraint between arbitrary atoms."^^xsd:string ;
    rdfs:subClassOf [ a owl:Restriction ;
            owl:onProperty :hasQuantity ;
            owl:someValuesFrom :constraint_parameters ],
        [ a owl:Restriction ;
            owl:onProperty :hasQuantity ;
            owl:someValuesFrom :number_of_atoms_per_constraint ],
        [ a owl:Restriction ;
            owl:onProperty :hasQuantity ;
            owl:someValuesFrom :constraint_kind ],
        [ a owl:Restriction ;
            owl:onProperty :hasQuantity ;
            owl:someValuesFrom :number_of_constraints ],
        [ a owl:Restriction ;
            owl:onProperty :hasQuantity ;
            owl:someValuesFrom :constraint_atoms ],
        :NMI_section .

:section_dft_plus_u_orbital a owl:Class ;
    rdfs:comment "Section for DFT+U-settings of a single orbital"^^xsd:string ;
    rdfs:subClassOf [ a owl:Restriction ;
            owl:onProperty :hasQuantity ;
            owl:someValuesFrom :dft_plus_u_orbital_J ],
        [ a owl:Restriction ;
            owl:onProperty :hasQuantity ;
            owl:someValuesFrom :dft_plus_u_orbital_label ],
        [ a owl:Restriction ;
            owl:onProperty :hasQuantity ;
            owl:someValuesFrom :dft_plus_u_orbital_atom ],
        [ a owl:Restriction ;
            owl:onProperty :hasQuantity ;
            owl:someValuesFrom :dft_plus_u_orbital_U_effective ],
        [ a owl:Restriction ;
            owl:onProperty :hasQuantity ;
            owl:someValuesFrom :dft_plus_u_orbital_U ],
        :NMI_section .

:section_dos a owl:Class ;
    rdfs:comment "Section collecting information of a (electronic-energy or vibrational-energy) density of states (DOS) evaluation."^^xsd:string ;
    rdfs:subClassOf [ a owl:Restriction ;
            owl:onProperty :hasQuantity ;
            owl:someValuesFrom :dos_kind ],
        [ a owl:Restriction ;
            owl:onProperty :hasQuantity ;
            owl:someValuesFrom :dos_energies_normalized ],
        [ a owl:Restriction ;
            owl:onProperty :hasQuantity ;
            owl:someValuesFrom :number_of_dos_lms ],
        [ a owl:Restriction ;
            owl:onProperty :hasQuantity ;
            owl:someValuesFrom :number_of_dos_values ],
        [ a owl:Restriction ;
            owl:onProperty :hasQuantity ;
            owl:someValuesFrom :dos_integrated_values ],
        [ a owl:Restriction ;
            owl:onProperty :hasQuantity ;
            owl:someValuesFrom :dos_energies ],
        [ a owl:Restriction ;
            owl:onProperty :hasQuantity ;
            owl:someValuesFrom :dos_values_lm ],
        [ a owl:Restriction ;
            owl:onProperty :hasQuantity ;
            owl:someValuesFrom :dos_values ],
        [ a owl:Restriction ;
            owl:onProperty :hasQuantity ;
            owl:someValuesFrom :dos_fermi_energy ],
        [ a owl:Restriction ;
            owl:onProperty :hasSubSection ;
            owl:someValuesFrom :section_dos_fingerprint ],
        [ a owl:Restriction ;
            owl:onProperty :hasQuantity ;
            owl:someValuesFrom :dos_values_normalized ],
        [ a owl:Restriction ;
            owl:onProperty :hasQuantity ;
            owl:someValuesFrom :dos_lm ],
        [ a owl:Restriction ;
            owl:onProperty :hasQuantity ;
            owl:someValuesFrom :dos_m_kind ],
        :NMI_section .

:section_dos_fingerprint a owl:Class ;
    rdfs:comment """Section for the fingerprint of the electronic density-of-states (DOS). DOS fingerprints are a modification of the D-Fingerprints reported in Chem. Mater. 2015, 27, 3, 735–743
(doi:10.1021/cm503507h). The fingerprint consists of a binary representation of the DOS,
that is used to evaluate the similarity of materials based on their electronic structure."""^^xsd:string ;
    rdfs:subClassOf [ a owl:Restriction ;
            owl:onProperty :hasQuantity ;
            owl:someValuesFrom :filling_factor ],
        [ a owl:Restriction ;
            owl:onProperty :hasQuantity ;
            owl:someValuesFrom :stepsize ],
        [ a owl:Restriction ;
            owl:onProperty :hasQuantity ;
            owl:someValuesFrom :grid_id ],
        [ a owl:Restriction ;
            owl:onProperty :hasQuantity ;
            owl:someValuesFrom :indices ],
        [ a owl:Restriction ;
            owl:onProperty :hasQuantity ;
            owl:someValuesFrom :bins ],
        :NMI_section .

:section_eigenvalues a owl:Class ;
    rdfs:comment """Section containing (electronic-energy) eigenvalues for one spin channel. If, for example, the eigenvalues of the Kohn-Sham operator are to be stored, a string
identifying this kind of eigenvalues is put in eigenvalues_kind, the coordinates of
the $k$-points at which the eigenvalues are evaluated is stored in
eigenvalues_kpoints, and the energy values of the eigenstates and their occupation is
stored in eigenvalues_values and eigenvalues_occupation, respectively."""^^xsd:string ;
    rdfs:subClassOf [ a owl:Restriction ;
            owl:onProperty :hasQuantity ;
            owl:someValuesFrom :eigenvalues_kind ],
        [ a owl:Restriction ;
            owl:onProperty :hasQuantity ;
            owl:someValuesFrom :eigenvalues_kpoints ],
        [ a owl:Restriction ;
            owl:onProperty :hasQuantity ;
            owl:someValuesFrom :number_of_eigenvalues ],
        [ a owl:Restriction ;
            owl:onProperty :hasQuantity ;
            owl:someValuesFrom :eigenvalues_kpoints_multiplicity ],
        [ a owl:Restriction ;
            owl:onProperty :hasQuantity ;
            owl:someValuesFrom :number_of_band_segment_eigenvalues ],
        [ a owl:Restriction ;
            owl:onProperty :hasQuantity ;
            owl:someValuesFrom :eigenvalues_kpoints_weights ],
        [ a owl:Restriction ;
            owl:onProperty :hasQuantity ;
            owl:someValuesFrom :number_of_normalized_band_segment_eigenvalues ],
        [ a owl:Restriction ;
            owl:onProperty :hasQuantity ;
            owl:someValuesFrom :number_of_eigenvalues_kpoints ],
        [ a owl:Restriction ;
            owl:onProperty :hasQuantity ;
            owl:someValuesFrom :eigenvalues_values ],
        [ a owl:Restriction ;
            owl:onProperty :hasQuantity ;
            owl:someValuesFrom :gw_qp_linearization_prefactor ],
        [ a owl:Restriction ;
            owl:onProperty :hasQuantity ;
            owl:someValuesFrom :eigenvalues_occupation ],
        :NMI_section .

:section_energy_code_independent a owl:Class ;
    rdfs:comment """Section describing a code-independent total energy obtained by subtracting some reference energy calculated with the same code. It contains the type in
energy_code_independent_kind and the computed code-independent total energy in
energy_code_independent_value. The computed energy allows for comparisons among
different codes and numerical settings."""^^xsd:string ;
    rdfs:subClassOf [ a owl:Restriction ;
            owl:onProperty :hasQuantity ;
            owl:someValuesFrom :energy_code_independent_value ],
        [ a owl:Restriction ;
            owl:onProperty :hasQuantity ;
            owl:someValuesFrom :energy_code_independent_kind ],
        :NMI_section .

:section_energy_van_der_Waals a owl:Class ;
    rdfs:comment """Section containing the Van der Waals energy value (energy_van_der_Waals_value) of type van_der_Waals_kind. This is used when more than one Van der Waals methods are applied
in the same *single configuration calculation*, see
section_single_configuration_calculation. The main Van der Waals method (the one
concurring to energy_current, and used, e.g., for evaluating the forces for a
relaxation or dynamics) is given in energy_van_der_Waals and is defined in
settings_van_der_Waals."""^^xsd:string ;
    rdfs:subClassOf [ a owl:Restriction ;
            owl:onProperty :hasQuantity ;
            owl:someValuesFrom :energy_van_der_Waals ],
        [ a owl:Restriction ;
            owl:onProperty :hasQuantity ;
            owl:someValuesFrom :energy_van_der_Waals_value ],
        [ a owl:Restriction ;
            owl:onProperty :hasQuantity ;
            owl:someValuesFrom :energy_van_der_Waals_kind ],
        :NMI_section .

:section_excited_states a owl:Class ;
    rdfs:comment "Excited states properties."^^xsd:string ;
    rdfs:subClassOf [ a owl:Restriction ;
            owl:onProperty :hasQuantity ;
            owl:someValuesFrom :number_of_excited_states ],
        [ a owl:Restriction ;
            owl:onProperty :hasQuantity ;
            owl:someValuesFrom :oscillator_strengths ],
        [ a owl:Restriction ;
            owl:onProperty :hasQuantity ;
            owl:someValuesFrom :transition_dipole_moments ],
        [ a owl:Restriction ;
            owl:onProperty :hasQuantity ;
            owl:someValuesFrom :excitation_energies ],
        :NMI_section .

:section_frame_sequence a owl:Class ;
    rdfs:comment """Section containing a sequence of frames, i.e. a trajectory which can have number_of_frames_in_sequence each representing one
section_single_configuration_calculation section evaluated with a sampling method
(e.g, molecular dynamics, Monte Carlo, geometry optimization). The sampling method
might be a subset of the whole trajectory.

Information on the method used for the sampling can be found in the
section_sampling_method section and information of each frame of the sequence are
found in the section_single_configuration_calculation section."""^^xsd:string ;
    rdfs:subClassOf [ a owl:Restriction ;
            owl:onProperty :hasQuantity ;
            owl:someValuesFrom :frame_sequence_conserved_quantity_stats ],
        [ a owl:Restriction ;
            owl:onProperty :hasQuantity ;
            owl:someValuesFrom :frame_sequence_conserved_quantity ],
        [ a owl:Restriction ;
            owl:onProperty :hasQuantity ;
            owl:someValuesFrom :number_of_temperatures_in_sequence ],
        [ a owl:Restriction ;
            owl:onProperty :hasQuantity ;
            owl:someValuesFrom :frame_sequence_local_frames_ref ],
        [ a owl:Restriction ;
            owl:onProperty :hasQuantity ;
            owl:someValuesFrom :frame_sequence_kinetic_energy ],
        [ a owl:Restriction ;
            owl:onProperty :hasSubSection ;
            owl:someValuesFrom :section_frame_sequence_user_quantity ],
        [ a owl:Restriction ;
            owl:onProperty :hasQuantity ;
            owl:someValuesFrom :previous_sequence_ref ],
        [ a owl:Restriction ;
            owl:onProperty :hasQuantity ;
            owl:someValuesFrom :frame_sequence_potential_energy_frames ],
        [ a owl:Restriction ;
            owl:onProperty :hasQuantity ;
            owl:someValuesFrom :geometry_optimization_converged ],
        [ a owl:Restriction ;
            owl:onProperty :hasQuantity ;
            owl:someValuesFrom :frame_sequence_temperature ],
        [ a owl:Restriction ;
            owl:onProperty :hasQuantity ;
            owl:someValuesFrom :frame_sequence_pressure_stats ],
        [ a owl:Restriction ;
            owl:onProperty :hasQuantity ;
            owl:someValuesFrom :number_of_conserved_quantity_evaluations_in_sequence ],
        [ a owl:Restriction ;
            owl:onProperty :hasQuantity ;
            owl:someValuesFrom :frame_sequence_time ],
        [ a owl:Restriction ;
            owl:onProperty :hasQuantity ;
            owl:someValuesFrom :frame_sequence_conserved_quantity_frames ],
        [ a owl:Restriction ;
            owl:onProperty :hasQuantity ;
            owl:someValuesFrom :frame_sequence_pressure ],
        [ a owl:Restriction ;
            owl:onProperty :hasQuantity ;
            owl:someValuesFrom :number_of_pressure_evaluations_in_sequence ],
        [ a owl:Restriction ;
            owl:onProperty :hasQuantity ;
            owl:someValuesFrom :frame_sequence_temperature_frames ],
        [ a owl:Restriction ;
            owl:onProperty :hasQuantity ;
            owl:someValuesFrom :frame_sequence_potential_energy ],
        [ a owl:Restriction ;
            owl:onProperty :hasQuantity ;
            owl:someValuesFrom :number_of_frames_in_sequence ],
        [ a owl:Restriction ;
            owl:onProperty :hasQuantity ;
            owl:someValuesFrom :frame_sequence_temperature_stats ],
        [ a owl:Restriction ;
            owl:onProperty :hasQuantity ;
            owl:someValuesFrom :frame_sequence_continuation_kind ],
        [ a owl:Restriction ;
            owl:onProperty :hasQuantity ;
            owl:someValuesFrom :number_of_kinetic_energies_in_sequence ],
        [ a owl:Restriction ;
            owl:onProperty :hasQuantity ;
            owl:someValuesFrom :number_of_potential_energies_in_sequence ],
        [ a owl:Restriction ;
            owl:onProperty :hasQuantity ;
            owl:someValuesFrom :frame_sequence_pressure_frames ],
        [ a owl:Restriction ;
            owl:onProperty :hasQuantity ;
            owl:someValuesFrom :frame_sequence_potential_energy_stats ],
        [ a owl:Restriction ;
            owl:onProperty :hasQuantity ;
            owl:someValuesFrom :frame_sequence_kinetic_energy_frames ],
        [ a owl:Restriction ;
            owl:onProperty :hasQuantity ;
            owl:someValuesFrom :frame_sequence_kinetic_energy_stats ],
        [ a owl:Restriction ;
            owl:onProperty :hasSubSection ;
            owl:someValuesFrom :section_thermodynamical_properties ],
        [ a owl:Restriction ;
            owl:onProperty :hasQuantity ;
            owl:someValuesFrom :frame_sequence_to_sampling_ref ],
        [ a owl:Restriction ;
            owl:onProperty :hasQuantity ;
            owl:someValuesFrom :frame_sequence_external_url ],
        :NMI_section .

:section_frame_sequence_user_quantity a owl:Class ;
    rdfs:comment "Section collecting some user-defined quantities evaluated along a sequence of frame."^^xsd:string ;
    rdfs:subClassOf [ a owl:Restriction ;
            owl:onProperty :hasQuantity ;
            owl:someValuesFrom :frame_sequence_user_quantity_stats ],
        [ a owl:Restriction ;
            owl:onProperty :hasQuantity ;
            owl:someValuesFrom :frame_sequence_user_quantity_frames ],
        [ a owl:Restriction ;
            owl:onProperty :hasQuantity ;
            owl:someValuesFrom :number_of_user_quantity_evaluations_in_sequence ],
        [ a owl:Restriction ;
            owl:onProperty :hasQuantity ;
            owl:someValuesFrom :frame_sequence_user_quantity_name ],
        [ a owl:Restriction ;
            owl:onProperty :hasQuantity ;
            owl:someValuesFrom :frame_sequence_user_quantity ],
        [ a owl:Restriction ;
            owl:onProperty :hasQuantity ;
            owl:someValuesFrom :number_of_frame_sequence_user_quantity_components ],
        :NMI_section .

:section_gaussian_basis_group a owl:Class ;
    rdfs:comment """Section that describes a group of Gaussian contractions. Groups allow one to calculate the primitive Gaussian integrals once for several different linear combinations of
them. This defines basis functions with radial part $f_i(r) = r^{l_i} \\\\sum_{j} c_{i
j} A(l_i, \\\\alpha_j) exp(-\\\\alpha_j r^2)$ where $A(l_i, \\\\alpha_j)$ is a the
normalization coefficient for primitive Gaussian basis functions. Here, $\\\\alpha_j$ is
defined in gaussian_basis_group_exponents, $l_i$ is given in gaussian_basis_group_ls,
and $c_{i j}$ is given in gaussian_basis_group_contractions, whereas the radial part
is given by the spherical harmonics $Y_{l m}$.

This section is defined only if the original basis function uses Gaussian basis
functions, and the sequence of radial functions $f_i$ across all
section_gaussian_basis_group in section_basis_set_atom_centered should match the one
of basis_set_atom_centered_radial_functions."""^^xsd:string ;
    rdfs:subClassOf [ a owl:Restriction ;
            owl:onProperty :hasQuantity ;
            owl:someValuesFrom :number_of_gaussian_basis_group_exponents ],
        [ a owl:Restriction ;
            owl:onProperty :hasQuantity ;
            owl:someValuesFrom :gaussian_basis_group_exponents ],
        [ a owl:Restriction ;
            owl:onProperty :hasQuantity ;
            owl:someValuesFrom :gaussian_basis_group_contractions ],
        [ a owl:Restriction ;
            owl:onProperty :hasQuantity ;
            owl:someValuesFrom :gaussian_basis_group_ls ],
        [ a owl:Restriction ;
            owl:onProperty :hasQuantity ;
            owl:someValuesFrom :number_of_gaussian_basis_group_contractions ],
        :NMI_section .

:section_interaction a owl:Class ;
    rdfs:comment "Section containing the description of a bonded interaction between arbitrary atoms."^^xsd:string ;
    rdfs:subClassOf [ a owl:Restriction ;
            owl:onProperty :hasQuantity ;
            owl:someValuesFrom :interaction_atoms ],
        [ a owl:Restriction ;
            owl:onProperty :hasQuantity ;
            owl:someValuesFrom :number_of_atoms_per_interaction ],
        [ a owl:Restriction ;
            owl:onProperty :hasQuantity ;
            owl:someValuesFrom :interaction_kind ],
        [ a owl:Restriction ;
            owl:onProperty :hasQuantity ;
            owl:someValuesFrom :interaction_parameters ],
        [ a owl:Restriction ;
            owl:onProperty :hasQuantity ;
            owl:someValuesFrom :number_of_interactions ],
        :NMI_section .

:section_k_band a owl:Class ;
    rdfs:comment """This section stores information on a $k$-band (electronic or vibrational band structure) evaluation along one-dimensional pathways in the $k$ or $q$ (reciprocal)
space given in section_k_band_segment. Eigenvalues calculated at the actual $k$-mesh
used for energy_total evaluations, can be found in the section_eigenvalues section."""^^xsd:string ;
    rdfs:subClassOf [ a owl:Restriction ;
            owl:onProperty :hasQuantity ;
            owl:someValuesFrom :band_structure_kind ],
        [ a owl:Restriction ;
            owl:onProperty :hasSubSection ;
            owl:someValuesFrom :section_brillouin_zone ],
        [ a owl:Restriction ;
            owl:onProperty :hasSubSection ;
            owl:someValuesFrom :section_k_band_segment ],
        [ a owl:Restriction ;
            owl:onProperty :hasQuantity ;
            owl:someValuesFrom :reciprocal_cell ],
        [ a owl:Restriction ;
            owl:onProperty :hasQuantity ;
            owl:someValuesFrom :is_standard_path ],
        [ a owl:Restriction ;
            owl:onProperty :hasSubSection ;
            owl:someValuesFrom :section_band_gap ],
        :NMI_section .

:section_k_band_normalized a owl:Class ;
    rdfs:comment """This section stores information on a normalized $k$-band (electronic band structure) evaluation along one-dimensional pathways in the $k$ (reciprocal) space given in
section_k_band_segment. Eigenvalues calculated at the actual $k$-mesh used for
energy_total evaluations, can be found in the section_eigenvalues section."""^^xsd:string ;
    rdfs:subClassOf [ a owl:Restriction ;
            owl:onProperty :hasQuantity ;
            owl:someValuesFrom :k_band_path_normalized_is_standard ],
        [ a owl:Restriction ;
            owl:onProperty :hasSubSection ;
            owl:someValuesFrom :section_k_band_segment_normalized ],
        :NMI_section .

:section_k_band_segment a owl:Class ;
    rdfs:comment """Section collecting the information on a $k$-band or $q$-band segment. This section stores band structures along a one-dimensional pathway in the $k$ or $q$ (reciprocal)
space.

Eigenvalues calculated at the actual $k$-mesh used for energy_total evaluations are
defined in section_eigenvalues and the band structures are represented as third-order
tensors: one dimension for the spin channels, one for the sequence of $k$ or $q$
points for the segment (given in number_of_k_points_per_segment), and one for the
sequence of eigenvalues at a given $k$ or $q$ point. The values of the $k$ or $q$
points in each segment are stored in band_k_points. The energies and occupation for
each eigenstate, at each $k$ or $q$ point, segment, and spin channel are stored in
band_energies and band_occupations, respectively. The labels for the segment are
specified in band_segm_labels."""^^xsd:string ;
    rdfs:subClassOf [ a owl:Restriction ;
            owl:onProperty :hasQuantity ;
            owl:someValuesFrom :band_segm_start_end ],
        [ a owl:Restriction ;
            owl:onProperty :hasQuantity ;
            owl:someValuesFrom :band_segm_labels ],
        [ a owl:Restriction ;
            owl:onProperty :hasQuantity ;
            owl:someValuesFrom :number_of_k_points_per_segment ],
        [ a owl:Restriction ;
            owl:onProperty :hasQuantity ;
            owl:someValuesFrom :band_occupations ],
        [ a owl:Restriction ;
            owl:onProperty :hasQuantity ;
            owl:someValuesFrom :band_k_points ],
        [ a owl:Restriction ;
            owl:onProperty :hasQuantity ;
            owl:someValuesFrom :band_energies ],
        :NMI_section .

:section_k_band_segment_normalized a owl:Class ;
    rdfs:comment """Section collecting the information on a normalized $k$-band segment. This section stores band structures along a one-dimensional pathway in the $k$ (reciprocal) space.

Eigenvalues calculated at the actual $k$-mesh used for energy_total evaluations are
defined in section_eigenvalues and the band structures are represented as third-order
tensors: one dimension for the spin channels, one for the sequence of $k$ points for
the segment (given in number_of_k_points_per_segment), and one for the sequence of
eigenvalues at a given $k$ point. The values of the $k$ points in each segment are
stored in band_k_points. The energies and occupation for each eigenstate, at each $k$
point, segment, and spin channel are stored in band_energies and band_occupations,
respectively. The labels for the segment are specified in band_segm_labels."""^^xsd:string ;
    rdfs:subClassOf [ a owl:Restriction ;
            owl:onProperty :hasQuantity ;
            owl:someValuesFrom :band_occupations_normalized ],
        [ a owl:Restriction ;
            owl:onProperty :hasQuantity ;
            owl:someValuesFrom :number_of_normalized_k_points_per_segment ],
        [ a owl:Restriction ;
            owl:onProperty :hasQuantity ;
            owl:someValuesFrom :band_segm_labels_normalized ],
        [ a owl:Restriction ;
            owl:onProperty :hasQuantity ;
            owl:someValuesFrom :band_segm_start_end_normalized ],
        [ a owl:Restriction ;
            owl:onProperty :hasQuantity ;
            owl:someValuesFrom :band_energies_normalized ],
        [ a owl:Restriction ;
            owl:onProperty :hasQuantity ;
            owl:someValuesFrom :band_k_points_normalized ],
        :NMI_section .

:section_method a owl:Class ;
    rdfs:comment """Section containing the various parameters that define the theory and the approximations (convergence, thresholds,...) to perform a *single configuration
calculation*, see section_single_configuration_calculation.

*NOTE*: This section does not contain settings for molecular dynamics, geometry
optimization etc. See section frame_sequence for these other settings instead."""^^xsd:string ;
    rdfs:subClassOf [ a owl:Restriction ;
            owl:onProperty :hasQuantity ;
            owl:someValuesFrom :number_of_k_mesh_points ],
        [ a owl:Restriction ;
            owl:onProperty :hasSubSection ;
            owl:someValuesFrom :section_dft_plus_u_orbital ],
        [ a owl:Restriction ;
            owl:onProperty :hasQuantity ;
            owl:someValuesFrom :gw_frequency_weights ],
        [ a owl:Restriction ;
            owl:onProperty :hasQuantity ;
            owl:someValuesFrom :dft_plus_u_projection_type ],
        [ a owl:Restriction ;
            owl:onProperty :hasQuantity ;
            owl:someValuesFrom :gw_basis_set ],
        [ a owl:Restriction ;
            owl:onProperty :hasQuantity ;
            owl:someValuesFrom :method_to_topology_ref ],
        [ a owl:Restriction ;
            owl:onProperty :hasQuantity ;
            owl:someValuesFrom :number_of_spin_channels ],
        [ a owl:Restriction ;
            owl:onProperty :hasQuantity ;
            owl:someValuesFrom :van_der_Waals_method ],
        [ a owl:Restriction ;
            owl:onProperty :hasQuantity ;
            owl:someValuesFrom :scf_threshold_energy_change ],
        [ a owl:Restriction ;
            owl:onProperty :hasQuantity ;
            owl:someValuesFrom :relativity_method ],
        [ a owl:Restriction ;
            owl:onProperty :hasQuantity ;
            owl:someValuesFrom :calculation_method_kind ],
        [ a owl:Restriction ;
            owl:onProperty :hasQuantity ;
            owl:someValuesFrom :calculation_method ],
        [ a owl:Restriction ;
            owl:onProperty :hasQuantity ;
            owl:someValuesFrom :total_charge ],
        [ a owl:Restriction ;
            owl:onProperty :hasQuantity ;
            owl:someValuesFrom :gw_starting_point ],
        [ a owl:Restriction ;
            owl:onProperty :hasQuantity ;
            owl:someValuesFrom :gw_type ],
        [ a owl:Restriction ;
            owl:onProperty :hasQuantity ;
            owl:someValuesFrom :gw_mixed_basis_gmax ],
        [ a owl:Restriction ;
            owl:onProperty :hasQuantity ;
            owl:someValuesFrom :gw_bare_coulomb_cutofftype ],
        [ a owl:Restriction ;
            owl:onProperty :hasQuantity ;
            owl:someValuesFrom :smearing_kind ],
        [ a owl:Restriction ;
            owl:onProperty :hasSubSection ;
            owl:someValuesFrom :section_method_basis_set ],
        [ a owl:Restriction ;
            owl:onProperty :hasQuantity ;
            owl:someValuesFrom :XC_method_current ],
        [ a owl:Restriction ;
            owl:onProperty :hasQuantity ;
            owl:someValuesFrom :gw_qp_equation_treatment ],
        [ a owl:Restriction ;
            owl:onProperty :hasQuantity ;
            owl:someValuesFrom :gw_screened_coulomb_volume_average ],
        [ a owl:Restriction ;
            owl:onProperty :hasQuantity ;
            owl:someValuesFrom :gw_type_test ],
        [ a owl:Restriction ;
            owl:onProperty :hasQuantity ;
            owl:someValuesFrom :spin_target_multiplicity ],
        [ a owl:Restriction ;
            owl:onProperty :hasQuantity ;
            owl:someValuesFrom :self_interaction_correction_method ],
        [ a owl:Restriction ;
            owl:onProperty :hasQuantity ;
            owl:someValuesFrom :gw_screened_Coulomb ],
        [ a owl:Restriction ;
            owl:onProperty :hasSubSection ;
            owl:someValuesFrom :section_XC_functionals ],
        [ a owl:Restriction ;
            owl:onProperty :hasQuantity ;
            owl:someValuesFrom :gw_ngridq ],
        [ a owl:Restriction ;
            owl:onProperty :hasQuantity ;
            owl:someValuesFrom :stress_tensor_method ],
        [ a owl:Restriction ;
            owl:onProperty :hasQuantity ;
            owl:someValuesFrom :dft_plus_u_functional ],
        [ a owl:Restriction ;
            owl:onProperty :hasQuantity ;
            owl:someValuesFrom :smearing_width ],
        [ a owl:Restriction ;
            owl:onProperty :hasQuantity ;
            owl:someValuesFrom :gw_frequency_number ],
        [ a owl:Restriction ;
            owl:onProperty :hasQuantity ;
            owl:someValuesFrom :gw_bare_coulomb_gmax ],
        [ a owl:Restriction ;
            owl:onProperty :hasQuantity ;
            owl:someValuesFrom :gw_self_energy_c_analytical_continuation ],
        [ a owl:Restriction ;
            owl:onProperty :hasSubSection ;
            owl:someValuesFrom :section_method_atom_kind ],
        [ a owl:Restriction ;
            owl:onProperty :hasQuantity ;
            owl:someValuesFrom :calculation_method_current ],
        [ a owl:Restriction ;
            owl:onProperty :hasQuantity ;
            owl:someValuesFrom :k_mesh_points ],
        [ a owl:Restriction ;
            owl:onProperty :hasQuantity ;
            owl:someValuesFrom :XC_functional ],
        [ a owl:Restriction ;
            owl:onProperty :hasQuantity ;
            owl:someValuesFrom :scf_max_iteration ],
        [ a owl:Restriction ;
            owl:onProperty :hasQuantity ;
            owl:someValuesFrom :gw_mixed_basis_lmax ],
        [ a owl:Restriction ;
            owl:onProperty :hasQuantity ;
            owl:someValuesFrom :gw_mixed_basis_tolerance ],
        [ a owl:Restriction ;
            owl:onProperty :hasQuantity ;
            owl:someValuesFrom :basis_set ],
        [ a owl:Restriction ;
            owl:onProperty :hasQuantity ;
            owl:someValuesFrom :gw_core_treatment ],
        [ a owl:Restriction ;
            owl:onProperty :hasQuantity ;
            owl:someValuesFrom :gw_polarizability_number_of_empty_states ],
        [ a owl:Restriction ;
            owl:onProperty :hasQuantity ;
            owl:someValuesFrom :gw_self_energy_c_number_of_poles ],
        [ a owl:Restriction ;
            owl:onProperty :hasQuantity ;
            owl:someValuesFrom :gw_frequency_values ],
        [ a owl:Restriction ;
            owl:onProperty :hasQuantity ;
            owl:someValuesFrom :electronic_structure_method ],
        [ a owl:Restriction ;
            owl:onProperty :hasQuantity ;
            owl:someValuesFrom :k_mesh_weights ],
        [ a owl:Restriction ;
            owl:onProperty :hasQuantity ;
            owl:someValuesFrom :gw_self_energy_c_number_of_empty_states ],
        [ a owl:Restriction ;
            owl:onProperty :hasQuantity ;
            owl:someValuesFrom :gw_max_frequency ],
        [ a owl:Restriction ;
            owl:onProperty :hasQuantity ;
            owl:someValuesFrom :gw_number_of_frequencies ],
        [ a owl:Restriction ;
            owl:onProperty :hasSubSection ;
            owl:someValuesFrom :section_method_to_method_refs ],
        [ a owl:Restriction ;
            owl:onProperty :hasQuantity ;
            owl:someValuesFrom :gw_self_energy_singularity_treatment ],
        [ a owl:Restriction ;
            owl:onProperty :hasQuantity ;
            owl:someValuesFrom :XC_method ],
        [ a owl:Restriction ;
            owl:onProperty :hasQuantity ;
            owl:someValuesFrom :gw_frequency_grid_type ],
        :NMI_section .

:section_method_atom_kind a owl:Class ;
    rdfs:comment """Every section_method_atom_kind section contains method-related information about a kind of atom, and is identified by one or more strings stored in
method_atom_kind_label.

This categorization into atom kinds is more flexible than just atomic species, because
to different atoms of the same species different atom-centered basis sets or pseudo-
potentials may be assigned. For instance, if two different oxygen atoms are assigned
to different basis sets or pseudo-potentials, they have to distinguished into two
different *kinds* of O atoms, by creating two distinct section_method_atom_kind
sections."""^^xsd:string ;
    rdfs:subClassOf [ a owl:Restriction ;
            owl:onProperty :hasQuantity ;
            owl:someValuesFrom :method_atom_kind_mass ],
        [ a owl:Restriction ;
            owl:onProperty :hasQuantity ;
            owl:someValuesFrom :method_atom_kind_explicit_electrons ],
        [ a owl:Restriction ;
            owl:onProperty :hasQuantity ;
            owl:someValuesFrom :method_atom_kind_pseudopotential_name ],
        [ a owl:Restriction ;
            owl:onProperty :hasQuantity ;
            owl:someValuesFrom :method_atom_kind_atom_number ],
        [ a owl:Restriction ;
            owl:onProperty :hasQuantity ;
            owl:someValuesFrom :method_atom_kind_label ],
        :NMI_section .

:section_method_basis_set a owl:Class ;
    rdfs:comment "This section contains the definition of the basis sets that are defined independently of the atomic configuration."^^xsd:string ;
    rdfs:subClassOf [ a owl:Restriction ;
            owl:onProperty :hasQuantity ;
            owl:someValuesFrom :method_basis_set_kind ],
        [ a owl:Restriction ;
            owl:onProperty :hasQuantity ;
            owl:someValuesFrom :mapping_section_method_basis_set_cell_associated ],
        [ a owl:Restriction ;
            owl:onProperty :hasQuantity ;
            owl:someValuesFrom :mapping_section_method_basis_set_atom_centered ],
        [ a owl:Restriction ;
            owl:onProperty :hasQuantity ;
            owl:someValuesFrom :number_of_basis_sets_atom_centered ],
        :NMI_section .

:section_method_to_method_refs a owl:Class ;
    rdfs:comment """Section that describes the relationship between different section_method sections. For instance, one calculation is a perturbation performed using a self-consistent
field (SCF) calculation as starting point, or a simulated system is partitioned in
regions with different but connected Hamiltonians (e.g., QM/MM, or a region treated
via Kohn-Sham DFT embedded into a region treated via orbital-free DFT).

The kind of relationship between the method defined in this section and the referenced
one is described by method_to_method_kind. The referenced section section_method is
identified via method_to_method_ref (typically used for a section_method section in
the same section_run) or method_to_method_external_url."""^^xsd:string ;
    rdfs:subClassOf [ a owl:Restriction ;
            owl:onProperty :hasQuantity ;
            owl:someValuesFrom :method_to_method_kind ],
        [ a owl:Restriction ;
            owl:onProperty :hasQuantity ;
            owl:someValuesFrom :method_to_method_external_url ],
        [ a owl:Restriction ;
            owl:onProperty :hasQuantity ;
            owl:someValuesFrom :method_to_method_ref ],
        :NMI_section .

:section_molecule_constraint a owl:Class ;
    rdfs:comment "Section describing a constraint between atoms within a molecule."^^xsd:string ;
    rdfs:subClassOf [ a owl:Restriction ;
            owl:onProperty :hasQuantity ;
            owl:someValuesFrom :number_of_atoms_per_molecule_constraint ],
        [ a owl:Restriction ;
            owl:onProperty :hasQuantity ;
            owl:someValuesFrom :molecule_constraint_atoms ],
        [ a owl:Restriction ;
            owl:onProperty :hasQuantity ;
            owl:someValuesFrom :molecule_constraint_parameters ],
        [ a owl:Restriction ;
            owl:onProperty :hasQuantity ;
            owl:someValuesFrom :number_of_molecule_constraints ],
        [ a owl:Restriction ;
            owl:onProperty :hasQuantity ;
            owl:someValuesFrom :molecule_constraint_kind ],
        :NMI_section .

:section_molecule_interaction a owl:Class ;
    rdfs:comment "Section describing a bonded interaction between atoms within a molecule."^^xsd:string ;
    rdfs:subClassOf [ a owl:Restriction ;
            owl:onProperty :hasQuantity ;
            owl:someValuesFrom :molecule_interaction_atoms ],
        [ a owl:Restriction ;
            owl:onProperty :hasQuantity ;
            owl:someValuesFrom :number_of_molecule_interactions ],
        [ a owl:Restriction ;
            owl:onProperty :hasQuantity ;
            owl:someValuesFrom :number_of_atoms_per_molecule_interaction ],
        [ a owl:Restriction ;
            owl:onProperty :hasQuantity ;
            owl:someValuesFrom :molecule_interaction_parameters ],
        [ a owl:Restriction ;
            owl:onProperty :hasQuantity ;
            owl:someValuesFrom :molecule_interaction_kind ],
        :NMI_section .

:section_molecule_type a owl:Class ;
    rdfs:comment "Section describing a type of molecule in the system."^^xsd:string ;
    rdfs:subClassOf [ a owl:Restriction ;
            owl:onProperty :hasQuantity ;
            owl:someValuesFrom :atom_in_molecule_to_atom_type_ref ],
        [ a owl:Restriction ;
            owl:onProperty :hasSubSection ;
            owl:someValuesFrom :section_molecule_constraint ],
        [ a owl:Restriction ;
            owl:onProperty :hasQuantity ;
            owl:someValuesFrom :molecule_type_name ],
        [ a owl:Restriction ;
            owl:onProperty :hasQuantity ;
            owl:someValuesFrom :atom_in_molecule_charge ],
        [ a owl:Restriction ;
            owl:onProperty :hasQuantity ;
            owl:someValuesFrom :atom_in_molecule_name ],
        [ a owl:Restriction ;
            owl:onProperty :hasQuantity ;
            owl:someValuesFrom :number_of_atoms_in_molecule ],
        [ a owl:Restriction ;
            owl:onProperty :hasSubSection ;
            owl:someValuesFrom :section_molecule_interaction ],
        :NMI_section .

:section_original_system a owl:Class ;
    rdfs:comment "Section containing symmetry information that is specific to the original system."^^xsd:string ;
    rdfs:subClassOf [ a owl:Restriction ;
            owl:onProperty :hasQuantity ;
            owl:someValuesFrom :equivalent_atoms_original ],
        [ a owl:Restriction ;
            owl:onProperty :hasQuantity ;
            owl:someValuesFrom :wyckoff_letters_original ],
        :NMI_section .

:section_primitive_system a owl:Class ;
    rdfs:comment """Section containing symmetry information that is specific to the primitive system. The primitive system is derived from the standardized system with a transformation that is
specific to the centring. The transformation matrices can be found e.g. from here:
https://atztogo.github.io/spglib/definition.html#transformation-to-the-primitive-cell"""^^xsd:string ;
    rdfs:subClassOf [ a owl:Restriction ;
            owl:onProperty :hasQuantity ;
            owl:someValuesFrom :atomic_numbers_primitive ],
        [ a owl:Restriction ;
            owl:onProperty :hasQuantity ;
            owl:someValuesFrom :atom_positions_primitive ],
        [ a owl:Restriction ;
            owl:onProperty :hasQuantity ;
            owl:someValuesFrom :number_of_atoms_primitive ],
        [ a owl:Restriction ;
            owl:onProperty :hasQuantity ;
            owl:someValuesFrom :equivalent_atoms_primitive ],
        [ a owl:Restriction ;
            owl:onProperty :hasQuantity ;
            owl:someValuesFrom :wyckoff_letters_primitive ],
        [ a owl:Restriction ;
            owl:onProperty :hasQuantity ;
            owl:someValuesFrom :lattice_vectors_primitive ],
        :NMI_section .

:section_prototype a owl:Class ;
    rdfs:comment "Information on the prototype corresponding to the current section."^^xsd:string ;
    rdfs:subClassOf [ a owl:Restriction ;
            owl:onProperty :hasQuantity ;
            owl:someValuesFrom :prototype_aflow_url ],
        [ a owl:Restriction ;
            owl:onProperty :hasQuantity ;
            owl:someValuesFrom :prototype_aflow_id ],
        [ a owl:Restriction ;
            owl:onProperty :hasQuantity ;
            owl:someValuesFrom :prototype_label ],
        [ a owl:Restriction ;
            owl:onProperty :hasQuantity ;
            owl:someValuesFrom :prototype_assignment_method ],
        :NMI_section .

:section_sampling_method a owl:Class ;
    rdfs:comment """Section containing the settings describing a (potential-energy surface) sampling method.

Results and monitored quantities of such sampling are collected in a sequence of
frames, section_frame_sequence."""^^xsd:string ;
    rdfs:subClassOf [ a owl:Restriction ;
            owl:onProperty :hasQuantity ;
            owl:someValuesFrom :geometry_optimization_geometry_change ],
        [ a owl:Restriction ;
            owl:onProperty :hasQuantity ;
            owl:someValuesFrom :ensemble_type ],
        [ a owl:Restriction ;
            owl:onProperty :hasQuantity ;
            owl:someValuesFrom :geometry_optimization_threshold_force ],
        [ a owl:Restriction ;
            owl:onProperty :hasQuantity ;
            owl:someValuesFrom :sampling_method_expansion_order ],
        [ a owl:Restriction ;
            owl:onProperty :hasQuantity ;
            owl:someValuesFrom :geometry_optimization_energy_change ],
        [ a owl:Restriction ;
            owl:onProperty :hasQuantity ;
            owl:someValuesFrom :geometry_optimization_method ],
        [ a owl:Restriction ;
            owl:onProperty :hasQuantity ;
            owl:someValuesFrom :sampling_method ],
        :NMI_section .

:section_scf_iteration a owl:Class ;
    rdfs:comment """Every section_scf_iteration represents a self-consistent field (SCF) iteration, see scf_info, and gives detailed information on the SCF procedure of the specified
quantities."""^^xsd:string ;
    rdfs:subClassOf [ a owl:Restriction ;
            owl:onProperty :hasQuantity ;
            owl:someValuesFrom :time_scf_iteration_date_end ],
        [ a owl:Restriction ;
            owl:onProperty :hasQuantity ;
            owl:someValuesFrom :energy_XC_scf_iteration ],
        [ a owl:Restriction ;
            owl:onProperty :hasQuantity ;
            owl:someValuesFrom :energy_correction_entropy_scf_iteration ],
        [ a owl:Restriction ;
            owl:onProperty :hasQuantity ;
            owl:someValuesFrom :time_scf_iteration_date_start ],
        [ a owl:Restriction ;
            owl:onProperty :hasQuantity ;
            owl:someValuesFrom :time_scf_iteration_wall_end ],
        [ a owl:Restriction ;
            owl:onProperty :hasQuantity ;
            owl:someValuesFrom :energy_electrostatic_scf_iteration ],
        [ a owl:Restriction ;
            owl:onProperty :hasQuantity ;
            owl:someValuesFrom :time_scf_iteration_wall_start ],
        [ a owl:Restriction ;
            owl:onProperty :hasQuantity ;
            owl:someValuesFrom :spin_S2_scf_iteration ],
        [ a owl:Restriction ;
            owl:onProperty :hasQuantity ;
            owl:someValuesFrom :energy_reference_lowest_unoccupied_iteration ],
        [ a owl:Restriction ;
            owl:onProperty :hasQuantity ;
            owl:someValuesFrom :energy_XC_potential_scf_iteration ],
        [ a owl:Restriction ;
            owl:onProperty :hasQuantity ;
            owl:someValuesFrom :time_scf_iteration_cpu1_end ],
        [ a owl:Restriction ;
            owl:onProperty :hasQuantity ;
            owl:someValuesFrom :energy_hartree_error_scf_iteration ],
        [ a owl:Restriction ;
            owl:onProperty :hasQuantity ;
            owl:someValuesFrom :energy_sum_eigenvalues_per_atom_scf_iteration ],
        [ a owl:Restriction ;
            owl:onProperty :hasQuantity ;
            owl:someValuesFrom :energy_free_per_atom_scf_iteration ],
        [ a owl:Restriction ;
            owl:onProperty :hasQuantity ;
            owl:someValuesFrom :energy_total_T0_scf_iteration ],
        [ a owl:Restriction ;
            owl:onProperty :hasQuantity ;
            owl:someValuesFrom :energy_correction_hartree_scf_iteration ],
        [ a owl:Restriction ;
            owl:onProperty :hasQuantity ;
            owl:someValuesFrom :energy_change_scf_iteration ],
        [ a owl:Restriction ;
            owl:onProperty :hasQuantity ;
            owl:someValuesFrom :energy_total_scf_iteration ],
        [ a owl:Restriction ;
            owl:onProperty :hasQuantity ;
            owl:someValuesFrom :energy_reference_fermi_iteration ],
        [ a owl:Restriction ;
            owl:onProperty :hasQuantity ;
            owl:someValuesFrom :energy_reference_highest_occupied_iteration ],
        [ a owl:Restriction ;
            owl:onProperty :hasQuantity ;
            owl:someValuesFrom :time_scf_iteration_cpu1_start ],
        [ a owl:Restriction ;
            owl:onProperty :hasQuantity ;
            owl:someValuesFrom :electronic_kinetic_energy_scf_iteration ],
        [ a owl:Restriction ;
            owl:onProperty :hasQuantity ;
            owl:someValuesFrom :energy_total_T0_per_atom_scf_iteration ],
        [ a owl:Restriction ;
            owl:onProperty :hasQuantity ;
            owl:someValuesFrom :energy_sum_eigenvalues_scf_iteration ],
        [ a owl:Restriction ;
            owl:onProperty :hasQuantity ;
            owl:someValuesFrom :energy_free_scf_iteration ],
        :NMI_section .

:section_single_configuration_calculation a owl:Class ;
    rdfs:comment """Every section_single_configuration_calculation section contains the values computed during a *single configuration calculation*, i.e. a calculation performed on a given
configuration of the system (as defined in section_system) and a given computational
method (e.g., exchange-correlation method, basis sets, as defined in section_method).

The link between the current section_single_configuration_calculation and the related
section_system and section_method sections is established by the values stored in
single_configuration_calculation_to_system_ref and
single_configuration_to_calculation_method_ref, respectively.

The reason why information on the system configuration and computational method is
stored separately is that several *single configuration calculations* can be performed
on the same system configuration, viz. several system configurations can be evaluated
with the same computational method. This storage strategy avoids redundancies."""^^xsd:string ;
    rdfs:subClassOf [ a owl:Restriction ;
            owl:onProperty :hasQuantity ;
            owl:someValuesFrom :energy_total ],
        [ a owl:Restriction ;
            owl:onProperty :hasQuantity ;
            owl:someValuesFrom :energy_total_T0 ],
        [ a owl:Restriction ;
            owl:onProperty :hasQuantity ;
            owl:someValuesFrom :energy_C ],
        [ a owl:Restriction ;
            owl:onProperty :hasQuantity ;
            owl:someValuesFrom :single_configuration_calculation_converged ],
        [ a owl:Restriction ;
            owl:onProperty :hasQuantity ;
            owl:someValuesFrom :atom_forces_free ],
        [ a owl:Restriction ;
            owl:onProperty :hasQuantity ;
            owl:someValuesFrom :atom_forces ],
        [ a owl:Restriction ;
            owl:onProperty :hasQuantity ;
            owl:someValuesFrom :stress_tensor ],
        [ a owl:Restriction ;
            owl:onProperty :hasQuantity ;
            owl:someValuesFrom :parsing_message_info_single_configuration ],
        [ a owl:Restriction ;
            owl:onProperty :hasSubSection ;
            owl:someValuesFrom :section_atom_projected_dos ],
        [ a owl:Restriction ;
            owl:onProperty :hasQuantity ;
            owl:someValuesFrom :energy_X_mGGA_scaled ],
        [ a owl:Restriction ;
            owl:onProperty :hasSubSection ;
            owl:someValuesFrom :section_atomic_multipoles ],
        [ a owl:Restriction ;
            owl:onProperty :hasQuantity ;
            owl:someValuesFrom :time_single_configuration_calculation_date_start ],
        [ a owl:Restriction ;
            owl:onProperty :hasQuantity ;
            owl:someValuesFrom :energy_correction_entropy ],
        [ a owl:Restriction ;
            owl:onProperty :hasQuantity ;
            owl:someValuesFrom :energy_T0_per_atom ],
        [ a owl:Restriction ;
            owl:onProperty :hasSubSection ;
            owl:someValuesFrom :section_calculation_to_folder_refs ],
        [ a owl:Restriction ;
            owl:onProperty :hasQuantity ;
            owl:someValuesFrom :energy_total_T0_per_atom ],
        [ a owl:Restriction ;
            owl:onProperty :hasSubSection ;
            owl:someValuesFrom :section_stress_tensor ],
        [ a owl:Restriction ;
            owl:onProperty :hasQuantity ;
            owl:someValuesFrom :hessian_matrix ],
        [ a owl:Restriction ;
            owl:onProperty :hasQuantity ;
            owl:someValuesFrom :energy_reference_highest_occupied ],
        [ a owl:Restriction ;
            owl:onProperty :hasSubSection ;
            owl:someValuesFrom :section_dos ],
        [ a owl:Restriction ;
            owl:onProperty :hasQuantity ;
            owl:someValuesFrom :gw_self_energy_x ],
        [ a owl:Restriction ;
            owl:onProperty :hasSubSection ;
            owl:someValuesFrom :section_species_projected_dos ],
        [ a owl:Restriction ;
            owl:onProperty :hasQuantity ;
            owl:someValuesFrom :electronic_kinetic_energy ],
        [ a owl:Restriction ;
            owl:onProperty :hasQuantity ;
            owl:someValuesFrom :parsing_message_debug_evaluation ],
        [ a owl:Restriction ;
            owl:onProperty :hasQuantity ;
            owl:someValuesFrom :energy_sum_eigenvalues ],
        [ a owl:Restriction ;
            owl:onProperty :hasQuantity ;
            owl:someValuesFrom :energy_method_current ],
        [ a owl:Restriction ;
            owl:onProperty :hasQuantity ;
            owl:someValuesFrom :energy_sum_eigenvalues_per_atom ],
        [ a owl:Restriction ;
            owl:onProperty :hasQuantity ;
            owl:someValuesFrom :atom_forces_free_raw ],
        [ a owl:Restriction ;
            owl:onProperty :hasQuantity ;
            owl:someValuesFrom :time_single_configuration_calculation_date_end ],
        [ a owl:Restriction ;
            owl:onProperty :hasQuantity ;
            owl:someValuesFrom :energy_hartree_fock_X ],
        [ a owl:Restriction ;
            owl:onProperty :hasQuantity ;
            owl:someValuesFrom :gw_fundamental_gap ],
        [ a owl:Restriction ;
            owl:onProperty :hasQuantity ;
            owl:someValuesFrom :time_single_configuration_calculation_wall_end ],
        [ a owl:Restriction ;
            owl:onProperty :hasQuantity ;
            owl:someValuesFrom :energy_C_mGGA ],
        [ a owl:Restriction ;
            owl:onProperty :hasQuantity ;
            owl:someValuesFrom :energy_correction_hartree ],
        [ a owl:Restriction ;
            owl:onProperty :hasSubSection ;
            owl:someValuesFrom :section_k_band_normalized ],
        [ a owl:Restriction ;
            owl:onProperty :hasQuantity ;
            owl:someValuesFrom :atom_forces_T0_raw ],
        [ a owl:Restriction ;
            owl:onProperty :hasSubSection ;
            owl:someValuesFrom :section_eigenvalues ],
        [ a owl:Restriction ;
            owl:onProperty :hasQuantity ;
            owl:someValuesFrom :gw_fermi_energy ],
        [ a owl:Restriction ;
            owl:onProperty :hasSubSection ;
            owl:someValuesFrom :section_volumetric_data ],
        [ a owl:Restriction ;
            owl:onProperty :hasQuantity ;
            owl:someValuesFrom :energy_X ],
        [ a owl:Restriction ;
            owl:onProperty :hasQuantity ;
            owl:someValuesFrom :energy_XC ],
        [ a owl:Restriction ;
            owl:onProperty :hasQuantity ;
            owl:someValuesFrom :energy_reference_fermi ],
        [ a owl:Restriction ;
            owl:onProperty :hasQuantity ;
            owl:someValuesFrom :zero_point_method ],
        [ a owl:Restriction ;
            owl:onProperty :hasQuantity ;
            owl:someValuesFrom :time_single_configuration_calculation_cpu1_start ],
        [ a owl:Restriction ;
            owl:onProperty :hasQuantity ;
            owl:someValuesFrom :gw_xc_potential ],
        [ a owl:Restriction ;
            owl:onProperty :hasQuantity ;
            owl:someValuesFrom :energy_hartree_fock_X_scaled ],
        [ a owl:Restriction ;
            owl:onProperty :hasQuantity ;
            owl:someValuesFrom :message_info_evaluation ],
        [ a owl:Restriction ;
            owl:onProperty :hasQuantity ;
            owl:someValuesFrom :energy_electrostatic ],
        [ a owl:Restriction ;
            owl:onProperty :hasSubSection ;
            owl:someValuesFrom :section_calculation_to_calculation_refs ],
        [ a owl:Restriction ;
            owl:onProperty :hasQuantity ;
            owl:someValuesFrom :time_calculation ],
        [ a owl:Restriction ;
            owl:onProperty :hasQuantity ;
            owl:someValuesFrom :parsing_message_warning_evaluation ],
        [ a owl:Restriction ;
            owl:onProperty :hasQuantity ;
            owl:someValuesFrom :energy_XC_functional ],
        [ a owl:Restriction ;
            owl:onProperty :hasQuantity ;
            owl:someValuesFrom :time_single_configuration_calculation_cpu1_end ],
        [ a owl:Restriction ;
            owl:onProperty :hasQuantity ;
            owl:someValuesFrom :energy_X_mGGA ],
        [ a owl:Restriction ;
            owl:onProperty :hasQuantity ;
            owl:someValuesFrom :single_configuration_to_calculation_method_ref ],
        [ a owl:Restriction ;
            owl:onProperty :hasQuantity ;
            owl:someValuesFrom :parsing_message_error_single_configuration ],
        [ a owl:Restriction ;
            owl:onProperty :hasSubSection ;
            owl:someValuesFrom :section_k_band ],
        [ a owl:Restriction ;
            owl:onProperty :hasQuantity ;
            owl:someValuesFrom :energy_free_per_atom ],
        [ a owl:Restriction ;
            owl:onProperty :hasQuantity ;
            owl:someValuesFrom :energy_XC_potential ],
        [ a owl:Restriction ;
            owl:onProperty :hasQuantity ;
            owl:someValuesFrom :message_debug_evaluation ],
        [ a owl:Restriction ;
            owl:onProperty :hasQuantity ;
            owl:someValuesFrom :number_of_scf_iterations ],
        [ a owl:Restriction ;
            owl:onProperty :hasQuantity ;
            owl:someValuesFrom :spin_S2 ],
        [ a owl:Restriction ;
            owl:onProperty :hasQuantity ;
            owl:someValuesFrom :gw_optical_gap ],
        [ a owl:Restriction ;
            owl:onProperty :hasQuantity ;
            owl:someValuesFrom :energy_zero_point ],
        [ a owl:Restriction ;
            owl:onProperty :hasQuantity ;
            owl:someValuesFrom :energy_free ],
        [ a owl:Restriction ;
            owl:onProperty :hasSubSection ;
            owl:someValuesFrom :section_excited_states ],
        [ a owl:Restriction ;
            owl:onProperty :hasSubSection ;
            owl:someValuesFrom :section_basis_set ],
        [ a owl:Restriction ;
            owl:onProperty :hasQuantity ;
            owl:someValuesFrom :gw_self_energy_c ],
        [ a owl:Restriction ;
            owl:onProperty :hasQuantity ;
            owl:someValuesFrom :message_error_evaluation ],
        [ a owl:Restriction ;
            owl:onProperty :hasQuantity ;
            owl:someValuesFrom :time_single_configuration_calculation_wall_start ],
        [ a owl:Restriction ;
            owl:onProperty :hasQuantity ;
            owl:someValuesFrom :atom_forces_raw ],
        [ a owl:Restriction ;
            owl:onProperty :hasQuantity ;
            owl:someValuesFrom :single_configuration_calculation_to_system_ref ],
        [ a owl:Restriction ;
            owl:onProperty :hasQuantity ;
            owl:someValuesFrom :energy_reference_lowest_unoccupied ],
        [ a owl:Restriction ;
            owl:onProperty :hasQuantity ;
            owl:someValuesFrom :energy_hartree_error ],
        [ a owl:Restriction ;
            owl:onProperty :hasSubSection ;
            owl:someValuesFrom :section_energy_code_independent ],
        [ a owl:Restriction ;
            owl:onProperty :hasQuantity ;
            owl:someValuesFrom :message_warning_evaluation ],
        [ a owl:Restriction ;
            owl:onProperty :hasSubSection ;
            owl:someValuesFrom :section_energy_van_der_Waals ],
        [ a owl:Restriction ;
            owl:onProperty :hasSubSection ;
            owl:someValuesFrom :section_scf_iteration ],
        [ a owl:Restriction ;
            owl:onProperty :hasQuantity ;
            owl:someValuesFrom :energy_current ],
        [ a owl:Restriction ;
            owl:onProperty :hasQuantity ;
            owl:someValuesFrom :atom_forces_T0 ],
        :NMI_section .

:section_soap a owl:Class ;
    rdfs:comment "Stores a soap descriptor for this configuration."^^xsd:string ;
    rdfs:subClassOf [ a owl:Restriction ;
            owl:onProperty :hasQuantity ;
            owl:someValuesFrom :soap_spectrum_gradients ],
        [ a owl:Restriction ;
            owl:onProperty :hasQuantity ;
            owl:someValuesFrom :soap_radial_basis_n ],
        [ a owl:Restriction ;
            owl:onProperty :hasQuantity ;
            owl:someValuesFrom :soap_radial_cutoff_rc ],
        [ a owl:Restriction ;
            owl:onProperty :hasQuantity ;
            owl:someValuesFrom :soap_angular_basis_L ],
        [ a owl:Restriction ;
            owl:onProperty :hasQuantity ;
            owl:someValuesFrom :soap_radial_basis_integration_steps ],
        [ a owl:Restriction ;
            owl:onProperty :hasSubSection ;
            owl:someValuesFrom :section_soap_coefficients ],
        [ a owl:Restriction ;
            owl:onProperty :hasQuantity ;
            owl:someValuesFrom :soap_radial_cutoff_center_weight ],
        [ a owl:Restriction ;
            owl:onProperty :hasQuantity ;
            owl:someValuesFrom :soap_radial_cutoff_type ],
        [ a owl:Restriction ;
            owl:onProperty :hasQuantity ;
            owl:someValuesFrom :soap_radial_basis_type ],
        [ a owl:Restriction ;
            owl:onProperty :hasQuantity ;
            owl:someValuesFrom :soap_kernel_adaptor ],
        [ a owl:Restriction ;
            owl:onProperty :hasQuantity ;
            owl:someValuesFrom :soap_spectrum_2l1_norm ],
        [ a owl:Restriction ;
            owl:onProperty :hasQuantity ;
            owl:someValuesFrom :soap_parameters_gid ],
        [ a owl:Restriction ;
            owl:onProperty :hasQuantity ;
            owl:someValuesFrom :soap_angular_basis_type ],
        [ a owl:Restriction ;
            owl:onProperty :hasQuantity ;
            owl:someValuesFrom :soap_radial_basis_sigma ],
        [ a owl:Restriction ;
            owl:onProperty :hasQuantity ;
            owl:someValuesFrom :soap_radial_cutoff_rc_width ],
        [ a owl:Restriction ;
            owl:onProperty :hasQuantity ;
            owl:someValuesFrom :soap_type_list ],
        [ a owl:Restriction ;
            owl:onProperty :hasQuantity ;
            owl:someValuesFrom :soap_radial_basis_mode ],
        [ a owl:Restriction ;
            owl:onProperty :hasQuantity ;
            owl:someValuesFrom :soap_spectrum_global ],
        :NMI_section .

:section_soap_coefficients a owl:Class ;
    rdfs:comment "Stores the soap coefficients for the pair of atoms given in soap_coefficients_atom_pair."^^xsd:string ;
    rdfs:subClassOf [ a owl:Restriction ;
            owl:onProperty :hasQuantity ;
            owl:someValuesFrom :number_of_soap_coefficients ],
        [ a owl:Restriction ;
            owl:onProperty :hasQuantity ;
            owl:someValuesFrom :soap_coefficients ],
        [ a owl:Restriction ;
            owl:onProperty :hasQuantity ;
            owl:someValuesFrom :soap_coefficients_atom_pair ],
        :NMI_section .

:section_species_projected_dos a owl:Class ;
    rdfs:comment "Section collecting the information on a species-projected density of states (DOS) evaluation."^^xsd:string ;
    rdfs:subClassOf [ a owl:Restriction ;
            owl:onProperty :hasQuantity ;
            owl:someValuesFrom :species_projected_dos_energies ],
        [ a owl:Restriction ;
            owl:onProperty :hasQuantity ;
            owl:someValuesFrom :species_projected_dos_m_kind ],
        [ a owl:Restriction ;
            owl:onProperty :hasQuantity ;
            owl:someValuesFrom :species_projected_dos_lm ],
        [ a owl:Restriction ;
            owl:onProperty :hasQuantity ;
            owl:someValuesFrom :number_of_species ],
        [ a owl:Restriction ;
            owl:onProperty :hasQuantity ;
            owl:someValuesFrom :number_of_lm_species_projected_dos ],
        [ a owl:Restriction ;
            owl:onProperty :hasQuantity ;
            owl:someValuesFrom :species_projected_dos_values_total ],
        [ a owl:Restriction ;
            owl:onProperty :hasQuantity ;
            owl:someValuesFrom :number_of_species_projected_dos_values ],
        [ a owl:Restriction ;
            owl:onProperty :hasQuantity ;
            owl:someValuesFrom :species_projected_dos_species_label ],
        [ a owl:Restriction ;
            owl:onProperty :hasQuantity ;
            owl:someValuesFrom :species_projected_dos_values_lm ],
        [ a owl:Restriction ;
            owl:onProperty :hasQuantity ;
            owl:someValuesFrom :species_projected_dos_energies_normalized ],
        :NMI_section .

:section_springer_id a owl:Class ;
    rdfs:comment "Identifiers used by Springer Materials"^^xsd:string ;
    rdfs:subClassOf :NMI_section .

:section_springer_material a owl:Class ;
    rdfs:comment """Every section_springer_material contains results of classification of materials with the same formula according to Springer Materials - it contains
section_springer_classsification, section_springer_compound, section_springer_id,
section_springer_references"""^^xsd:string ;
    rdfs:subClassOf [ a owl:Restriction ;
            owl:onProperty :hasQuantity ;
            owl:someValuesFrom :springer_compound_class ],
        [ a owl:Restriction ;
            owl:onProperty :hasQuantity ;
            owl:someValuesFrom :springer_url ],
        [ a owl:Restriction ;
            owl:onProperty :hasSubSection ;
            owl:someValuesFrom :section_springer_id ],
        [ a owl:Restriction ;
            owl:onProperty :hasQuantity ;
            owl:someValuesFrom :springer_classification ],
        [ a owl:Restriction ;
            owl:onProperty :hasQuantity ;
            owl:someValuesFrom :springer_alphabetical_formula ],
        [ a owl:Restriction ;
            owl:onProperty :hasQuantity ;
            owl:someValuesFrom :springer_id ],
        :NMI_section .

:section_std_system a owl:Class ;
    rdfs:comment """Section containing symmetry information that is specific to the standardized system. The standardized system is defined as given by spglib and the details can be found
from https://arxiv.org/abs/1506.01455"""^^xsd:string ;
    rdfs:subClassOf [ a owl:Restriction ;
            owl:onProperty :hasQuantity ;
            owl:someValuesFrom :equivalent_atoms_std ],
        [ a owl:Restriction ;
            owl:onProperty :hasQuantity ;
            owl:someValuesFrom :atomic_numbers_std ],
        [ a owl:Restriction ;
            owl:onProperty :hasQuantity ;
            owl:someValuesFrom :number_of_atoms_std ],
        [ a owl:Restriction ;
            owl:onProperty :hasQuantity ;
            owl:someValuesFrom :lattice_vectors_std ],
        [ a owl:Restriction ;
            owl:onProperty :hasQuantity ;
            owl:someValuesFrom :atom_positions_std ],
        [ a owl:Restriction ;
            owl:onProperty :hasQuantity ;
            owl:someValuesFrom :wyckoff_letters_std ],
        :NMI_section .

:section_stress_tensor a owl:Class ;
    rdfs:comment """Section collecting alternative values to stress_tensor that have been calculated. This section allows the storage of multiple definitions and evaluated values of the
stress tensor, while only one definition is used for, e.g., molecular dynamics or
geometry optimization (if needed)."""^^xsd:string ;
    rdfs:subClassOf [ a owl:Restriction ;
            owl:onProperty :hasQuantity ;
            owl:someValuesFrom :stress_tensor_value ],
        [ a owl:Restriction ;
            owl:onProperty :hasQuantity ;
            owl:someValuesFrom :stress_tensor_kind ],
        :NMI_section .

:section_symmetry a owl:Class ;
    rdfs:comment "Section containing information about the symmetry properties of the system."^^xsd:string ;
    rdfs:subClassOf [ a owl:Restriction ;
            owl:onProperty :hasQuantity ;
            owl:someValuesFrom :crystal_system ],
        [ a owl:Restriction ;
            owl:onProperty :hasQuantity ;
            owl:someValuesFrom :bravais_lattice ],
        [ a owl:Restriction ;
            owl:onProperty :hasQuantity ;
            owl:someValuesFrom :transformation_matrix ],
        [ a owl:Restriction ;
            owl:onProperty :hasSubSection ;
            owl:someValuesFrom :section_primitive_system ],
        [ a owl:Restriction ;
            owl:onProperty :hasQuantity ;
            owl:someValuesFrom :hall_symbol ],
        [ a owl:Restriction ;
            owl:onProperty :hasQuantity ;
            owl:someValuesFrom :space_group_number ],
        [ a owl:Restriction ;
            owl:onProperty :hasQuantity ;
            owl:someValuesFrom :point_group ],
        [ a owl:Restriction ;
            owl:onProperty :hasSubSection ;
            owl:someValuesFrom :section_original_system ],
        [ a owl:Restriction ;
            owl:onProperty :hasQuantity ;
            owl:someValuesFrom :international_short_symbol ],
        [ a owl:Restriction ;
            owl:onProperty :hasQuantity ;
            owl:someValuesFrom :hall_number ],
        [ a owl:Restriction ;
            owl:onProperty :hasSubSection ;
            owl:someValuesFrom :section_std_system ],
        [ a owl:Restriction ;
            owl:onProperty :hasQuantity ;
            owl:someValuesFrom :origin_shift ],
        [ a owl:Restriction ;
            owl:onProperty :hasQuantity ;
            owl:someValuesFrom :symmetry_method ],
        [ a owl:Restriction ;
            owl:onProperty :hasQuantity ;
            owl:someValuesFrom :choice ],
        :NMI_section .

:section_system a owl:Class ;
    rdfs:comment """Every section_system contains all needed properties required to describe the simulated physical system, e.g. the given atomic configuration, the definition of periodic cell
(if present), the external potentials and other parameters."""^^xsd:string ;
    rdfs:subClassOf [ a owl:Restriction ;
            owl:onProperty :hasQuantity ;
            owl:someValuesFrom :number_of_atoms ],
        [ a owl:Restriction ;
            owl:onProperty :hasQuantity ;
            owl:someValuesFrom :system_reweighted_composition ],
        [ a owl:Restriction ;
            owl:onProperty :hasQuantity ;
            owl:someValuesFrom :chemical_composition_reduced ],
        [ a owl:Restriction ;
            owl:onProperty :hasQuantity ;
            owl:someValuesFrom :configuration_periodic_dimensions ],
        [ a owl:Restriction ;
            owl:onProperty :hasQuantity ;
            owl:someValuesFrom :chemical_composition_bulk_reduced ],
        [ a owl:Restriction ;
            owl:onProperty :hasQuantity ;
            owl:someValuesFrom :topology_ref ],
        [ a owl:Restriction ;
            owl:onProperty :hasQuantity ;
            owl:someValuesFrom :is_representative ],
        [ a owl:Restriction ;
            owl:onProperty :hasQuantity ;
            owl:someValuesFrom :atom_atom_number ],
        [ a owl:Restriction ;
            owl:onProperty :hasQuantity ;
            owl:someValuesFrom :system_composition ],
        [ a owl:Restriction ;
            owl:onProperty :hasQuantity ;
            owl:someValuesFrom :local_rotations ],
        [ a owl:Restriction ;
            owl:onProperty :hasQuantity ;
            owl:someValuesFrom :lattice_vectors ],
        [ a owl:Restriction ;
            owl:onProperty :hasQuantity ;
            owl:someValuesFrom :system_type ],
        [ a owl:Restriction ;
            owl:onProperty :hasSubSection ;
            owl:someValuesFrom :section_soap ],
        [ a owl:Restriction ;
            owl:onProperty :hasQuantity ;
            owl:someValuesFrom :configuration_raw_gid ],
        [ a owl:Restriction ;
            owl:onProperty :hasQuantity ;
            owl:someValuesFrom :system_name ],
        [ a owl:Restriction ;
            owl:onProperty :hasQuantity ;
            owl:someValuesFrom :atom_positions ],
        [ a owl:Restriction ;
            owl:onProperty :hasQuantity ;
            owl:someValuesFrom :atom_species ],
        [ a owl:Restriction ;
            owl:onProperty :hasQuantity ;
            owl:someValuesFrom :system_configuration_consistent ],
        [ a owl:Restriction ;
            owl:onProperty :hasQuantity ;
            owl:someValuesFrom :number_of_sites ],
        [ a owl:Restriction ;
            owl:onProperty :hasQuantity ;
            owl:someValuesFrom :symmorphic ],
        [ a owl:Restriction ;
            owl:onProperty :hasSubSection ;
            owl:someValuesFrom :section_springer_material ],
        [ a owl:Restriction ;
            owl:onProperty :hasQuantity ;
            owl:someValuesFrom :SC_matrix ],
        [ a owl:Restriction ;
            owl:onProperty :hasSubSection ;
            owl:someValuesFrom :section_symmetry ],
        [ a owl:Restriction ;
            owl:onProperty :hasQuantity ;
            owl:someValuesFrom :atom_labels ],
        [ a owl:Restriction ;
            owl:onProperty :hasSubSection ;
            owl:someValuesFrom :section_prototype ],
        [ a owl:Restriction ;
            owl:onProperty :hasQuantity ;
            owl:someValuesFrom :atom_concentrations ],
        [ a owl:Restriction ;
            owl:onProperty :hasQuantity ;
            owl:someValuesFrom :time_reversal_symmetry ],
        [ a owl:Restriction ;
            owl:onProperty :hasQuantity ;
            owl:someValuesFrom :chemical_composition ],
        [ a owl:Restriction ;
            owl:onProperty :hasQuantity ;
            owl:someValuesFrom :atom_velocities ],
        [ a owl:Restriction ;
            owl:onProperty :hasQuantity ;
            owl:someValuesFrom :simulation_cell ],
        [ a owl:Restriction ;
            owl:onProperty :hasQuantity ;
            owl:someValuesFrom :embedded_system ],
        [ a owl:Restriction ;
            owl:onProperty :hasSubSection ;
            owl:someValuesFrom :section_system_to_system_refs ],
        [ a owl:Restriction ;
            owl:onProperty :hasQuantity ;
            owl:someValuesFrom :number_of_electrons ],
        :NMI_section .

:section_system_to_system_refs a owl:Class ;
    rdfs:comment """Section that describes the relationship between different section_system sections. For instance, if a phonon calculation using a finite difference approach is performed
the force evaluation is typically done in a larger supercell but the properties such
as the phonon band structure are still calculated for the primitive cell.

The kind of relationship between the system defined in this section and the referenced
one is described by system_to_system_kind. The referenced section_system is identified
via system_to_system_ref."""^^xsd:string ;
    rdfs:subClassOf [ a owl:Restriction ;
            owl:onProperty :hasQuantity ;
            owl:someValuesFrom :system_to_system_kind ],
        [ a owl:Restriction ;
            owl:onProperty :hasQuantity ;
            owl:someValuesFrom :system_to_system_ref ],
        :NMI_section .

:section_thermodynamical_properties a owl:Class ;
    rdfs:comment "Section that defines thermodynamical properties about the system in a section_frame_sequence."^^xsd:string ;
    rdfs:subClassOf [ a owl:Restriction ;
            owl:onProperty :hasQuantity ;
            owl:someValuesFrom :number_of_thermodynamical_property_values ],
        [ a owl:Restriction ;
            owl:onProperty :hasQuantity ;
            owl:someValuesFrom :thermodynamical_property_temperature ],
        [ a owl:Restriction ;
            owl:onProperty :hasQuantity ;
            owl:someValuesFrom :specific_heat_capacity ],
        [ a owl:Restriction ;
            owl:onProperty :hasQuantity ;
            owl:someValuesFrom :specific_vibrational_free_energy_at_constant_volume ],
        [ a owl:Restriction ;
            owl:onProperty :hasQuantity ;
            owl:someValuesFrom :helmholz_free_energy ],
        [ a owl:Restriction ;
            owl:onProperty :hasQuantity ;
            owl:someValuesFrom :thermodynamical_property_heat_capacity_C_v ],
        [ a owl:Restriction ;
            owl:onProperty :hasQuantity ;
            owl:someValuesFrom :vibrational_free_energy_at_constant_volume ],
        [ a owl:Restriction ;
            owl:onProperty :hasQuantity ;
            owl:someValuesFrom :thermodynamical_properties_calculation_method ],
        :NMI_section .

:section_topology a owl:Class ;
    rdfs:comment "Section containing the definition of topology (connectivity among atoms in force fileds), force field, and constraints of a system."^^xsd:string ;
    rdfs:subClassOf [ a owl:Restriction ;
            owl:onProperty :hasSubSection ;
            owl:someValuesFrom :section_molecule_type ],
        [ a owl:Restriction ;
            owl:onProperty :hasQuantity ;
            owl:someValuesFrom :atom_to_molecule ],
        [ a owl:Restriction ;
            owl:onProperty :hasQuantity ;
            owl:someValuesFrom :molecule_to_molecule_type_map ],
        [ a owl:Restriction ;
            owl:onProperty :hasQuantity ;
            owl:someValuesFrom :number_of_topology_molecules ],
        [ a owl:Restriction ;
            owl:onProperty :hasSubSection ;
            owl:someValuesFrom :section_interaction ],
        [ a owl:Restriction ;
            owl:onProperty :hasQuantity ;
            owl:someValuesFrom :topology_force_field_name ],
        [ a owl:Restriction ;
            owl:onProperty :hasQuantity ;
            owl:someValuesFrom :number_of_topology_atoms ],
        [ a owl:Restriction ;
            owl:onProperty :hasSubSection ;
            owl:someValuesFrom :section_atom_type ],
        [ a owl:Restriction ;
            owl:onProperty :hasSubSection ;
            owl:someValuesFrom :section_constraint ],
        :NMI_section .

:section_volumetric_data a owl:Class ;
    rdfs:comment """Section defining a set of volumetric data on a uniform real-space grid.

To store an array (e.g. a density or a potential), define:

* three grid point displacement vectors ("displacements")

* number of grid points along each axis ("nx", "ny" and "nz")

* the origin of the coordinate system, i.e. coordinates of the first grid

point ("origin")

* how many spatial functions are represented, e.g., two for a

normal spin-polarized density ("multiplicity")

* the values for each grid point ("values")

* the unit that applies to each value ("units")

* the kind of array represented by the volumetric data ("kind").

Allowed kinds are (please add new kinds as necessary): "density",

"potential_hartree" and "potential_effective".  Densities and

potentials that are spin-polarized should have multiplicity two.

Rules for more complex spins are to be decided when necessary."""^^xsd:string ;
    rdfs:subClassOf [ a owl:Restriction ;
            owl:onProperty :hasQuantity ;
            owl:someValuesFrom :volumetric_data_kind ],
        [ a owl:Restriction ;
            owl:onProperty :hasQuantity ;
            owl:someValuesFrom :volumetric_data_values ],
        [ a owl:Restriction ;
            owl:onProperty :hasQuantity ;
            owl:someValuesFrom :volumetric_data_origin ],
        [ a owl:Restriction ;
            owl:onProperty :hasQuantity ;
            owl:someValuesFrom :volumetric_data_nz ],
        [ a owl:Restriction ;
            owl:onProperty :hasQuantity ;
            owl:someValuesFrom :volumetric_data_multiplicity ],
        [ a owl:Restriction ;
            owl:onProperty :hasQuantity ;
            owl:someValuesFrom :volumetric_data_displacements ],
        [ a owl:Restriction ;
            owl:onProperty :hasQuantity ;
            owl:someValuesFrom :volumetric_data_nx ],
        [ a owl:Restriction ;
            owl:onProperty :hasQuantity ;
            owl:someValuesFrom :volumetric_data_ny ],
        :NMI_section .

:self_interaction_correction_method a owl:Class ;
    rdfs:comment """Contains the name for the self-interaction correction (SIC) treatment used to
calculate the final energy and related quantities. If skipped or empty, no special
correction is applied.

The following SIC methods are available:

| SIC method                | Description                       |

| ------------------------- | --------------------------------  |

| `""`                      | No correction                     |

| `"SIC_AD"`                | The average density correction    |

| `"SIC_SOSEX"`             | Second order screened exchange    |

| `"SIC_EXPLICIT_ORBITALS"` | (scaled) Perdew-Zunger correction explicitly on a
set of orbitals |

| `"SIC_MAURI_SPZ"`         | (scaled) Perdew-Zunger expression on the spin
density / doublet unpaired orbital |

| `"SIC_MAURI_US"`          | A (scaled) correction proposed by Mauri and co-
workers on the spin density / doublet unpaired orbital |"""^^xsd:string ;
    rdfs:subClassOf [ a owl:Restriction ;
            owl:onProperty :hasCategory ;
            owl:someValuesFrom :settings_self_interaction_correction ],
        [ a owl:Restriction ;
            owl:hasValue 0 ;
            owl:onProperty :hasNumberOfDimensions ],
        [ a owl:Restriction ;
            owl:allValuesFrom <http://emmo.info/emmo/middle/perceptual#EMMO_50ea1ec5_f157_41b0_b46b_a9032f17ca10> ;
            owl:onProperty :hasDatatype ],
        [ a owl:Restriction ;
            owl:onProperty :hasCategory ;
            owl:someValuesFrom :settings_potential_energy_surface ],
        [ a owl:Restriction ;
            owl:onProperty :hasCategory ;
            owl:someValuesFrom :settings_XC ],
        :NMI_quantity .

:settings_XC_functional a owl:Class ;
    rdfs:comment """Contain parameters connected with the definition of the exchange-correlation (XC)
functional (see section_XC_functionals and XC_functional)."""^^xsd:string ;
    rdfs:subClassOf :settings_XC .

:settings_numerical_parameter a owl:Class ;
    rdfs:comment """A parameter that can influence the convergence, but not the physics (unlike
settings_physical_parameter)"""^^xsd:string ;
    rdfs:subClassOf :NMI_category .

:settings_relativity a owl:Class ;
    rdfs:comment """Contains parameters and information connected with the relativistic treatment used in
the calculation."""^^xsd:string ;
    rdfs:subClassOf :settings_XC .

:settings_self_interaction_correction a owl:Class ;
    rdfs:comment """Contains parameters and information connected with the self-interaction correction
(SIC) method being used in self_interaction_correction_method."""^^xsd:string ;
    rdfs:subClassOf :settings_XC .

:settings_stress_tensor a owl:Class ;
    rdfs:comment """Settings to calculate the stress tensor (stress_tensor) consistent with the total
energy of the system given in energy_total."""^^xsd:string ;
    rdfs:subClassOf :NMI_category .

:settings_van_der_Waals a owl:Class ;
    rdfs:comment """Contain parameters and information connected with the Van der Waals treatment used in
the calculation to compute the Van der Waals energy (energy_van_der_Waals)."""^^xsd:string ;
    rdfs:subClassOf :settings_XC .

:simulation_cell a owl:Class ;
    rdfs:comment """DEPRECATED, use lattice_vectors instead. Holds the lattice vectors (in Cartesian
coordinates) of the simulation cell. The last (fastest) index runs over the
$x,y,z$ Cartesian coordinates, and the first index runs over the 3 lattice
vectors."""^^xsd:string ;
    rdfs:subClassOf [ a owl:Restriction ;
            owl:hasValue 3 ;
            owl:onProperty :hasFixDim2 ],
        [ a owl:Restriction ;
            owl:allValuesFrom <http://emmo.info/emmo/middle/math#EMMO_18d180e4_5e3e_42f7_820c_e08951223486> ;
            owl:onProperty :hasDatatype ],
        [ a owl:Restriction ;
            owl:allValuesFrom <http://emmo.info/emmo/middle/siunits#EMMO_7db11dbf_a643_464a_9b56_07eabcc3e9c5> ;
            owl:onProperty <http://emmo.info/emmo/middle/metrology#EMMO_67fc0a36_8dcb_4ffa_9a43_31074efa3296> ],
        [ a owl:Restriction ;
            owl:hasValue 3 ;
            owl:onProperty :hasFixDim1 ],
        [ a owl:Restriction ;
            owl:hasValue 2 ;
            owl:onProperty :hasNumberOfDimensions ],
        [ a owl:Restriction ;
            owl:onProperty :hasCategory ;
            owl:someValuesFrom :configuration_core ],
        :NMI_quantity .

:single_configuration_calculation_converged a owl:Class ;
    rdfs:comment """Determines whether a *single configuration calculation* in
section_single_configuration_calculation is converged."""^^xsd:string ;
    rdfs:subClassOf [ a owl:Restriction ;
            owl:allValuesFrom <http://emmo.info/emmo/middle/math#EMMO_54dc83cb_06e1_4739_9e45_bc09cead7f48> ;
            owl:onProperty :hasDatatype ],
        [ a owl:Restriction ;
            owl:hasValue 0 ;
            owl:onProperty :hasNumberOfDimensions ],
        :NMI_quantity .

:single_configuration_calculation_to_system_ref a owl:Class ;
    rdfs:comment """Reference to the system (atomic configuration, cell, ...) that is calculated in
section_single_configuration_calculation."""^^xsd:string ;
    rdfs:subClassOf [ a owl:Restriction ;
            owl:hasValue 0 ;
            owl:onProperty :hasNumberOfDimensions ],
        :NMI_quantity .

:single_configuration_to_calculation_method_ref a owl:Class ;
    rdfs:comment """Reference to the method used for the calculation in
section_single_configuration_calculation."""^^xsd:string ;
    rdfs:subClassOf [ a owl:Restriction ;
            owl:hasValue 0 ;
            owl:onProperty :hasNumberOfDimensions ],
        :NMI_quantity .

:smearing_kind a owl:Class ;
    rdfs:comment """Specifies the kind of smearing on the electron occupation used to calculate the
free energy (see energy_free)

Valid values are:

| Smearing kind             | Description                       |

| ------------------------- | --------------------------------- |

| `"empty"`                 | No smearing is applied            |

| `"gaussian"`              | Gaussian smearing                 |

| `"fermi"`                 | Fermi smearing                    |

| `"marzari-vanderbilt"`    | Marzari-Vanderbilt smearing       |

| `"methfessel-paxton"`     | Methfessel-Paxton smearing        |

| `"tetrahedra"`            | Interpolation of state energies and occupations
(ignores smearing_width) |"""^^xsd:string ;
    rdfs:subClassOf [ a owl:Restriction ;
            owl:onProperty :hasCategory ;
            owl:someValuesFrom :settings_smearing ],
        [ a owl:Restriction ;
            owl:allValuesFrom <http://emmo.info/emmo/middle/perceptual#EMMO_50ea1ec5_f157_41b0_b46b_a9032f17ca10> ;
            owl:onProperty :hasDatatype ],
        [ a owl:Restriction ;
            owl:hasValue 0 ;
            owl:onProperty :hasNumberOfDimensions ],
        :NMI_quantity .

:smearing_width a owl:Class ;
    rdfs:comment """Specifies the width of the smearing in energy for the electron occupation used to
calculate the free energy (see energy_free).

*NOTE:* Not all methods specified in smearing_kind uses this value."""^^xsd:string ;
    rdfs:subClassOf [ a owl:Restriction ;
            owl:allValuesFrom <http://emmo.info/emmo/middle/math#EMMO_18d180e4_5e3e_42f7_820c_e08951223486> ;
            owl:onProperty :hasDatatype ],
        [ a owl:Restriction ;
            owl:hasValue 0 ;
            owl:onProperty :hasNumberOfDimensions ],
        [ a owl:Restriction ;
            owl:onProperty :hasCategory ;
            owl:someValuesFrom :settings_smearing ],
        :NMI_quantity .

:soap_angular_basis_L a owl:Class ;
    rdfs:comment "angular basis L"^^xsd:string ;
    rdfs:subClassOf [ a owl:Restriction ;
            owl:hasValue 0 ;
            owl:onProperty :hasNumberOfDimensions ],
        [ a owl:Restriction ;
            owl:onProperty :hasCategory ;
            owl:someValuesFrom :soap_parameter ],
        [ a owl:Restriction ;
            owl:allValuesFrom <http://emmo.info/emmo/middle/math#EMMO_f8bd64d5_5d3e_4ad4_a46e_c30714fecb7f> ;
            owl:onProperty :hasDatatype ],
        [ a owl:Restriction ;
            owl:allValuesFrom <http://emmo.info/emmo/middle/math#EMMO_f8bd64d5_5d3e_4ad4_a46e_c30714fecb7f> ;
            owl:onProperty <http://emmo.info/emmo/middle/metrology#EMMO_67fc0a36_8dcb_4ffa_9a43_31074efa3296> ],
        :NMI_dimension,
        :NMI_quantity .

:soap_angular_basis_type a owl:Class ;
    rdfs:comment "angular basis type"^^xsd:string ;
    rdfs:subClassOf [ a owl:Restriction ;
            owl:onProperty :hasCategory ;
            owl:someValuesFrom :soap_parameter ],
        [ a owl:Restriction ;
            owl:hasValue 0 ;
            owl:onProperty :hasNumberOfDimensions ],
        [ a owl:Restriction ;
            owl:allValuesFrom <http://emmo.info/emmo/middle/perceptual#EMMO_50ea1ec5_f157_41b0_b46b_a9032f17ca10> ;
            owl:onProperty :hasDatatype ],
        :NMI_quantity .

:soap_coefficients a owl:Class ;
    rdfs:comment """Compressed coefficient of the soap descriptor for the atom pair
soap_coefficients_atom_pair"""^^xsd:string ;
    rdfs:subClassOf [ a owl:Restriction ;
            owl:hasValue 1 ;
            owl:onProperty :hasNumberOfDimensions ],
        [ a owl:Restriction ;
            owl:allValuesFrom <http://emmo.info/emmo/middle/math#EMMO_18d180e4_5e3e_42f7_820c_e08951223486> ;
            owl:onProperty :hasDatatype ],
        [ a owl:Restriction ;
            owl:hasValue :number_of_soap_coefficients ;
            owl:onProperty :hasVarDim1 ],
        :NMI_quantity .

:soap_coefficients_atom_pair a owl:Class ;
    rdfs:comment "Pair of atoms described in the current section"^^xsd:string ;
    rdfs:subClassOf [ a owl:Restriction ;
            owl:allValuesFrom <http://emmo.info/emmo/middle/perceptual#EMMO_50ea1ec5_f157_41b0_b46b_a9032f17ca10> ;
            owl:onProperty :hasDatatype ],
        [ a owl:Restriction ;
            owl:hasValue 0 ;
            owl:onProperty :hasNumberOfDimensions ],
        :NMI_quantity .

:soap_kernel_adaptor a owl:Class ;
    rdfs:comment "kernel adaptor"^^xsd:string ;
    rdfs:subClassOf [ a owl:Restriction ;
            owl:onProperty :hasCategory ;
            owl:someValuesFrom :soap_parameter ],
        [ a owl:Restriction ;
            owl:allValuesFrom <http://emmo.info/emmo/middle/perceptual#EMMO_50ea1ec5_f157_41b0_b46b_a9032f17ca10> ;
            owl:onProperty :hasDatatype ],
        [ a owl:Restriction ;
            owl:hasValue 0 ;
            owl:onProperty :hasNumberOfDimensions ],
        :NMI_quantity .

:soap_parameters_gid a owl:Class ;
    rdfs:comment """Unique checksum of all the soap parameters (all those with abstract type
soap_parameter) with prefix psoap"""^^xsd:string ;
    rdfs:subClassOf [ a owl:Restriction ;
            owl:allValuesFrom <http://emmo.info/emmo/middle/perceptual#EMMO_50ea1ec5_f157_41b0_b46b_a9032f17ca10> ;
            owl:onProperty :hasDatatype ],
        [ a owl:Restriction ;
            owl:hasValue 0 ;
            owl:onProperty :hasNumberOfDimensions ],
        :NMI_quantity .

:soap_radial_basis_integration_steps a owl:Class ;
    rdfs:comment "radial basis integration steps"^^xsd:string ;
    rdfs:subClassOf [ a owl:Restriction ;
            owl:onProperty :hasCategory ;
            owl:someValuesFrom :soap_parameter ],
        [ a owl:Restriction ;
            owl:allValuesFrom <http://emmo.info/emmo/middle/math#EMMO_f8bd64d5_5d3e_4ad4_a46e_c30714fecb7f> ;
            owl:onProperty <http://emmo.info/emmo/middle/metrology#EMMO_67fc0a36_8dcb_4ffa_9a43_31074efa3296> ],
        [ a owl:Restriction ;
            owl:allValuesFrom <http://emmo.info/emmo/middle/math#EMMO_f8bd64d5_5d3e_4ad4_a46e_c30714fecb7f> ;
            owl:onProperty :hasDatatype ],
        [ a owl:Restriction ;
            owl:hasValue 0 ;
            owl:onProperty :hasNumberOfDimensions ],
        :NMI_dimension,
        :NMI_quantity .

:soap_radial_basis_mode a owl:Class ;
    rdfs:comment "radial basis mode"^^xsd:string ;
    rdfs:subClassOf [ a owl:Restriction ;
            owl:onProperty :hasCategory ;
            owl:someValuesFrom :soap_parameter ],
        [ a owl:Restriction ;
            owl:allValuesFrom <http://emmo.info/emmo/middle/perceptual#EMMO_50ea1ec5_f157_41b0_b46b_a9032f17ca10> ;
            owl:onProperty :hasDatatype ],
        [ a owl:Restriction ;
            owl:hasValue 0 ;
            owl:onProperty :hasNumberOfDimensions ],
        :NMI_quantity .

:soap_radial_basis_n a owl:Class ;
    rdfs:comment "radial basis N"^^xsd:string ;
    rdfs:subClassOf [ a owl:Restriction ;
            owl:allValuesFrom <http://emmo.info/emmo/middle/math#EMMO_f8bd64d5_5d3e_4ad4_a46e_c30714fecb7f> ;
            owl:onProperty <http://emmo.info/emmo/middle/metrology#EMMO_67fc0a36_8dcb_4ffa_9a43_31074efa3296> ],
        [ a owl:Restriction ;
            owl:allValuesFrom <http://emmo.info/emmo/middle/math#EMMO_f8bd64d5_5d3e_4ad4_a46e_c30714fecb7f> ;
            owl:onProperty :hasDatatype ],
        [ a owl:Restriction ;
            owl:onProperty :hasCategory ;
            owl:someValuesFrom :soap_parameter ],
        [ a owl:Restriction ;
            owl:hasValue 0 ;
            owl:onProperty :hasNumberOfDimensions ],
        :NMI_dimension,
        :NMI_quantity .

:soap_radial_basis_sigma a owl:Class ;
    rdfs:comment "radial basis sigma"^^xsd:string ;
    rdfs:subClassOf [ a owl:Restriction ;
            owl:onProperty :hasCategory ;
            owl:someValuesFrom :soap_parameter ],
        [ a owl:Restriction ;
            owl:allValuesFrom <http://emmo.info/emmo/middle/math#EMMO_18d180e4_5e3e_42f7_820c_e08951223486> ;
            owl:onProperty :hasDatatype ],
        [ a owl:Restriction ;
            owl:hasValue 0 ;
            owl:onProperty :hasNumberOfDimensions ],
        :NMI_quantity .

:soap_radial_basis_type a owl:Class ;
    rdfs:comment "radial basis type"^^xsd:string ;
    rdfs:subClassOf [ a owl:Restriction ;
            owl:allValuesFrom <http://emmo.info/emmo/middle/perceptual#EMMO_50ea1ec5_f157_41b0_b46b_a9032f17ca10> ;
            owl:onProperty :hasDatatype ],
        [ a owl:Restriction ;
            owl:onProperty :hasCategory ;
            owl:someValuesFrom :soap_parameter ],
        [ a owl:Restriction ;
            owl:hasValue 0 ;
            owl:onProperty :hasNumberOfDimensions ],
        :NMI_quantity .

:soap_radial_cutoff_center_weight a owl:Class ;
    rdfs:comment "radial cutoff center weight"^^xsd:string ;
    rdfs:subClassOf [ a owl:Restriction ;
            owl:allValuesFrom <http://emmo.info/emmo/middle/math#EMMO_18d180e4_5e3e_42f7_820c_e08951223486> ;
            owl:onProperty :hasDatatype ],
        [ a owl:Restriction ;
            owl:hasValue 0 ;
            owl:onProperty :hasNumberOfDimensions ],
        [ a owl:Restriction ;
            owl:onProperty :hasCategory ;
            owl:someValuesFrom :soap_parameter ],
        :NMI_quantity .

:soap_radial_cutoff_rc a owl:Class ;
    rdfs:comment "radial cutoff"^^xsd:string ;
    rdfs:subClassOf [ a owl:Restriction ;
            owl:onProperty :hasCategory ;
            owl:someValuesFrom :soap_parameter ],
        [ a owl:Restriction ;
            owl:hasValue 0 ;
            owl:onProperty :hasNumberOfDimensions ],
        [ a owl:Restriction ;
            owl:allValuesFrom <http://emmo.info/emmo/middle/math#EMMO_18d180e4_5e3e_42f7_820c_e08951223486> ;
            owl:onProperty :hasDatatype ],
        :NMI_quantity .

:soap_radial_cutoff_rc_width a owl:Class ;
    rdfs:comment "radial cutoff width"^^xsd:string ;
    rdfs:subClassOf [ a owl:Restriction ;
            owl:allValuesFrom <http://emmo.info/emmo/middle/math#EMMO_f8bd64d5_5d3e_4ad4_a46e_c30714fecb7f> ;
            owl:onProperty :hasDatatype ],
        [ a owl:Restriction ;
            owl:hasValue 0 ;
            owl:onProperty :hasNumberOfDimensions ],
        [ a owl:Restriction ;
            owl:allValuesFrom <http://emmo.info/emmo/middle/math#EMMO_f8bd64d5_5d3e_4ad4_a46e_c30714fecb7f> ;
            owl:onProperty <http://emmo.info/emmo/middle/metrology#EMMO_67fc0a36_8dcb_4ffa_9a43_31074efa3296> ],
        [ a owl:Restriction ;
            owl:onProperty :hasCategory ;
            owl:someValuesFrom :soap_parameter ],
        :NMI_dimension,
        :NMI_quantity .

:soap_radial_cutoff_type a owl:Class ;
    rdfs:comment "radial cutoff type"^^xsd:string ;
    rdfs:subClassOf [ a owl:Restriction ;
            owl:allValuesFrom <http://emmo.info/emmo/middle/perceptual#EMMO_50ea1ec5_f157_41b0_b46b_a9032f17ca10> ;
            owl:onProperty :hasDatatype ],
        [ a owl:Restriction ;
            owl:onProperty :hasCategory ;
            owl:someValuesFrom :soap_parameter ],
        [ a owl:Restriction ;
            owl:hasValue 0 ;
            owl:onProperty :hasNumberOfDimensions ],
        :NMI_quantity .

:soap_spectrum_2l1_norm a owl:Class ;
    rdfs:comment "2l1 norm spectrum"^^xsd:string ;
    rdfs:subClassOf [ a owl:Restriction ;
            owl:hasValue 0 ;
            owl:onProperty :hasNumberOfDimensions ],
        [ a owl:Restriction ;
            owl:onProperty :hasCategory ;
            owl:someValuesFrom :soap_parameter ],
        [ a owl:Restriction ;
            owl:allValuesFrom <http://emmo.info/emmo/middle/math#EMMO_54dc83cb_06e1_4739_9e45_bc09cead7f48> ;
            owl:onProperty :hasDatatype ],
        :NMI_quantity .

:soap_spectrum_global a owl:Class ;
    rdfs:comment "global spectrum"^^xsd:string ;
    rdfs:subClassOf [ a owl:Restriction ;
            owl:allValuesFrom <http://emmo.info/emmo/middle/math#EMMO_54dc83cb_06e1_4739_9e45_bc09cead7f48> ;
            owl:onProperty :hasDatatype ],
        [ a owl:Restriction ;
            owl:hasValue 0 ;
            owl:onProperty :hasNumberOfDimensions ],
        [ a owl:Restriction ;
            owl:onProperty :hasCategory ;
            owl:someValuesFrom :soap_parameter ],
        :NMI_quantity .

:soap_spectrum_gradients a owl:Class ;
    rdfs:comment "gradients in specturm"^^xsd:string ;
    rdfs:subClassOf [ a owl:Restriction ;
            owl:allValuesFrom <http://emmo.info/emmo/middle/math#EMMO_54dc83cb_06e1_4739_9e45_bc09cead7f48> ;
            owl:onProperty :hasDatatype ],
        [ a owl:Restriction ;
            owl:onProperty :hasCategory ;
            owl:someValuesFrom :soap_parameter ],
        [ a owl:Restriction ;
            owl:hasValue 0 ;
            owl:onProperty :hasNumberOfDimensions ],
        :NMI_quantity .

:soap_type_list a owl:Class ;
    rdfs:comment "Type list"^^xsd:string ;
    rdfs:subClassOf [ a owl:Restriction ;
            owl:onProperty :hasCategory ;
            owl:someValuesFrom :soap_parameter ],
        [ a owl:Restriction ;
            owl:allValuesFrom <http://emmo.info/emmo/middle/perceptual#EMMO_50ea1ec5_f157_41b0_b46b_a9032f17ca10> ;
            owl:onProperty :hasDatatype ],
        [ a owl:Restriction ;
            owl:hasValue 0 ;
            owl:onProperty :hasNumberOfDimensions ],
        :NMI_quantity .

:space_group_number a owl:Class ;
    rdfs:comment """Specifies the International Union of Crystallography (IUC) number of the 3D space
group of this system."""^^xsd:string ;
    rdfs:subClassOf [ a owl:Restriction ;
            owl:hasValue 0 ;
            owl:onProperty :hasNumberOfDimensions ],
        [ a owl:Restriction ;
            owl:allValuesFrom <http://emmo.info/emmo/middle/math#EMMO_f8bd64d5_5d3e_4ad4_a46e_c30714fecb7f> ;
            owl:onProperty <http://emmo.info/emmo/middle/metrology#EMMO_67fc0a36_8dcb_4ffa_9a43_31074efa3296> ],
        [ a owl:Restriction ;
            owl:allValuesFrom <http://emmo.info/emmo/middle/math#EMMO_f8bd64d5_5d3e_4ad4_a46e_c30714fecb7f> ;
            owl:onProperty :hasDatatype ],
        :NMI_dimension,
        :NMI_quantity .

:species_projected_dos_energies a owl:Class ;
    rdfs:comment """Contains the set of discrete energy values for the species-projected density of
states (DOS)."""^^xsd:string ;
    rdfs:subClassOf [ a owl:Restriction ;
            owl:allValuesFrom <http://emmo.info/emmo/middle/siunits#EMMO_8a70dea4_d6ab_4260_b931_a3e990982416> ;
            owl:onProperty <http://emmo.info/emmo/middle/metrology#EMMO_67fc0a36_8dcb_4ffa_9a43_31074efa3296> ],
        [ a owl:Restriction ;
            owl:allValuesFrom <http://emmo.info/emmo/middle/math#EMMO_18d180e4_5e3e_42f7_820c_e08951223486> ;
            owl:onProperty :hasDatatype ],
        [ a owl:Restriction ;
            owl:hasValue 1 ;
            owl:onProperty :hasNumberOfDimensions ],
        [ a owl:Restriction ;
            owl:hasValue :number_of_species_projected_dos_values ;
            owl:onProperty :hasVarDim1 ],
        :NMI_quantity .

:species_projected_dos_energies_normalized a owl:Class ;
    rdfs:comment """Contains the set of discrete energy values with respect to the top of the valence
band for the species-projected density of states (DOS). It is derived from the
species_projected_dos_energies species field."""^^xsd:string ;
    rdfs:subClassOf [ a owl:Restriction ;
            owl:allValuesFrom <http://emmo.info/emmo/middle/math#EMMO_18d180e4_5e3e_42f7_820c_e08951223486> ;
            owl:onProperty :hasDatatype ],
        [ a owl:Restriction ;
            owl:hasValue :number_of_species_projected_dos_values ;
            owl:onProperty :hasVarDim1 ],
        [ a owl:Restriction ;
            owl:allValuesFrom <http://emmo.info/emmo/middle/siunits#EMMO_8a70dea4_d6ab_4260_b931_a3e990982416> ;
            owl:onProperty <http://emmo.info/emmo/middle/metrology#EMMO_67fc0a36_8dcb_4ffa_9a43_31074efa3296> ],
        [ a owl:Restriction ;
            owl:hasValue 1 ;
            owl:onProperty :hasNumberOfDimensions ],
        :NMI_quantity .

:species_projected_dos_lm a owl:Class ;
    rdfs:comment """Consists of tuples of $l$ and $m$ values for all given values in the
species_projected_dos_values_lm species field.

The quantum number $l$ represents the azimuthal quantum number, whereas for the
quantum number $m$, besides the conventional use as magnetic quantum number ($l+1$
integer values from $-l$ to $l$), a set of different conventions is accepted. The
adopted convention is specified by atom_projected_dos_m_kind."""^^xsd:string ;
    rdfs:subClassOf [ a owl:Restriction ;
            owl:hasValue :number_of_lm_species_projected_dos ;
            owl:onProperty :hasVarDim1 ],
        [ a owl:Restriction ;
            owl:hasValue 2 ;
            owl:onProperty :hasNumberOfDimensions ],
        [ a owl:Restriction ;
            owl:hasValue 2 ;
            owl:onProperty :hasFixDim2 ],
        [ a owl:Restriction ;
            owl:allValuesFrom <http://emmo.info/emmo/middle/math#EMMO_f8bd64d5_5d3e_4ad4_a46e_c30714fecb7f> ;
            owl:onProperty :hasDatatype ],
        :NMI_quantity .

:species_projected_dos_m_kind a owl:Class ;
    rdfs:comment """Specifies the kind of the integer numbers $m$ used in species_projected_dos_lm.

Allowed values are listed in the [m_kind wiki
page](https://gitlab.rzg.mpg.de/nomad-lab/nomad-meta-info/wikis/metainfo/m-kind)
and can be (quantum) numbers of

* spherical

* polynomial

* real_orbital

* integrated

functions or values."""^^xsd:string ;
    rdfs:subClassOf [ a owl:Restriction ;
            owl:hasValue 0 ;
            owl:onProperty :hasNumberOfDimensions ],
        [ a owl:Restriction ;
            owl:allValuesFrom <http://emmo.info/emmo/middle/perceptual#EMMO_50ea1ec5_f157_41b0_b46b_a9032f17ca10> ;
            owl:onProperty :hasDatatype ],
        :NMI_quantity .

:species_projected_dos_species_label a owl:Class ;
    rdfs:comment """Contains labels of the atomic species for the species-projected density of states
(DOS).

Differently from atom_labels, which allow more than one label for the same atomic
species (by adding a number or a string to the label), this list is expected to
refer to actual atomic species, i.e. belonging to the periodic table of elements.
Thus, the species-projected DOS are expected to be as many as the different atomic
species in the system."""^^xsd:string ;
    rdfs:subClassOf [ a owl:Restriction ;
            owl:allValuesFrom <http://emmo.info/emmo/middle/perceptual#EMMO_50ea1ec5_f157_41b0_b46b_a9032f17ca10> ;
            owl:onProperty :hasDatatype ],
        [ a owl:Restriction ;
            owl:hasValue :number_of_species ;
            owl:onProperty :hasVarDim1 ],
        [ a owl:Restriction ;
            owl:hasValue 1 ;
            owl:onProperty :hasNumberOfDimensions ],
        :NMI_quantity .

:species_projected_dos_values_lm a owl:Class ;
    rdfs:comment """Holds species-projected density of states (DOS) values, divided into contributions
from each $l,m$ channel.

Here, there are as many species-projected DOS as the number of species,
number_of_species. The list of labels of the species is given in
species_projected_dos_species_label."""^^xsd:string ;
    rdfs:subClassOf [ a owl:Restriction ;
            owl:hasValue :number_of_spin_channels ;
            owl:onProperty :hasVarDim2 ],
        [ a owl:Restriction ;
            owl:hasValue 4 ;
            owl:onProperty :hasNumberOfDimensions ],
        [ a owl:Restriction ;
            owl:hasValue :number_of_species_projected_dos_values ;
            owl:onProperty :hasVarDim4 ],
        [ a owl:Restriction ;
            owl:hasValue :number_of_species ;
            owl:onProperty :hasVarDim3 ],
        [ a owl:Restriction ;
            owl:allValuesFrom <http://emmo.info/emmo/middle/math#EMMO_18d180e4_5e3e_42f7_820c_e08951223486> ;
            owl:onProperty :hasDatatype ],
        [ a owl:Restriction ;
            owl:hasValue :number_of_lm_species_projected_dos ;
            owl:onProperty :hasVarDim1 ],
        :NMI_quantity .

:species_projected_dos_values_total a owl:Class ;
    rdfs:comment """Holds species-projected density of states (DOS) values, summed up over all
azimuthal quantum numbers $l$.

Here, there are as many species-projected DOS as the number of species,
number_of_species. The list of labels of the species is given in
species_projected_dos_species_label."""^^xsd:string ;
    rdfs:subClassOf [ a owl:Restriction ;
            owl:hasValue :number_of_species ;
            owl:onProperty :hasVarDim2 ],
        [ a owl:Restriction ;
            owl:hasValue :number_of_spin_channels ;
            owl:onProperty :hasVarDim1 ],
        [ a owl:Restriction ;
            owl:allValuesFrom <http://emmo.info/emmo/middle/math#EMMO_18d180e4_5e3e_42f7_820c_e08951223486> ;
            owl:onProperty :hasDatatype ],
        [ a owl:Restriction ;
            owl:hasValue 3 ;
            owl:onProperty :hasNumberOfDimensions ],
        [ a owl:Restriction ;
            owl:hasValue :number_of_species_projected_dos_values ;
            owl:onProperty :hasVarDim3 ],
        :NMI_quantity .

:specific_heat_capacity a owl:Class ;
    rdfs:comment "Stores the specific heat capacity at constant volume."^^xsd:string ;
    rdfs:subClassOf [ a owl:Restriction ;
            owl:allValuesFrom <http://emmo.info/emmo/middle/math#EMMO_18d180e4_5e3e_42f7_820c_e08951223486> ;
            owl:onProperty :hasDatatype ],
        [ a owl:Restriction ;
            owl:allValuesFrom <https://nomad-coe.eu/ontology/properties#JouleKilogramPerKelvin> ;
            owl:onProperty <http://emmo.info/emmo/middle/metrology#EMMO_67fc0a36_8dcb_4ffa_9a43_31074efa3296> ],
        [ a owl:Restriction ;
            owl:hasValue :number_of_thermodynamical_property_values ;
            owl:onProperty :hasVarDim1 ],
        [ a owl:Restriction ;
            owl:hasValue 1 ;
            owl:onProperty :hasNumberOfDimensions ],
        :NMI_quantity .

:specific_vibrational_free_energy_at_constant_volume a owl:Class ;
    rdfs:comment "Stores the specific vibrational free energy at constant volume."^^xsd:string ;
    rdfs:subClassOf [ a owl:Restriction ;
            owl:allValuesFrom <https://nomad-coe.eu/ontology/properties#JoulePerKilogram> ;
            owl:onProperty <http://emmo.info/emmo/middle/metrology#EMMO_67fc0a36_8dcb_4ffa_9a43_31074efa3296> ],
        [ a owl:Restriction ;
            owl:hasValue 1 ;
            owl:onProperty :hasNumberOfDimensions ],
        [ a owl:Restriction ;
            owl:allValuesFrom <http://emmo.info/emmo/middle/math#EMMO_18d180e4_5e3e_42f7_820c_e08951223486> ;
            owl:onProperty :hasDatatype ],
        [ a owl:Restriction ;
            owl:hasValue :number_of_thermodynamical_property_values ;
            owl:onProperty :hasVarDim1 ],
        :NMI_quantity .

:spin_S2 a owl:Class ;
    rdfs:comment """Stores the value of the total spin moment operator $S^2$ for the converged
wavefunctions calculated with the XC_method. It can be used to calculate the spin
contamination in spin-unrestricted calculations."""^^xsd:string ;
    rdfs:subClassOf [ a owl:Restriction ;
            owl:hasValue 0 ;
            owl:onProperty :hasNumberOfDimensions ],
        [ a owl:Restriction ;
            owl:allValuesFrom <http://emmo.info/emmo/middle/math#EMMO_18d180e4_5e3e_42f7_820c_e08951223486> ;
            owl:onProperty :hasDatatype ],
        :NMI_quantity .

:spin_S2_scf_iteration a owl:Class ;
    rdfs:comment """Stores the value of the total spin moment operator $S^2$ during the self-
consistent field (SCF) iterations of the XC_method. It can be used to calculate
the spin contamination in spin-unrestricted calculations."""^^xsd:string ;
    rdfs:subClassOf [ a owl:Restriction ;
            owl:hasValue 0 ;
            owl:onProperty :hasNumberOfDimensions ],
        [ a owl:Restriction ;
            owl:allValuesFrom <http://emmo.info/emmo/middle/math#EMMO_18d180e4_5e3e_42f7_820c_e08951223486> ;
            owl:onProperty :hasDatatype ],
        :NMI_quantity .

:spin_target_multiplicity a owl:Class ;
    rdfs:comment """Stores the target (user-imposed) value of the spin multiplicity $M=2S+1$, where
$S$ is the total spin. It is an integer number. This value is not necessarily the
value obtained at the end of the calculation. See spin_S2 for the converged value
of the spin moment."""^^xsd:string ;
    rdfs:subClassOf [ a owl:Restriction ;
            owl:allValuesFrom <http://emmo.info/emmo/middle/math#EMMO_f8bd64d5_5d3e_4ad4_a46e_c30714fecb7f> ;
            owl:onProperty <http://emmo.info/emmo/middle/metrology#EMMO_67fc0a36_8dcb_4ffa_9a43_31074efa3296> ],
        [ a owl:Restriction ;
            owl:allValuesFrom <http://emmo.info/emmo/middle/math#EMMO_f8bd64d5_5d3e_4ad4_a46e_c30714fecb7f> ;
            owl:onProperty :hasDatatype ],
        [ a owl:Restriction ;
            owl:hasValue 0 ;
            owl:onProperty :hasNumberOfDimensions ],
        :NMI_dimension,
        :NMI_quantity .

:springer_alphabetical_formula a owl:Class ;
    rdfs:comment "The alphabetical formula of the material according to Springer Materials Database"^^xsd:string ;
    rdfs:subClassOf [ a owl:Restriction ;
            owl:allValuesFrom <http://emmo.info/emmo/middle/perceptual#EMMO_50ea1ec5_f157_41b0_b46b_a9032f17ca10> ;
            owl:onProperty :hasDatatype ],
        [ a owl:Restriction ;
            owl:hasValue 0 ;
            owl:onProperty :hasNumberOfDimensions ],
        :NMI_quantity .

:springer_classification a owl:Class ;
    rdfs:comment """Contains the classification name of the current material according to Springer
Materials"""^^xsd:string ;
    rdfs:subClassOf [ a owl:Restriction ;
            owl:hasValue 1 ;
            owl:onProperty :hasNumberOfDimensions ],
        [ a owl:Restriction ;
            owl:allValuesFrom <http://emmo.info/emmo/middle/perceptual#EMMO_50ea1ec5_f157_41b0_b46b_a9032f17ca10> ;
            owl:onProperty :hasDatatype ],
        :NMI_quantity .

:springer_compound_class a owl:Class ;
    rdfs:comment """Name of a class of the current compound, as defined in by Springer Materials. This
is a property of the chemical formula of the compound"""^^xsd:string ;
    rdfs:subClassOf [ a owl:Restriction ;
            owl:hasValue 1 ;
            owl:onProperty :hasNumberOfDimensions ],
        [ a owl:Restriction ;
            owl:allValuesFrom <http://emmo.info/emmo/middle/perceptual#EMMO_50ea1ec5_f157_41b0_b46b_a9032f17ca10> ;
            owl:onProperty :hasDatatype ],
        :NMI_quantity .

:springer_id a owl:Class ;
    rdfs:comment "Id of the classified material according to Springer Materials"^^xsd:string ;
    rdfs:subClassOf [ a owl:Restriction ;
            owl:hasValue 0 ;
            owl:onProperty :hasNumberOfDimensions ],
        [ a owl:Restriction ;
            owl:allValuesFrom <http://emmo.info/emmo/middle/perceptual#EMMO_50ea1ec5_f157_41b0_b46b_a9032f17ca10> ;
            owl:onProperty :hasDatatype ],
        :NMI_quantity .

:springer_url a owl:Class ;
    rdfs:comment "Url to the source page in Springer Materials describing the current entry"^^xsd:string ;
    rdfs:subClassOf [ a owl:Restriction ;
            owl:allValuesFrom <http://emmo.info/emmo/middle/perceptual#EMMO_50ea1ec5_f157_41b0_b46b_a9032f17ca10> ;
            owl:onProperty :hasDatatype ],
        [ a owl:Restriction ;
            owl:hasValue 0 ;
            owl:onProperty :hasNumberOfDimensions ],
        :NMI_quantity .

:stepsize a owl:Class ;
    rdfs:comment "Stepsize of interpolation in the first step of the generation of DOS fingerprints."^^xsd:string ;
    rdfs:subClassOf [ a owl:Restriction ;
            owl:hasValue 0 ;
            owl:onProperty :hasNumberOfDimensions ],
        [ a owl:Restriction ;
            owl:allValuesFrom <http://emmo.info/emmo/middle/math#EMMO_18d180e4_5e3e_42f7_820c_e08951223486> ;
            owl:onProperty :hasDatatype ],
        :NMI_quantity .

:stress_tensor a owl:Class ;
    rdfs:comment """Stores the final value of the default stress tensor consistent with energy_total
and calculated with the method specified in stress_tensor_method.

This value is used (if needed) for, e.g., molecular dynamics and geometry
optimization. Alternative definitions of the stress tensor can be assigned with
stress_tensor_kind"""^^xsd:string ;
    rdfs:subClassOf [ a owl:Restriction ;
            owl:hasValue 2 ;
            owl:onProperty :hasNumberOfDimensions ],
        [ a owl:Restriction ;
            owl:allValuesFrom <http://emmo.info/emmo/middle/math#EMMO_18d180e4_5e3e_42f7_820c_e08951223486> ;
            owl:onProperty :hasDatatype ],
        [ a owl:Restriction ;
            owl:hasValue 3 ;
            owl:onProperty :hasFixDim1 ],
        [ a owl:Restriction ;
            owl:hasValue 3 ;
            owl:onProperty :hasFixDim2 ],
        [ a owl:Restriction ;
            owl:onProperty :hasCategory ;
            owl:someValuesFrom :stress_tensor_type ],
        [ a owl:Restriction ;
            owl:allValuesFrom <http://emmo.info/emmo/middle/siunits#EMMO_a80dc6f5_b1aa_41a7_a3a8_cd5040da2162> ;
            owl:onProperty <http://emmo.info/emmo/middle/metrology#EMMO_67fc0a36_8dcb_4ffa_9a43_31074efa3296> ],
        :NMI_quantity .

:stress_tensor_kind a owl:Class ;
    rdfs:comment """Specifies the method used to compute the stress tensor stored in
stress_tensor_value. This is an *alternative* to the stress tensor defined in
stress_tensor_method, which is stored in stress_tensor.

This field allows for multiple definitions and evaluated values of the stress
tensor, while only one definition is used for, e.g., molecular dynamics and
geometry optimization."""^^xsd:string ;
    rdfs:subClassOf [ a owl:Restriction ;
            owl:allValuesFrom <http://emmo.info/emmo/middle/perceptual#EMMO_50ea1ec5_f157_41b0_b46b_a9032f17ca10> ;
            owl:onProperty :hasDatatype ],
        [ a owl:Restriction ;
            owl:hasValue 0 ;
            owl:onProperty :hasNumberOfDimensions ],
        :NMI_quantity .

:stress_tensor_method a owl:Class ;
    rdfs:comment """Specifies the method used to calculate stress_tensor for, e.g., molecular dynamics
and geometry optimization.

The allowed values are:

* numeric

* analytic"""^^xsd:string ;
    rdfs:subClassOf [ a owl:Restriction ;
            owl:onProperty :hasCategory ;
            owl:someValuesFrom :settings_stress_tensor ],
        [ a owl:Restriction ;
            owl:allValuesFrom <http://emmo.info/emmo/middle/perceptual#EMMO_50ea1ec5_f157_41b0_b46b_a9032f17ca10> ;
            owl:onProperty :hasDatatype ],
        [ a owl:Restriction ;
            owl:hasValue 0 ;
            owl:onProperty :hasNumberOfDimensions ],
        :NMI_quantity .

:stress_tensor_value a owl:Class ;
    rdfs:comment """Contains the value of the stress tensor of the kind defined in stress_tensor_kind.
This is an *alternative* to the stress tensor defined in stress_tensor_method.

This field allows for multiple definitions and evaluated values of the stress
tensor, while only one definition is used for, e.g., molecular dynamics and
geometry optimization."""^^xsd:string ;
    rdfs:subClassOf [ a owl:Restriction ;
            owl:hasValue 2 ;
            owl:onProperty :hasNumberOfDimensions ],
        [ a owl:Restriction ;
            owl:hasValue 3 ;
            owl:onProperty :hasFixDim1 ],
        [ a owl:Restriction ;
            owl:allValuesFrom <http://emmo.info/emmo/middle/math#EMMO_18d180e4_5e3e_42f7_820c_e08951223486> ;
            owl:onProperty :hasDatatype ],
        [ a owl:Restriction ;
            owl:allValuesFrom <http://emmo.info/emmo/middle/siunits#EMMO_a80dc6f5_b1aa_41a7_a3a8_cd5040da2162> ;
            owl:onProperty <http://emmo.info/emmo/middle/metrology#EMMO_67fc0a36_8dcb_4ffa_9a43_31074efa3296> ],
        [ a owl:Restriction ;
            owl:onProperty :hasCategory ;
            owl:someValuesFrom :stress_tensor_type ],
        [ a owl:Restriction ;
            owl:hasValue 3 ;
            owl:onProperty :hasFixDim2 ],
        :NMI_quantity .

:symmetry_method a owl:Class ;
    rdfs:comment """Identifies the source of the symmetry information contained within this section.
If equal to 'spg_normalized' the information comes from a normalization step."""^^xsd:string ;
    rdfs:subClassOf [ a owl:Restriction ;
            owl:hasValue 0 ;
            owl:onProperty :hasNumberOfDimensions ],
        [ a owl:Restriction ;
            owl:allValuesFrom <http://emmo.info/emmo/middle/perceptual#EMMO_50ea1ec5_f157_41b0_b46b_a9032f17ca10> ;
            owl:onProperty :hasDatatype ],
        :NMI_quantity .

:symmorphic a owl:Class ;
    rdfs:comment "Is the space group symmorphic? Set to True if all translations are zero."^^xsd:string ;
    rdfs:subClassOf [ a owl:Restriction ;
            owl:allValuesFrom <http://emmo.info/emmo/middle/math#EMMO_54dc83cb_06e1_4739_9e45_bc09cead7f48> ;
            owl:onProperty :hasDatatype ],
        [ a owl:Restriction ;
            owl:hasValue 0 ;
            owl:onProperty :hasNumberOfDimensions ],
        :NMI_quantity .

:system_composition a owl:Class ;
    rdfs:comment """Composition, i.e. cumulative chemical formula with atoms ordered by decreasing
atomic number Z."""^^xsd:string ;
    rdfs:subClassOf [ a owl:Restriction ;
            owl:allValuesFrom <http://emmo.info/emmo/middle/perceptual#EMMO_50ea1ec5_f157_41b0_b46b_a9032f17ca10> ;
            owl:onProperty :hasDatatype ],
        [ a owl:Restriction ;
            owl:hasValue 0 ;
            owl:onProperty :hasNumberOfDimensions ],
        :NMI_quantity .

:system_configuration_consistent a owl:Class ;
    rdfs:comment "Flag set is the configuration is consistent"^^xsd:string ;
    rdfs:subClassOf [ a owl:Restriction ;
            owl:hasValue 0 ;
            owl:onProperty :hasNumberOfDimensions ],
        [ a owl:Restriction ;
            owl:allValuesFrom <http://emmo.info/emmo/middle/math#EMMO_54dc83cb_06e1_4739_9e45_bc09cead7f48> ;
            owl:onProperty :hasDatatype ],
        :NMI_quantity .

:system_name a owl:Class ;
    rdfs:comment """Specifies the name of the system. This information is provided by the user in some
codes and is stored here for debugging or visualization purposes."""^^xsd:string ;
    rdfs:subClassOf [ a owl:Restriction ;
            owl:hasValue 0 ;
            owl:onProperty :hasNumberOfDimensions ],
        [ a owl:Restriction ;
            owl:allValuesFrom <http://emmo.info/emmo/middle/perceptual#EMMO_50ea1ec5_f157_41b0_b46b_a9032f17ca10> ;
            owl:onProperty :hasDatatype ],
        :NMI_quantity .

:system_reweighted_composition a owl:Class ;
    rdfs:comment """Composition, i.e. cumulative chemical with atoms ordered by decreasing atomic
number Z reweighted so that the sum is close to 100, and values are rounded up,
and are stable (i.e. it is a fixed point)."""^^xsd:string ;
    rdfs:subClassOf [ a owl:Restriction ;
            owl:allValuesFrom <http://emmo.info/emmo/middle/perceptual#EMMO_50ea1ec5_f157_41b0_b46b_a9032f17ca10> ;
            owl:onProperty :hasDatatype ],
        [ a owl:Restriction ;
            owl:hasValue 0 ;
            owl:onProperty :hasNumberOfDimensions ],
        :NMI_quantity .

:system_to_system_kind a owl:Class ;
    rdfs:comment """String defining the relationship between the referenced section_system and the
present section_system. Often systems are connected for example if a phonon
calculation using finite differences is performed the force ealuation is done in a
larger supercell but properties such as the phonon band structure are still
calculated for the primitive cell. Hence, the need of keeping track of these
connected systems. The referenced system is identified via system_to_system_ref."""^^xsd:string ;
    rdfs:subClassOf [ a owl:Restriction ;
            owl:hasValue 0 ;
            owl:onProperty :hasNumberOfDimensions ],
        [ a owl:Restriction ;
            owl:allValuesFrom <http://emmo.info/emmo/middle/perceptual#EMMO_50ea1ec5_f157_41b0_b46b_a9032f17ca10> ;
            owl:onProperty :hasDatatype ],
        :NMI_quantity .

:system_to_system_ref a owl:Class ;
    rdfs:comment """Reference to another system. The kind of relationship between the present and the
referenced section_system is specified by system_to_system_kind."""^^xsd:string ;
    rdfs:subClassOf [ a owl:Restriction ;
            owl:hasValue 0 ;
            owl:onProperty :hasNumberOfDimensions ],
        :NMI_quantity .

:system_type a owl:Class ;
    rdfs:comment "Type of the system"^^xsd:string ;
    rdfs:subClassOf [ a owl:Restriction ;
            owl:hasValue 0 ;
            owl:onProperty :hasNumberOfDimensions ],
        [ a owl:Restriction ;
            owl:allValuesFrom <http://emmo.info/emmo/middle/perceptual#EMMO_50ea1ec5_f157_41b0_b46b_a9032f17ca10> ;
            owl:onProperty :hasDatatype ],
        :NMI_quantity .

:thermodynamical_properties_calculation_method a owl:Class ;
    rdfs:comment """Method used to calculate the thermodynamic quantities.

Valid values:

* harmonic"""^^xsd:string ;
    rdfs:subClassOf [ a owl:Restriction ;
            owl:allValuesFrom <http://emmo.info/emmo/middle/perceptual#EMMO_50ea1ec5_f157_41b0_b46b_a9032f17ca10> ;
            owl:onProperty :hasDatatype ],
        [ a owl:Restriction ;
            owl:hasValue 0 ;
            owl:onProperty :hasNumberOfDimensions ],
        :NMI_quantity .

:thermodynamical_property_heat_capacity_C_v a owl:Class ;
    rdfs:comment "Stores the heat capacity per cell unit at constant volume."^^xsd:string ;
    rdfs:subClassOf [ a owl:Restriction ;
            owl:allValuesFrom <https://nomad-coe.eu/ontology/properties#JoulePerKelvin> ;
            owl:onProperty <http://emmo.info/emmo/middle/metrology#EMMO_67fc0a36_8dcb_4ffa_9a43_31074efa3296> ],
        [ a owl:Restriction ;
            owl:hasValue 1 ;
            owl:onProperty :hasNumberOfDimensions ],
        [ a owl:Restriction ;
            owl:hasValue :number_of_thermodynamical_property_values ;
            owl:onProperty :hasVarDim1 ],
        [ a owl:Restriction ;
            owl:allValuesFrom <http://emmo.info/emmo/middle/math#EMMO_18d180e4_5e3e_42f7_820c_e08951223486> ;
            owl:onProperty :hasDatatype ],
        :NMI_quantity .

:thermodynamical_property_temperature a owl:Class ;
    rdfs:comment """Specifies the temperatures at which properties such as the Helmholtz free energy
are calculated."""^^xsd:string ;
    rdfs:subClassOf [ a owl:Restriction ;
            owl:hasValue 1 ;
            owl:onProperty :hasNumberOfDimensions ],
        [ a owl:Restriction ;
            owl:hasValue :number_of_thermodynamical_property_values ;
            owl:onProperty :hasVarDim1 ],
        [ a owl:Restriction ;
            owl:allValuesFrom <http://emmo.info/emmo/middle/math#EMMO_18d180e4_5e3e_42f7_820c_e08951223486> ;
            owl:onProperty :hasDatatype ],
        [ a owl:Restriction ;
            owl:allValuesFrom <http://emmo.info/emmo/middle/siunits#EMMO_2e5e45fc_f52c_4294_bdc2_5ed7a06dfce7> ;
            owl:onProperty <http://emmo.info/emmo/middle/metrology#EMMO_67fc0a36_8dcb_4ffa_9a43_31074efa3296> ],
        :NMI_quantity .

:time_calculation a owl:Class ;
    rdfs:comment """Stores the wall-clock time needed for a calculation using
calculation_method_current. Basically, it tracks the real time that has been
elapsed from start to end."""^^xsd:string ;
    rdfs:subClassOf [ a owl:Restriction ;
            owl:onProperty :hasCategory ;
            owl:someValuesFrom :accessory_info ],
        [ a owl:Restriction ;
            owl:allValuesFrom <http://emmo.info/emmo/middle/math#EMMO_18d180e4_5e3e_42f7_820c_e08951223486> ;
            owl:onProperty :hasDatatype ],
        [ a owl:Restriction ;
            owl:onProperty :hasCategory ;
            owl:someValuesFrom :time_info ],
        [ a owl:Restriction ;
            owl:allValuesFrom <http://emmo.info/emmo/middle/siunits#EMMO_314ba716_2d3d_4462_9a4f_d3419ae1df43> ;
            owl:onProperty <http://emmo.info/emmo/middle/metrology#EMMO_67fc0a36_8dcb_4ffa_9a43_31074efa3296> ],
        [ a owl:Restriction ;
            owl:hasValue 0 ;
            owl:onProperty :hasNumberOfDimensions ],
        :NMI_quantity .

:time_reversal_symmetry a owl:Class ;
    rdfs:comment "Is time-reversal symmetry present?"^^xsd:string ;
    rdfs:subClassOf [ a owl:Restriction ;
            owl:allValuesFrom <http://emmo.info/emmo/middle/math#EMMO_54dc83cb_06e1_4739_9e45_bc09cead7f48> ;
            owl:onProperty :hasDatatype ],
        [ a owl:Restriction ;
            owl:hasValue 0 ;
            owl:onProperty :hasNumberOfDimensions ],
        :NMI_quantity .

:time_run_cpu1_end a owl:Class ;
    rdfs:comment "Stores the end time of the run on CPU 1."^^xsd:string ;
    rdfs:subClassOf [ a owl:Restriction ;
            owl:onProperty :hasCategory ;
            owl:someValuesFrom :time_info ],
        [ a owl:Restriction ;
            owl:hasValue 0 ;
            owl:onProperty :hasNumberOfDimensions ],
        [ a owl:Restriction ;
            owl:allValuesFrom <http://emmo.info/emmo/middle/siunits#EMMO_314ba716_2d3d_4462_9a4f_d3419ae1df43> ;
            owl:onProperty <http://emmo.info/emmo/middle/metrology#EMMO_67fc0a36_8dcb_4ffa_9a43_31074efa3296> ],
        [ a owl:Restriction ;
            owl:onProperty :hasCategory ;
            owl:someValuesFrom :accessory_info ],
        [ a owl:Restriction ;
            owl:allValuesFrom <http://emmo.info/emmo/middle/math#EMMO_18d180e4_5e3e_42f7_820c_e08951223486> ;
            owl:onProperty :hasDatatype ],
        :NMI_quantity .

:time_run_cpu1_start a owl:Class ;
    rdfs:comment "Stores the start time of the run on CPU 1."^^xsd:string ;
    rdfs:subClassOf [ a owl:Restriction ;
            owl:onProperty :hasCategory ;
            owl:someValuesFrom :accessory_info ],
        [ a owl:Restriction ;
            owl:allValuesFrom <http://emmo.info/emmo/middle/math#EMMO_18d180e4_5e3e_42f7_820c_e08951223486> ;
            owl:onProperty :hasDatatype ],
        [ a owl:Restriction ;
            owl:hasValue 0 ;
            owl:onProperty :hasNumberOfDimensions ],
        [ a owl:Restriction ;
            owl:onProperty :hasCategory ;
            owl:someValuesFrom :time_info ],
        [ a owl:Restriction ;
            owl:allValuesFrom <http://emmo.info/emmo/middle/siunits#EMMO_314ba716_2d3d_4462_9a4f_d3419ae1df43> ;
            owl:onProperty <http://emmo.info/emmo/middle/metrology#EMMO_67fc0a36_8dcb_4ffa_9a43_31074efa3296> ],
        :NMI_quantity .

:time_run_date_end a owl:Class ;
    rdfs:comment """Stores the end date of the run as time since the *Unix epoch* (00:00:00 UTC on 1
January 1970) in seconds. For date and times without a timezone, the default
timezone GMT is used."""^^xsd:string ;
    rdfs:subClassOf [ a owl:Restriction ;
            owl:onProperty :hasCategory ;
            owl:someValuesFrom :time_info ],
        [ a owl:Restriction ;
            owl:hasValue 0 ;
            owl:onProperty :hasNumberOfDimensions ],
        [ a owl:Restriction ;
            owl:onProperty :hasCategory ;
            owl:someValuesFrom :accessory_info ],
        [ a owl:Restriction ;
            owl:allValuesFrom <http://emmo.info/emmo/middle/math#EMMO_18d180e4_5e3e_42f7_820c_e08951223486> ;
            owl:onProperty :hasDatatype ],
        [ a owl:Restriction ;
            owl:allValuesFrom <http://emmo.info/emmo/middle/siunits#EMMO_314ba716_2d3d_4462_9a4f_d3419ae1df43> ;
            owl:onProperty <http://emmo.info/emmo/middle/metrology#EMMO_67fc0a36_8dcb_4ffa_9a43_31074efa3296> ],
        :NMI_quantity .

:time_run_date_start a owl:Class ;
    rdfs:comment """Stores the start date of the run as time since the *Unix epoch* (00:00:00 UTC on 1
January 1970) in seconds. For date and times without a timezone, the default
timezone GMT is used."""^^xsd:string ;
    rdfs:subClassOf [ a owl:Restriction ;
            owl:onProperty :hasCategory ;
            owl:someValuesFrom :accessory_info ],
        [ a owl:Restriction ;
            owl:allValuesFrom <http://emmo.info/emmo/middle/siunits#EMMO_314ba716_2d3d_4462_9a4f_d3419ae1df43> ;
            owl:onProperty <http://emmo.info/emmo/middle/metrology#EMMO_67fc0a36_8dcb_4ffa_9a43_31074efa3296> ],
        [ a owl:Restriction ;
            owl:allValuesFrom <http://emmo.info/emmo/middle/math#EMMO_18d180e4_5e3e_42f7_820c_e08951223486> ;
            owl:onProperty :hasDatatype ],
        [ a owl:Restriction ;
            owl:onProperty :hasCategory ;
            owl:someValuesFrom :time_info ],
        [ a owl:Restriction ;
            owl:hasValue 0 ;
            owl:onProperty :hasNumberOfDimensions ],
        :NMI_quantity .

:time_run_wall_end a owl:Class ;
    rdfs:comment "Stores the internal wall-clock time at the end of the run."^^xsd:string ;
    rdfs:subClassOf [ a owl:Restriction ;
            owl:hasValue 0 ;
            owl:onProperty :hasNumberOfDimensions ],
        [ a owl:Restriction ;
            owl:onProperty :hasCategory ;
            owl:someValuesFrom :time_info ],
        [ a owl:Restriction ;
            owl:onProperty :hasCategory ;
            owl:someValuesFrom :accessory_info ],
        [ a owl:Restriction ;
            owl:allValuesFrom <http://emmo.info/emmo/middle/siunits#EMMO_314ba716_2d3d_4462_9a4f_d3419ae1df43> ;
            owl:onProperty <http://emmo.info/emmo/middle/metrology#EMMO_67fc0a36_8dcb_4ffa_9a43_31074efa3296> ],
        [ a owl:Restriction ;
            owl:allValuesFrom <http://emmo.info/emmo/middle/math#EMMO_18d180e4_5e3e_42f7_820c_e08951223486> ;
            owl:onProperty :hasDatatype ],
        :NMI_quantity .

:time_run_wall_start a owl:Class ;
    rdfs:comment "Stores the internal wall-clock time from the start of the run."^^xsd:string ;
    rdfs:subClassOf [ a owl:Restriction ;
            owl:onProperty :hasCategory ;
            owl:someValuesFrom :time_info ],
        [ a owl:Restriction ;
            owl:allValuesFrom <http://emmo.info/emmo/middle/math#EMMO_18d180e4_5e3e_42f7_820c_e08951223486> ;
            owl:onProperty :hasDatatype ],
        [ a owl:Restriction ;
            owl:allValuesFrom <http://emmo.info/emmo/middle/siunits#EMMO_314ba716_2d3d_4462_9a4f_d3419ae1df43> ;
            owl:onProperty <http://emmo.info/emmo/middle/metrology#EMMO_67fc0a36_8dcb_4ffa_9a43_31074efa3296> ],
        [ a owl:Restriction ;
            owl:onProperty :hasCategory ;
            owl:someValuesFrom :accessory_info ],
        [ a owl:Restriction ;
            owl:hasValue 0 ;
            owl:onProperty :hasNumberOfDimensions ],
        :NMI_quantity .

:time_scf_iteration_cpu1_end a owl:Class ;
    rdfs:comment "Stores the end time of a self-consistent field (SCF) iteration on CPU 1."^^xsd:string ;
    rdfs:subClassOf [ a owl:Restriction ;
            owl:allValuesFrom <http://emmo.info/emmo/middle/math#EMMO_18d180e4_5e3e_42f7_820c_e08951223486> ;
            owl:onProperty :hasDatatype ],
        [ a owl:Restriction ;
            owl:onProperty :hasCategory ;
            owl:someValuesFrom :accessory_info ],
        [ a owl:Restriction ;
            owl:hasValue 0 ;
            owl:onProperty :hasNumberOfDimensions ],
        [ a owl:Restriction ;
            owl:onProperty :hasCategory ;
            owl:someValuesFrom :time_info ],
        [ a owl:Restriction ;
            owl:allValuesFrom <http://emmo.info/emmo/middle/siunits#EMMO_314ba716_2d3d_4462_9a4f_d3419ae1df43> ;
            owl:onProperty <http://emmo.info/emmo/middle/metrology#EMMO_67fc0a36_8dcb_4ffa_9a43_31074efa3296> ],
        :NMI_quantity .

:time_scf_iteration_cpu1_start a owl:Class ;
    rdfs:comment "Stores the start time of a self-consistent field (SCF) iteration on CPU 1."^^xsd:string ;
    rdfs:subClassOf [ a owl:Restriction ;
            owl:hasValue 0 ;
            owl:onProperty :hasNumberOfDimensions ],
        [ a owl:Restriction ;
            owl:allValuesFrom <http://emmo.info/emmo/middle/math#EMMO_18d180e4_5e3e_42f7_820c_e08951223486> ;
            owl:onProperty :hasDatatype ],
        [ a owl:Restriction ;
            owl:onProperty :hasCategory ;
            owl:someValuesFrom :accessory_info ],
        [ a owl:Restriction ;
            owl:onProperty :hasCategory ;
            owl:someValuesFrom :time_info ],
        [ a owl:Restriction ;
            owl:allValuesFrom <http://emmo.info/emmo/middle/siunits#EMMO_314ba716_2d3d_4462_9a4f_d3419ae1df43> ;
            owl:onProperty <http://emmo.info/emmo/middle/metrology#EMMO_67fc0a36_8dcb_4ffa_9a43_31074efa3296> ],
        :NMI_quantity .

:time_scf_iteration_date_end a owl:Class ;
    rdfs:comment """Stores the end date of a self-consistent field (SCF) iteration as time since the
*Unix epoch* (00:00:00 UTC on 1 January 1970) in seconds. For date and times
without a timezone, the default timezone GMT is used."""^^xsd:string ;
    rdfs:subClassOf [ a owl:Restriction ;
            owl:allValuesFrom <http://emmo.info/emmo/middle/siunits#EMMO_314ba716_2d3d_4462_9a4f_d3419ae1df43> ;
            owl:onProperty <http://emmo.info/emmo/middle/metrology#EMMO_67fc0a36_8dcb_4ffa_9a43_31074efa3296> ],
        [ a owl:Restriction ;
            owl:onProperty :hasCategory ;
            owl:someValuesFrom :accessory_info ],
        [ a owl:Restriction ;
            owl:hasValue 0 ;
            owl:onProperty :hasNumberOfDimensions ],
        [ a owl:Restriction ;
            owl:allValuesFrom <http://emmo.info/emmo/middle/math#EMMO_18d180e4_5e3e_42f7_820c_e08951223486> ;
            owl:onProperty :hasDatatype ],
        [ a owl:Restriction ;
            owl:onProperty :hasCategory ;
            owl:someValuesFrom :time_info ],
        :NMI_quantity .

:time_scf_iteration_date_start a owl:Class ;
    rdfs:comment """Stores the start date of a self-consistent field (SCF) iteration as time since the
*Unix epoch* (00:00:00 UTC on 1 January 1970) in seconds. For date and times
without a timezone, the default timezone GMT is used."""^^xsd:string ;
    rdfs:subClassOf [ a owl:Restriction ;
            owl:onProperty :hasCategory ;
            owl:someValuesFrom :time_info ],
        [ a owl:Restriction ;
            owl:allValuesFrom <http://emmo.info/emmo/middle/siunits#EMMO_314ba716_2d3d_4462_9a4f_d3419ae1df43> ;
            owl:onProperty <http://emmo.info/emmo/middle/metrology#EMMO_67fc0a36_8dcb_4ffa_9a43_31074efa3296> ],
        [ a owl:Restriction ;
            owl:onProperty :hasCategory ;
            owl:someValuesFrom :accessory_info ],
        [ a owl:Restriction ;
            owl:hasValue 0 ;
            owl:onProperty :hasNumberOfDimensions ],
        [ a owl:Restriction ;
            owl:allValuesFrom <http://emmo.info/emmo/middle/math#EMMO_18d180e4_5e3e_42f7_820c_e08951223486> ;
            owl:onProperty :hasDatatype ],
        :NMI_quantity .

:time_scf_iteration_wall_end a owl:Class ;
    rdfs:comment """Stores the internal wall-clock time at the end of a self-consistent field (SCF)
iteration."""^^xsd:string ;
    rdfs:subClassOf [ a owl:Restriction ;
            owl:hasValue 0 ;
            owl:onProperty :hasNumberOfDimensions ],
        [ a owl:Restriction ;
            owl:allValuesFrom <http://emmo.info/emmo/middle/siunits#EMMO_314ba716_2d3d_4462_9a4f_d3419ae1df43> ;
            owl:onProperty <http://emmo.info/emmo/middle/metrology#EMMO_67fc0a36_8dcb_4ffa_9a43_31074efa3296> ],
        [ a owl:Restriction ;
            owl:onProperty :hasCategory ;
            owl:someValuesFrom :time_info ],
        [ a owl:Restriction ;
            owl:onProperty :hasCategory ;
            owl:someValuesFrom :accessory_info ],
        [ a owl:Restriction ;
            owl:allValuesFrom <http://emmo.info/emmo/middle/math#EMMO_18d180e4_5e3e_42f7_820c_e08951223486> ;
            owl:onProperty :hasDatatype ],
        :NMI_quantity .

:time_scf_iteration_wall_start a owl:Class ;
    rdfs:comment """Stores the internal wall-clock time from the start of a self-consistent field
(SCF) iteration."""^^xsd:string ;
    rdfs:subClassOf [ a owl:Restriction ;
            owl:hasValue 0 ;
            owl:onProperty :hasNumberOfDimensions ],
        [ a owl:Restriction ;
            owl:allValuesFrom <http://emmo.info/emmo/middle/math#EMMO_18d180e4_5e3e_42f7_820c_e08951223486> ;
            owl:onProperty :hasDatatype ],
        [ a owl:Restriction ;
            owl:onProperty :hasCategory ;
            owl:someValuesFrom :accessory_info ],
        [ a owl:Restriction ;
            owl:allValuesFrom <http://emmo.info/emmo/middle/siunits#EMMO_314ba716_2d3d_4462_9a4f_d3419ae1df43> ;
            owl:onProperty <http://emmo.info/emmo/middle/metrology#EMMO_67fc0a36_8dcb_4ffa_9a43_31074efa3296> ],
        [ a owl:Restriction ;
            owl:onProperty :hasCategory ;
            owl:someValuesFrom :time_info ],
        :NMI_quantity .

:time_single_configuration_calculation_cpu1_end a owl:Class ;
    rdfs:comment """Stores the end time of the *single configuration calculation* (see
section_single_configuration_calculation) on CPU 1."""^^xsd:string ;
    rdfs:subClassOf [ a owl:Restriction ;
            owl:allValuesFrom <http://emmo.info/emmo/middle/math#EMMO_18d180e4_5e3e_42f7_820c_e08951223486> ;
            owl:onProperty :hasDatatype ],
        [ a owl:Restriction ;
            owl:onProperty :hasCategory ;
            owl:someValuesFrom :time_info ],
        [ a owl:Restriction ;
            owl:hasValue 0 ;
            owl:onProperty :hasNumberOfDimensions ],
        [ a owl:Restriction ;
            owl:allValuesFrom <http://emmo.info/emmo/middle/siunits#EMMO_314ba716_2d3d_4462_9a4f_d3419ae1df43> ;
            owl:onProperty <http://emmo.info/emmo/middle/metrology#EMMO_67fc0a36_8dcb_4ffa_9a43_31074efa3296> ],
        [ a owl:Restriction ;
            owl:onProperty :hasCategory ;
            owl:someValuesFrom :accessory_info ],
        :NMI_quantity .

:time_single_configuration_calculation_cpu1_start a owl:Class ;
    rdfs:comment """Stores the start time of the *single configuration calculation* (see
section_single_configuration_calculation) on CPU 1."""^^xsd:string ;
    rdfs:subClassOf [ a owl:Restriction ;
            owl:hasValue 0 ;
            owl:onProperty :hasNumberOfDimensions ],
        [ a owl:Restriction ;
            owl:allValuesFrom <http://emmo.info/emmo/middle/math#EMMO_18d180e4_5e3e_42f7_820c_e08951223486> ;
            owl:onProperty :hasDatatype ],
        [ a owl:Restriction ;
            owl:onProperty :hasCategory ;
            owl:someValuesFrom :accessory_info ],
        [ a owl:Restriction ;
            owl:onProperty :hasCategory ;
            owl:someValuesFrom :time_info ],
        [ a owl:Restriction ;
            owl:allValuesFrom <http://emmo.info/emmo/middle/siunits#EMMO_314ba716_2d3d_4462_9a4f_d3419ae1df43> ;
            owl:onProperty <http://emmo.info/emmo/middle/metrology#EMMO_67fc0a36_8dcb_4ffa_9a43_31074efa3296> ],
        :NMI_quantity .

:time_single_configuration_calculation_date_end a owl:Class ;
    rdfs:comment """Stores the end date of the *single configuration calculation* (see
section_single_configuration_calculation) as time since the *Unix epoch* (00:00:00
UTC on 1 January 1970) in seconds. For date and times without a timezone, the
default timezone GMT is used."""^^xsd:string ;
    rdfs:subClassOf [ a owl:Restriction ;
            owl:allValuesFrom <http://emmo.info/emmo/middle/siunits#EMMO_314ba716_2d3d_4462_9a4f_d3419ae1df43> ;
            owl:onProperty <http://emmo.info/emmo/middle/metrology#EMMO_67fc0a36_8dcb_4ffa_9a43_31074efa3296> ],
        [ a owl:Restriction ;
            owl:onProperty :hasCategory ;
            owl:someValuesFrom :accessory_info ],
        [ a owl:Restriction ;
            owl:hasValue 0 ;
            owl:onProperty :hasNumberOfDimensions ],
        [ a owl:Restriction ;
            owl:onProperty :hasCategory ;
            owl:someValuesFrom :time_info ],
        [ a owl:Restriction ;
            owl:allValuesFrom <http://emmo.info/emmo/middle/math#EMMO_18d180e4_5e3e_42f7_820c_e08951223486> ;
            owl:onProperty :hasDatatype ],
        :NMI_quantity .

:time_single_configuration_calculation_date_start a owl:Class ;
    rdfs:comment """Stores the start date of the *single configuration calculation* (see
section_single_configuration_calculation) as time since the *Unix epoch* (00:00:00
UTC on 1 January 1970) in seconds. For date and times without a timezone, the
default timezone GMT is used."""^^xsd:string ;
    rdfs:subClassOf [ a owl:Restriction ;
            owl:onProperty :hasCategory ;
            owl:someValuesFrom :time_info ],
        [ a owl:Restriction ;
            owl:hasValue 0 ;
            owl:onProperty :hasNumberOfDimensions ],
        [ a owl:Restriction ;
            owl:onProperty :hasCategory ;
            owl:someValuesFrom :accessory_info ],
        [ a owl:Restriction ;
            owl:allValuesFrom <http://emmo.info/emmo/middle/math#EMMO_18d180e4_5e3e_42f7_820c_e08951223486> ;
            owl:onProperty :hasDatatype ],
        [ a owl:Restriction ;
            owl:allValuesFrom <http://emmo.info/emmo/middle/siunits#EMMO_314ba716_2d3d_4462_9a4f_d3419ae1df43> ;
            owl:onProperty <http://emmo.info/emmo/middle/metrology#EMMO_67fc0a36_8dcb_4ffa_9a43_31074efa3296> ],
        :NMI_quantity .

:time_single_configuration_calculation_wall_end a owl:Class ;
    rdfs:comment """Stores the internal wall-clock time at the end of the *single configuration
calculation* (see section_single_configuration_calculation)."""^^xsd:string ;
    rdfs:subClassOf [ a owl:Restriction ;
            owl:hasValue 0 ;
            owl:onProperty :hasNumberOfDimensions ],
        [ a owl:Restriction ;
            owl:allValuesFrom <http://emmo.info/emmo/middle/siunits#EMMO_314ba716_2d3d_4462_9a4f_d3419ae1df43> ;
            owl:onProperty <http://emmo.info/emmo/middle/metrology#EMMO_67fc0a36_8dcb_4ffa_9a43_31074efa3296> ],
        [ a owl:Restriction ;
            owl:allValuesFrom <http://emmo.info/emmo/middle/math#EMMO_18d180e4_5e3e_42f7_820c_e08951223486> ;
            owl:onProperty :hasDatatype ],
        [ a owl:Restriction ;
            owl:onProperty :hasCategory ;
            owl:someValuesFrom :time_info ],
        [ a owl:Restriction ;
            owl:onProperty :hasCategory ;
            owl:someValuesFrom :accessory_info ],
        :NMI_quantity .

:time_single_configuration_calculation_wall_start a owl:Class ;
    rdfs:comment """Stores the internal wall-clock time from the start of the *single configuration
calculation* (see section_single_configuration_calculation)."""^^xsd:string ;
    rdfs:subClassOf [ a owl:Restriction ;
            owl:onProperty :hasCategory ;
            owl:someValuesFrom :time_info ],
        [ a owl:Restriction ;
            owl:allValuesFrom <http://emmo.info/emmo/middle/siunits#EMMO_314ba716_2d3d_4462_9a4f_d3419ae1df43> ;
            owl:onProperty <http://emmo.info/emmo/middle/metrology#EMMO_67fc0a36_8dcb_4ffa_9a43_31074efa3296> ],
        [ a owl:Restriction ;
            owl:onProperty :hasCategory ;
            owl:someValuesFrom :accessory_info ],
        [ a owl:Restriction ;
            owl:allValuesFrom <http://emmo.info/emmo/middle/math#EMMO_18d180e4_5e3e_42f7_820c_e08951223486> ;
            owl:onProperty :hasDatatype ],
        [ a owl:Restriction ;
            owl:hasValue 0 ;
            owl:onProperty :hasNumberOfDimensions ],
        :NMI_quantity .

:topology_force_field_name a owl:Class ;
    rdfs:comment """A unique string idenfiying the force field defined in this section. Strategies to
define it are discussed in the
[topology\\_force\\_field\\_name](https://gitlab.mpcdf.mpg.de/nomad-lab/nomad-meta-
info/wikis/metainfo/topology-force-field-name)."""^^xsd:string ;
    rdfs:subClassOf [ a owl:Restriction ;
            owl:allValuesFrom <http://emmo.info/emmo/middle/perceptual#EMMO_50ea1ec5_f157_41b0_b46b_a9032f17ca10> ;
            owl:onProperty :hasDatatype ],
        [ a owl:Restriction ;
            owl:hasValue 0 ;
            owl:onProperty :hasNumberOfDimensions ],
        :NMI_quantity .

:topology_ref a owl:Class ;
    rdfs:comment """Reference to the topology used for this system; if not given, the trivial topology
should be assumed."""^^xsd:string ;
    rdfs:subClassOf [ a owl:Restriction ;
            owl:hasValue 0 ;
            owl:onProperty :hasNumberOfDimensions ],
        :NMI_quantity .

:total_charge a owl:Class ;
    rdfs:comment "Provides the total amount of charge of the system in a run."^^xsd:string ;
    rdfs:subClassOf [ a owl:Restriction ;
            owl:allValuesFrom <http://emmo.info/emmo/middle/math#EMMO_f8bd64d5_5d3e_4ad4_a46e_c30714fecb7f> ;
            owl:onProperty :hasDatatype ],
        [ a owl:Restriction ;
            owl:allValuesFrom <http://emmo.info/emmo/middle/siunits#EMMO_696ed548_9477_45ea_993c_6a8f5271914a> ;
            owl:onProperty <http://emmo.info/emmo/middle/metrology#EMMO_67fc0a36_8dcb_4ffa_9a43_31074efa3296> ],
        [ a owl:Restriction ;
            owl:hasValue 0 ;
            owl:onProperty :hasNumberOfDimensions ],
        :NMI_quantity .

:transformation_matrix a owl:Class ;
    rdfs:comment """Matrix $\\mathbf{P}$ that is used to transform the standardized coordinates to the
original coordinates. Together with the vector $\\mathbf{p}$, found in
space_group_3D_origin_shift, the transformation between the standardized
coordinates $\\mathbf{x}_s$ and original coordinates $\\mathbf{x}$ is then given by
$\\mathbf{x}_s = \\mathbf{P} \\mathbf{x} + \\mathbf{p}$."""^^xsd:string ;
    rdfs:subClassOf [ a owl:Restriction ;
            owl:allValuesFrom <http://emmo.info/emmo/middle/math#EMMO_18d180e4_5e3e_42f7_820c_e08951223486> ;
            owl:onProperty :hasDatatype ],
        [ a owl:Restriction ;
            owl:hasValue 2 ;
            owl:onProperty :hasNumberOfDimensions ],
        [ a owl:Restriction ;
            owl:hasValue 3 ;
            owl:onProperty :hasFixDim2 ],
        [ a owl:Restriction ;
            owl:hasValue 3 ;
            owl:onProperty :hasFixDim1 ],
        :NMI_quantity .

:transition_dipole_moments a owl:Class ;
    rdfs:comment "Transition dipole moments."^^xsd:string ;
    rdfs:subClassOf [ a owl:Restriction ;
            owl:allValuesFrom <http://emmo.info/emmo/middle/math#EMMO_18d180e4_5e3e_42f7_820c_e08951223486> ;
            owl:onProperty :hasDatatype ],
        [ a owl:Restriction ;
            owl:hasValue 3 ;
            owl:onProperty :hasFixDim2 ],
        [ a owl:Restriction ;
            owl:hasValue 2 ;
            owl:onProperty :hasNumberOfDimensions ],
        [ a owl:Restriction ;
            owl:hasValue :number_of_excited_states ;
            owl:onProperty :hasVarDim1 ],
        :NMI_quantity .

:type a owl:Class ;
    rdfs:comment "Type of band gap."^^xsd:string ;
    rdfs:subClassOf [ a owl:Restriction ;
            owl:hasValue 0 ;
            owl:onProperty :hasNumberOfDimensions ],
        :NMI_quantity .

:valence_band_max_energy a owl:Class ;
    rdfs:comment "Valence band maximum energy."^^xsd:string ;
    rdfs:subClassOf [ a owl:Restriction ;
            owl:allValuesFrom <http://emmo.info/emmo/middle/siunits#EMMO_8a70dea4_d6ab_4260_b931_a3e990982416> ;
            owl:onProperty <http://emmo.info/emmo/middle/metrology#EMMO_67fc0a36_8dcb_4ffa_9a43_31074efa3296> ],
        [ a owl:Restriction ;
            owl:allValuesFrom <http://emmo.info/emmo/middle/math#EMMO_18d180e4_5e3e_42f7_820c_e08951223486> ;
            owl:onProperty :hasDatatype ],
        [ a owl:Restriction ;
            owl:hasValue 0 ;
            owl:onProperty :hasNumberOfDimensions ],
        :NMI_quantity .

:valence_band_max_k_point a owl:Class ;
    rdfs:comment "Coordinate of the valence band minimum in k-space."^^xsd:string ;
    rdfs:subClassOf [ a owl:Restriction ;
            owl:allValuesFrom <https://nomad-coe.eu/ontology/properties#PerMetre> ;
            owl:onProperty <http://emmo.info/emmo/middle/metrology#EMMO_67fc0a36_8dcb_4ffa_9a43_31074efa3296> ],
        [ a owl:Restriction ;
            owl:hasValue 1 ;
            owl:onProperty :hasNumberOfDimensions ],
        [ a owl:Restriction ;
            owl:allValuesFrom <http://emmo.info/emmo/middle/math#EMMO_18d180e4_5e3e_42f7_820c_e08951223486> ;
            owl:onProperty :hasDatatype ],
        [ a owl:Restriction ;
            owl:hasValue 3 ;
            owl:onProperty :hasFixDim1 ],
        :NMI_quantity .

:value a owl:Class ;
    rdfs:comment """Band gap energy. Value of zero corresponds to a band structure without
a band gap."""^^xsd:string ;
    rdfs:subClassOf [ a owl:Restriction ;
            owl:hasValue 0 ;
            owl:onProperty :hasNumberOfDimensions ],
        [ a owl:Restriction ;
            owl:allValuesFrom <http://emmo.info/emmo/middle/math#EMMO_18d180e4_5e3e_42f7_820c_e08951223486> ;
            owl:onProperty :hasDatatype ],
        [ a owl:Restriction ;
            owl:allValuesFrom <http://emmo.info/emmo/middle/siunits#EMMO_8a70dea4_d6ab_4260_b931_a3e990982416> ;
            owl:onProperty <http://emmo.info/emmo/middle/metrology#EMMO_67fc0a36_8dcb_4ffa_9a43_31074efa3296> ],
        :NMI_quantity .

:van_der_Waals_method a owl:Class ;
    rdfs:comment """Describes the Van der Waals method. If skipped or an empty string is used, it
means no Van der Waals correction is applied.

Allowed values are:

| Van der Waals method  | Description                               |

| --------------------- | ----------------------------------------- |

| `""`                  | No Van der Waals correction               |

| `"TS"`                | A. Tkatchenko and M. Scheffler, [Phys. Rev. Lett.
**102**, 073005 (2009)](http://dx.doi.org/10.1103/PhysRevLett.102.073005) |

| `"OBS"`               | F. Ortmann, F. Bechstedt, and W. G. Schmidt, [Phys. Rev.
B **73**, 205101 (2006)](http://dx.doi.org/10.1103/PhysRevB.73.205101) |

| `"G06"`               | S. Grimme, [J. Comput. Chem. **27**, 1787
(2006)](http://dx.doi.org/10.1002/jcc.20495) |

| `"JCHS"`              | P. Jurečka, J. Černý, P. Hobza, and D. R. Salahub,
[Journal of Computational Chemistry **28**, 555
(2007)](http://dx.doi.org/10.1002/jcc.20570) |

| `"MDB"`               | Many-body dispersion. A. Tkatchenko, R. A. Di Stasio Jr,
R. Car, and M. Scheffler, [Physical Review Letters **108**, 236402
(2012)](http://dx.doi.org/10.1103/PhysRevLett.108.236402) and A. Ambrosetti, A. M.
Reilly, R. A. Di Stasio Jr, and A. Tkatchenko, [The Journal of Chemical Physics
**140**, 18A508 (2014)](http://dx.doi.org/10.1063/1.4865104) |

| `"XC"`                | The method to calculate the Van der Waals energy uses a
non-local functional which is described in section_XC_functionals. |"""^^xsd:string ;
    rdfs:subClassOf [ a owl:Restriction ;
            owl:onProperty :hasCategory ;
            owl:someValuesFrom :settings_potential_energy_surface ],
        [ a owl:Restriction ;
            owl:onProperty :hasCategory ;
            owl:someValuesFrom :settings_XC ],
        [ a owl:Restriction ;
            owl:onProperty :hasCategory ;
            owl:someValuesFrom :settings_van_der_Waals ],
        [ a owl:Restriction ;
            owl:hasValue 0 ;
            owl:onProperty :hasNumberOfDimensions ],
        [ a owl:Restriction ;
            owl:allValuesFrom <http://emmo.info/emmo/middle/perceptual#EMMO_50ea1ec5_f157_41b0_b46b_a9032f17ca10> ;
            owl:onProperty :hasDatatype ],
        :NMI_quantity .

:vertices a owl:Class ;
    rdfs:comment "The vertices of the Brillouin zone corners as 3D coordinates in reciprocal space."^^xsd:string ;
    rdfs:subClassOf [ a owl:Restriction ;
            owl:hasValue 2 ;
            owl:onProperty :hasNumberOfDimensions ],
        [ a owl:Restriction ;
            owl:hasValue 3 ;
            owl:onProperty :hasFixDim1 ],
        [ a owl:Restriction ;
            owl:allValuesFrom <http://emmo.info/emmo/middle/math#EMMO_18d180e4_5e3e_42f7_820c_e08951223486> ;
            owl:onProperty :hasDatatype ],
        :NMI_quantity .

:vibrational_free_energy_at_constant_volume a owl:Class ;
    rdfs:comment "Holds the vibrational free energy per atom at constant volume."^^xsd:string ;
    rdfs:subClassOf [ a owl:Restriction ;
            owl:hasValue :number_of_thermodynamical_property_values ;
            owl:onProperty :hasVarDim1 ],
        [ a owl:Restriction ;
            owl:allValuesFrom <http://emmo.info/emmo/middle/math#EMMO_18d180e4_5e3e_42f7_820c_e08951223486> ;
            owl:onProperty :hasDatatype ],
        [ a owl:Restriction ;
            owl:allValuesFrom <http://emmo.info/emmo/middle/siunits#EMMO_8a70dea4_d6ab_4260_b931_a3e990982416> ;
            owl:onProperty <http://emmo.info/emmo/middle/metrology#EMMO_67fc0a36_8dcb_4ffa_9a43_31074efa3296> ],
        [ a owl:Restriction ;
            owl:hasValue 1 ;
            owl:onProperty :hasNumberOfDimensions ],
        :NMI_quantity .

:volumetric_data_displacements a owl:Class ;
    rdfs:comment """displacement vectors between grid points along each axis; same indexing rules as
lattice_vectors.  In many cases, displacements and number of points are related to
lattice_vectors through: [displacement] * [number of points + N] =
[lattice_vector],where N is 1 for periodic directions and 0 for non-periodic ones"""^^xsd:string ;
    rdfs:subClassOf [ a owl:Restriction ;
            owl:hasValue 3 ;
            owl:onProperty :hasFixDim1 ],
        [ a owl:Restriction ;
            owl:hasValue 2 ;
            owl:onProperty :hasNumberOfDimensions ],
        [ a owl:Restriction ;
            owl:hasValue 3 ;
            owl:onProperty :hasFixDim2 ],
        [ a owl:Restriction ;
            owl:allValuesFrom <http://emmo.info/emmo/middle/siunits#EMMO_7db11dbf_a643_464a_9b56_07eabcc3e9c5> ;
            owl:onProperty <http://emmo.info/emmo/middle/metrology#EMMO_67fc0a36_8dcb_4ffa_9a43_31074efa3296> ],
        [ a owl:Restriction ;
            owl:allValuesFrom <http://emmo.info/emmo/middle/math#EMMO_18d180e4_5e3e_42f7_820c_e08951223486> ;
            owl:onProperty :hasDatatype ],
        :NMI_quantity .

:volumetric_data_kind a owl:Class ;
    rdfs:comment """The kind of function, e.g. density, potential_hartree, potential_effective.  The
unit of measurement for "volumetric_data_values" depends on the kind: Densities
are 1/m^3 and potentials are J/m^3.  See [full specification on the
wiki](https://gitlab.mpcdf.mpg.de/nomad-lab/nomad-meta-
info/wikis/metainfo/volumetric-data)."""^^xsd:string ;
    rdfs:subClassOf [ a owl:Restriction ;
            owl:allValuesFrom <http://emmo.info/emmo/middle/perceptual#EMMO_50ea1ec5_f157_41b0_b46b_a9032f17ca10> ;
            owl:onProperty :hasDatatype ],
        [ a owl:Restriction ;
            owl:hasValue 0 ;
            owl:onProperty :hasNumberOfDimensions ],
        :NMI_quantity .

:volumetric_data_origin a owl:Class ;
    rdfs:comment """location of the first grid point; same coordinate system as atom_positions when
applicable."""^^xsd:string ;
    rdfs:subClassOf [ a owl:Restriction ;
            owl:hasValue 3 ;
            owl:onProperty :hasFixDim1 ],
        [ a owl:Restriction ;
            owl:hasValue 1 ;
            owl:onProperty :hasNumberOfDimensions ],
        [ a owl:Restriction ;
            owl:allValuesFrom <http://emmo.info/emmo/middle/math#EMMO_18d180e4_5e3e_42f7_820c_e08951223486> ;
            owl:onProperty :hasDatatype ],
        :NMI_quantity .

:volumetric_data_values a owl:Class ;
    rdfs:comment """Array of shape (multiplicity, nx, ny, nz) containing the values.  The units of
these values depend on which kind of data the values represent; see
"volumetric_data_kind"."""^^xsd:string ;
    rdfs:subClassOf [ a owl:Restriction ;
            owl:hasValue :volumetric_data_nx ;
            owl:onProperty :hasVarDim2 ],
        [ a owl:Restriction ;
            owl:hasValue :volumetric_data_nz ;
            owl:onProperty :hasVarDim4 ],
        [ a owl:Restriction ;
            owl:allValuesFrom <http://emmo.info/emmo/middle/math#EMMO_18d180e4_5e3e_42f7_820c_e08951223486> ;
            owl:onProperty :hasDatatype ],
        [ a owl:Restriction ;
            owl:hasValue :volumetric_data_ny ;
            owl:onProperty :hasVarDim3 ],
        [ a owl:Restriction ;
            owl:hasValue 4 ;
            owl:onProperty :hasNumberOfDimensions ],
        [ a owl:Restriction ;
            owl:hasValue :volumetric_data_multiplicity ;
            owl:onProperty :hasVarDim1 ],
        :NMI_quantity .

:wyckoff_letters_original a owl:Class ;
    rdfs:comment "Wyckoff letters for atoms in the original cell."^^xsd:string ;
    rdfs:subClassOf [ a owl:Restriction ;
            owl:hasValue 1 ;
            owl:onProperty :hasNumberOfDimensions ],
        [ a owl:Restriction ;
            owl:allValuesFrom <http://emmo.info/emmo/middle/perceptual#EMMO_50ea1ec5_f157_41b0_b46b_a9032f17ca10> ;
            owl:onProperty :hasDatatype ],
        [ a owl:Restriction ;
            owl:hasValue :number_of_atoms ;
            owl:onProperty :hasVarDim1 ],
        :NMI_quantity .

:wyckoff_letters_primitive a owl:Class ;
    rdfs:comment "Wyckoff letters for atoms in the primitive cell."^^xsd:string ;
    rdfs:subClassOf [ a owl:Restriction ;
            owl:hasValue :number_of_atoms_primitive ;
            owl:onProperty :hasVarDim1 ],
        [ a owl:Restriction ;
            owl:allValuesFrom <http://emmo.info/emmo/middle/perceptual#EMMO_50ea1ec5_f157_41b0_b46b_a9032f17ca10> ;
            owl:onProperty :hasDatatype ],
        [ a owl:Restriction ;
            owl:hasValue 1 ;
            owl:onProperty :hasNumberOfDimensions ],
        :NMI_quantity .

:wyckoff_letters_std a owl:Class ;
    rdfs:comment "Wyckoff letters for atoms in the standardized cell."^^xsd:string ;
    rdfs:subClassOf [ a owl:Restriction ;
            owl:hasValue 1 ;
            owl:onProperty :hasNumberOfDimensions ],
        [ a owl:Restriction ;
            owl:allValuesFrom <http://emmo.info/emmo/middle/perceptual#EMMO_50ea1ec5_f157_41b0_b46b_a9032f17ca10> ;
            owl:onProperty :hasDatatype ],
        [ a owl:Restriction ;
            owl:hasValue :number_of_atoms_std ;
            owl:onProperty :hasVarDim1 ],
        :NMI_quantity .

:zero_point_method a owl:Class ;
    rdfs:comment """Describes the zero-point vibrations method. If skipped or an empty string is used,
it means no zero-point vibrations correction is applied."""^^xsd:string ;
    rdfs:subClassOf [ a owl:Restriction ;
            owl:allValuesFrom <http://emmo.info/emmo/middle/perceptual#EMMO_50ea1ec5_f157_41b0_b46b_a9032f17ca10> ;
            owl:onProperty :hasDatatype ],
        [ a owl:Restriction ;
            owl:hasValue 0 ;
            owl:onProperty :hasNumberOfDimensions ],
        :NMI_quantity .

:energy_type_C a owl:Class ;
    rdfs:comment "This metadata stores the correlation (C) energy."^^xsd:string ;
    rdfs:subClassOf :energy_component .

:energy_type_XC a owl:Class ;
    rdfs:comment "This metadata stores the exchange-correlation (XC) energy."^^xsd:string ;
    rdfs:subClassOf :energy_component .

:energy_type_van_der_Waals a owl:Class ;
    rdfs:comment "This metadata stores the converged van der Waals energy."^^xsd:string ;
    rdfs:subClassOf :energy_component .

:message_error a owl:Class ;
    rdfs:comment "An error message of the computational program."^^xsd:string ;
    rdfs:subClassOf :message_warning .

:number_of_atoms_per_constraint a owl:Class ;
    rdfs:comment "Number of atoms involved in this constraint."^^xsd:string ;
    rdfs:subClassOf [ a owl:Restriction ;
            owl:hasValue 0 ;
            owl:onProperty :hasNumberOfDimensions ],
        [ a owl:Restriction ;
            owl:allValuesFrom <http://emmo.info/emmo/middle/math#EMMO_f8bd64d5_5d3e_4ad4_a46e_c30714fecb7f> ;
            owl:onProperty :hasDatatype ],
        [ a owl:Restriction ;
            owl:allValuesFrom <http://emmo.info/emmo/middle/math#EMMO_f8bd64d5_5d3e_4ad4_a46e_c30714fecb7f> ;
            owl:onProperty <http://emmo.info/emmo/middle/metrology#EMMO_67fc0a36_8dcb_4ffa_9a43_31074efa3296> ],
        :NMI_dimension,
        :NMI_quantity .

:number_of_atoms_per_interaction a owl:Class ;
    rdfs:comment "Number of atoms involved in this interaction."^^xsd:string ;
    rdfs:subClassOf [ a owl:Restriction ;
            owl:allValuesFrom <http://emmo.info/emmo/middle/math#EMMO_f8bd64d5_5d3e_4ad4_a46e_c30714fecb7f> ;
            owl:onProperty :hasDatatype ],
        [ a owl:Restriction ;
            owl:allValuesFrom <http://emmo.info/emmo/middle/math#EMMO_f8bd64d5_5d3e_4ad4_a46e_c30714fecb7f> ;
            owl:onProperty <http://emmo.info/emmo/middle/metrology#EMMO_67fc0a36_8dcb_4ffa_9a43_31074efa3296> ],
        [ a owl:Restriction ;
            owl:hasValue 0 ;
            owl:onProperty :hasNumberOfDimensions ],
        :NMI_dimension,
        :NMI_quantity .

:number_of_atoms_per_molecule_constraint a owl:Class ;
    rdfs:comment "Number of atoms, in this molecule, involved in this constraint."^^xsd:string ;
    rdfs:subClassOf [ a owl:Restriction ;
            owl:allValuesFrom <http://emmo.info/emmo/middle/math#EMMO_f8bd64d5_5d3e_4ad4_a46e_c30714fecb7f> ;
            owl:onProperty :hasDatatype ],
        [ a owl:Restriction ;
            owl:hasValue 0 ;
            owl:onProperty :hasNumberOfDimensions ],
        [ a owl:Restriction ;
            owl:allValuesFrom <http://emmo.info/emmo/middle/math#EMMO_f8bd64d5_5d3e_4ad4_a46e_c30714fecb7f> ;
            owl:onProperty <http://emmo.info/emmo/middle/metrology#EMMO_67fc0a36_8dcb_4ffa_9a43_31074efa3296> ],
        :NMI_dimension,
        :NMI_quantity .

:number_of_atoms_per_molecule_interaction a owl:Class ;
    rdfs:comment "Number of atoms, in this molecule, involved in this interaction."^^xsd:string ;
    rdfs:subClassOf [ a owl:Restriction ;
            owl:hasValue 0 ;
            owl:onProperty :hasNumberOfDimensions ],
        [ a owl:Restriction ;
            owl:allValuesFrom <http://emmo.info/emmo/middle/math#EMMO_f8bd64d5_5d3e_4ad4_a46e_c30714fecb7f> ;
            owl:onProperty :hasDatatype ],
        [ a owl:Restriction ;
            owl:allValuesFrom <http://emmo.info/emmo/middle/math#EMMO_f8bd64d5_5d3e_4ad4_a46e_c30714fecb7f> ;
            owl:onProperty <http://emmo.info/emmo/middle/metrology#EMMO_67fc0a36_8dcb_4ffa_9a43_31074efa3296> ],
        :NMI_dimension,
        :NMI_quantity .

:number_of_basis_sets_atom_centered a owl:Class ;
    rdfs:comment """String describing the use of the basis set, i.e, if it used for expanding a
wavefunction or an electron density. Allowed values are listed in the
[basis\\_set\\_kind wiki page](https://gitlab.mpcdf.mpg.de/nomad-lab/nomad-meta-
info/wikis/metainfo/basis-set-kind)."""^^xsd:string ;
    rdfs:subClassOf [ a owl:Restriction ;
            owl:allValuesFrom <http://emmo.info/emmo/middle/math#EMMO_f8bd64d5_5d3e_4ad4_a46e_c30714fecb7f> ;
            owl:onProperty :hasDatatype ],
        [ a owl:Restriction ;
            owl:allValuesFrom <http://emmo.info/emmo/middle/math#EMMO_f8bd64d5_5d3e_4ad4_a46e_c30714fecb7f> ;
            owl:onProperty <http://emmo.info/emmo/middle/metrology#EMMO_67fc0a36_8dcb_4ffa_9a43_31074efa3296> ],
        [ a owl:Restriction ;
            owl:hasValue 0 ;
            owl:onProperty :hasNumberOfDimensions ],
        :NMI_dimension,
        :NMI_quantity .

:number_of_constraints a owl:Class ;
    rdfs:comment "Number of constraints of this type."^^xsd:string ;
    rdfs:subClassOf [ a owl:Restriction ;
            owl:allValuesFrom <http://emmo.info/emmo/middle/math#EMMO_f8bd64d5_5d3e_4ad4_a46e_c30714fecb7f> ;
            owl:onProperty :hasDatatype ],
        [ a owl:Restriction ;
            owl:hasValue 0 ;
            owl:onProperty :hasNumberOfDimensions ],
        [ a owl:Restriction ;
            owl:allValuesFrom <http://emmo.info/emmo/middle/math#EMMO_f8bd64d5_5d3e_4ad4_a46e_c30714fecb7f> ;
            owl:onProperty <http://emmo.info/emmo/middle/metrology#EMMO_67fc0a36_8dcb_4ffa_9a43_31074efa3296> ],
        :NMI_dimension,
        :NMI_quantity .

:number_of_interactions a owl:Class ;
    rdfs:comment "Number of interactions of this type."^^xsd:string ;
    rdfs:subClassOf [ a owl:Restriction ;
            owl:allValuesFrom <http://emmo.info/emmo/middle/math#EMMO_f8bd64d5_5d3e_4ad4_a46e_c30714fecb7f> ;
            owl:onProperty <http://emmo.info/emmo/middle/metrology#EMMO_67fc0a36_8dcb_4ffa_9a43_31074efa3296> ],
        [ a owl:Restriction ;
            owl:allValuesFrom <http://emmo.info/emmo/middle/math#EMMO_f8bd64d5_5d3e_4ad4_a46e_c30714fecb7f> ;
            owl:onProperty :hasDatatype ],
        [ a owl:Restriction ;
            owl:hasValue 0 ;
            owl:onProperty :hasNumberOfDimensions ],
        :NMI_dimension,
        :NMI_quantity .

:number_of_molecule_constraints a owl:Class ;
    rdfs:comment "Number of constraints of this type."^^xsd:string ;
    rdfs:subClassOf [ a owl:Restriction ;
            owl:allValuesFrom <http://emmo.info/emmo/middle/math#EMMO_f8bd64d5_5d3e_4ad4_a46e_c30714fecb7f> ;
            owl:onProperty <http://emmo.info/emmo/middle/metrology#EMMO_67fc0a36_8dcb_4ffa_9a43_31074efa3296> ],
        [ a owl:Restriction ;
            owl:hasValue 0 ;
            owl:onProperty :hasNumberOfDimensions ],
        [ a owl:Restriction ;
            owl:allValuesFrom <http://emmo.info/emmo/middle/math#EMMO_f8bd64d5_5d3e_4ad4_a46e_c30714fecb7f> ;
            owl:onProperty :hasDatatype ],
        :NMI_dimension,
        :NMI_quantity .

:number_of_molecule_interactions a owl:Class ;
    rdfs:comment "Number of bonded interactions of this type."^^xsd:string ;
    rdfs:subClassOf [ a owl:Restriction ;
            owl:allValuesFrom <http://emmo.info/emmo/middle/math#EMMO_f8bd64d5_5d3e_4ad4_a46e_c30714fecb7f> ;
            owl:onProperty <http://emmo.info/emmo/middle/metrology#EMMO_67fc0a36_8dcb_4ffa_9a43_31074efa3296> ],
        [ a owl:Restriction ;
            owl:hasValue 0 ;
            owl:onProperty :hasNumberOfDimensions ],
        [ a owl:Restriction ;
            owl:allValuesFrom <http://emmo.info/emmo/middle/math#EMMO_f8bd64d5_5d3e_4ad4_a46e_c30714fecb7f> ;
            owl:onProperty :hasDatatype ],
        :NMI_dimension,
        :NMI_quantity .

:number_of_sites a owl:Class ;
    rdfs:comment """number of sites in a variable composition representation. By default (no variable
composition) it is the same as number_of_atoms."""^^xsd:string ;
    rdfs:subClassOf [ a owl:Restriction ;
            owl:hasValue 0 ;
            owl:onProperty :hasNumberOfDimensions ],
        [ a owl:Restriction ;
            owl:allValuesFrom <http://emmo.info/emmo/middle/math#EMMO_f8bd64d5_5d3e_4ad4_a46e_c30714fecb7f> ;
            owl:onProperty <http://emmo.info/emmo/middle/metrology#EMMO_67fc0a36_8dcb_4ffa_9a43_31074efa3296> ],
        [ a owl:Restriction ;
            owl:allValuesFrom <http://emmo.info/emmo/middle/math#EMMO_f8bd64d5_5d3e_4ad4_a46e_c30714fecb7f> ;
            owl:onProperty :hasDatatype ],
        :NMI_dimension,
        :NMI_quantity .

:number_of_soap_coefficients a owl:Class ;
    rdfs:comment "number of soap coefficients"^^xsd:string ;
    rdfs:subClassOf [ a owl:Restriction ;
            owl:allValuesFrom <http://emmo.info/emmo/middle/math#EMMO_f8bd64d5_5d3e_4ad4_a46e_c30714fecb7f> ;
            owl:onProperty :hasDatatype ],
        [ a owl:Restriction ;
            owl:allValuesFrom <http://emmo.info/emmo/middle/math#EMMO_f8bd64d5_5d3e_4ad4_a46e_c30714fecb7f> ;
            owl:onProperty <http://emmo.info/emmo/middle/metrology#EMMO_67fc0a36_8dcb_4ffa_9a43_31074efa3296> ],
        [ a owl:Restriction ;
            owl:hasValue 0 ;
            owl:onProperty :hasNumberOfDimensions ],
        :NMI_dimension,
        :NMI_quantity .

:number_of_topology_atoms a owl:Class ;
    rdfs:comment "Number of atoms in the system described by this topology."^^xsd:string ;
    rdfs:subClassOf [ a owl:Restriction ;
            owl:allValuesFrom <http://emmo.info/emmo/middle/math#EMMO_f8bd64d5_5d3e_4ad4_a46e_c30714fecb7f> ;
            owl:onProperty :hasDatatype ],
        [ a owl:Restriction ;
            owl:hasValue 0 ;
            owl:onProperty :hasNumberOfDimensions ],
        [ a owl:Restriction ;
            owl:allValuesFrom <http://emmo.info/emmo/middle/math#EMMO_f8bd64d5_5d3e_4ad4_a46e_c30714fecb7f> ;
            owl:onProperty <http://emmo.info/emmo/middle/metrology#EMMO_67fc0a36_8dcb_4ffa_9a43_31074efa3296> ],
        :NMI_dimension,
        :NMI_quantity .

:number_of_topology_molecules a owl:Class ;
    rdfs:comment "Number of molecules in the system, as described by this topology."^^xsd:string ;
    rdfs:subClassOf [ a owl:Restriction ;
            owl:allValuesFrom <http://emmo.info/emmo/middle/math#EMMO_f8bd64d5_5d3e_4ad4_a46e_c30714fecb7f> ;
            owl:onProperty :hasDatatype ],
        [ a owl:Restriction ;
            owl:hasValue 0 ;
            owl:onProperty :hasNumberOfDimensions ],
        [ a owl:Restriction ;
            owl:allValuesFrom <http://emmo.info/emmo/middle/math#EMMO_f8bd64d5_5d3e_4ad4_a46e_c30714fecb7f> ;
            owl:onProperty <http://emmo.info/emmo/middle/metrology#EMMO_67fc0a36_8dcb_4ffa_9a43_31074efa3296> ],
        :NMI_dimension,
        :NMI_quantity .

:parsing_message_error a owl:Class ;
    rdfs:comment "This field is used for error messages of the parsing program."^^xsd:string ;
    rdfs:subClassOf :parsing_message_warning .

:settings_scf a owl:Class ;
    rdfs:comment """Contains parameters connected with the convergence of the self-consistent field (SCF)
iterations."""^^xsd:string ;
    rdfs:subClassOf :NMI_category .

:settings_smearing a owl:Class ;
    rdfs:comment """Contain parameters that control the smearing of the orbital occupation at finite
electronic temperatures."""^^xsd:string ;
    rdfs:subClassOf :NMI_category .

:stress_tensor_type a owl:Class ;
    rdfs:comment """Contains the final value of the default stress tensor (stress_tensor) and/or the value
of the stress tensor (stress_tensor_value) of the kind defined in stress_tensor_kind."""^^xsd:string ;
    rdfs:subClassOf :NMI_category .

:volumetric_data_multiplicity a owl:Class ;
    rdfs:comment "number of functions stored"^^xsd:string ;
    rdfs:subClassOf [ a owl:Restriction ;
            owl:allValuesFrom <http://emmo.info/emmo/middle/math#EMMO_f8bd64d5_5d3e_4ad4_a46e_c30714fecb7f> ;
            owl:onProperty <http://emmo.info/emmo/middle/metrology#EMMO_67fc0a36_8dcb_4ffa_9a43_31074efa3296> ],
        [ a owl:Restriction ;
            owl:hasValue 0 ;
            owl:onProperty :hasNumberOfDimensions ],
        [ a owl:Restriction ;
            owl:allValuesFrom <http://emmo.info/emmo/middle/math#EMMO_f8bd64d5_5d3e_4ad4_a46e_c30714fecb7f> ;
            owl:onProperty :hasDatatype ],
        :NMI_dimension,
        :NMI_quantity .

:volumetric_data_nx a owl:Class ;
    rdfs:comment "number of points along x axis"^^xsd:string ;
    rdfs:subClassOf [ a owl:Restriction ;
            owl:allValuesFrom <http://emmo.info/emmo/middle/math#EMMO_f8bd64d5_5d3e_4ad4_a46e_c30714fecb7f> ;
            owl:onProperty <http://emmo.info/emmo/middle/metrology#EMMO_67fc0a36_8dcb_4ffa_9a43_31074efa3296> ],
        [ a owl:Restriction ;
            owl:allValuesFrom <http://emmo.info/emmo/middle/math#EMMO_f8bd64d5_5d3e_4ad4_a46e_c30714fecb7f> ;
            owl:onProperty :hasDatatype ],
        [ a owl:Restriction ;
            owl:hasValue 0 ;
            owl:onProperty :hasNumberOfDimensions ],
        :NMI_dimension,
        :NMI_quantity .

:volumetric_data_ny a owl:Class ;
    rdfs:comment "number of points along y axis"^^xsd:string ;
    rdfs:subClassOf [ a owl:Restriction ;
            owl:hasValue 0 ;
            owl:onProperty :hasNumberOfDimensions ],
        [ a owl:Restriction ;
            owl:allValuesFrom <http://emmo.info/emmo/middle/math#EMMO_f8bd64d5_5d3e_4ad4_a46e_c30714fecb7f> ;
            owl:onProperty <http://emmo.info/emmo/middle/metrology#EMMO_67fc0a36_8dcb_4ffa_9a43_31074efa3296> ],
        [ a owl:Restriction ;
            owl:allValuesFrom <http://emmo.info/emmo/middle/math#EMMO_f8bd64d5_5d3e_4ad4_a46e_c30714fecb7f> ;
            owl:onProperty :hasDatatype ],
        :NMI_dimension,
        :NMI_quantity .

:volumetric_data_nz a owl:Class ;
    rdfs:comment "number of points along z axis"^^xsd:string ;
    rdfs:subClassOf [ a owl:Restriction ;
            owl:hasValue 0 ;
            owl:onProperty :hasNumberOfDimensions ],
        [ a owl:Restriction ;
            owl:allValuesFrom <http://emmo.info/emmo/middle/math#EMMO_f8bd64d5_5d3e_4ad4_a46e_c30714fecb7f> ;
            owl:onProperty <http://emmo.info/emmo/middle/metrology#EMMO_67fc0a36_8dcb_4ffa_9a43_31074efa3296> ],
        [ a owl:Restriction ;
            owl:allValuesFrom <http://emmo.info/emmo/middle/math#EMMO_f8bd64d5_5d3e_4ad4_a46e_c30714fecb7f> ;
            owl:onProperty :hasDatatype ],
        :NMI_dimension,
        :NMI_quantity .

:NMI_type a owl:Class ;
    rdfs:subClassOf owl:Thing .

:energy_total_potential_per_atom a owl:Class ;
    rdfs:comment """A value of the total potential energy per atom. Note that a direct comparison may not
be possible because of a difference in the methods for computing total energies and
numerical implementations of various codes might leads to different energy zeros (see
section_energy_code_independent for a code-independent definition of the energy)."""^^xsd:string ;
    rdfs:subClassOf :energy_component .

:energy_type_X a owl:Class ;
    rdfs:comment "This metadata stores the exchange (X) energy."^^xsd:string ;
    rdfs:subClassOf :energy_component .

:hasFixDim3 a owl:DatatypeProperty,
        owl:FunctionalProperty ;
    rdfs:domain :NMI_quantity ;
    rdfs:range [ a rdfs:Datatype ;
            owl:onDatatype xsd:integer ;
            owl:withRestrictions ( [ xsd:minInclusive 1 ] ) ] .

:number_of_band_segment_eigenvalues a owl:Class ;
    rdfs:comment "Gives the number of eigenvalues in a band segment, see band_energies."^^xsd:string ;
    rdfs:subClassOf [ a owl:Restriction ;
            owl:allValuesFrom <http://emmo.info/emmo/middle/math#EMMO_f8bd64d5_5d3e_4ad4_a46e_c30714fecb7f> ;
            owl:onProperty :hasDatatype ],
        [ a owl:Restriction ;
            owl:allValuesFrom <http://emmo.info/emmo/middle/math#EMMO_f8bd64d5_5d3e_4ad4_a46e_c30714fecb7f> ;
            owl:onProperty <http://emmo.info/emmo/middle/metrology#EMMO_67fc0a36_8dcb_4ffa_9a43_31074efa3296> ],
        [ a owl:Restriction ;
            owl:hasValue 0 ;
            owl:onProperty :hasNumberOfDimensions ],
        :NMI_dimension,
        :NMI_quantity .

:number_of_conserved_quantity_evaluations_in_sequence a owl:Class ;
    rdfs:comment """Gives the number of conserved quantity evaluations in this sequence. A sequence is
a trajectory, which can have number_of_frames_in_sequence each representing one
section_single_configuration_calculation section."""^^xsd:string ;
    rdfs:subClassOf [ a owl:Restriction ;
            owl:allValuesFrom <http://emmo.info/emmo/middle/math#EMMO_f8bd64d5_5d3e_4ad4_a46e_c30714fecb7f> ;
            owl:onProperty :hasDatatype ],
        [ a owl:Restriction ;
            owl:allValuesFrom <http://emmo.info/emmo/middle/math#EMMO_f8bd64d5_5d3e_4ad4_a46e_c30714fecb7f> ;
            owl:onProperty <http://emmo.info/emmo/middle/metrology#EMMO_67fc0a36_8dcb_4ffa_9a43_31074efa3296> ],
        [ a owl:Restriction ;
            owl:hasValue 0 ;
            owl:onProperty :hasNumberOfDimensions ],
        :NMI_dimension,
        :NMI_quantity .

:number_of_dos_lms a owl:Class ;
    rdfs:comment """Gives the number of $l$, $m$ combinations for the given projected density of
states (DOS) in dos_values and dos_values_lm."""^^xsd:string ;
    rdfs:subClassOf [ a owl:Restriction ;
            owl:allValuesFrom <http://emmo.info/emmo/middle/math#EMMO_f8bd64d5_5d3e_4ad4_a46e_c30714fecb7f> ;
            owl:onProperty <http://emmo.info/emmo/middle/metrology#EMMO_67fc0a36_8dcb_4ffa_9a43_31074efa3296> ],
        [ a owl:Restriction ;
            owl:hasValue 0 ;
            owl:onProperty :hasNumberOfDimensions ],
        [ a owl:Restriction ;
            owl:allValuesFrom <http://emmo.info/emmo/middle/math#EMMO_f8bd64d5_5d3e_4ad4_a46e_c30714fecb7f> ;
            owl:onProperty :hasDatatype ],
        :NMI_dimension,
        :NMI_quantity .

:number_of_frame_sequence_user_quantity_components a owl:Class ;
    rdfs:comment """Gives the number of user-defined quantity defined by
frame_sequence_user_quantity_name and monitored in a sequence of frames. A
sequence is a trajectory, which can have number_of_frames_in_sequence each
representing one section_single_configuration_calculation section.

Dedicated metadata monitored along a sequence of frames are created for the
conserved energy-like quantity (frame_sequence_conserved_quantity), the kinetic
and potential energies ([frame_sequence_kinetic_energy and
frame_sequence_potential_energy](frame_sequence_kinetic_energy and
frame_sequence_potential_energy)), the instantaneous temperature
(frame_sequence_temperature) and the pressure (frame_sequence_pressure)."""^^xsd:string ;
    rdfs:subClassOf [ a owl:Restriction ;
            owl:hasValue 0 ;
            owl:onProperty :hasNumberOfDimensions ],
        [ a owl:Restriction ;
            owl:allValuesFrom <http://emmo.info/emmo/middle/math#EMMO_f8bd64d5_5d3e_4ad4_a46e_c30714fecb7f> ;
            owl:onProperty <http://emmo.info/emmo/middle/metrology#EMMO_67fc0a36_8dcb_4ffa_9a43_31074efa3296> ],
        [ a owl:Restriction ;
            owl:allValuesFrom <http://emmo.info/emmo/middle/math#EMMO_f8bd64d5_5d3e_4ad4_a46e_c30714fecb7f> ;
            owl:onProperty :hasDatatype ],
        :NMI_dimension,
        :NMI_quantity .

:number_of_frames_in_sequence a owl:Class ;
    rdfs:comment """Gives the number of frames in a sequence. A sequence is a trajectory, which can
have number_of_frames_in_sequence each representing one
section_single_configuration_calculation section."""^^xsd:string ;
    rdfs:subClassOf [ a owl:Restriction ;
            owl:allValuesFrom <http://emmo.info/emmo/middle/math#EMMO_f8bd64d5_5d3e_4ad4_a46e_c30714fecb7f> ;
            owl:onProperty :hasDatatype ],
        [ a owl:Restriction ;
            owl:allValuesFrom <http://emmo.info/emmo/middle/math#EMMO_f8bd64d5_5d3e_4ad4_a46e_c30714fecb7f> ;
            owl:onProperty <http://emmo.info/emmo/middle/metrology#EMMO_67fc0a36_8dcb_4ffa_9a43_31074efa3296> ],
        [ a owl:Restriction ;
            owl:hasValue 0 ;
            owl:onProperty :hasNumberOfDimensions ],
        :NMI_dimension,
        :NMI_quantity .

:number_of_gaussian_basis_group_contractions a owl:Class ;
    rdfs:comment """Gives the number of different contractions, i.e. resulting basis functions in a
section_gaussian_basis_group section."""^^xsd:string ;
    rdfs:subClassOf [ a owl:Restriction ;
            owl:hasValue 0 ;
            owl:onProperty :hasNumberOfDimensions ],
        [ a owl:Restriction ;
            owl:allValuesFrom <http://emmo.info/emmo/middle/math#EMMO_f8bd64d5_5d3e_4ad4_a46e_c30714fecb7f> ;
            owl:onProperty <http://emmo.info/emmo/middle/metrology#EMMO_67fc0a36_8dcb_4ffa_9a43_31074efa3296> ],
        [ a owl:Restriction ;
            owl:allValuesFrom <http://emmo.info/emmo/middle/math#EMMO_f8bd64d5_5d3e_4ad4_a46e_c30714fecb7f> ;
            owl:onProperty :hasDatatype ],
        :NMI_dimension,
        :NMI_quantity .

:number_of_gaussian_basis_group_exponents a owl:Class ;
    rdfs:comment """Gives the number of different Gaussian exponents in a section_gaussian_basis_group
section."""^^xsd:string ;
    rdfs:subClassOf [ a owl:Restriction ;
            owl:hasValue 0 ;
            owl:onProperty :hasNumberOfDimensions ],
        [ a owl:Restriction ;
            owl:allValuesFrom <http://emmo.info/emmo/middle/math#EMMO_f8bd64d5_5d3e_4ad4_a46e_c30714fecb7f> ;
            owl:onProperty <http://emmo.info/emmo/middle/metrology#EMMO_67fc0a36_8dcb_4ffa_9a43_31074efa3296> ],
        [ a owl:Restriction ;
            owl:allValuesFrom <http://emmo.info/emmo/middle/math#EMMO_f8bd64d5_5d3e_4ad4_a46e_c30714fecb7f> ;
            owl:onProperty :hasDatatype ],
        :NMI_dimension,
        :NMI_quantity .

:number_of_k_mesh_points a owl:Class ;
    rdfs:comment "number of k points in the mesh (i.e. the k points used to evaluate energy_total)."^^xsd:string ;
    rdfs:subClassOf [ a owl:Restriction ;
            owl:allValuesFrom <http://emmo.info/emmo/middle/math#EMMO_f8bd64d5_5d3e_4ad4_a46e_c30714fecb7f> ;
            owl:onProperty <http://emmo.info/emmo/middle/metrology#EMMO_67fc0a36_8dcb_4ffa_9a43_31074efa3296> ],
        [ a owl:Restriction ;
            owl:onProperty :hasCategory ;
            owl:someValuesFrom :settings_potential_energy_surface ],
        [ a owl:Restriction ;
            owl:onProperty :hasCategory ;
            owl:someValuesFrom :settings_k_points ],
        [ a owl:Restriction ;
            owl:allValuesFrom <http://emmo.info/emmo/middle/math#EMMO_f8bd64d5_5d3e_4ad4_a46e_c30714fecb7f> ;
            owl:onProperty :hasDatatype ],
        [ a owl:Restriction ;
            owl:hasValue 0 ;
            owl:onProperty :hasNumberOfDimensions ],
        :NMI_dimension,
        :NMI_quantity .

:number_of_kinds_in_basis_set_atom_centered a owl:Class ;
    rdfs:comment """Gives the number of different *kinds* of radial basis functions in the
section_basis_set_atom_centered section. Specifically, basis functions with the
same $n$ and $l$ quantum numbers are grouped in sets. Each set counts as one
*kind*."""^^xsd:string ;
    rdfs:subClassOf [ a owl:Restriction ;
            owl:allValuesFrom <http://emmo.info/emmo/middle/math#EMMO_f8bd64d5_5d3e_4ad4_a46e_c30714fecb7f> ;
            owl:onProperty <http://emmo.info/emmo/middle/metrology#EMMO_67fc0a36_8dcb_4ffa_9a43_31074efa3296> ],
        [ a owl:Restriction ;
            owl:hasValue 0 ;
            owl:onProperty :hasNumberOfDimensions ],
        [ a owl:Restriction ;
            owl:allValuesFrom <http://emmo.info/emmo/middle/math#EMMO_f8bd64d5_5d3e_4ad4_a46e_c30714fecb7f> ;
            owl:onProperty :hasDatatype ],
        :NMI_dimension,
        :NMI_quantity .

:number_of_kinetic_energies_in_sequence a owl:Class ;
    rdfs:comment """Gives the number of kinetic energy evaluations in this sequence of frames, see
frame_sequence_kinetic_energy."""^^xsd:string ;
    rdfs:subClassOf [ a owl:Restriction ;
            owl:allValuesFrom <http://emmo.info/emmo/middle/math#EMMO_f8bd64d5_5d3e_4ad4_a46e_c30714fecb7f> ;
            owl:onProperty <http://emmo.info/emmo/middle/metrology#EMMO_67fc0a36_8dcb_4ffa_9a43_31074efa3296> ],
        [ a owl:Restriction ;
            owl:hasValue 0 ;
            owl:onProperty :hasNumberOfDimensions ],
        [ a owl:Restriction ;
            owl:allValuesFrom <http://emmo.info/emmo/middle/math#EMMO_f8bd64d5_5d3e_4ad4_a46e_c30714fecb7f> ;
            owl:onProperty :hasDatatype ],
        :NMI_dimension,
        :NMI_quantity .

:number_of_lm_atom_projected_dos a owl:Class ;
    rdfs:comment """Gives the number of $l$, $m$ combinations for the atom projected density of states
(DOS) defined in section_atom_projected_dos."""^^xsd:string ;
    rdfs:subClassOf [ a owl:Restriction ;
            owl:allValuesFrom <http://emmo.info/emmo/middle/math#EMMO_f8bd64d5_5d3e_4ad4_a46e_c30714fecb7f> ;
            owl:onProperty :hasDatatype ],
        [ a owl:Restriction ;
            owl:hasValue 0 ;
            owl:onProperty :hasNumberOfDimensions ],
        [ a owl:Restriction ;
            owl:allValuesFrom <http://emmo.info/emmo/middle/math#EMMO_f8bd64d5_5d3e_4ad4_a46e_c30714fecb7f> ;
            owl:onProperty <http://emmo.info/emmo/middle/metrology#EMMO_67fc0a36_8dcb_4ffa_9a43_31074efa3296> ],
        :NMI_dimension,
        :NMI_quantity .

:number_of_lm_atomic_multipoles a owl:Class ;
    rdfs:comment """Gives the number of $l$, $m$ combinations for atomic multipoles
atomic_multipole_lm."""^^xsd:string ;
    rdfs:subClassOf [ a owl:Restriction ;
            owl:allValuesFrom <http://emmo.info/emmo/middle/math#EMMO_f8bd64d5_5d3e_4ad4_a46e_c30714fecb7f> ;
            owl:onProperty :hasDatatype ],
        [ a owl:Restriction ;
            owl:allValuesFrom <http://emmo.info/emmo/middle/math#EMMO_f8bd64d5_5d3e_4ad4_a46e_c30714fecb7f> ;
            owl:onProperty <http://emmo.info/emmo/middle/metrology#EMMO_67fc0a36_8dcb_4ffa_9a43_31074efa3296> ],
        [ a owl:Restriction ;
            owl:hasValue 0 ;
            owl:onProperty :hasNumberOfDimensions ],
        :NMI_dimension,
        :NMI_quantity .

:number_of_lm_species_projected_dos a owl:Class ;
    rdfs:comment """Gives the number of $l$, $m$ combinations for the species-projected density of
states (DOS) defined in section_species_projected_dos."""^^xsd:string ;
    rdfs:subClassOf [ a owl:Restriction ;
            owl:allValuesFrom <http://emmo.info/emmo/middle/math#EMMO_f8bd64d5_5d3e_4ad4_a46e_c30714fecb7f> ;
            owl:onProperty <http://emmo.info/emmo/middle/metrology#EMMO_67fc0a36_8dcb_4ffa_9a43_31074efa3296> ],
        [ a owl:Restriction ;
            owl:allValuesFrom <http://emmo.info/emmo/middle/math#EMMO_f8bd64d5_5d3e_4ad4_a46e_c30714fecb7f> ;
            owl:onProperty :hasDatatype ],
        [ a owl:Restriction ;
            owl:hasValue 0 ;
            owl:onProperty :hasNumberOfDimensions ],
        :NMI_dimension,
        :NMI_quantity .

:number_of_normalized_band_segment_eigenvalues a owl:Class ;
    rdfs:comment """Gives the number of normalized eigenvalues in a band segment, see

band_energies_normalized."""^^xsd:string ;
    rdfs:subClassOf [ a owl:Restriction ;
            owl:allValuesFrom <http://emmo.info/emmo/middle/math#EMMO_f8bd64d5_5d3e_4ad4_a46e_c30714fecb7f> ;
            owl:onProperty :hasDatatype ],
        [ a owl:Restriction ;
            owl:allValuesFrom <http://emmo.info/emmo/middle/math#EMMO_f8bd64d5_5d3e_4ad4_a46e_c30714fecb7f> ;
            owl:onProperty <http://emmo.info/emmo/middle/metrology#EMMO_67fc0a36_8dcb_4ffa_9a43_31074efa3296> ],
        [ a owl:Restriction ;
            owl:hasValue 0 ;
            owl:onProperty :hasNumberOfDimensions ],
        :NMI_dimension,
        :NMI_quantity .

:number_of_potential_energies_in_sequence a owl:Class ;
    rdfs:comment """Gives the number of potential energies evaluation in this sequence. A sequence is
a trajectory, which can have number_of_frames_in_sequence each representing one
section_single_configuration_calculation section."""^^xsd:string ;
    rdfs:subClassOf [ a owl:Restriction ;
            owl:allValuesFrom <http://emmo.info/emmo/middle/math#EMMO_f8bd64d5_5d3e_4ad4_a46e_c30714fecb7f> ;
            owl:onProperty <http://emmo.info/emmo/middle/metrology#EMMO_67fc0a36_8dcb_4ffa_9a43_31074efa3296> ],
        [ a owl:Restriction ;
            owl:allValuesFrom <http://emmo.info/emmo/middle/math#EMMO_f8bd64d5_5d3e_4ad4_a46e_c30714fecb7f> ;
            owl:onProperty :hasDatatype ],
        [ a owl:Restriction ;
            owl:hasValue 0 ;
            owl:onProperty :hasNumberOfDimensions ],
        :NMI_dimension,
        :NMI_quantity .

:number_of_pressure_evaluations_in_sequence a owl:Class ;
    rdfs:comment """Gives the number of pressure evaluations in this sequence. A sequence is a
trajectory, which can have number_of_frames_in_sequence each representing one
section_single_configuration_calculation section."""^^xsd:string ;
    rdfs:subClassOf [ a owl:Restriction ;
            owl:hasValue 0 ;
            owl:onProperty :hasNumberOfDimensions ],
        [ a owl:Restriction ;
            owl:allValuesFrom <http://emmo.info/emmo/middle/math#EMMO_f8bd64d5_5d3e_4ad4_a46e_c30714fecb7f> ;
            owl:onProperty <http://emmo.info/emmo/middle/metrology#EMMO_67fc0a36_8dcb_4ffa_9a43_31074efa3296> ],
        [ a owl:Restriction ;
            owl:allValuesFrom <http://emmo.info/emmo/middle/math#EMMO_f8bd64d5_5d3e_4ad4_a46e_c30714fecb7f> ;
            owl:onProperty :hasDatatype ],
        :NMI_dimension,
        :NMI_quantity .

:number_of_temperatures_in_sequence a owl:Class ;
    rdfs:comment """Gives the number of temperature frames (frame_sequence_temperature) used in the
section_frame_sequence. A sequence is a trajectory, which can have
number_of_frames_in_sequence each representing one
section_single_configuration_calculation section."""^^xsd:string ;
    rdfs:subClassOf [ a owl:Restriction ;
            owl:allValuesFrom <http://emmo.info/emmo/middle/math#EMMO_f8bd64d5_5d3e_4ad4_a46e_c30714fecb7f> ;
            owl:onProperty <http://emmo.info/emmo/middle/metrology#EMMO_67fc0a36_8dcb_4ffa_9a43_31074efa3296> ],
        [ a owl:Restriction ;
            owl:allValuesFrom <http://emmo.info/emmo/middle/math#EMMO_f8bd64d5_5d3e_4ad4_a46e_c30714fecb7f> ;
            owl:onProperty :hasDatatype ],
        [ a owl:Restriction ;
            owl:hasValue 0 ;
            owl:onProperty :hasNumberOfDimensions ],
        :NMI_dimension,
        :NMI_quantity .

:number_of_user_quantity_evaluations_in_sequence a owl:Class ;
    rdfs:comment """Gives the number of user defined quantity evaluations along a sequence of
frame_sequence_user_quantity frames. A sequence is a trajectory, which can have
number_of_frames_in_sequence each representing one
section_single_configuration_calculation section."""^^xsd:string ;
    rdfs:subClassOf [ a owl:Restriction ;
            owl:allValuesFrom <http://emmo.info/emmo/middle/math#EMMO_f8bd64d5_5d3e_4ad4_a46e_c30714fecb7f> ;
            owl:onProperty <http://emmo.info/emmo/middle/metrology#EMMO_67fc0a36_8dcb_4ffa_9a43_31074efa3296> ],
        [ a owl:Restriction ;
            owl:allValuesFrom <http://emmo.info/emmo/middle/math#EMMO_f8bd64d5_5d3e_4ad4_a46e_c30714fecb7f> ;
            owl:onProperty :hasDatatype ],
        [ a owl:Restriction ;
            owl:hasValue 0 ;
            owl:onProperty :hasNumberOfDimensions ],
        :NMI_dimension,
        :NMI_quantity .

:settings_atom_in_molecule a owl:Class ;
    rdfs:comment "Parameters of an atom within a molecule."^^xsd:string ;
    rdfs:subClassOf :NMI_category .

:settings_k_points a owl:Class ;
    rdfs:comment "Contains parameters that control the $k$-point mesh."^^xsd:string ;
    rdfs:subClassOf :settings_potential_energy_surface .

:settings_molecular_dynamics a owl:Class ;
    rdfs:comment "Contains parameters that control the molecular dynamics sampling."^^xsd:string ;
    rdfs:subClassOf :settings_sampling .

:energy_component_per_atom a owl:Class ;
    rdfs:comment """A value of an energy component per atom, concurring in defining the total energy per
atom."""^^xsd:string ;
    rdfs:subClassOf :energy_value .

:error_estimate_contribution a owl:Class ;
    rdfs:comment "An estimate of a partial quantity contributing to the error for a given quantity."^^xsd:string ;
    rdfs:subClassOf :NMI_category .

:hasVarDim4 a owl:ObjectProperty ;
    rdfs:domain :NMI_quantity ;
    rdfs:range :NMI_dimension ;
    rdfs:subPropertyOf <http://emmo.info/emmo/middle/semiotics#EMMO_eb3518bf_f799_4f9e_8c3e_ce59af11453b> .

:number_of_atom_projected_dos_values a owl:Class ;
    rdfs:comment """Gives the number of energy values for the atom-projected density of states (DOS)
based on atom_projected_dos_values_lm and atom_projected_dos_values_total."""^^xsd:string ;
    rdfs:subClassOf [ a owl:Restriction ;
            owl:allValuesFrom <http://emmo.info/emmo/middle/math#EMMO_f8bd64d5_5d3e_4ad4_a46e_c30714fecb7f> ;
            owl:onProperty :hasDatatype ],
        [ a owl:Restriction ;
            owl:hasValue 0 ;
            owl:onProperty :hasNumberOfDimensions ],
        [ a owl:Restriction ;
            owl:allValuesFrom <http://emmo.info/emmo/middle/math#EMMO_f8bd64d5_5d3e_4ad4_a46e_c30714fecb7f> ;
            owl:onProperty <http://emmo.info/emmo/middle/metrology#EMMO_67fc0a36_8dcb_4ffa_9a43_31074efa3296> ],
        :NMI_dimension,
        :NMI_quantity .

:number_of_atoms_in_molecule a owl:Class ;
    rdfs:comment "Number of atoms in this molecule."^^xsd:string ;
    rdfs:subClassOf [ a owl:Restriction ;
            owl:allValuesFrom <http://emmo.info/emmo/middle/math#EMMO_f8bd64d5_5d3e_4ad4_a46e_c30714fecb7f> ;
            owl:onProperty <http://emmo.info/emmo/middle/metrology#EMMO_67fc0a36_8dcb_4ffa_9a43_31074efa3296> ],
        [ a owl:Restriction ;
            owl:allValuesFrom <http://emmo.info/emmo/middle/math#EMMO_f8bd64d5_5d3e_4ad4_a46e_c30714fecb7f> ;
            owl:onProperty :hasDatatype ],
        [ a owl:Restriction ;
            owl:hasValue 0 ;
            owl:onProperty :hasNumberOfDimensions ],
        :NMI_dimension,
        :NMI_quantity .

:number_of_excited_states a owl:Class ;
    rdfs:comment "Number of excited states."^^xsd:string ;
    rdfs:subClassOf [ a owl:Restriction ;
            owl:allValuesFrom <http://emmo.info/emmo/middle/math#EMMO_f8bd64d5_5d3e_4ad4_a46e_c30714fecb7f> ;
            owl:onProperty <http://emmo.info/emmo/middle/metrology#EMMO_67fc0a36_8dcb_4ffa_9a43_31074efa3296> ],
        [ a owl:Restriction ;
            owl:hasValue 0 ;
            owl:onProperty :hasNumberOfDimensions ],
        [ a owl:Restriction ;
            owl:allValuesFrom <http://emmo.info/emmo/middle/math#EMMO_f8bd64d5_5d3e_4ad4_a46e_c30714fecb7f> ;
            owl:onProperty :hasDatatype ],
        :NMI_dimension,
        :NMI_quantity .

:number_of_k_points_per_segment a owl:Class ;
    rdfs:comment """Gives the number of $k$ points in the segment of the band structure, see
section_k_band_segment."""^^xsd:string ;
    rdfs:subClassOf [ a owl:Restriction ;
            owl:allValuesFrom <http://emmo.info/emmo/middle/math#EMMO_f8bd64d5_5d3e_4ad4_a46e_c30714fecb7f> ;
            owl:onProperty <http://emmo.info/emmo/middle/metrology#EMMO_67fc0a36_8dcb_4ffa_9a43_31074efa3296> ],
        [ a owl:Restriction ;
            owl:hasValue 0 ;
            owl:onProperty :hasNumberOfDimensions ],
        [ a owl:Restriction ;
            owl:allValuesFrom <http://emmo.info/emmo/middle/math#EMMO_f8bd64d5_5d3e_4ad4_a46e_c30714fecb7f> ;
            owl:onProperty :hasDatatype ],
        :NMI_dimension,
        :NMI_quantity .

:number_of_normalized_k_points_per_segment a owl:Class ;
    rdfs:comment """Gives the number of $k$ points in the segment of the normalized band structure
(see section_k_band_segment_normalized)."""^^xsd:string ;
    rdfs:subClassOf [ a owl:Restriction ;
            owl:allValuesFrom <http://emmo.info/emmo/middle/math#EMMO_f8bd64d5_5d3e_4ad4_a46e_c30714fecb7f> ;
            owl:onProperty :hasDatatype ],
        [ a owl:Restriction ;
            owl:allValuesFrom <http://emmo.info/emmo/middle/math#EMMO_f8bd64d5_5d3e_4ad4_a46e_c30714fecb7f> ;
            owl:onProperty <http://emmo.info/emmo/middle/metrology#EMMO_67fc0a36_8dcb_4ffa_9a43_31074efa3296> ],
        [ a owl:Restriction ;
            owl:hasValue 0 ;
            owl:onProperty :hasNumberOfDimensions ],
        :NMI_dimension,
        :NMI_quantity .

:number_of_species a owl:Class ;
    rdfs:comment """Gives the number of species for the species-projected density of states (DOS)
defined in section_species_projected_dos."""^^xsd:string ;
    rdfs:subClassOf [ a owl:Restriction ;
            owl:hasValue 0 ;
            owl:onProperty :hasNumberOfDimensions ],
        [ a owl:Restriction ;
            owl:allValuesFrom <http://emmo.info/emmo/middle/math#EMMO_f8bd64d5_5d3e_4ad4_a46e_c30714fecb7f> ;
            owl:onProperty <http://emmo.info/emmo/middle/metrology#EMMO_67fc0a36_8dcb_4ffa_9a43_31074efa3296> ],
        [ a owl:Restriction ;
            owl:allValuesFrom <http://emmo.info/emmo/middle/math#EMMO_f8bd64d5_5d3e_4ad4_a46e_c30714fecb7f> ;
            owl:onProperty :hasDatatype ],
        :NMI_dimension,
        :NMI_quantity .

:program_info a owl:Class ;
    rdfs:comment """Contains information on the program that generated the data, i.e. the program_name,
program_version, program_compilation_host and program_compilation_datetime as direct
children of this field."""^^xsd:string ;
    rdfs:subClassOf :accessory_info .

:settings_geometry_optimization a owl:Class ;
    rdfs:comment "Contains parameters controlling the geometry optimization."^^xsd:string ;
    rdfs:subClassOf :settings_sampling .

:settings_physical_parameter a owl:Class ;
    rdfs:comment """A parameter that defines the physical model used. Use settings_numerical_parameter for
parameters that that influence only the convergence/accuracy."""^^xsd:string ;
    rdfs:subClassOf :NMI_category .

:message_warning a owl:Class ;
    rdfs:comment "A warning message of the computational program."^^xsd:string ;
    rdfs:subClassOf :message_info .

:number_of_atoms_primitive a owl:Class ;
    rdfs:comment "Number of atoms in primitive system."^^xsd:string ;
    rdfs:subClassOf [ a owl:Restriction ;
            owl:allValuesFrom <http://emmo.info/emmo/middle/math#EMMO_f8bd64d5_5d3e_4ad4_a46e_c30714fecb7f> ;
            owl:onProperty :hasDatatype ],
        [ a owl:Restriction ;
            owl:allValuesFrom <http://emmo.info/emmo/middle/math#EMMO_f8bd64d5_5d3e_4ad4_a46e_c30714fecb7f> ;
            owl:onProperty <http://emmo.info/emmo/middle/metrology#EMMO_67fc0a36_8dcb_4ffa_9a43_31074efa3296> ],
        [ a owl:Restriction ;
            owl:hasValue 0 ;
            owl:onProperty :hasNumberOfDimensions ],
        :NMI_dimension,
        :NMI_quantity .

:number_of_atoms_std a owl:Class ;
    rdfs:comment "Number of atoms in standardized system."^^xsd:string ;
    rdfs:subClassOf [ a owl:Restriction ;
            owl:hasValue 0 ;
            owl:onProperty :hasNumberOfDimensions ],
        [ a owl:Restriction ;
            owl:allValuesFrom <http://emmo.info/emmo/middle/math#EMMO_f8bd64d5_5d3e_4ad4_a46e_c30714fecb7f> ;
            owl:onProperty :hasDatatype ],
        [ a owl:Restriction ;
            owl:allValuesFrom <http://emmo.info/emmo/middle/math#EMMO_f8bd64d5_5d3e_4ad4_a46e_c30714fecb7f> ;
            owl:onProperty <http://emmo.info/emmo/middle/metrology#EMMO_67fc0a36_8dcb_4ffa_9a43_31074efa3296> ],
        :NMI_dimension,
        :NMI_quantity .

:number_of_species_projected_dos_values a owl:Class ;
    rdfs:comment """Gives the number of energy values for the species-projected density of states
(DOS) defined in section_species_projected_dos."""^^xsd:string ;
    rdfs:subClassOf [ a owl:Restriction ;
            owl:allValuesFrom <http://emmo.info/emmo/middle/math#EMMO_f8bd64d5_5d3e_4ad4_a46e_c30714fecb7f> ;
            owl:onProperty <http://emmo.info/emmo/middle/metrology#EMMO_67fc0a36_8dcb_4ffa_9a43_31074efa3296> ],
        [ a owl:Restriction ;
            owl:allValuesFrom <http://emmo.info/emmo/middle/math#EMMO_f8bd64d5_5d3e_4ad4_a46e_c30714fecb7f> ;
            owl:onProperty :hasDatatype ],
        [ a owl:Restriction ;
            owl:hasValue 0 ;
            owl:onProperty :hasNumberOfDimensions ],
        :NMI_dimension,
        :NMI_quantity .

:parsing_message_warning a owl:Class ;
    rdfs:comment "This field is used for warning messages of the parsing program."^^xsd:string ;
    rdfs:subClassOf :parsing_message_info .

:settings_post_hartree_fock a owl:Class ;
    rdfs:comment "Contains parameters for the post Hartree-Fock method."^^xsd:string ;
    rdfs:subClassOf :settings_XC .

:atom_forces_type a owl:Class ;
    rdfs:comment """The types of forces acting on the atoms (i.e., minus derivatives of the specific type
of energy with respect to the atom position)."""^^xsd:string ;
    rdfs:subClassOf :NMI_category .

:energy_type_reference a owl:Class ;
    rdfs:comment "This metadata stores an energy used as reference point."^^xsd:string ;
    rdfs:subClassOf :energy_value .

:configuration_core a owl:Class ;
    rdfs:comment "Properties defining the current configuration."^^xsd:string ;
    rdfs:subClassOf :NMI_category .

:message_info a owl:Class ;
    rdfs:comment "An information message of the computational program."^^xsd:string ;
    rdfs:subClassOf :message_debug .

:number_of_dos_values a owl:Class ;
    rdfs:comment """Gives the number of energy values for the density of states (DOS), see
dos_energies."""^^xsd:string ;
    rdfs:subClassOf [ a owl:Restriction ;
            owl:allValuesFrom <http://emmo.info/emmo/middle/math#EMMO_f8bd64d5_5d3e_4ad4_a46e_c30714fecb7f> ;
            owl:onProperty :hasDatatype ],
        [ a owl:Restriction ;
            owl:allValuesFrom <http://emmo.info/emmo/middle/math#EMMO_f8bd64d5_5d3e_4ad4_a46e_c30714fecb7f> ;
            owl:onProperty <http://emmo.info/emmo/middle/metrology#EMMO_67fc0a36_8dcb_4ffa_9a43_31074efa3296> ],
        [ a owl:Restriction ;
            owl:hasValue 0 ;
            owl:onProperty :hasNumberOfDimensions ],
        :NMI_dimension,
        :NMI_quantity .

:number_of_eigenvalues a owl:Class ;
    rdfs:comment "Gives the number of eigenvalues, see eigenvalues_values."^^xsd:string ;
    rdfs:subClassOf [ a owl:Restriction ;
            owl:hasValue 0 ;
            owl:onProperty :hasNumberOfDimensions ],
        [ a owl:Restriction ;
            owl:allValuesFrom <http://emmo.info/emmo/middle/math#EMMO_f8bd64d5_5d3e_4ad4_a46e_c30714fecb7f> ;
            owl:onProperty :hasDatatype ],
        [ a owl:Restriction ;
            owl:allValuesFrom <http://emmo.info/emmo/middle/math#EMMO_f8bd64d5_5d3e_4ad4_a46e_c30714fecb7f> ;
            owl:onProperty <http://emmo.info/emmo/middle/metrology#EMMO_67fc0a36_8dcb_4ffa_9a43_31074efa3296> ],
        :NMI_dimension,
        :NMI_quantity .

:number_of_thermodynamical_property_values a owl:Class ;
    rdfs:comment """Gives the number of thermal properties values available in
section_thermodynamical_properties."""^^xsd:string ;
    rdfs:subClassOf [ a owl:Restriction ;
            owl:allValuesFrom <http://emmo.info/emmo/middle/math#EMMO_f8bd64d5_5d3e_4ad4_a46e_c30714fecb7f> ;
            owl:onProperty <http://emmo.info/emmo/middle/metrology#EMMO_67fc0a36_8dcb_4ffa_9a43_31074efa3296> ],
        [ a owl:Restriction ;
            owl:allValuesFrom <http://emmo.info/emmo/middle/math#EMMO_f8bd64d5_5d3e_4ad4_a46e_c30714fecb7f> ;
            owl:onProperty :hasDatatype ],
        [ a owl:Restriction ;
            owl:hasValue 0 ;
            owl:onProperty :hasNumberOfDimensions ],
        :NMI_dimension,
        :NMI_quantity .

:parsing_message_info a owl:Class ;
    rdfs:comment "This field is used for info messages of the parsing program."^^xsd:string ;
    rdfs:subClassOf :parsing_message_debug .

:energy_total_potential a owl:Class ;
    rdfs:comment """A value of the total potential energy. Note that a direct comparison may not be
possible because of a difference in the methods for computing total energies and
numerical implementations of various codes might leads to different energy zeros (see
section_energy_code_independent for a code-independent definition of the energy)."""^^xsd:string ;
    rdfs:subClassOf :energy_component .

:settings_sampling a owl:Class ;
    rdfs:comment "Contains parameters controlling the sampling."^^xsd:string ;
    rdfs:subClassOf :NMI_category .

:message_debug a owl:Class ;
    rdfs:comment "A debugging message of the computational program."^^xsd:string ;
    rdfs:subClassOf :NMI_category .

:parsing_message_debug a owl:Class ;
    rdfs:comment "This field is used for debugging messages of the parsing program."^^xsd:string ;
    rdfs:subClassOf :NMI_category .

:number_of_eigenvalues_kpoints a owl:Class ;
    rdfs:comment """Gives the number of $k$ points, see eigenvalues_kpoints. $k$ points are calculated
within a run and are irreducible if a symmetry is used."""^^xsd:string ;
    rdfs:subClassOf [ a owl:Restriction ;
            owl:allValuesFrom <http://emmo.info/emmo/middle/math#EMMO_f8bd64d5_5d3e_4ad4_a46e_c30714fecb7f> ;
            owl:onProperty :hasDatatype ],
        [ a owl:Restriction ;
            owl:hasValue 0 ;
            owl:onProperty :hasNumberOfDimensions ],
        [ a owl:Restriction ;
            owl:allValuesFrom <http://emmo.info/emmo/middle/math#EMMO_f8bd64d5_5d3e_4ad4_a46e_c30714fecb7f> ;
            owl:onProperty <http://emmo.info/emmo/middle/metrology#EMMO_67fc0a36_8dcb_4ffa_9a43_31074efa3296> ],
        :NMI_dimension,
        :NMI_quantity .

:settings_XC a owl:Class ;
    rdfs:comment """Contains parameters connected with the definition of the exchange-correlation (XC)
*method*. Here, the term *method* is a more general concept than just *functionals*
and include, e.g., post Hartree-Fock methods, too."""^^xsd:string ;
    rdfs:subClassOf :settings_potential_energy_surface .

:settings_potential_energy_surface a owl:Class ;
    rdfs:comment "Contains parameters that control the potential energy surface."^^xsd:string ;
    rdfs:subClassOf :NMI_category .

:hasVarDim3 a owl:ObjectProperty ;
    rdfs:domain :NMI_quantity ;
    rdfs:range :NMI_dimension ;
    rdfs:subPropertyOf <http://emmo.info/emmo/middle/semiotics#EMMO_eb3518bf_f799_4f9e_8c3e_ce59af11453b> .

:soap_parameter a owl:Class ;
    rdfs:comment "A soap parameter"^^xsd:string ;
    rdfs:subClassOf :NMI_category .

:time_info a owl:Class ;
    rdfs:comment """Stores information on the date and timings of the calculation. They are useful for,
e.g., debugging or visualization purposes."""^^xsd:string ;
    rdfs:subClassOf :accessory_info .

:number_of_atoms a owl:Class ;
    rdfs:comment """Stores the total number of atoms used in the calculation. For alloys where
concentrations of species are given for each site in the unit cell, it stores the
number of sites."""^^xsd:string ;
    rdfs:subClassOf [ a owl:Restriction ;
            owl:hasValue 0 ;
            owl:onProperty :hasNumberOfDimensions ],
        [ a owl:Restriction ;
            owl:allValuesFrom <http://emmo.info/emmo/middle/math#EMMO_f8bd64d5_5d3e_4ad4_a46e_c30714fecb7f> ;
            owl:onProperty <http://emmo.info/emmo/middle/metrology#EMMO_67fc0a36_8dcb_4ffa_9a43_31074efa3296> ],
        [ a owl:Restriction ;
            owl:allValuesFrom <http://emmo.info/emmo/middle/math#EMMO_f8bd64d5_5d3e_4ad4_a46e_c30714fecb7f> ;
            owl:onProperty :hasDatatype ],
        :NMI_dimension,
        :NMI_quantity .

:NMI_category a owl:Class ;
    rdfs:subClassOf :NMI_type .

:number_of_spin_channels a owl:Class ;
    rdfs:comment "Gives the number of spin channels, see section_method."^^xsd:string ;
    rdfs:subClassOf [ a owl:Restriction ;
            owl:hasValue 0 ;
            owl:onProperty :hasNumberOfDimensions ],
        [ a owl:Restriction ;
            owl:allValuesFrom <http://emmo.info/emmo/middle/math#EMMO_f8bd64d5_5d3e_4ad4_a46e_c30714fecb7f> ;
            owl:onProperty :hasDatatype ],
        [ a owl:Restriction ;
            owl:allValuesFrom <http://emmo.info/emmo/middle/math#EMMO_f8bd64d5_5d3e_4ad4_a46e_c30714fecb7f> ;
            owl:onProperty <http://emmo.info/emmo/middle/metrology#EMMO_67fc0a36_8dcb_4ffa_9a43_31074efa3296> ],
        :NMI_dimension,
        :NMI_quantity .

:accessory_info a owl:Class ;
    rdfs:comment """Information that *in theory* should not affect the results of the calculations (e.g.,
timing)."""^^xsd:string ;
    rdfs:subClassOf :NMI_category .

:hasFixDim1 a owl:DatatypeProperty,
        owl:FunctionalProperty ;
    rdfs:domain :NMI_quantity ;
    rdfs:range [ a rdfs:Datatype ;
            owl:onDatatype xsd:integer ;
            owl:withRestrictions ( [ xsd:minInclusive 1 ] ) ] .

:hasVarDim2 a owl:ObjectProperty ;
    rdfs:domain :NMI_quantity ;
    rdfs:range :NMI_dimension ;
    rdfs:subPropertyOf <http://emmo.info/emmo/middle/semiotics#EMMO_eb3518bf_f799_4f9e_8c3e_ce59af11453b> .

:hasFixDim2 a owl:DatatypeProperty,
        owl:FunctionalProperty ;
    rdfs:domain :NMI_quantity ;
    rdfs:range [ a rdfs:Datatype ;
            owl:onDatatype xsd:integer ;
            owl:withRestrictions ( [ xsd:minInclusive 1 ] ) ] .

:energy_component a owl:Class ;
    rdfs:comment "A value of an energy component, expected to be an extensive property."^^xsd:string ;
    rdfs:subClassOf :energy_value .

:hasSubSection a owl:ObjectProperty ;
    rdfs:domain :NMI_section ;
    rdfs:range :NMI_section ;
    rdfs:subPropertyOf <http://emmo.info/emmo/top/mereotopology#EMMO_17e27c22_37e1_468c_9dd7_95e137f73e7f> .

:energy_value a owl:Class ;
    rdfs:comment "This metadata stores an energy value."^^xsd:string ;
    rdfs:subClassOf :NMI_category .

:NMI_section a owl:Class ;
    rdfs:subClassOf :NMI_type .

:NMI_dimension a owl:Class ;
    rdfs:subClassOf :NMI_quantity .

:hasVarDim1 a owl:ObjectProperty ;
    rdfs:domain :NMI_quantity ;
    rdfs:range :NMI_dimension ;
    rdfs:subPropertyOf <http://emmo.info/emmo/middle/semiotics#EMMO_eb3518bf_f799_4f9e_8c3e_ce59af11453b> .

:hasCategory a owl:ObjectProperty ;
    rdfs:domain :NMI_quantity ;
    rdfs:range :NMI_category ;
    rdfs:subPropertyOf <http://emmo.info/emmo/middle/semiotics#EMMO_eb3518bf_f799_4f9e_8c3e_ce59af11453b> .

:hasDatatype a owl:ObjectProperty ;
    rdfs:domain :NMI_quantity ;
    rdfs:subPropertyOf <http://emmo.info/emmo/middle/semiotics#EMMO_eb3518bf_f799_4f9e_8c3e_ce59af11453b> .

:hasNumberOfDimensions a owl:DatatypeProperty,
        owl:FunctionalProperty ;
    rdfs:range [ a rdfs:Datatype ;
            owl:onDatatype xsd:integer ;
            owl:withRestrictions ( [ xsd:minInclusive 0 ] ) ] .

:hasQuantity a owl:ObjectProperty ;
    rdfs:domain :NMI_section ;
    rdfs:range :NMI_quantity ;
    rdfs:subPropertyOf <http://emmo.info/emmo/middle/reductionistic#EMMO_b2282816_b7a3_44c6_b2cb_3feff1ceb7fe> .

:NMI_quantity a owl:Class ;
    rdfs:subClassOf :NMI_type .

